PREFIX : <http://def.isotc211.org/iso19115/-1/2018/SpatialRepresentationInformation/code/MD_TopologyLevelCode/>
PREFIX cs: <http://def.isotc211.org/iso19115/-1/2018/SpatialRepresentationInformation/code/MD_TopologyLevelCode>
PREFIX prov: <http://www.w3.org/ns/prov#>
PREFIX rdfs: <http://www.w3.org/2000/01/rdf-schema#>
PREFIX reg: <http://purl.org/linked-data/registry#>
PREFIX schema: <https://schema.org/>
PREFIX skos: <http://www.w3.org/2004/02/skos/core#>
PREFIX status: <http://def.isotc211.org/iso19135/-1/2015/CoreModel/code/RE_ItemStatus/>
PREFIX xsd: <http://www.w3.org/2001/XMLSchema#>

:abstract
    a skos:Concept ;
    reg:status status:stable ;
    rdfs:isDefinedBy cs: ;
    skos:definition "topological complex without any specified geometric realisation" ;
    skos:inScheme cs: ;
    skos:prefLabel "abstract"@en ;
    skos:topConceptOf cs: ;
    schema:identifier "abstract"^^xsd:token ;
    skos:historyNote "Presented in the original standard's codelist"@en ;
.

:fullPlanarGraph
    a skos:Concept ;
    reg:status status:stable ;
    rdfs:isDefinedBy cs: ;
    skos:definition "2-dimensional topological complex that is planar. (A 2-dimensional topological complex is commonly called 'full topology' in a cartographic 2D environment.)" ;
    skos:inScheme cs: ;
    skos:prefLabel "full planar graph"@en ;
    skos:topConceptOf cs: ;
    schema:identifier "fullPlanarGraph"^^xsd:token ;
    skos:historyNote "Presented in the original standard's codelist"@en ;
.

:fullSurfaceGraph
    a skos:Concept ;
    reg:status status:stable ;
    rdfs:isDefinedBy cs: ;
    skos:definition "2-dimensional topological complex that is isomorphic to a subset of a surface" ;
    skos:inScheme cs: ;
    skos:prefLabel "full surface graph"@en ;
    skos:topConceptOf cs: ;
    schema:identifier "fullSurfaceGraph"^^xsd:token ;
    skos:historyNote "Presented in the original standard's codelist"@en ;
.

:fullTopology3D
    a skos:Concept ;
    reg:status status:stable ;
    rdfs:isDefinedBy cs: ;
    skos:definition "complete coverage of a 3D Euclidean coordinate space" ;
    skos:inScheme cs: ;
    skos:prefLabel "full topology3d"@en ;
    skos:topConceptOf cs: ;
    schema:identifier "fullTopology3D"^^xsd:token ;
    skos:historyNote "Presented in the original standard's codelist"@en ;
.

:geometryOnly
    a skos:Concept ;
    reg:status status:stable ;
    rdfs:isDefinedBy cs: ;
    skos:definition "geometry objects without any additional structure which describes topology" ;
    skos:inScheme cs: ;
    skos:prefLabel "geometry only"@en ;
    skos:topConceptOf cs: ;
    schema:identifier "geometryOnly"^^xsd:token ;
    skos:historyNote "Presented in the original standard's codelist"@en ;
.

:planarGraph
    a skos:Concept ;
    reg:status status:stable ;
    rdfs:isDefinedBy cs: ;
    skos:definition "1-dimensional topological complex that is planar. (A planar graph is a graph that can be drawn in a plane in such a way that no two edges intersect except at a vertex.)" ;
    skos:inScheme cs: ;
    skos:prefLabel "planar graph"@en ;
    skos:topConceptOf cs: ;
    schema:identifier "planarGraph"^^xsd:token ;
    skos:historyNote "Presented in the original standard's codelist"@en ;
.

:surfaceGraph
    a skos:Concept ;
    reg:status status:stable ;
    rdfs:isDefinedBy cs: ;
    skos:definition "1-dimensional topological complex that is isomorphic to a subset of a surface. (A geometric complex is isomorphic to a topological complex if their elements are in a one-to-one, dimensional-and boundary-preserving correspondence to one another.)" ;
    skos:inScheme cs: ;
    skos:prefLabel "surface graph"@en ;
    skos:topConceptOf cs: ;
    schema:identifier "surfaceGraph"^^xsd:token ;
    skos:historyNote "Presented in the original standard's codelist"@en ;
.

:topology1D
    a skos:Concept ;
    reg:status status:stable ;
    rdfs:isDefinedBy cs: ;
    skos:definition "1-dimensional topological complex - commonly called 'chain-node' topology" ;
    skos:inScheme cs: ;
    skos:prefLabel "topology1d"@en ;
    skos:topConceptOf cs: ;
    schema:identifier "topology1D"^^xsd:token ;
    skos:historyNote "Presented in the original standard's codelist"@en ;
.

:topology3D
    a skos:Concept ;
    reg:status status:stable ;
    rdfs:isDefinedBy cs: ;
    skos:definition "3-dimensional topological complex. (A topological complex is a collection of topological primitives that are closed under the boundary operations.)" ;
    skos:inScheme cs: ;
    skos:prefLabel "topology3d"@en ;
    skos:topConceptOf cs: ;
    schema:identifier "topology3D"^^xsd:token ;
    skos:historyNote "Presented in the original standard's codelist"@en ;
.

cs:
    a skos:ConceptScheme ;
    reg:status status:valid ;
    skos:definition "degree of complexity of the spatial relationships"@en ;
    skos:hasTopConcept
        :abstract ,
        :fullPlanarGraph ,
        :fullSurfaceGraph ,
        :fullTopology3D ,
        :geometryOnly ,
        :planarGraph ,
        :surfaceGraph ,
        :topology1D ,
        :topology3D ;
    skos:prefLabel "MD Topology Level Code"@en ;
    prov:qualifiedDerivation
        [
            prov:entity <http://example.com/none> ;
            prov:hadRole <https://linked.data.gov.au/def/vocab-derivation-modes/none> ;
        ] ;
    schema:citation "http://standards.iso.org/iso/19115/-1/ed-1/en/"^^xsd:anyURI ;
    schema:creator <https://committee.iso.org/home/tc211> ;
    schema:dateCreated "2000-01-01"^^xsd:date ;
    schema:dateModified "2000-01-01"^^xsd:date ;
    schema:identifier "MD_TopologyLevelCode"^^xsd:token ;
    schema:isFormatOf <http://def.isotc211.org/iso19115/-1/2018/SpatialRepresentationInformation#MD_TopologyLevelCode> ;
    schema:issued "2000-01-01"^^xsd:date ;
    skos:historyNote "Derived from TC211-produced RDF versions of the standard's UML"@en ;
    schema:publisher <https://committee.iso.org/home/tc211> ;
.
