# baseURI: http://def.isotc211.org/iso19115/-1/2014/ReferenceSystemInformation
# imports: http://def.isotc211.org/iso19115/-1/2014/CommonClasses
# imports: http://def.isotc211.org/iso19150/-2/2012/base

@prefix dct: <http://purl.org/dc/terms/> .
@prefix iso19115-1: <http://def.isotc211.org/iso19115/-1/2014/ReferenceSystemInformation#> .
@prefix iso19115-1Code: <http://def.isotc211.org/iso19115/-1/2014/ReferenceSystemInformation/code/> .
@prefix iso19115-1_2358: <http://def.isotc211.org/iso19115/-1/2014/CommonClasses#> .
@prefix owl: <http://www.w3.org/2002/07/owl#> .
@prefix rdf: <http://www.w3.org/1999/02/22-rdf-syntax-ns#> .
@prefix rdfs: <http://www.w3.org/2000/01/rdf-schema#> .
@prefix skos: <http://www.w3.org/2004/02/skos/core#> .
@prefix xsd: <http://www.w3.org/2001/XMLSchema#> .

<http://def.isotc211.org/iso19115/-1/2014/ReferenceSystemInformation>
  rdf:type owl:Ontology ;
  dct:source "http://standards.iso.org/iso/19115/-1/ed-1/en/" ;
  rdfs:label "ISO 19115-1:2014 Reference system information" ;
  owl:imports <http://def.isotc211.org/iso19115/-1/2014/CommonClasses> ;
  owl:imports <http://def.isotc211.org/iso19150/-2/2012/base> ;
  owl:versionInfo "2014" ;
.
iso19115-1:MD_ReferenceSystem
  rdf:type owl:Class ;
  rdfs:isDefinedBy <http://standards.iso.org/iso/19115/-1/ed-1/en/> ;
  rdfs:label "MD_ReferenceSystem" ;
  rdfs:subClassOf [
      rdf:type owl:Restriction ;
      owl:allValuesFrom iso19115-1_2358:MD_Identifier ;
      owl:onProperty <http://def.isotc211.org/iso19115/-1/2014/ReferenceSystemInformation#MD_ReferenceSystem.referenceSystemIdentifier> ;
    ] ;
  rdfs:subClassOf [
      rdf:type owl:Restriction ;
      owl:allValuesFrom iso19115-1:MD_ReferenceSystemTypeCode ;
      owl:onProperty <http://def.isotc211.org/iso19115/-1/2014/ReferenceSystemInformation#MD_ReferenceSystem.referenceSystemType> ;
    ] ;
  rdfs:subClassOf [
      rdf:type owl:Restriction ;
      owl:maxCardinality "1"^^xsd:nonNegativeInteger ;
      owl:onProperty <http://def.isotc211.org/iso19115/-1/2014/ReferenceSystemInformation#MD_ReferenceSystem.referenceSystemIdentifier> ;
    ] ;
  rdfs:subClassOf [
      rdf:type owl:Restriction ;
      owl:maxCardinality "1"^^xsd:nonNegativeInteger ;
      owl:onProperty <http://def.isotc211.org/iso19115/-1/2014/ReferenceSystemInformation#MD_ReferenceSystem.referenceSystemType> ;
    ] ;
  skos:definition "information about the reference system" ;
.
<http://def.isotc211.org/iso19115/-1/2014/ReferenceSystemInformation#MD_ReferenceSystem.referenceSystemIdentifier>
  rdf:type owl:ObjectProperty ;
  rdfs:domain iso19115-1:MD_ReferenceSystem ;
  rdfs:isDefinedBy <http://standards.iso.org/iso/19115/-1/ed-1/en/> ;
  rdfs:label "referenceSystemIdentifier" ;
  rdfs:range iso19115-1_2358:MD_Identifier ;
.
<http://def.isotc211.org/iso19115/-1/2014/ReferenceSystemInformation#MD_ReferenceSystem.referenceSystemType>
  rdf:type owl:ObjectProperty ;
  rdfs:domain iso19115-1:MD_ReferenceSystem ;
  rdfs:isDefinedBy <http://standards.iso.org/iso/19115/-1/ed-1/en/> ;
  rdfs:label "referenceSystemType" ;
  rdfs:range iso19115-1:MD_ReferenceSystemTypeCode ;
.
iso19115-1:MD_ReferenceSystemTypeCode
  rdf:type owl:Class ;
  rdfs:isDefinedBy <http://standards.iso.org/iso/19115/-1/ed-1/en/> ;
  rdfs:label "MD_ReferenceSystemTypeCode" ;
  rdfs:subClassOf skos:Concept ;
.
iso19115-1Code:MD_ReferenceSystemTypeCode
  rdf:type skos:ConceptScheme ;
  dct:description "defines type of reference system used"^^xsd:string ;
  dct:isFormatOf iso19115-1:MD_ReferenceSystemTypeCode ;
  rdfs:isDefinedBy <http://standards.iso.org/iso/19115/-1/ed-1/en/> ;
  rdfs:label "MD Reference System Type Code - Concept Scheme"^^xsd:string ;
  skos:definition "defines type of reference system used"^^xsd:string ;
  skos:prefLabel "MD_ReferenceSystemTypeCode - ConceptScheme" ;
.
<http://def.isotc211.org/iso19115/-1/2014/ReferenceSystemInformation/code/MD_ReferenceSystemTypeCode/compoundEngineeringParametric>
  rdf:type iso19115-1:MD_ReferenceSystemTypeCode ;
  rdf:type skos:Concept ;
  dct:description """compound spatio-parametric coordinate reference system containing an engineering coordinate reference system and a parametric reference system 

EXAMPLE [local] x, y, pressure"""^^xsd:string ;
  rdfs:isDefinedBy <http://standards.iso.org/iso/19115/-1/ed-1/en/> ;
  rdfs:label "compound Engineering Parametric" ;
  skos:definition """compound spatio-parametric coordinate reference system containing an engineering coordinate reference system and a parametric reference system 

EXAMPLE [local] x, y, pressure"""^^xsd:string ;
  skos:inScheme iso19115-1Code:MD_ReferenceSystemTypeCode ;
  skos:prefLabel "compoundEngineeringParametric" ;
.
<http://def.isotc211.org/iso19115/-1/2014/ReferenceSystemInformation/code/MD_ReferenceSystemTypeCode/compoundEngineeringParametricTemporal>
  rdf:type iso19115-1:MD_ReferenceSystemTypeCode ;
  rdf:type skos:Concept ;
  dct:description """compound spatio-parametric-temporal coordinate reference system containing an engineering, a parametric, and a temporal coordinate reference system 

EXAMPLE [local] x, y, pressure, time"""^^xsd:string ;
  rdfs:isDefinedBy <http://standards.iso.org/iso/19115/-1/ed-1/en/> ;
  rdfs:label "compound Engineering Parametric Temporal" ;
  skos:definition """compound spatio-parametric-temporal coordinate reference system containing an engineering, a parametric, and a temporal coordinate reference system 

EXAMPLE [local] x, y, pressure, time"""^^xsd:string ;
  skos:inScheme iso19115-1Code:MD_ReferenceSystemTypeCode ;
  skos:prefLabel "compoundEngineeringParametricTemporal" ;
.
<http://def.isotc211.org/iso19115/-1/2014/ReferenceSystemInformation/code/MD_ReferenceSystemTypeCode/compoundEngineeringTemporal>
  rdf:type iso19115-1:MD_ReferenceSystemTypeCode ;
  rdf:type skos:Concept ;
  dct:description """compound spatio-temporal coordinate reference system containing an engineering and a temporal coordinate reference system 

EXAMPLE [local] x, y, time"""^^xsd:string ;
  rdfs:isDefinedBy <http://standards.iso.org/iso/19115/-1/ed-1/en/> ;
  rdfs:label "compound Engineering Temporal" ;
  skos:definition """compound spatio-temporal coordinate reference system containing an engineering and a temporal coordinate reference system 

EXAMPLE [local] x, y, time"""^^xsd:string ;
  skos:inScheme iso19115-1Code:MD_ReferenceSystemTypeCode ;
  skos:prefLabel "compoundEngineeringTemporal" ;
.
<http://def.isotc211.org/iso19115/-1/2014/ReferenceSystemInformation/code/MD_ReferenceSystemTypeCode/compoundEngineeringVertical>
  rdf:type iso19115-1:MD_ReferenceSystemTypeCode ;
  rdf:type skos:Concept ;
  dct:description """compound spatial reference system containing a horizontal engineering coordinate reference system and a vertical coordinate reference system 

EXAMPLE [local] x, y, height"""^^xsd:string ;
  rdfs:isDefinedBy <http://standards.iso.org/iso/19115/-1/ed-1/en/> ;
  rdfs:label "compound Engineering Vertical" ;
  skos:definition """compound spatial reference system containing a horizontal engineering coordinate reference system and a vertical coordinate reference system 

EXAMPLE [local] x, y, height"""^^xsd:string ;
  skos:inScheme iso19115-1Code:MD_ReferenceSystemTypeCode ;
  skos:prefLabel "compoundEngineeringVertical" ;
.
<http://def.isotc211.org/iso19115/-1/2014/ReferenceSystemInformation/code/MD_ReferenceSystemTypeCode/compoundEngineeringVerticalTemporal>
  rdf:type iso19115-1:MD_ReferenceSystemTypeCode ;
  rdf:type skos:Concept ;
  dct:description """compound spatio-temporal coordinate reference system containing an engineering, a vertical, and a temporal coordinate reference system 

EXAMPLE [local] x, y, height, time"""^^xsd:string ;
  rdfs:isDefinedBy <http://standards.iso.org/iso/19115/-1/ed-1/en/> ;
  rdfs:label "compound Engineering Vertical Temporal" ;
  skos:definition """compound spatio-temporal coordinate reference system containing an engineering, a vertical, and a temporal coordinate reference system 

EXAMPLE [local] x, y, height, time"""^^xsd:string ;
  skos:inScheme iso19115-1Code:MD_ReferenceSystemTypeCode ;
  skos:prefLabel "compoundEngineeringVerticalTemporal" ;
.
<http://def.isotc211.org/iso19115/-1/2014/ReferenceSystemInformation/code/MD_ReferenceSystemTypeCode/compoundGeographic2DParametric>
  rdf:type iso19115-1:MD_ReferenceSystemTypeCode ;
  rdf:type skos:Concept ;
  dct:description """compound spatio-parametric coordinate reference system containing a 2 dimensional geographic horizontal coordinate reference system and a parametric reference system 

EXAMPLE latitude, longitude, pressure"""^^xsd:string ;
  rdfs:isDefinedBy <http://standards.iso.org/iso/19115/-1/ed-1/en/> ;
  rdfs:label "compound Geographic 2D Parametric" ;
  skos:definition """compound spatio-parametric coordinate reference system containing a 2 dimensional geographic horizontal coordinate reference system and a parametric reference system 

EXAMPLE latitude, longitude, pressure"""^^xsd:string ;
  skos:inScheme iso19115-1Code:MD_ReferenceSystemTypeCode ;
  skos:prefLabel "compoundGeographic2DParametric" ;
.
<http://def.isotc211.org/iso19115/-1/2014/ReferenceSystemInformation/code/MD_ReferenceSystemTypeCode/compoundGeographic2DParametricTemporal>
  rdf:type iso19115-1:MD_ReferenceSystemTypeCode ;
  rdf:type skos:Concept ;
  dct:description """compound spatio-parametric-temporal coordinate reference system containing a 2 dimensional geographic horizontal, a parametric and a temporal coordinate reference system 

EXAMPLE latitude, longitude, pressure, time"""^^xsd:string ;
  rdfs:isDefinedBy <http://standards.iso.org/iso/19115/-1/ed-1/en/> ;
  rdfs:label "compound Geographic 2D Parametric Temporal" ;
  skos:definition """compound spatio-parametric-temporal coordinate reference system containing a 2 dimensional geographic horizontal, a parametric and a temporal coordinate reference system 

EXAMPLE latitude, longitude, pressure, time"""^^xsd:string ;
  skos:inScheme iso19115-1Code:MD_ReferenceSystemTypeCode ;
  skos:prefLabel "compoundGeographic2DParametricTemporal" ;
.
<http://def.isotc211.org/iso19115/-1/2014/ReferenceSystemInformation/code/MD_ReferenceSystemTypeCode/compoundGeographic2DTemporal>
  rdf:type iso19115-1:MD_ReferenceSystemTypeCode ;
  rdf:type skos:Concept ;
  dct:description """compound spatio-temporal coordinate reference system containing a 2 dimensional geographic horizontal coordinate reference system and a temporal reference system 

EXAMPLE latitude, longitude, time"""^^xsd:string ;
  rdfs:isDefinedBy <http://standards.iso.org/iso/19115/-1/ed-1/en/> ;
  rdfs:label "compound Geographic 2D Temporal" ;
  skos:definition """compound spatio-temporal coordinate reference system containing a 2 dimensional geographic horizontal coordinate reference system and a temporal reference system 

EXAMPLE latitude, longitude, time"""^^xsd:string ;
  skos:inScheme iso19115-1Code:MD_ReferenceSystemTypeCode ;
  skos:prefLabel "compoundGeographic2DTemporal" ;
.
<http://def.isotc211.org/iso19115/-1/2014/ReferenceSystemInformation/code/MD_ReferenceSystemTypeCode/compoundGeographic2DVertical>
  rdf:type iso19115-1:MD_ReferenceSystemTypeCode ;
  rdf:type skos:Concept ;
  dct:description """compound coordinate reference system in which one constituent coordinate reference system is a horizontal geodetic coordinate reference system and one is a vertical coordinate reference system 

EXAMPLE latitude, longitude, [gravity-related] height or depth"""^^xsd:string ;
  rdfs:isDefinedBy <http://standards.iso.org/iso/19115/-1/ed-1/en/> ;
  rdfs:label "compound Geographic 2D Vertical" ;
  skos:definition """compound coordinate reference system in which one constituent coordinate reference system is a horizontal geodetic coordinate reference system and one is a vertical coordinate reference system 

EXAMPLE latitude, longitude, [gravity-related] height or depth"""^^xsd:string ;
  skos:inScheme iso19115-1Code:MD_ReferenceSystemTypeCode ;
  skos:prefLabel "compoundGeographic2DVertical" ;
.
<http://def.isotc211.org/iso19115/-1/2014/ReferenceSystemInformation/code/MD_ReferenceSystemTypeCode/compoundGeographic2DVerticalTemporal>
  rdf:type iso19115-1:MD_ReferenceSystemTypeCode ;
  rdf:type skos:Concept ;
  dct:description """compound spatio-temporal coordinate reference system containing a 2 dimensional geographic horizontal, a vertical, and a temporal coordinate reference system 

EXAMPLE latitude, longitude, height, time"""^^xsd:string ;
  rdfs:isDefinedBy <http://standards.iso.org/iso/19115/-1/ed-1/en/> ;
  rdfs:label "compound Geographic 2D Vertical Temporal" ;
  skos:definition """compound spatio-temporal coordinate reference system containing a 2 dimensional geographic horizontal, a vertical, and a temporal coordinate reference system 

EXAMPLE latitude, longitude, height, time"""^^xsd:string ;
  skos:inScheme iso19115-1Code:MD_ReferenceSystemTypeCode ;
  skos:prefLabel "compoundGeographic2DVerticalTemporal" ;
.
<http://def.isotc211.org/iso19115/-1/2014/ReferenceSystemInformation/code/MD_ReferenceSystemTypeCode/compoundGeographic3DTemporal>
  rdf:type iso19115-1:MD_ReferenceSystemTypeCode ;
  rdf:type skos:Concept ;
  dct:description """compound spatio-temporal coordinate reference system containing a 3 dimensional geographic and a temporal coordinate reference system 

EXAMPLE latitude, longitude, ellipsoidal height, time"""^^xsd:string ;
  rdfs:isDefinedBy <http://standards.iso.org/iso/19115/-1/ed-1/en/> ;
  rdfs:label "compound Geographic 3D Temporal" ;
  skos:definition """compound spatio-temporal coordinate reference system containing a 3 dimensional geographic and a temporal coordinate reference system 

EXAMPLE latitude, longitude, ellipsoidal height, time"""^^xsd:string ;
  skos:inScheme iso19115-1Code:MD_ReferenceSystemTypeCode ;
  skos:prefLabel "compoundGeographic3DTemporal" ;
.
<http://def.isotc211.org/iso19115/-1/2014/ReferenceSystemInformation/code/MD_ReferenceSystemTypeCode/compoundProjected2DParametric>
  rdf:type iso19115-1:MD_ReferenceSystemTypeCode ;
  rdf:type skos:Concept ;
  dct:description """compound spatio-parametric coordinate reference system containing a projected horizontal coordinate reference system and a parametric reference system 

EXAMPLE easting, northing, density"""^^xsd:string ;
  rdfs:isDefinedBy <http://standards.iso.org/iso/19115/-1/ed-1/en/> ;
  rdfs:label "compound Projected 2D Parametric" ;
  skos:definition """compound spatio-parametric coordinate reference system containing a projected horizontal coordinate reference system and a parametric reference system 

EXAMPLE easting, northing, density"""^^xsd:string ;
  skos:inScheme iso19115-1Code:MD_ReferenceSystemTypeCode ;
  skos:prefLabel "compoundProjected2DParametric" ;
.
<http://def.isotc211.org/iso19115/-1/2014/ReferenceSystemInformation/code/MD_ReferenceSystemTypeCode/compoundProjected2DParametricTemporal>
  rdf:type iso19115-1:MD_ReferenceSystemTypeCode ;
  rdf:type skos:Concept ;
  dct:description """compound spatio-parametric-temporal coordinate reference system containing a projected horizontal, a parametric, and a temporal coordinate reference system 

EXAMPLE easting, northing, density, time"""^^xsd:string ;
  rdfs:isDefinedBy <http://standards.iso.org/iso/19115/-1/ed-1/en/> ;
  rdfs:label "compound Projected 2D Parametric Temporal" ;
  skos:definition """compound spatio-parametric-temporal coordinate reference system containing a projected horizontal, a parametric, and a temporal coordinate reference system 

EXAMPLE easting, northing, density, time"""^^xsd:string ;
  skos:inScheme iso19115-1Code:MD_ReferenceSystemTypeCode ;
  skos:prefLabel "compoundProjected2DParametricTemporal" ;
.
<http://def.isotc211.org/iso19115/-1/2014/ReferenceSystemInformation/code/MD_ReferenceSystemTypeCode/compoundProjectedTemporal>
  rdf:type iso19115-1:MD_ReferenceSystemTypeCode ;
  rdf:type skos:Concept ;
  dct:description """compound spatio-temporal coordinate reference system containing a projected horizontal and a temporal coordinate reference system 

EXAMPLE easting, northing, time"""^^xsd:string ;
  rdfs:isDefinedBy <http://standards.iso.org/iso/19115/-1/ed-1/en/> ;
  rdfs:label "compound Projected Temporal" ;
  skos:definition """compound spatio-temporal coordinate reference system containing a projected horizontal and a temporal coordinate reference system 

EXAMPLE easting, northing, time"""^^xsd:string ;
  skos:inScheme iso19115-1Code:MD_ReferenceSystemTypeCode ;
  skos:prefLabel "compoundProjectedTemporal" ;
.
<http://def.isotc211.org/iso19115/-1/2014/ReferenceSystemInformation/code/MD_ReferenceSystemTypeCode/compoundProjectedVertical>
  rdf:type iso19115-1:MD_ReferenceSystemTypeCode ;
  rdf:type skos:Concept ;
  dct:description """compound spatial reference system containing a horizontal projected coordinate reference system and a vertical coordinate reference system 

EXAMPLE easting, northing, [gravity-related] height or depth"""^^xsd:string ;
  rdfs:isDefinedBy <http://standards.iso.org/iso/19115/-1/ed-1/en/> ;
  rdfs:label "compound Projected Vertical" ;
  skos:definition """compound spatial reference system containing a horizontal projected coordinate reference system and a vertical coordinate reference system 

EXAMPLE easting, northing, [gravity-related] height or depth"""^^xsd:string ;
  skos:inScheme iso19115-1Code:MD_ReferenceSystemTypeCode ;
  skos:prefLabel "compoundProjectedVertical" ;
.
<http://def.isotc211.org/iso19115/-1/2014/ReferenceSystemInformation/code/MD_ReferenceSystemTypeCode/compoundProjectedVerticalTemporal>
  rdf:type iso19115-1:MD_ReferenceSystemTypeCode ;
  rdf:type skos:Concept ;
  dct:description """compound spatio-temporal coordinate reference system containing a projected horizontal, a vertical, and a temporal coordinate reference system 

EXAMPLE easting, northing, height, time"""^^xsd:string ;
  rdfs:isDefinedBy <http://standards.iso.org/iso/19115/-1/ed-1/en/> ;
  rdfs:label "compound Projected Vertical Temporal" ;
  skos:definition """compound spatio-temporal coordinate reference system containing a projected horizontal, a vertical, and a temporal coordinate reference system 

EXAMPLE easting, northing, height, time"""^^xsd:string ;
  skos:inScheme iso19115-1Code:MD_ReferenceSystemTypeCode ;
  skos:prefLabel "compoundProjectedVerticalTemporal" ;
.
<http://def.isotc211.org/iso19115/-1/2014/ReferenceSystemInformation/code/MD_ReferenceSystemTypeCode/engineering>
  rdf:type iso19115-1:MD_ReferenceSystemTypeCode ;
  rdf:type skos:Concept ;
  dct:description """coordinate reference system based on an engineering datum (datum describing the relationship of a coordinate system to a local reference) 

EXAMPLE [local] x,y"""^^xsd:string ;
  rdfs:isDefinedBy <http://standards.iso.org/iso/19115/-1/ed-1/en/> ;
  rdfs:label "engineering" ;
  skos:definition """coordinate reference system based on an engineering datum (datum describing the relationship of a coordinate system to a local reference) 

EXAMPLE [local] x,y"""^^xsd:string ;
  skos:inScheme iso19115-1Code:MD_ReferenceSystemTypeCode ;
  skos:prefLabel "engineering" ;
.
<http://def.isotc211.org/iso19115/-1/2014/ReferenceSystemInformation/code/MD_ReferenceSystemTypeCode/engineeringDesign>
  rdf:type iso19115-1:MD_ReferenceSystemTypeCode ;
  rdf:type skos:Concept ;
  dct:description """engineering coordinate reference system in which the base representation of a moving object is specified 

EXAMPLE [local] x,y"""^^xsd:string ;
  rdfs:isDefinedBy <http://standards.iso.org/iso/19115/-1/ed-1/en/> ;
  rdfs:label "engineering Design" ;
  skos:definition """engineering coordinate reference system in which the base representation of a moving object is specified 

EXAMPLE [local] x,y"""^^xsd:string ;
  skos:inScheme iso19115-1Code:MD_ReferenceSystemTypeCode ;
  skos:prefLabel "engineeringDesign" ;
.
<http://def.isotc211.org/iso19115/-1/2014/ReferenceSystemInformation/code/MD_ReferenceSystemTypeCode/engineeringImage>
  rdf:type iso19115-1:MD_ReferenceSystemTypeCode ;
  rdf:type skos:Concept ;
  dct:description """coordinate reference system based on an image datum (engineering datum which defines the relationship of a coordinate system to an image) 

EXAMPLE row, column"""^^xsd:string ;
  rdfs:isDefinedBy <http://standards.iso.org/iso/19115/-1/ed-1/en/> ;
  rdfs:label "engineering Image" ;
  skos:definition """coordinate reference system based on an image datum (engineering datum which defines the relationship of a coordinate system to an image) 

EXAMPLE row, column"""^^xsd:string ;
  skos:inScheme iso19115-1Code:MD_ReferenceSystemTypeCode ;
  skos:prefLabel "engineeringImage" ;
.
<http://def.isotc211.org/iso19115/-1/2014/ReferenceSystemInformation/code/MD_ReferenceSystemTypeCode/geodeticGeocentric>
  rdf:type iso19115-1:MD_ReferenceSystemTypeCode ;
  rdf:type skos:Concept ;
  dct:description """geodetic CRS having a Cartesian 3D coordinate system 

EXAMPLE [geocentric] X,Y,Z"""^^xsd:string ;
  rdfs:isDefinedBy <http://standards.iso.org/iso/19115/-1/ed-1/en/> ;
  rdfs:label "geodetic Geocentric" ;
  skos:definition """geodetic CRS having a Cartesian 3D coordinate system 

EXAMPLE [geocentric] X,Y,Z"""^^xsd:string ;
  skos:inScheme iso19115-1Code:MD_ReferenceSystemTypeCode ;
  skos:prefLabel "geodeticGeocentric" ;
.
<http://def.isotc211.org/iso19115/-1/2014/ReferenceSystemInformation/code/MD_ReferenceSystemTypeCode/geodeticGeographic2D>
  rdf:type iso19115-1:MD_ReferenceSystemTypeCode ;
  rdf:type skos:Concept ;
  dct:description """geodetic CRS having an ellipsoidal 2D coordinate system 

EXAMPLE latitude, longitude"""^^xsd:string ;
  rdfs:isDefinedBy <http://standards.iso.org/iso/19115/-1/ed-1/en/> ;
  rdfs:label "geodetic Geographic 2D" ;
  skos:definition """geodetic CRS having an ellipsoidal 2D coordinate system 

EXAMPLE latitude, longitude"""^^xsd:string ;
  skos:inScheme iso19115-1Code:MD_ReferenceSystemTypeCode ;
  skos:prefLabel "geodeticGeographic2D" ;
.
<http://def.isotc211.org/iso19115/-1/2014/ReferenceSystemInformation/code/MD_ReferenceSystemTypeCode/geodeticGeographic3D>
  rdf:type iso19115-1:MD_ReferenceSystemTypeCode ;
  rdf:type skos:Concept ;
  dct:description """geodetic CRS having an ellipsoidal 3D coordinate system 

EXAMPLE latitude, longitude, ellipsoidal height"""^^xsd:string ;
  rdfs:isDefinedBy <http://standards.iso.org/iso/19115/-1/ed-1/en/> ;
  rdfs:label "geodetic Geographic 3D" ;
  skos:definition """geodetic CRS having an ellipsoidal 3D coordinate system 

EXAMPLE latitude, longitude, ellipsoidal height"""^^xsd:string ;
  skos:inScheme iso19115-1Code:MD_ReferenceSystemTypeCode ;
  skos:prefLabel "geodeticGeographic3D" ;
.
<http://def.isotc211.org/iso19115/-1/2014/ReferenceSystemInformation/code/MD_ReferenceSystemTypeCode/geographicIdentifier>
  rdf:type iso19115-1:MD_ReferenceSystemTypeCode ;
  rdf:type skos:Concept ;
  dct:description """spatial reference in the form of a label or code that identifies a location 

EXAMPLE post code"""^^xsd:string ;
  rdfs:isDefinedBy <http://standards.iso.org/iso/19115/-1/ed-1/en/> ;
  rdfs:label "geographic Identifier" ;
  skos:definition """spatial reference in the form of a label or code that identifies a location 

EXAMPLE post code"""^^xsd:string ;
  skos:inScheme iso19115-1Code:MD_ReferenceSystemTypeCode ;
  skos:prefLabel "geographicIdentifier" ;
.
<http://def.isotc211.org/iso19115/-1/2014/ReferenceSystemInformation/code/MD_ReferenceSystemTypeCode/linear>
  rdf:type iso19115-1:MD_ReferenceSystemTypeCode ;
  rdf:type skos:Concept ;
  dct:description """reference system that identifies a location by reference to a segment of a linear geographic feature and distance along that segment from a given point 

EXAMPLE x km along road"""^^xsd:string ;
  rdfs:isDefinedBy <http://standards.iso.org/iso/19115/-1/ed-1/en/> ;
  rdfs:label "linear" ;
  skos:definition """reference system that identifies a location by reference to a segment of a linear geographic feature and distance along that segment from a given point 

EXAMPLE x km along road"""^^xsd:string ;
  skos:inScheme iso19115-1Code:MD_ReferenceSystemTypeCode ;
  skos:prefLabel "linear" ;
.
<http://def.isotc211.org/iso19115/-1/2014/ReferenceSystemInformation/code/MD_ReferenceSystemTypeCode/parametric>
  rdf:type iso19115-1:MD_ReferenceSystemTypeCode ;
  rdf:type skos:Concept ;
  dct:description """coordinate reference system based on a parametric datum (datum describing the relationship of a parametric coordinate system to an object) 

EXAMPLE pressure"""^^xsd:string ;
  rdfs:isDefinedBy <http://standards.iso.org/iso/19115/-1/ed-1/en/> ;
  rdfs:label "parametric" ;
  skos:definition """coordinate reference system based on a parametric datum (datum describing the relationship of a parametric coordinate system to an object) 

EXAMPLE pressure"""^^xsd:string ;
  skos:inScheme iso19115-1Code:MD_ReferenceSystemTypeCode ;
  skos:prefLabel "parametric" ;
.
<http://def.isotc211.org/iso19115/-1/2014/ReferenceSystemInformation/code/MD_ReferenceSystemTypeCode/projected>
  rdf:type iso19115-1:MD_ReferenceSystemTypeCode ;
  rdf:type skos:Concept ;
  dct:description """coordinate reference system derived from a two-dimensional geodetic coordinate reference system by applying a map projection 

EXAMPLE easting, northing"""^^xsd:string ;
  rdfs:isDefinedBy <http://standards.iso.org/iso/19115/-1/ed-1/en/> ;
  rdfs:label "projected" ;
  skos:definition """coordinate reference system derived from a two-dimensional geodetic coordinate reference system by applying a map projection 

EXAMPLE easting, northing"""^^xsd:string ;
  skos:inScheme iso19115-1Code:MD_ReferenceSystemTypeCode ;
  skos:prefLabel "projected" ;
.
<http://def.isotc211.org/iso19115/-1/2014/ReferenceSystemInformation/code/MD_ReferenceSystemTypeCode/temporal>
  rdf:type iso19115-1:MD_ReferenceSystemTypeCode ;
  rdf:type skos:Concept ;
  dct:description """reference system against which time is measured 

EXAMPLE time"""^^xsd:string ;
  rdfs:isDefinedBy <http://standards.iso.org/iso/19115/-1/ed-1/en/> ;
  rdfs:label "temporal" ;
  skos:definition """reference system against which time is measured 

EXAMPLE time"""^^xsd:string ;
  skos:inScheme iso19115-1Code:MD_ReferenceSystemTypeCode ;
  skos:prefLabel "temporal" ;
.
<http://def.isotc211.org/iso19115/-1/2014/ReferenceSystemInformation/code/MD_ReferenceSystemTypeCode/vertical>
  rdf:type iso19115-1:MD_ReferenceSystemTypeCode ;
  rdf:type skos:Concept ;
  dct:description """one-dimensional coordinate reference system based on a vertical datum (datum describing the relation of gravity-related heights or depths to the Earth) 

EXAMPLE [gravity-related] height or depth"""^^xsd:string ;
  rdfs:isDefinedBy <http://standards.iso.org/iso/19115/-1/ed-1/en/> ;
  rdfs:label "vertical" ;
  skos:definition """one-dimensional coordinate reference system based on a vertical datum (datum describing the relation of gravity-related heights or depths to the Earth) 

EXAMPLE [gravity-related] height or depth"""^^xsd:string ;
  skos:inScheme iso19115-1Code:MD_ReferenceSystemTypeCode ;
  skos:prefLabel "vertical" ;
.
iso19115-1Code:MD_ReferenceSystemTypeCodeCollection
  rdf:type skos:Collection ;
  skos:members (
      [
        rdf:type skos:Concept ;
      ]
      [
        rdf:type skos:Concept ;
      ]
      [
        rdf:type skos:Concept ;
      ]
      [
        rdf:type skos:Concept ;
      ]
      [
        rdf:type skos:Concept ;
      ]
      [
        rdf:type skos:Concept ;
      ]
      [
        rdf:type skos:Concept ;
      ]
      [
        rdf:type skos:Concept ;
      ]
      [
        rdf:type skos:Concept ;
      ]
      [
        rdf:type skos:Concept ;
      ]
      [
        rdf:type skos:Concept ;
      ]
      [
        rdf:type skos:Concept ;
      ]
      [
        rdf:type skos:Concept ;
      ]
      [
        rdf:type skos:Concept ;
      ]
      [
        rdf:type skos:Concept ;
      ]
      [
        rdf:type skos:Concept ;
      ]
      [
        rdf:type skos:Concept ;
      ]
      [
        rdf:type skos:Concept ;
      ]
      [
        rdf:type skos:Concept ;
      ]
      [
        rdf:type skos:Concept ;
      ]
      [
        rdf:type skos:Concept ;
      ]
      [
        rdf:type skos:Concept ;
      ]
      [
        rdf:type skos:Concept ;
      ]
      [
        rdf:type skos:Concept ;
      ]
      [
        rdf:type skos:Concept ;
      ]
      [
        rdf:type skos:Concept ;
      ]
      [
        rdf:type skos:Concept ;
      ]
      [
        rdf:type skos:Concept ;
      ]
    ) ;
  skos:prefLabel "MD_ReferenceSystemTypeCode - Collection" ;
.
