<?xml version="1.0"?>

<!DOCTYPE rdf:RDF [
  <!ENTITY owl "http://www.w3.org/2002/07/owl#" >
  <!ENTITY xsd "http://www.w3.org/2001/XMLSchema#" >
  <!ENTITY rdfs "http://www.w3.org/2000/01/rdf-schema#" >
  <!ENTITY rdf "http://www.w3.org/1999/02/22-rdf-syntax-ns#" >
  <!ENTITY dc "http://purl.org/dc/elements/1.1/" >
  <!ENTITY dct "http://purl.org/dc/terms/" >
  <!ENTITY skos "http://www.w3.org/2004/02/skos/core#" >
  <!ENTITY iso19150-2 "http://def.isotc211.org/iso19150/-2/2012/base#" >
  <!ENTITY iso19103_333 "http://def.isotc211.org/iso19103/2005/UnitsOfMeasure#" >
  <!ENTITY iso19103_342 "http://def.isotc211.org/iso19103/2005/Numerics#" >
  <!ENTITY iso19133_1920 "http://def.isotc211.org/iso19133/2005/CostFunction#" >
  <!ENTITY iso19134 "http://def.isotc211.org/iso19134/2007/MultimodalCostFunction#" >
  <!ENTITY iso19134Code "http://def.isotc211.org/iso19134/2007/MultimodalCostFunction/code/">

]>

  <!--+++++++++++++++++++++++++++++++++++++++++++++++++++++++-->
  <!-- File name:         iso19134MultimodalCostFunction.rdf -->
  <!-- Generator:         GOM_Technologies::UML2OWL          -->
  <!-- Generator version: 2.5                                -->
  <!-- File date:         18-11-2016                         -->
  <!--+++++++++++++++++++++++++++++++++++++++++++++++++++++++-->

<rdf:RDF xmlns="http://def.isotc211.org/iso19134/2007/MultimodalCostFunction#"
  xml:base="http://def.isotc211.org/iso19134/2007/MultimodalCostFunction"
  xmlns:owl="http://www.w3.org/2002/07/owl#"
  xmlns:xsd="http://www.w3.org/2001/XMLSchema#"
  xmlns:rdfs="http://www.w3.org/2000/01/rdf-schema#"
  xmlns:rdf="http://www.w3.org/1999/02/22-rdf-syntax-ns#"
  xmlns:dc="http://purl.org/dc/elements/1.1/"
  xmlns:dct="http://purl.org/dc/terms/"
  xmlns:skos="http://www.w3.org/2004/02/skos/core#"
  xmlns:iso19150-2="http://def.isotc211.org/iso19150/-2/2012/base#"
  xmlns:iso19103_333="http://def.isotc211.org/iso19103/2005/UnitsOfMeasure#"
  xmlns:iso19103_342="http://def.isotc211.org/iso19103/2005/Numerics#"
  xmlns:iso19133_1920="http://def.isotc211.org/iso19133/2005/CostFunction#"
  xmlns:iso19134="http://def.isotc211.org/iso19134/2007/MultimodalCostFunction#"
  xmlns:iso19134Code="http://def.isotc211.org/iso19134/2007/MultimodalCostFunction/code/">

  <!--+++++++++++++++++++++++++++++++++++++++++++++++++++-->
  <!-- Ontology: ISO 19134:2007 Multimodal Cost Function -->
  <!--+++++++++++++++++++++++++++++++++++++++++++++++++++-->
  <owl:Ontology rdf:about="http://def.isotc211.org/iso19134/2007/MultimodalCostFunction">
    <rdfs:label>ISO 19134:2007 Multimodal Cost Function</rdfs:label>
    <dct:source>http://standards.iso.org/iso/19134/ed-1/en/</dct:source>
    <owl:versionInfo>2007-02-01</owl:versionInfo>
    <!--owl:imports rdf:resource="http://def.isotc211.org/iso19103/2005/UnitsOfMeasure"/-->
    <!--owl:imports rdf:resource="http://def.isotc211.org/iso19103/2005/Numerics"/-->
    <!--owl:imports rdf:resource="http://def.isotc211.org/iso19133/2005/CostFunction"/-->
    <owl:imports rdf:resource="http://def.isotc211.org/iso19150/-2/2012/base"/>
  </owl:Ontology>

  <!--+++++++++++++++++++++++-->
  <!-- Class: MN_CostElement -->
  <!--+++++++++++++++++++++++-->
  <owl:Class rdf:about="&iso19134;MN_CostElement">
    <rdfs:label>MN_CostElement</rdfs:label>
    <skos:definition>The data type .gu.MN_CostElement.gu. is the root of the collection of data types used to define cost functions.  MN_CostElement is a variant type of NS_CostElement in ISO 19133. </skos:definition>
    <rdfs:isDefinedBy>http://standards.iso.org/iso/19134/ed-1/en/</rdfs:isDefinedBy>
    <rdfs:subClassOf rdf:resource="&iso19134;MN_CostFunction"/>
  </owl:Class>

  <!--++++++++++++++++++++++++-->
  <!-- Class: MN_CostFunction -->
  <!--++++++++++++++++++++++++-->
  <owl:Class rdf:about="&iso19134;MN_CostFunction">
    <rdfs:label>MN_CostFunction</rdfs:label>
    <skos:definition>The data type .gu.MN_CostFunction.gu. is a variant subtype of .gu.NS_CostFunction.gu. in ISO 19133. </skos:definition>
    <rdfs:isDefinedBy>http://standards.iso.org/iso/19134/ed-1/en/</rdfs:isDefinedBy>
    <rdfs:subClassOf rdf:resource="&iso19133_1920;NS_CostFunction"/>
  </owl:Class>

  <!--++++++++++++++++++-->
  <!-- Class: MN_Counts -->
  <!--++++++++++++++++++-->
  <owl:Class rdf:about="&iso19134;MN_Counts">
    <rdfs:label>MN_Counts</rdfs:label>
    <skos:definition>The data type .gu.MN_ Counts.gu. is the root class for all types that have a count-valued cost.</skos:definition>
    <rdfs:isDefinedBy>http://standards.iso.org/iso/19134/ed-1/en/</rdfs:isDefinedBy>
    <rdfs:subClassOf rdf:resource="&iso19134;MN_CostElement"/>
  </owl:Class>

  <!--++++++++++++++++++++-->
  <!-- Class: MN_Distance -->
  <!--++++++++++++++++++++-->
  <owl:Class rdf:about="&iso19134;MN_Distance">
    <rdfs:label>MN_Distance</rdfs:label>
    <skos:definition>The data type .gu.MN_ Distance.gu. is the root class for all types that have a distance-valued cost. </skos:definition>
    <rdfs:isDefinedBy>http://standards.iso.org/iso/19134/ed-1/en/</rdfs:isDefinedBy>
    <rdfs:subClassOf rdf:resource="&iso19134;MN_CostElement"/>
  </owl:Class>

  <!--+++++++++++++++++-->
  <!-- Class: MN_Fares -->
  <!--+++++++++++++++++-->
  <owl:Class rdf:about="&iso19134;MN_Fares">
    <rdfs:label>MN_Fares</rdfs:label>
    <skos:definition>The data type .gu.MN_Fares.gu. is used for describing monetary cost arising from out-of-pocket costs for travel. </skos:definition>
    <rdfs:isDefinedBy>http://standards.iso.org/iso/19134/ed-1/en/</rdfs:isDefinedBy>
    <rdfs:subClassOf rdf:resource="&iso19134;MN_MonetaryCost"/>
  </owl:Class>

  <!--++++++++++++++++++++++++-->
  <!-- Class: MN_MonetaryCost -->
  <!--++++++++++++++++++++++++-->
  <owl:Class rdf:about="&iso19134;MN_MonetaryCost">
    <rdfs:label>MN_MonetaryCost</rdfs:label>
    <skos:definition>The data type .gu.MN_MonetaryCost.gu. is the root class for all types that have a monetary-valued cost.</skos:definition>
    <rdfs:isDefinedBy>http://standards.iso.org/iso/19134/ed-1/en/</rdfs:isDefinedBy>
    <rdfs:subClassOf rdf:resource="&iso19134;MN_CostElement"/>
  </owl:Class>

  <!--+++++++++++++++++++++++++++++-->
  <!-- Class: MN_NumberOfTransfers -->
  <!--+++++++++++++++++++++++++++++-->
  <owl:Class rdf:about="&iso19134;MN_NumberOfTransfers">
    <rdfs:label>MN_NumberOfTransfers</rdfs:label>
    <skos:definition>The data type .gu.MN_NumberOfTransfer.gu. is the cost element used for counting modal transfers. </skos:definition>
    <rdfs:isDefinedBy>http://standards.iso.org/iso/19134/ed-1/en/</rdfs:isDefinedBy>
    <rdfs:subClassOf rdf:resource="&iso19134;MN_Counts"/>
  </owl:Class>

  <!--++++++++++++++++-->
  <!-- Class: MN_Time -->
  <!--++++++++++++++++-->
  <owl:Class rdf:about="&iso19134;MN_Time">
    <rdfs:label>MN_Time</rdfs:label>
    <skos:definition>The data type .gu.MN_Time.gu. is the root class for all types that have a time-valued cost. </skos:definition>
    <rdfs:isDefinedBy>http://standards.iso.org/iso/19134/ed-1/en/</rdfs:isDefinedBy>
    <rdfs:subClassOf rdf:resource="&iso19134;MN_CostElement"/>
  </owl:Class>

  <!--+++++++++++++++++++++-->
  <!-- Class: MN_TotalCost -->
  <!--+++++++++++++++++++++-->
  <owl:Class rdf:about="&iso19134;MN_TotalCost">
    <rdfs:label>MN_TotalCost</rdfs:label>
    <skos:definition>The data type .gu.MN_TotalCost.gu. is used for describing monetary cost arising from total travel activities.  For example, the total cost is composed of time, distance, out-of-pocket costs including parking fees, and cost related to waypoint activities such as shopping. Detailed explanation for MN_TotalCost can be found in Annex B. </skos:definition>
    <rdfs:isDefinedBy>http://standards.iso.org/iso/19134/ed-1/en/</rdfs:isDefinedBy>
    <rdfs:subClassOf rdf:resource="&iso19134;MN_MonetaryCost"/>
  </owl:Class>

  <!--++++++++++++++++++++++-->
  <!-- Class: MN_TravelTime -->
  <!--++++++++++++++++++++++-->
  <owl:Class rdf:about="&iso19134;MN_TravelTime">
    <rdfs:label>MN_TravelTime</rdfs:label>
    <skos:definition>The data type .gu.MN_TravelTime.gu. is used for describing cost arising from line-haul travel time along the multimodal route. </skos:definition>
    <rdfs:isDefinedBy>http://standards.iso.org/iso/19134/ed-1/en/</rdfs:isDefinedBy>
    <rdfs:subClassOf rdf:resource="&iso19134;MN_Time"/>
  </owl:Class>

  <!--+++++++++++++++++++++++-->
  <!-- Class: MN_WaitingTime -->
  <!--+++++++++++++++++++++++-->
  <owl:Class rdf:about="&iso19134;MN_WaitingTime">
    <rdfs:label>MN_WaitingTime</rdfs:label>
    <skos:definition>The data type .gu.MN_WaitingTime.gu. is used for describing cost arising from waiting time at transfer points along the multimodal route.  </skos:definition>
    <rdfs:isDefinedBy>http://standards.iso.org/iso/19134/ed-1/en/</rdfs:isDefinedBy>
    <rdfs:subClassOf rdf:resource="&iso19134;MN_Time"/>
  </owl:Class>

  <!--+++++++++++++++++++++++++-->
  <!-- Class: MN_WayPointsCost -->
  <!--+++++++++++++++++++++++++-->
  <owl:Class rdf:about="&iso19134;MN_WayPointsCost">
    <rdfs:label>MN_WayPointsCost</rdfs:label>
    <skos:definition>The data type .gu.MN_WayPointsCost.gu. is used for describing monetary cost related to waypoint activities such as shopping. </skos:definition>
    <rdfs:isDefinedBy>http://standards.iso.org/iso/19134/ed-1/en/</rdfs:isDefinedBy>
    <rdfs:subClassOf rdf:resource="&iso19134;MN_MonetaryCost"/>
  </owl:Class>

  <!--++++++++++++++++++++++++-->
  <!-- Class: MN_WeightedCost -->
  <!--++++++++++++++++++++++++-->
  <owl:Class rdf:about="&iso19134;MN_WeightedCost">
    <rdfs:label>MN_WeightedCost</rdfs:label>
    <skos:definition>The type .gu.MN_WeightedCost.gu. is a cost function that is the sum of the numeric values of other cost functions with weights. MN_WeightedCost is a variant type of NS_WeightedCost in ISO 19133.</skos:definition>
    <rdfs:isDefinedBy>http://standards.iso.org/iso/19134/ed-1/en/</rdfs:isDefinedBy>
    <rdfs:subClassOf rdf:resource="&iso19134;MN_CostFunction"/>
    <rdfs:subClassOf>
      <owl:Restriction>
        <owl:onProperty rdf:resource="&iso19134;MN_WeightedCost.targetUnit"/>
        <owl:maxCardinality rdf:datatype="&xsd;nonNegativeInteger">1</owl:maxCardinality>
      </owl:Restriction>
    </rdfs:subClassOf>
    <rdfs:subClassOf>
      <owl:Restriction>
        <owl:onProperty rdf:resource="&iso19134;MN_WeightedCost.targetUnit"/>
        <owl:allValuesFrom rdf:resource="&iso19103_333;UnitOfMeasure"/>
      </owl:Restriction>
    </rdfs:subClassOf>
    <rdfs:subClassOf>
      <owl:Restriction>
        <owl:onProperty rdf:resource="&iso19134;MN_WeightedCost.term"/>
        <owl:minCardinality rdf:datatype="&xsd;nonNegativeInteger">1</owl:minCardinality>
      </owl:Restriction>
    </rdfs:subClassOf>
    <rdfs:subClassOf>
      <owl:Restriction>
        <owl:onProperty rdf:resource="&iso19134;MN_WeightedCost.term"/>
        <owl:allValuesFrom rdf:resource="&iso19134;MN_WeightedCostFunctionTerm"/>
      </owl:Restriction>
    </rdfs:subClassOf>
  </owl:Class>

  <!--++++++++++++++++++++++++++++++++++++-->
  <!-- Class: MN_WeightedCostFunctionTerm -->
  <!--++++++++++++++++++++++++++++++++++++-->
  <owl:Class rdf:about="&iso19134;MN_WeightedCostFunctionTerm">
    <rdfs:label>MN_WeightedCostFunctionTerm</rdfs:label>
    <skos:definition>The data type .gu.MN_WeightedCostFunctionTerm.gu. is a component of a cost function that is the sum of the numeric values of other cost functions with weights.</skos:definition>
    <rdfs:isDefinedBy>http://standards.iso.org/iso/19134/ed-1/en/</rdfs:isDefinedBy>
    <rdfs:subClassOf>
      <owl:Restriction>
        <owl:onProperty rdf:resource="&iso19134;MN_WeightedCostFunctionTerm.unit"/>
        <owl:cardinality rdf:datatype="&xsd;nonNegativeInteger">1</owl:cardinality>
      </owl:Restriction>
    </rdfs:subClassOf>
    <rdfs:subClassOf>
      <owl:Restriction>
        <owl:onProperty rdf:resource="&iso19134;MN_WeightedCostFunctionTerm.unit"/>
        <owl:allValuesFrom rdf:resource="&iso19103_333;UnitOfMeasure"/>
      </owl:Restriction>
    </rdfs:subClassOf>
    <rdfs:subClassOf>
      <owl:Restriction>
        <owl:onProperty rdf:resource="&iso19134;MN_WeightedCostFunctionTerm.type"/>
        <owl:cardinality rdf:datatype="&xsd;nonNegativeInteger">1</owl:cardinality>
      </owl:Restriction>
    </rdfs:subClassOf>
    <rdfs:subClassOf>
      <owl:Restriction>
        <owl:onProperty rdf:resource="&iso19134;MN_WeightedCostFunctionTerm.type"/>
        <owl:allValuesFrom rdf:resource="&iso19134;MN_CostType"/>
      </owl:Restriction>
    </rdfs:subClassOf>
    <rdfs:subClassOf>
      <owl:Restriction>
        <owl:onProperty rdf:resource="&iso19134;MN_WeightedCostFunctionTerm.weight"/>
        <owl:cardinality rdf:datatype="&xsd;nonNegativeInteger">1</owl:cardinality>
      </owl:Restriction>
    </rdfs:subClassOf>
    <rdfs:subClassOf>
      <owl:Restriction>
        <owl:onProperty rdf:resource="&iso19134;MN_WeightedCostFunctionTerm.weight"/>
        <owl:allValuesFrom rdf:resource="&iso19103_342;Number"/>
      </owl:Restriction>
    </rdfs:subClassOf>
  </owl:Class>

  <!--++++++++++++++++++++++++++++++++++++++++++++-->
  <!-- ObjectProperty: MN_WeightedCost.targetUnit -->
  <!--++++++++++++++++++++++++++++++++++++++++++++-->
  <owl:ObjectProperty rdf:about="&iso19134;MN_WeightedCost.targetUnit">
    <rdfs:label>targetUnit</rdfs:label>
    <rdfs:isDefinedBy>http://standards.iso.org/iso/19134/ed-1/en/</rdfs:isDefinedBy>
    <rdfs:domain rdf:resource="&iso19134;MN_WeightedCost"/>
    <rdfs:range rdf:resource="&iso19103_333;UnitOfMeasure"/>
  </owl:ObjectProperty>

  <!--++++++++++++++++++++++++++++++++++++++++++++++++++-->
  <!-- ObjectProperty: MN_WeightedCostFunctionTerm.unit -->
  <!--++++++++++++++++++++++++++++++++++++++++++++++++++-->
  <owl:ObjectProperty rdf:about="&iso19134;MN_WeightedCostFunctionTerm.unit">
    <rdfs:label>unit</rdfs:label>
    <rdfs:isDefinedBy>http://standards.iso.org/iso/19134/ed-1/en/</rdfs:isDefinedBy>
    <rdfs:domain rdf:resource="&iso19134;MN_WeightedCostFunctionTerm"/>
    <rdfs:range rdf:resource="&iso19103_333;UnitOfMeasure"/>
  </owl:ObjectProperty>

  <!--++++++++++++++++++++++++++++++++++++++++++++++++++-->
  <!-- ObjectProperty: MN_WeightedCostFunctionTerm.type -->
  <!--++++++++++++++++++++++++++++++++++++++++++++++++++-->
  <owl:ObjectProperty rdf:about="&iso19134;MN_WeightedCostFunctionTerm.type">
    <rdfs:label>type</rdfs:label>
    <rdfs:isDefinedBy>http://standards.iso.org/iso/19134/ed-1/en/</rdfs:isDefinedBy>
    <rdfs:domain rdf:resource="&iso19134;MN_WeightedCostFunctionTerm"/>
    <rdfs:range rdf:resource="&iso19134;MN_CostType"/>
  </owl:ObjectProperty>

  <!--++++++++++++++++++++++++++++++++++++++++++++++++++++-->
  <!-- ObjectProperty: MN_WeightedCostFunctionTerm.weight -->
  <!--++++++++++++++++++++++++++++++++++++++++++++++++++++-->
  <owl:ObjectProperty rdf:about="&iso19134;MN_WeightedCostFunctionTerm.weight">
    <rdfs:label>weight</rdfs:label>
    <rdfs:isDefinedBy>http://standards.iso.org/iso/19134/ed-1/en/</rdfs:isDefinedBy>
    <rdfs:domain rdf:resource="&iso19134;MN_WeightedCostFunctionTerm"/>
    <rdfs:range rdf:resource="&iso19103_342;Number"/>
  </owl:ObjectProperty>

  <!--++++++++++++++++++++++++++++++++++++++-->
  <!-- ObjectProperty: MN_WeightedCost.term -->
  <!--++++++++++++++++++++++++++++++++++++++-->
  <owl:ObjectProperty rdf:about="&iso19134;MN_WeightedCost.term">
    <rdfs:label>term</rdfs:label>
    <rdfs:isDefinedBy>http://standards.iso.org/iso/19134/ed-1/en/</rdfs:isDefinedBy>
    <iso19150-2:aggregationType>partOfCompositeAggregation</iso19150-2:aggregationType>
    <rdfs:domain rdf:resource="&iso19134;MN_WeightedCost"/>
    <rdfs:range rdf:resource="&iso19134;MN_WeightedCostFunctionTerm"/>
  </owl:ObjectProperty>

  <!--+++++++++++++++++++++++-->
  <!-- Codelist: MN_CostType -->
  <!--+++++++++++++++++++++++-->
  <owl:Class rdf:about="&iso19134;MN_CostType">
    <rdfs:label>MN_CostType</rdfs:label>
    <rdfs:isDefinedBy>http://standards.iso.org/iso/19134/ed-1/en/</rdfs:isDefinedBy>
    <rdfs:subClassOf rdf:resource="&skos;Concept"/>
  </owl:Class>
  <skos:ConceptScheme rdf:about="&iso19134Code;MN_CostType">
    <skos:prefLabel>MN_CostType - ConceptScheme</skos:prefLabel>
    <rdfs:isDefinedBy>http://standards.iso.org/iso/19134/ed-1/en/</rdfs:isDefinedBy>
    <dct:isFormatOf rdf:resource="&iso19134;MN_CostType"/>
  </skos:ConceptScheme>
  <iso19134:MN_CostType rdf:about="&iso19134Code;MN_CostType/waitingTime">
    <rdf:type rdf:resource="&skos;Concept"/>
    <skos:prefLabel>waitingTime</skos:prefLabel>
    <skos:inScheme rdf:resource="&iso19134Code;MN_CostType"/>
    <rdfs:isDefinedBy>http://standards.iso.org/iso/19134/ed-1/en/</rdfs:isDefinedBy>
  </iso19134:MN_CostType>
  <iso19134:MN_CostType rdf:about="&iso19134Code;MN_CostType/travelTime">
    <rdf:type rdf:resource="&skos;Concept"/>
    <skos:prefLabel>travelTime</skos:prefLabel>
    <skos:inScheme rdf:resource="&iso19134Code;MN_CostType"/>
    <rdfs:isDefinedBy>http://standards.iso.org/iso/19134/ed-1/en/</rdfs:isDefinedBy>
  </iso19134:MN_CostType>
  <iso19134:MN_CostType rdf:about="&iso19134Code;MN_CostType/totalCost">
    <rdf:type rdf:resource="&skos;Concept"/>
    <skos:prefLabel>totalCost</skos:prefLabel>
    <skos:inScheme rdf:resource="&iso19134Code;MN_CostType"/>
    <rdfs:isDefinedBy>http://standards.iso.org/iso/19134/ed-1/en/</rdfs:isDefinedBy>
  </iso19134:MN_CostType>
  <iso19134:MN_CostType rdf:about="&iso19134Code;MN_CostType/fares">
    <rdf:type rdf:resource="&skos;Concept"/>
    <skos:prefLabel>fares</skos:prefLabel>
    <skos:inScheme rdf:resource="&iso19134Code;MN_CostType"/>
    <rdfs:isDefinedBy>http://standards.iso.org/iso/19134/ed-1/en/</rdfs:isDefinedBy>
  </iso19134:MN_CostType>
  <iso19134:MN_CostType rdf:about="&iso19134Code;MN_CostType/wayPointsCost">
    <rdf:type rdf:resource="&skos;Concept"/>
    <skos:prefLabel>wayPointsCost</skos:prefLabel>
    <skos:inScheme rdf:resource="&iso19134Code;MN_CostType"/>
    <rdfs:isDefinedBy>http://standards.iso.org/iso/19134/ed-1/en/</rdfs:isDefinedBy>
  </iso19134:MN_CostType>
  <iso19134:MN_CostType rdf:about="&iso19134Code;MN_CostType/numberOfTransfers">
    <rdf:type rdf:resource="&skos;Concept"/>
    <skos:prefLabel>numberOfTransfers</skos:prefLabel>
    <skos:inScheme rdf:resource="&iso19134Code;MN_CostType"/>
    <rdfs:isDefinedBy>http://standards.iso.org/iso/19134/ed-1/en/</rdfs:isDefinedBy>
  </iso19134:MN_CostType>
  <iso19134:MN_CostType rdf:about="&iso19134Code;MN_CostType/distance">
    <rdf:type rdf:resource="&skos;Concept"/>
    <skos:prefLabel>distance</skos:prefLabel>
    <skos:inScheme rdf:resource="&iso19134Code;MN_CostType"/>
    <rdfs:isDefinedBy>http://standards.iso.org/iso/19134/ed-1/en/</rdfs:isDefinedBy>
  </iso19134:MN_CostType>
  <skos:Collection rdf:about="&iso19134Code;MN_CostTypeCollection">
    <skos:prefLabel>MN_CostType - Collection</skos:prefLabel>
    <skos:member rdf:resource="&iso19134Code;MN_CostType/waitingTime"/>
    <skos:member rdf:resource="&iso19134Code;MN_CostType/travelTime"/>
    <skos:member rdf:resource="&iso19134Code;MN_CostType/totalCost"/>
    <skos:member rdf:resource="&iso19134Code;MN_CostType/fares"/>
    <skos:member rdf:resource="&iso19134Code;MN_CostType/wayPointsCost"/>
    <skos:member rdf:resource="&iso19134Code;MN_CostType/numberOfTransfers"/>
    <skos:member rdf:resource="&iso19134Code;MN_CostType/distance"/>
  </skos:Collection>

</rdf:RDF>

