<?xml version="1.0"?>

<!DOCTYPE rdf:RDF [
  <!ENTITY owl "http://www.w3.org/2002/07/owl#" >
  <!ENTITY xsd "http://www.w3.org/2001/XMLSchema#" >
  <!ENTITY rdfs "http://www.w3.org/2000/01/rdf-schema#" >
  <!ENTITY rdf "http://www.w3.org/1999/02/22-rdf-syntax-ns#" >
  <!ENTITY dc "http://purl.org/dc/elements/1.1/" >
  <!ENTITY dct "http://purl.org/dc/terms/" >
  <!ENTITY skos "http://www.w3.org/2004/02/skos/core#" >
  <!ENTITY iso19150-2 "http://def.isotc211.org/iso19150/-2/2012/base#" >
  <!ENTITY iso19103 "http://def.isotc211.org/iso19103/2005/Names#" >

]>

<rdf:RDF xmlns="http://def.isotc211.org/iso19103/2005/Names#"
  xml:base="http://def.isotc211.org/iso19103/2005/Names"
  xmlns:owl="http://www.w3.org/2002/07/owl#"
  xmlns:xsd="http://www.w3.org/2001/XMLSchema#"
  xmlns:rdfs="http://www.w3.org/2000/01/rdf-schema#"
  xmlns:rdf="http://www.w3.org/1999/02/22-rdf-syntax-ns#"
  xmlns:dc="http://purl.org/dc/elements/1.1/"
  xmlns:dct="http://purl.org/dc/terms/"
  xmlns:skos="http://www.w3.org/2004/02/skos/core#"
  xmlns:iso19150-2="http://def.isotc211.org/iso19150/-2/2012/base#"
  xmlns:iso19103="http://def.isotc211.org/iso19103/2005/Names#">
  <owl:Ontology rdf:about="http://def.isotc211.org/iso19103/2005/Names">
    <rdfs:label>ISO 19103:2005 Names</rdfs:label>
    <dct:source>http://standards.iso.org/iso/19103/ed-1/en/</dct:source>
    <owl:versionInfo>2005-07-15</owl:versionInfo>
    <owl:imports rdf:resource="http://def.isotc211.org/iso19150/-2/2012/base"/>
  </owl:Ontology>
  <owl:Class rdf:about="&iso19103;GenericName">
    <rdfs:label>GenericName</rdfs:label>
    <skos:definition>Generic Name is the abstract class for all names in a NameSpace. Each instance of a GenericName is either a LocalName or a ScopedName. A LocalName references a local object directly accessible from the NameSpace. A ScopedName is a composite of a LocalName for locating another NameSpace and a GenericName valid in that NameSpace.</skos:definition>
    <rdfs:isDefinedBy>http://standards.iso.org/iso/19103/ed-1/en/</rdfs:isDefinedBy>
    <iso19150-2:isAbstract rdf:datatype="&xsd;boolean">true</iso19150-2:isAbstract>
    <rdfs:subClassOf>
      <owl:Restriction>
        <owl:onProperty rdf:resource="&iso19103;GenericName.scope"/>
        <owl:cardinality rdf:datatype="&xsd;nonNegativeInteger">1</owl:cardinality>
      </owl:Restriction>
    </rdfs:subClassOf>
    <rdfs:subClassOf>
      <owl:Restriction>
        <owl:onProperty rdf:resource="&iso19103;GenericName.scope"/>
        <owl:allValuesFrom rdf:resource="&iso19103;NameSpace"/>
      </owl:Restriction>
    </rdfs:subClassOf>
  </owl:Class>
  <owl:Class rdf:about="&iso19103;LocalName">
    <rdfs:label>LocalName</rdfs:label>
    <skos:definition>A LocalName references a local object directly accessible the NameSpace.</skos:definition>
    <rdfs:isDefinedBy>http://standards.iso.org/iso/19103/ed-1/en/</rdfs:isDefinedBy>
    <iso19150-2:constraint>self .eq. parsedName()</iso19150-2:constraint>
    <iso19150-2:constraint>self .eq. parsedName()</iso19150-2:constraint>
    <rdfs:subClassOf rdf:resource="&iso19103;GenericName"/>
  </owl:Class>
  <owl:Class rdf:about="&iso19103;MemberName">
    <rdfs:label>MemberName</rdfs:label>
    <skos:definition>A MemberName is a LocalName that references either an attribute slot in a record or  recordType or an attribute, operation, or association role in an object instance or  type description in some form of schema. The stored value "aName" is the returned value for the "aName()" operation.  </skos:definition>
    <rdfs:isDefinedBy>http://standards.iso.org/iso/19103/ed-1/en/</rdfs:isDefinedBy>
    <rdfs:subClassOf rdf:resource="&iso19103;LocalName"/>
    <rdfs:subClassOf>
      <owl:Restriction>
        <owl:onProperty rdf:resource="&iso19103;MemberName.aName"/>
        <owl:cardinality rdf:datatype="&xsd;nonNegativeInteger">1</owl:cardinality>
      </owl:Restriction>
    </rdfs:subClassOf>
    <rdfs:subClassOf>
      <owl:Restriction>
        <owl:onProperty rdf:resource="&iso19103;MemberName.aName"/>
        <owl:allValuesFrom rdf:resource="&xsd;string"/>
      </owl:Restriction>
    </rdfs:subClassOf>
    <rdfs:subClassOf>
      <owl:Restriction>
        <owl:onProperty rdf:resource="&iso19103;MemberName.attributeType"/>
        <owl:cardinality rdf:datatype="&xsd;nonNegativeInteger">1</owl:cardinality>
      </owl:Restriction>
    </rdfs:subClassOf>
    <rdfs:subClassOf>
      <owl:Restriction>
        <owl:onProperty rdf:resource="&iso19103;MemberName.attributeType"/>
        <owl:allValuesFrom rdf:resource="&iso19103;TypeName"/>
      </owl:Restriction>
    </rdfs:subClassOf>
  </owl:Class>
  <owl:Class rdf:about="&iso19103;NameSpace">
    <rdfs:label>NameSpace</rdfs:label>
    <skos:definition>A Name Space is a domain in which "names" given by character strings (possibly under local constrains constraints enforced by the Name Space) can be mapped to objects via a getObejct operation. Examples include objects which form a Name Space for their attributes, operations and associations, or Schemas that form Name Spaces for their included data types or classes. Not all methods for NameSpaces need to be made publicly accessible.</skos:definition>
    <rdfs:isDefinedBy>http://standards.iso.org/iso/19103/ed-1/en/</rdfs:isDefinedBy>
    <rdfs:subClassOf>
      <owl:Restriction>
        <owl:onProperty rdf:resource="&iso19103;NameSpace.isGlobal"/>
        <owl:cardinality rdf:datatype="&xsd;nonNegativeInteger">1</owl:cardinality>
      </owl:Restriction>
    </rdfs:subClassOf>
    <rdfs:subClassOf>
      <owl:Restriction>
        <owl:onProperty rdf:resource="&iso19103;NameSpace.isGlobal"/>
        <owl:allValuesFrom rdf:resource="&xsd;boolean"/>
      </owl:Restriction>
    </rdfs:subClassOf>
    <rdfs:subClassOf>
      <owl:Restriction>
        <owl:onProperty rdf:resource="&iso19103;NameSpace.acceptableClassList"/>
        <owl:allValuesFrom rdf:resource="&iso19103;TypeName"/>
      </owl:Restriction>
    </rdfs:subClassOf>
    <rdfs:subClassOf>
      <owl:Restriction>
        <owl:onProperty rdf:resource="&iso19103;NameSpace.name"/>
        <owl:allValuesFrom rdf:resource="&iso19103;GenericName"/>
      </owl:Restriction>
    </rdfs:subClassOf>
  </owl:Class>
  <owl:Class rdf:about="&iso19103;NULL">
    <rdfs:label>NULL</rdfs:label>
    <skos:definition>.lt.UsedBy.gt..lt.NameSpace.gt.ISO 19103 Conceptual Schema Language.lt..sl.NameSpace.gt..lt.Class.gt.CircularSequence.lt..sl.Class.gt..lt.Package.gt.Collections.lt..sl.Package.gt..lt.Operation.gt.last.lt..sl.Operation.gt..lt.Parameter.gt.Return.lt..sl.Parameter.gt..lt.Type.gt.NULL.lt..sl.Type.gt..lt.UsedBy.gt.</skos:definition>
    <rdfs:isDefinedBy>http://standards.iso.org/iso/19103/ed-1/en/</rdfs:isDefinedBy>
  </owl:Class>
  <owl:Class rdf:about="&iso19103;Reference">
    <rdfs:label>Reference</rdfs:label>
    <skos:definition>.lt.UsedBy.gt..lt.NameSpace.gt.ISO 19103 Conceptual Schema Language.lt..sl.NameSpace.gt..lt.Class.gt.NameSpace.lt..sl.Class.gt..lt.Package.gt.Names.lt..sl.Package.gt..lt.Operation.gt.registerID.lt..sl.Operation.gt..lt.Parameter.gt.registeredObj.lt..sl.Parameter.gt..lt.Type.gt.Reference.lt..sl.Type.gt..lt.UsedBy.gt.</skos:definition>
    <rdfs:isDefinedBy>http://standards.iso.org/iso/19103/ed-1/en/</rdfs:isDefinedBy>
  </owl:Class>
  <owl:Class rdf:about="&iso19103;ScopedName">
    <rdfs:label>ScopedName</rdfs:label>
    <skos:definition>A ScopedName is a composite of a LocalName for anther NameSpace and a GenericName valid in that NameSpace.This is the value returned by the getObject() operations. In a cascade for of TypeNames and Attribute names, the usual notation is a sequence of name separated by dots ".".</skos:definition>
    <rdfs:isDefinedBy>http://standards.iso.org/iso/19103/ed-1/en/</rdfs:isDefinedBy>
    <iso19150-2:constraint>push(S:Scope).scope .eq. S</iso19150-2:constraint>
    <iso19150-2:constraint>push(S:Scope).scope .eq. S</iso19150-2:constraint>
    <iso19150-2:constraint>push(S:Scope).scope .eq. S</iso19150-2:constraint>
    <rdfs:subClassOf rdf:resource="&iso19103;GenericName"/>
  </owl:Class>
  <owl:Class rdf:about="&iso19103;TypeName">
    <rdfs:label>TypeName</rdfs:label>
    <skos:definition>A TypeName is a LocalName that references either a recordType or object type in some form of schema. The stored value "aName" is the returned value for the "aName()" operation. This is the types name. For parsing from types (or objects) the parsible name normally uses a "." navigation separator, so that it is of the form  .lt.class.gt...lt.member.gt...lt.memberOfMember.gt.. ...)</skos:definition>
    <rdfs:isDefinedBy>http://standards.iso.org/iso/19103/ed-1/en/</rdfs:isDefinedBy>
    <rdfs:subClassOf rdf:resource="&iso19103;LocalName"/>
    <rdfs:subClassOf>
      <owl:Restriction>
        <owl:onProperty rdf:resource="&iso19103;TypeName.aName"/>
        <owl:cardinality rdf:datatype="&xsd;nonNegativeInteger">1</owl:cardinality>
      </owl:Restriction>
    </rdfs:subClassOf>
    <rdfs:subClassOf>
      <owl:Restriction>
        <owl:onProperty rdf:resource="&iso19103;TypeName.aName"/>
        <owl:allValuesFrom rdf:resource="&xsd;string"/>
      </owl:Restriction>
    </rdfs:subClassOf>
  </owl:Class>
  <owl:Class rdf:about="&iso19103;void">
    <rdfs:label>void</rdfs:label>
    <skos:definition>.lt.UsedBy.gt..lt.NameSpace.gt.Informative Models.lt..sl.NameSpace.gt..lt.Class.gt.GC_GeoParser.lt..sl.Class.gt..lt.Package.gt.Services.lt..sl.Package.gt..lt.Operation.gt.getFeature.lt..sl.Operation.gt..lt.Parameter.gt.Return.lt..sl.Parameter.gt..lt.Type.gt.void.lt..sl.Type.gt..lt.UsedBy.gt.</skos:definition>
    <rdfs:isDefinedBy>http://standards.iso.org/iso/19103/ed-1/en/</rdfs:isDefinedBy>
  </owl:Class>
  <owl:DatatypeProperty rdf:about="&iso19103;MemberName.aName">
    <rdfs:label>aName</rdfs:label>
    <rdfs:isDefinedBy>http://standards.iso.org/iso/19103/ed-1/en/</rdfs:isDefinedBy>
    <rdfs:domain rdf:resource="&iso19103;MemberName"/>
    <rdfs:range rdf:resource="&xsd;string"/>
  </owl:DatatypeProperty>
  <owl:ObjectProperty rdf:about="&iso19103;MemberName.attributeType">
    <rdfs:label>attributeType</rdfs:label>
    <rdfs:isDefinedBy>http://standards.iso.org/iso/19103/ed-1/en/</rdfs:isDefinedBy>
    <rdfs:domain rdf:resource="&iso19103;MemberName"/>
    <rdfs:range rdf:resource="&iso19103;TypeName"/>
  </owl:ObjectProperty>
  <owl:DatatypeProperty rdf:about="&iso19103;NameSpace.isGlobal">
    <rdfs:label>isGlobal</rdfs:label>
    <rdfs:isDefinedBy>http://standards.iso.org/iso/19103/ed-1/en/</rdfs:isDefinedBy>
    <rdfs:domain rdf:resource="&iso19103;NameSpace"/>
    <rdfs:range rdf:resource="&xsd;boolean"/>
  </owl:DatatypeProperty>
  <owl:ObjectProperty rdf:about="&iso19103;NameSpace.acceptableClassList">
    <rdfs:label>acceptableClassList</rdfs:label>
    <rdfs:isDefinedBy>http://standards.iso.org/iso/19103/ed-1/en/</rdfs:isDefinedBy>
    <rdfs:domain rdf:resource="&iso19103;NameSpace"/>
    <rdfs:range rdf:resource="&iso19103;TypeName"/>
  </owl:ObjectProperty>
  <owl:DatatypeProperty rdf:about="&iso19103;TypeName.aName">
    <rdfs:label>aName</rdfs:label>
    <rdfs:isDefinedBy>http://standards.iso.org/iso/19103/ed-1/en/</rdfs:isDefinedBy>
    <rdfs:domain rdf:resource="&iso19103;TypeName"/>
    <rdfs:range rdf:resource="&xsd;string"/>
  </owl:DatatypeProperty>
  <owl:ObjectProperty rdf:about="&iso19103;GenericName.scope">
    <rdfs:label>scope</rdfs:label>
    <rdfs:isDefinedBy>http://standards.iso.org/iso/19103/ed-1/en/</rdfs:isDefinedBy>
    <iso19150-2:aggregationType>partOfSharedAggregation</iso19150-2:aggregationType>
    <iso19150-2:associationName>Scope</iso19150-2:associationName>
    <rdfs:domain rdf:resource="&iso19103;GenericName"/>
    <rdfs:range rdf:resource="&iso19103;NameSpace"/>
  </owl:ObjectProperty>
  <owl:ObjectProperty rdf:about="&iso19103;NameSpace.name">
    <rdfs:label>name</rdfs:label>
    <rdfs:isDefinedBy>http://standards.iso.org/iso/19103/ed-1/en/</rdfs:isDefinedBy>
    <iso19150-2:associationName>Scope</iso19150-2:associationName>
    <rdfs:domain rdf:resource="&iso19103;NameSpace"/>
    <rdfs:range rdf:resource="&iso19103;GenericName"/>
    <owl:inverseOf rdf:resource="&iso19103;GenericName.scope"/>
  </owl:ObjectProperty>
  <owl:ObjectProperty rdf:about="&iso19103;GenericName.scope">
    <rdfs:label>scope</rdfs:label>
    <rdfs:isDefinedBy>http://standards.iso.org/iso/19103/ed-1/en/</rdfs:isDefinedBy>
    <iso19150-2:aggregationType>partOfSharedAggregation</iso19150-2:aggregationType>
    <iso19150-2:associationName>Scope</iso19150-2:associationName>
    <rdfs:domain rdf:resource="&iso19103;GenericName"/>
    <rdfs:range rdf:resource="&iso19103;NameSpace"/>
  </owl:ObjectProperty>
  <owl:ObjectProperty rdf:about="&iso19103;NameSpace.name">
    <rdfs:label>name</rdfs:label>
    <rdfs:isDefinedBy>http://standards.iso.org/iso/19103/ed-1/en/</rdfs:isDefinedBy>
    <iso19150-2:associationName>Scope</iso19150-2:associationName>
    <rdfs:domain rdf:resource="&iso19103;NameSpace"/>
    <rdfs:range rdf:resource="&iso19103;GenericName"/>
    <owl:inverseOf rdf:resource="&iso19103;GenericName.scope"/>
  </owl:ObjectProperty>
</rdf:RDF>

