PREFIX cs: <http://def.isotc211.org/iso19135/-1/2015/CoreModel/code/RE_ItemStatus>
PREFIX prov: <http://www.w3.org/ns/prov#>
PREFIX rdfs: <http://www.w3.org/2000/01/rdf-schema#>
PREFIX reg: <http://purl.org/linked-data/registry#>
PREFIX schema: <https://schema.org/>
PREFIX skos: <http://www.w3.org/2004/02/skos/core#>
PREFIX status: <http://def.isotc211.org/iso19135/-1/2015/CoreModel/code/RE_ItemStatus/>
PREFIX xsd: <http://www.w3.org/2001/XMLSchema#>

status:stable
    a skos:Concept ;
    reg:status status:experimental ;
    rdfs:isDefinedBy cs: ;
    skos:broader status:valid ;
    skos:definition "The item valid and expected to remain unchanged. It may be used widely"@en ;
    skos:inScheme cs: ;
    skos:prefLabel "stable"@en ;
    schema:provenance "Added to this codelist by GOM, 2023"@en ;
.

status:invalid
    a skos:Concept ;
    reg:status status:original ;
    rdfs:isDefinedBy cs: ;
    skos:definition "A decision has been made that a previously valid register item contains a substantial error and is invalid, and will normally have been replaced by a corrected item"@en ;
    skos:inScheme cs: ;
    skos:prefLabel "invalid"@en ;
    skos:topConceptOf cs: ;
    schema:provenance "Supplied within the original issuance of the vocabulary"@en ;
.

status:retired
    a skos:Concept ;
    reg:status status:original ;
    rdfs:isDefinedBy cs: ;
    skos:definition "A decision has been made that the item is no longer recommended for use. It has not been superseded by another item"@en ;
    skos:inScheme cs: ;
    skos:prefLabel "retired"@en ;
    skos:topConceptOf cs: ;
    schema:provenance "Supplied within the original issuance of the vocabulary"@en ;
.

status:submitted
    a skos:Concept ;
    reg:status status:original ;
    rdfs:isDefinedBy cs: ;
    skos:definition "The item has been entered into the register, but the control body has not accepted the proposal to add it"@en ;
    skos:inScheme cs: ;
    skos:prefLabel "submitted"@en ;
    skos:topConceptOf cs: ;
    schema:provenance "Supplied within the original issuance of the vocabulary"@en ;
.

status:superseded
    a skos:Concept ;
    reg:status status:original ;
    rdfs:isDefinedBy cs: ;
    skos:definition "The item has been superseded by another item and is no longer recommended for use"@en ;
    skos:inScheme cs: ;
    skos:prefLabel "superseded"@en ;
    skos:topConceptOf cs: ;
    schema:provenance "Supplied within the original issuance of the vocabulary"@en ;
.

status:addition
    a skos:Concept ;
    reg:status status:addition ;
    rdfs:isDefinedBy cs: ;
    skos:broader status:valid ;
    skos:definition "The item is valid and was supplied to the vocabulary after initial creation"@en ;
    skos:inScheme cs: ;
    skos:prefLabel "addition"@en ;
    schema:provenance "Added to this codelist by GOM, 2022"@en ;
.

status:experimental
    a skos:Concept ;
    reg:status status:experimental ;
    rdfs:isDefinedBy cs: ;
    skos:broader status:valid ;
    skos:definition "The item is valid but is experimental in nature and should be used with caution"@en ;
    skos:inScheme cs: ;
    skos:prefLabel "valid"@en ;
    schema:provenance "Added to this codelist by GOM, 2023"@en ;
.

status:valid
    a skos:Concept ;
    reg:status status:original ;
    rdfs:isDefinedBy cs: ;
    skos:definition "The item has been accepted, is recommended for use, and has not been superseded or retired"@en ;
    skos:inScheme cs: ;
    skos:prefLabel "valid"@en ;
    skos:topConceptOf cs: ;
    schema:provenance "Supplied within the original issuance of the vocabulary"@en ;
.

status:original
    a skos:Concept ;
    reg:status status:addition ;
    rdfs:isDefinedBy cs: ;
    skos:broader status:valid ;
    skos:definition "Supplied within the original issuance of the vocabulary"@en ;
    skos:inScheme cs: ;
    skos:prefLabel "original"@en ;
    schema:provenance "Added to this codelist by GOM, 2022"@en ;
.

cs:
    a skos:ConceptScheme ;
    reg:status status:experimental ;
    skos:definition "Instances of RE_ItemStatus that identify the registration status of a RegisterItem"@en ;
    skos:hasTopConcept
        status:addition ,
        status:invalid ,
        status:original ,
        status:retired ,
        status:submitted ,
        status:superseded ,
        status:valid ;
    skos:prefLabel "Register Item Status Codes"@en ;
    prov:qualifiedDerivation
        [
            prov:entity <http://example.com/none> ;
            prov:hadRole <https://linked.data.gov.au/def/vocab-derivation-modes/none> ;
        ] ;
    schema:citation "http://standards.iso.org/iso/19135/-1/ed-1/en/"^^xsd:anyURI ;
    schema:creator <https://committee.iso.org/home/tc211> ;
    schema:dateCreated "2000-01-01"^^xsd:date ;
    schema:dateModified "2023-05-16"^^xsd:date ;
    schema:identifier "RE_ItemStatus"^^xsd:token ;
    schema:issued "2000-01-01"^^xsd:date ;
    schema:provenance "Derived from TC211-produced RDF versions of the standard's UML"@en ;
    schema:publisher <https://committee.iso.org/home/tc211> ;
.
