@base          <http://def.isotc211.org/iso19115/-1/2014/Metadata-Fundamentals> .
@prefix dc:    <http://purl.org/dc/elements/1.1/> .
@prefix dct:   <http://purl.org/dc/terms/> .
@prefix owl:   <http://www.w3.org/2002/07/owl#> .
@prefix rdf:   <http://www.w3.org/1999/02/22-rdf-syntax-ns#> .
@prefix rdfs:  <http://www.w3.org/2000/01/rdf-schema#> .
@prefix reg:    <http://purl.org/linked-data/registry#>.
@prefix skos:  <http://www.w3.org/2004/02/skos/core#> .

@prefix application: <http://def.isotc211.org/iso19115/-1/2014/ApplicationSchemaInformation#> .
@prefix citation: <http://def.isotc211.org/iso19115/-1/2014/CitationAndResponsiblePartyInformation#> .
@prefix common: <http://def.isotc211.org/iso19115/-1/2014/CommonClasses#> .
@prefix constraint: <http://def.isotc211.org/iso19115/-1/2014/ConstraintInformation#> .
@prefix content: <http://def.isotc211.org/iso19115/-1/2014/ContentInformation#> .
@prefix crs:   <http://def.isotc211.org/iso19111/2007/CoordinateReferenceSystems#> .
@prefix distribution: <http://def.isotc211.org/iso19115/-1/2014/DistributionInformation#> .
@prefix extended: <http://def.isotc211.org/iso19115/-1/2014/ExampleOfExtendedMatadata#> .
@prefix extent: <http://def.isotc211.org/iso19115/-1/2014/ExtentInformation#> .
@prefix fc:    <http://def.isotc211.org/iso19110/2005/MethodologyForFeatureCataloguing#> .
@prefix fundamentals: <http://def.isotc211.org/iso19115/-1/2014/Metadata-Fundamentals#> .
@prefix identification: <http://def.isotc211.org/iso19115/-1/2014/IdentificationInformation#> .
@prefix lineage: <http://def.isotc211.org/iso19115/-1/2014/LineageInformation#> .
@prefix localization: <http://def.isotc211.org/iso19115/-1/2014/Language-CharactersetLocalizationInformation#> .
@prefix maintenance: <http://def.isotc211.org/iso19115/-1/2014/MaintenanceInformation#> .
@prefix metapp: <http://def.isotc211.org/iso19115/-1/2014/MetadataApplicationInformation#> .
@prefix metext: <http://def.isotc211.org/iso19115/-1/2014/MetadataExtensionInformation#> .
@prefix metinf: <http://def.isotc211.org/iso19115/-1/2014/MetadataInformation#> .
@prefix portrayal: <http://def.isotc211.org/iso19115/-1/2014/PortrayalCatalogueInformation#> .
@prefix rs:    <http://def.isotc211.org/iso19115/-1/2014/ReferenceSystemInformation#> .
@prefix service: <http://def.isotc211.org/iso19115/-1/2014/ServiceMetadataInformation#> . 
@prefix sr:    <http://def.isotc211.org/iso19115/-1/2014/SpatialRepresentationInformation#> .

@prefix iso00639_65: <http://def.isotc211.org/iso00639/-2/LanguageCodes#> .
@prefix iso19110_2259: <http://def.isotc211.org/iso19110/2005/MethodologyForFeatureCataloguing#> .
@prefix iso19107_2211: <http://def.isotc211.org/iso19107/2003/GeometryRoot#> .
@prefix iso19107_2210: <http://def.isotc211.org/iso19107/2003/GeometricPrimitive#> .
@prefix iso19115-1Code: <http://def.isotc211.org/iso19115/-1/2014/CitationAndResponsiblePartyInformation/code/> .
@prefix iso19108_891: <http://def.isotc211.org/iso19108/2006/TemporalObjects#> .
@prefix iso19139_709: <http://def.isotc211.org/iso19139/2007/CulturalAndLinguisticAdapdability#> .
@prefix iso19115-1: <http://def.isotc211.org/iso19115/-1/2014/CitationAndResponsiblePartyInformation#> .
@prefix iso19111_1300: <http://def.isotc211.org/iso19111/2007/CoordinateReferenceSystems#> .
@prefix iso19103_2176: <http://def.isotc211.org/iso19103/2015/RecordTypes#> .
@prefix iso19103_2174: <http://def.isotc211.org/iso19103/2015/NameTypes#> .
@prefix iso03166_66: <http://def.isotc211.org/iso03166/-1/CountryCodes#> .
@prefix iso19115-1_2364: <http://def.isotc211.org/iso19115/-1/2014/ConstraintInformation#> .
@prefix iso19115-1_2376: <http://def.isotc211.org/iso19115/-1/2014/SpatialRepresentationInformation#> .
@prefix iso19115-1_2375: <http://def.isotc211.org/iso19115/-1/2014/ReferenceSystemInformation#> .
@prefix iso19115-1_2365: <http://def.isotc211.org/iso19115/-1/2014/ContentInformation#> .
@prefix iso19115-1_2374: <http://def.isotc211.org/iso19115/-1/2014/PortrayalCatalogueInformation#> .
@prefix iso19115-1_2362: <http://def.isotc211.org/iso19115/-1/2014/ApplicationSchemaInformation#> .
@prefix iso19115-1_2363: <http://def.isotc211.org/iso19115/-1/2014/CitationAndResponsiblePartyInformation#> .
@prefix iso19115-1_2373: <http://def.isotc211.org/iso19115/-1/2014/MetadataExtensionInformation#> .
@prefix iso19115-1_2368: <http://def.isotc211.org/iso19115/-1/2014/ExtentInformation#> .
@prefix iso19115-1_2369: <http://def.isotc211.org/iso19115/-1/2014/IdentificationInformation#> .
@prefix iso19115-1_2366: <http://def.isotc211.org/iso19115/-1/2014/LineageInformation#> .
@prefix iso19103_2178: <http://def.isotc211.org/iso19103/2015/WebEnvironment#> .
@prefix iso19115-1_2367: <http://def.isotc211.org/iso19115/-1/2014/DistributionInformation#> .
@prefix iso19103_2179: <http://def.isotc211.org/iso19103/2015/MeasureTypes#> .
@prefix iso19157_1164: <http://def.isotc211.org/iso19157/2013/DataQuality#> .
@prefix iso19115-1_2371: <http://def.isotc211.org/iso19115/-1/2014/MetadataApplicationInformation#> .
@prefix iso19115-1_2360: <http://def.isotc211.org/iso19115/-1/2014/Language-CharactersetLocalizationInformation#> .
@prefix iso19115-1_2372: <http://def.isotc211.org/iso19115/-1/2014/MetadataInformation#> .
@prefix iso19115-1_2370: <http://def.isotc211.org/iso19115/-1/2014/MaintenanceInformation#> .
@prefix iso19150-2: <http://def.isotc211.org/iso19150/-2/2012/base#> .
@prefix iso19115-1_2358: <http://def.isotc211.org/iso19115/-1/2014/CommonClasses#> .


<ContentInformation/code/MD_CoverageContentTypeCode/auxilliaryInformation>
        a                 iso19115-1_2365:MD_CoverageContentTypeCode , skos:Concept ;
        rdfs:isDefinedBy  <http://standards.iso.org/iso/19115/-1/ed-1/en/> ;
        rdfs:label        "auxilliary Information" ;
        dct:description   "calculation of the primary physicalMeasurement coverages in the dataset\r\n\r\nEXAMPLE Grid of aerosol optical thickness used in the calculation of a sea surface temperature product."^^xsd:string ;
        skos:definition   "calculation of the primary physicalMeasurement coverages in the dataset\r\n\r\nEXAMPLE Grid of aerosol optical thickness used in the calculation of a sea surface temperature product."^^xsd:string ;
        skos:inScheme     <ContentInformation/code/MD_CoverageContentTypeCode> ;
        skos:prefLabel    "auxilliaryInformation" .

<ContentInformation/code/MD_CoverageContentTypeCode/image>
        a                 iso19115-1_2365:MD_CoverageContentTypeCode , skos:Concept ;
        rdfs:isDefinedBy  <http://standards.iso.org/iso/19115/-1/ed-1/en/> ;
        rdfs:label        "image" ;
        dct:description   "meaningful numerical representation of a physical parameter that is not the actual value of the physical parameter"^^xsd:string ;
        skos:definition   "meaningful numerical representation of a physical parameter that is not the actual value of the physical parameter"^^xsd:string ;
        skos:inScheme     <ContentInformation/code/MD_CoverageContentTypeCode> ;
        skos:prefLabel    "image" .

<ContentInformation/code/MD_CoverageContentTypeCode/coordinate>
        a                 iso19115-1_2365:MD_CoverageContentTypeCode , skos:Concept ;
        rdfs:isDefinedBy  <http://standards.iso.org/iso/19115/-1/ed-1/en/> ;
        rdfs:label        "coordinate" ;
        dct:description   "data used to provide coordinate axis values"^^xsd:string ;
        skos:definition   "data used to provide coordinate axis values"^^xsd:string ;
        skos:inScheme     <ContentInformation/code/MD_CoverageContentTypeCode> ;
        skos:prefLabel    "coordinate" .

<ContentInformation/code/MD_CoverageContentTypeCode/qualityInformation>
        a                 iso19115-1_2365:MD_CoverageContentTypeCode , skos:Concept ;
        rdfs:isDefinedBy  <http://standards.iso.org/iso/19115/-1/ed-1/en/> ;
        rdfs:label        "quality Information" ;
        dct:description   "data used to characterize the quality of the physicalMeasurement coverages in the dataset.\r\nNOTE Typically included in a gmi:QE_CoverageResult."^^xsd:string ;
        skos:definition   "data used to characterize the quality of the physicalMeasurement coverages in the dataset.\r\nNOTE Typically included in a gmi:QE_CoverageResult."^^xsd:string ;
        skos:inScheme     <ContentInformation/code/MD_CoverageContentTypeCode> ;
        skos:prefLabel    "qualityInformation" .

<ContentInformation/code/MD_CoverageContentTypeCode/referenceInformation>
        a                 iso19115-1_2365:MD_CoverageContentTypeCode , skos:Concept ;
        rdfs:isDefinedBy  <http://standards.iso.org/iso/19115/-1/ed-1/en/> ;
        rdfs:label        "reference Information" ;
        dct:description   "reference information used to support the calculation or use of the physicalMeasurement coverages in the dataset\r\nEXAMPLE Grids of latitude/longitude used to geolocate the physical measurements."^^xsd:string ;
        skos:definition   "reference information used to support the calculation or use of the physicalMeasurement coverages in the dataset\r\nEXAMPLE Grids of latitude/longitude used to geolocate the physical measurements."^^xsd:string ;
        skos:inScheme     <ContentInformation/code/MD_CoverageContentTypeCode> ;
        skos:prefLabel    "referenceInformation" .

<ContentInformation/code/MD_CoverageContentTypeCode/physicalMeasurement>
        a                 iso19115-1_2365:MD_CoverageContentTypeCode , skos:Concept ;
        rdfs:isDefinedBy  <http://standards.iso.org/iso/19115/-1/ed-1/en/> ;
        rdfs:label        "physical Measurement" ;
        dct:description   "value in physical units of the quantity being measured"^^xsd:string ;
        skos:definition   "value in physical units of the quantity being measured"^^xsd:string ;
        skos:inScheme     <ContentInformation/code/MD_CoverageContentTypeCode> ;
        skos:prefLabel    "physicalMeasurement" .

<ContentInformation/code/MD_CoverageContentTypeCode/thematicClassification>
        a                 iso19115-1_2365:MD_CoverageContentTypeCode , skos:Concept ;
        rdfs:isDefinedBy  <http://standards.iso.org/iso/19115/-1/ed-1/en/> ;
        rdfs:label        "thematic Classification" ;
        dct:description   "code value with no quantitative meaning, used to represent a physical quantity"^^xsd:string ;
        skos:definition   "code value with no quantitative meaning, used to represent a physical quantity"^^xsd:string ;
        skos:inScheme     <ContentInformation/code/MD_CoverageContentTypeCode> ;
        skos:prefLabel    "thematicClassification" .

<ContentInformation/code/MD_CoverageContentTypeCode/modelResult>
        a                 iso19115-1_2365:MD_CoverageContentTypeCode , skos:Concept ;
        rdfs:isDefinedBy  <http://standards.iso.org/iso/19115/-1/ed-1/en/> ;
        rdfs:label        "model Result" ;
        dct:description   "resources with values that are calculated using a model rather than being observed or calculated from observations"^^xsd:string ;
        skos:definition   "resources with values that are calculated using a model rather than being observed or calculated from observations"^^xsd:string ;
        skos:inScheme     <ContentInformation/code/MD_CoverageContentTypeCode> ;
        skos:prefLabel    "modelResult" .
