@base          <http://def.isotc211.org/iso19115/-1/2014/Metadata-Fundamentals> .
@prefix dc:    <http://purl.org/dc/elements/1.1/> .
@prefix dct:   <http://purl.org/dc/terms/> .
@prefix owl:   <http://www.w3.org/2002/07/owl#> .
@prefix rdf:   <http://www.w3.org/1999/02/22-rdf-syntax-ns#> .
@prefix rdfs:  <http://www.w3.org/2000/01/rdf-schema#> .
@prefix reg:    <http://purl.org/linked-data/registry#>.
@prefix skos:  <http://www.w3.org/2004/02/skos/core#> .

@prefix application: <http://def.isotc211.org/iso19115/-1/2014/ApplicationSchemaInformation#> .
@prefix citation: <http://def.isotc211.org/iso19115/-1/2014/CitationAndResponsiblePartyInformation#> .
@prefix common: <http://def.isotc211.org/iso19115/-1/2014/CommonClasses#> .
@prefix constraint: <http://def.isotc211.org/iso19115/-1/2014/ConstraintInformation#> .
@prefix content: <http://def.isotc211.org/iso19115/-1/2014/ContentInformation#> .
@prefix crs:   <http://def.isotc211.org/iso19111/2007/CoordinateReferenceSystems#> .
@prefix distribution: <http://def.isotc211.org/iso19115/-1/2014/DistributionInformation#> .
@prefix extended: <http://def.isotc211.org/iso19115/-1/2014/ExampleOfExtendedMatadata#> .
@prefix extent: <http://def.isotc211.org/iso19115/-1/2014/ExtentInformation#> .
@prefix fc:    <http://def.isotc211.org/iso19110/2005/MethodologyForFeatureCataloguing#> .
@prefix fundamentals: <http://def.isotc211.org/iso19115/-1/2014/Metadata-Fundamentals#> .
@prefix identification: <http://def.isotc211.org/iso19115/-1/2014/IdentificationInformation#> .
@prefix lineage: <http://def.isotc211.org/iso19115/-1/2014/LineageInformation#> .
@prefix localization: <http://def.isotc211.org/iso19115/-1/2014/Language-CharactersetLocalizationInformation#> .
@prefix maintenance: <http://def.isotc211.org/iso19115/-1/2014/MaintenanceInformation#> .
@prefix metapp: <http://def.isotc211.org/iso19115/-1/2014/MetadataApplicationInformation#> .
@prefix metext: <http://def.isotc211.org/iso19115/-1/2014/MetadataExtensionInformation#> .
@prefix metinf: <http://def.isotc211.org/iso19115/-1/2014/MetadataInformation#> .
@prefix portrayal: <http://def.isotc211.org/iso19115/-1/2014/PortrayalCatalogueInformation#> .
@prefix rs:    <http://def.isotc211.org/iso19115/-1/2014/ReferenceSystemInformation#> .
@prefix service: <http://def.isotc211.org/iso19115/-1/2014/ServiceMetadataInformation#> . 
@prefix sr:    <http://def.isotc211.org/iso19115/-1/2014/SpatialRepresentationInformation#> .

@prefix iso00639_65: <http://def.isotc211.org/iso00639/-2/LanguageCodes#> .
@prefix iso19110_2259: <http://def.isotc211.org/iso19110/2005/MethodologyForFeatureCataloguing#> .
@prefix iso19107_2211: <http://def.isotc211.org/iso19107/2003/GeometryRoot#> .
@prefix iso19107_2210: <http://def.isotc211.org/iso19107/2003/GeometricPrimitive#> .
@prefix iso19115-1Code: <http://def.isotc211.org/iso19115/-1/2014/CitationAndResponsiblePartyInformation/code/> .
@prefix iso19108_891: <http://def.isotc211.org/iso19108/2006/TemporalObjects#> .
@prefix iso19139_709: <http://def.isotc211.org/iso19139/2007/CulturalAndLinguisticAdapdability#> .
@prefix iso19115-1: <http://def.isotc211.org/iso19115/-1/2014/CitationAndResponsiblePartyInformation#> .
@prefix iso19111_1300: <http://def.isotc211.org/iso19111/2007/CoordinateReferenceSystems#> .
@prefix iso19103_2176: <http://def.isotc211.org/iso19103/2015/RecordTypes#> .
@prefix iso19103_2174: <http://def.isotc211.org/iso19103/2015/NameTypes#> .
@prefix iso03166_66: <http://def.isotc211.org/iso03166/-1/CountryCodes#> .
@prefix iso19115-1_2364: <http://def.isotc211.org/iso19115/-1/2014/ConstraintInformation#> .
@prefix iso19115-1_2376: <http://def.isotc211.org/iso19115/-1/2014/SpatialRepresentationInformation#> .
@prefix iso19115-1_2375: <http://def.isotc211.org/iso19115/-1/2014/ReferenceSystemInformation#> .
@prefix iso19115-1_2365: <http://def.isotc211.org/iso19115/-1/2014/ContentInformation#> .
@prefix iso19115-1_2374: <http://def.isotc211.org/iso19115/-1/2014/PortrayalCatalogueInformation#> .
@prefix iso19115-1_2362: <http://def.isotc211.org/iso19115/-1/2014/ApplicationSchemaInformation#> .
@prefix iso19115-1_2363: <http://def.isotc211.org/iso19115/-1/2014/CitationAndResponsiblePartyInformation#> .
@prefix iso19115-1_2373: <http://def.isotc211.org/iso19115/-1/2014/MetadataExtensionInformation#> .
@prefix iso19115-1_2368: <http://def.isotc211.org/iso19115/-1/2014/ExtentInformation#> .
@prefix iso19115-1_2369: <http://def.isotc211.org/iso19115/-1/2014/IdentificationInformation#> .
@prefix iso19115-1_2366: <http://def.isotc211.org/iso19115/-1/2014/LineageInformation#> .
@prefix iso19103_2178: <http://def.isotc211.org/iso19103/2015/WebEnvironment#> .
@prefix iso19115-1_2367: <http://def.isotc211.org/iso19115/-1/2014/DistributionInformation#> .
@prefix iso19103_2179: <http://def.isotc211.org/iso19103/2015/MeasureTypes#> .
@prefix iso19157_1164: <http://def.isotc211.org/iso19157/2013/DataQuality#> .
@prefix iso19115-1_2371: <http://def.isotc211.org/iso19115/-1/2014/MetadataApplicationInformation#> .
@prefix iso19115-1_2360: <http://def.isotc211.org/iso19115/-1/2014/Language-CharactersetLocalizationInformation#> .
@prefix iso19115-1_2372: <http://def.isotc211.org/iso19115/-1/2014/MetadataInformation#> .
@prefix iso19115-1_2370: <http://def.isotc211.org/iso19115/-1/2014/MaintenanceInformation#> .
@prefix iso19150-2: <http://def.isotc211.org/iso19150/-2/2012/base#> .
@prefix iso19115-1_2358: <http://def.isotc211.org/iso19115/-1/2014/CommonClasses#> .


<MetadataExtensionInformation/code/MD_DatatypeCode/enumeration>
        a                 iso19115-1_2373:MD_DatatypeCode , skos:Concept ;
        rdfs:isDefinedBy  <http://standards.iso.org/iso/19115/-1/ed-1/en/> ;
        rdfs:label        "enumeration" ;
        dct:description   "data type whose instances form a list of named literal values, not extendable"^^xsd:string ;
        skos:definition   "data type whose instances form a list of named literal values, not extendable"^^xsd:string ;
        skos:inScheme     <MetadataExtensionInformation/code/MD_DatatypeCode> ;
        skos:prefLabel    "enumeration" .

<MetadataExtensionInformation/code/MD_DatatypeCode/integer>
        a                 iso19115-1_2373:MD_DatatypeCode , skos:Concept ;
        rdfs:isDefinedBy  <http://standards.iso.org/iso/19115/-1/ed-1/en/> ;
        rdfs:label        "integer" ;
        dct:description   "numerical field"^^xsd:string ;
        skos:definition   "numerical field"^^xsd:string ;
        skos:inScheme     <MetadataExtensionInformation/code/MD_DatatypeCode> ;
        skos:prefLabel    "integer" .

<MetadataExtensionInformation/code/MD_DatatypeCode/class>
        a                 iso19115-1_2373:MD_DatatypeCode , skos:Concept ;
        rdfs:isDefinedBy  <http://standards.iso.org/iso/19115/-1/ed-1/en/> ;
        rdfs:label        "class" ;
        dct:description   "descriptor of a set of objects that share the same attributes, operations, methods, relationships, and behaviour"^^xsd:string ;
        skos:definition   "descriptor of a set of objects that share the same attributes, operations, methods, relationships, and behaviour"^^xsd:string ;
        skos:inScheme     <MetadataExtensionInformation/code/MD_DatatypeCode> ;
        skos:prefLabel    "class" .

<MetadataExtensionInformation/code/MD_DatatypeCode/abstractClass>
        a                 iso19115-1_2373:MD_DatatypeCode , skos:Concept ;
        rdfs:isDefinedBy  <http://standards.iso.org/iso/19115/-1/ed-1/en/> ;
        rdfs:label        "abstract Class" ;
        dct:description   "class that cannot be directly instantiated"^^xsd:string ;
        skos:definition   "class that cannot be directly instantiated"^^xsd:string ;
        skos:inScheme     <MetadataExtensionInformation/code/MD_DatatypeCode> ;
        skos:prefLabel    "abstractClass" .

<MetadataExtensionInformation/code/MD_DatatypeCode/typeClass>
        a                 iso19115-1_2373:MD_DatatypeCode , skos:Concept ;
        rdfs:isDefinedBy  <http://standards.iso.org/iso/19115/-1/ed-1/en/> ;
        rdfs:label        "type Class" ;
        dct:description   "class used for specification of a domain of instances (objects), together with the operations applicable to the objects. A type may have attributes and associations"^^xsd:string ;
        skos:definition   "class used for specification of a domain of instances (objects), together with the operations applicable to the objects. A type may have attributes and associations"^^xsd:string ;
        skos:inScheme     <MetadataExtensionInformation/code/MD_DatatypeCode> ;
        skos:prefLabel    "typeClass" .

<MetadataExtensionInformation/code/MD_DatatypeCode/codelistElement>
        a                 iso19115-1_2373:MD_DatatypeCode , skos:Concept ;
        rdfs:isDefinedBy  <http://standards.iso.org/iso/19115/-1/ed-1/en/> ;
        rdfs:label        "codelist Element" ;
        dct:description   "permissible value for a codelist or enumeration"^^xsd:string ;
        skos:definition   "permissible value for a codelist or enumeration"^^xsd:string ;
        skos:inScheme     <MetadataExtensionInformation/code/MD_DatatypeCode> ;
        skos:prefLabel    "codelistElement" .

<MetadataExtensionInformation/code/MD_DatatypeCode/metaClass>
        a                 iso19115-1_2373:MD_DatatypeCode , skos:Concept ;
        rdfs:isDefinedBy  <http://standards.iso.org/iso/19115/-1/ed-1/en/> ;
        rdfs:label        "meta Class" ;
        dct:description   "class whose instances are classes"^^xsd:string ;
        skos:definition   "class whose instances are classes"^^xsd:string ;
        skos:inScheme     <MetadataExtensionInformation/code/MD_DatatypeCode> ;
        skos:prefLabel    "metaClass" .

<MetadataExtensionInformation/code/MD_DatatypeCode/datatypeClass>
        a                 iso19115-1_2373:MD_DatatypeCode , skos:Concept ;
        rdfs:isDefinedBy  <http://standards.iso.org/iso/19115/-1/ed-1/en/> ;
        rdfs:label        "datatype Class" ;
        dct:description   "class with few or no operations whose primary purpose is to hold the abstract state of another class for transmittal, storage, encoding or persistent storage"^^xsd:string ;
        skos:definition   "class with few or no operations whose primary purpose is to hold the abstract state of another class for transmittal, storage, encoding or persistent storage"^^xsd:string ;
        skos:inScheme     <MetadataExtensionInformation/code/MD_DatatypeCode> ;
        skos:prefLabel    "datatypeClass" .

<MetadataExtensionInformation/code/MD_DatatypeCode/specifiedClass>
        a                 iso19115-1_2373:MD_DatatypeCode , skos:Concept ;
        rdfs:isDefinedBy  <http://standards.iso.org/iso/19115/-1/ed-1/en/> ;
        rdfs:label        "specified Class" ;
        dct:description   "subclass that may be substituted for its superclass"^^xsd:string ;
        skos:definition   "subclass that may be substituted for its superclass"^^xsd:string ;
        skos:inScheme     <MetadataExtensionInformation/code/MD_DatatypeCode> ;
        skos:prefLabel    "specifiedClass" .

<MetadataExtensionInformation/code/MD_DatatypeCode/aggregateClass>
        a                 iso19115-1_2373:MD_DatatypeCode , skos:Concept ;
        rdfs:isDefinedBy  <http://standards.iso.org/iso/19115/-1/ed-1/en/> ;
        rdfs:label        "aggregate Class" ;
        dct:description   "class that is composed of classes it is connected to by an aggregate relationship"^^xsd:string ;
        skos:definition   "class that is composed of classes it is connected to by an aggregate relationship"^^xsd:string ;
        skos:inScheme     <MetadataExtensionInformation/code/MD_DatatypeCode> ;
        skos:prefLabel    "aggregateClass" .

<MetadataExtensionInformation/code/MD_DatatypeCode/unionClass>
        a                 iso19115-1_2373:MD_DatatypeCode , skos:Concept ;
        rdfs:isDefinedBy  <http://standards.iso.org/iso/19115/-1/ed-1/en/> ;
        rdfs:label        "union Class" ;
        dct:description   "class describing a selection of one of the specified types"^^xsd:string ;
        skos:definition   "class describing a selection of one of the specified types"^^xsd:string ;
        skos:inScheme     <MetadataExtensionInformation/code/MD_DatatypeCode> ;
        skos:prefLabel    "unionClass" .

<MetadataExtensionInformation/code/MD_DatatypeCode/association>
        a                 iso19115-1_2373:MD_DatatypeCode , skos:Concept ;
        rdfs:isDefinedBy  <http://standards.iso.org/iso/19115/-1/ed-1/en/> ;
        rdfs:label        "association" ;
        dct:description   "semantic relationship between two classes that involves connections among their instances"^^xsd:string ;
        skos:definition   "semantic relationship between two classes that involves connections among their instances"^^xsd:string ;
        skos:inScheme     <MetadataExtensionInformation/code/MD_DatatypeCode> ;
        skos:prefLabel    "association" .

<MetadataExtensionInformation/code/MD_DatatypeCode/codelist>
        a                 iso19115-1_2373:MD_DatatypeCode , skos:Concept ;
        rdfs:isDefinedBy  <http://standards.iso.org/iso/19115/-1/ed-1/en/> ;
        rdfs:label        "codelist" ;
        dct:description   "flexible enumeration useful for expressing a long list of values, can be extended"^^xsd:string ;
        skos:definition   "flexible enumeration useful for expressing a long list of values, can be extended"^^xsd:string ;
        skos:inScheme     <MetadataExtensionInformation/code/MD_DatatypeCode> ;
        skos:prefLabel    "codelist" .

<MetadataExtensionInformation/code/MD_DatatypeCode/interfaceClass>
        a                 iso19115-1_2373:MD_DatatypeCode , skos:Concept ;
        rdfs:isDefinedBy  <http://standards.iso.org/iso/19115/-1/ed-1/en/> ;
        rdfs:label        "interface Class" ;
        dct:description   "named set of operations that characterize the behaviour of an element"^^xsd:string ;
        skos:definition   "named set of operations that characterize the behaviour of an element"^^xsd:string ;
        skos:inScheme     <MetadataExtensionInformation/code/MD_DatatypeCode> ;
        skos:prefLabel    "interfaceClass" .

<MetadataExtensionInformation/code/MD_DatatypeCode/characterString>
        a                 iso19115-1_2373:MD_DatatypeCode , skos:Concept ;
        rdfs:isDefinedBy  <http://standards.iso.org/iso/19115/-1/ed-1/en/> ;
        rdfs:label        "character String" ;
        dct:description   "textual information"^^xsd:string ;
        skos:definition   "textual information"^^xsd:string ;
        skos:inScheme     <MetadataExtensionInformation/code/MD_DatatypeCode> ;
        skos:prefLabel    "characterString" .
