@base          <http://def.isotc211.org/iso19115/-1/2014/Metadata-Fundamentals> .
@prefix dc:    <http://purl.org/dc/elements/1.1/> .
@prefix dct:   <http://purl.org/dc/terms/> .
@prefix owl:   <http://www.w3.org/2002/07/owl#> .
@prefix rdf:   <http://www.w3.org/1999/02/22-rdf-syntax-ns#> .
@prefix rdfs:  <http://www.w3.org/2000/01/rdf-schema#> .
@prefix reg:    <http://purl.org/linked-data/registry#>.
@prefix skos:  <http://www.w3.org/2004/02/skos/core#> .

@prefix application: <http://def.isotc211.org/iso19115/-1/2014/ApplicationSchemaInformation#> .
@prefix citation: <http://def.isotc211.org/iso19115/-1/2014/CitationAndResponsiblePartyInformation#> .
@prefix common: <http://def.isotc211.org/iso19115/-1/2014/CommonClasses#> .
@prefix constraint: <http://def.isotc211.org/iso19115/-1/2014/ConstraintInformation#> .
@prefix content: <http://def.isotc211.org/iso19115/-1/2014/ContentInformation#> .
@prefix crs:   <http://def.isotc211.org/iso19111/2007/CoordinateReferenceSystems#> .
@prefix distribution: <http://def.isotc211.org/iso19115/-1/2014/DistributionInformation#> .
@prefix extended: <http://def.isotc211.org/iso19115/-1/2014/ExampleOfExtendedMatadata#> .
@prefix extent: <http://def.isotc211.org/iso19115/-1/2014/ExtentInformation#> .
@prefix fc:    <http://def.isotc211.org/iso19110/2005/MethodologyForFeatureCataloguing#> .
@prefix fundamentals: <http://def.isotc211.org/iso19115/-1/2014/Metadata-Fundamentals#> .
@prefix identification: <http://def.isotc211.org/iso19115/-1/2014/IdentificationInformation#> .
@prefix lineage: <http://def.isotc211.org/iso19115/-1/2014/LineageInformation#> .
@prefix localization: <http://def.isotc211.org/iso19115/-1/2014/Language-CharactersetLocalizationInformation#> .
@prefix maintenance: <http://def.isotc211.org/iso19115/-1/2014/MaintenanceInformation#> .
@prefix metapp: <http://def.isotc211.org/iso19115/-1/2014/MetadataApplicationInformation#> .
@prefix metext: <http://def.isotc211.org/iso19115/-1/2014/MetadataExtensionInformation#> .
@prefix metinf: <http://def.isotc211.org/iso19115/-1/2014/MetadataInformation#> .
@prefix portrayal: <http://def.isotc211.org/iso19115/-1/2014/PortrayalCatalogueInformation#> .
@prefix rs:    <http://def.isotc211.org/iso19115/-1/2014/ReferenceSystemInformation#> .
@prefix service: <http://def.isotc211.org/iso19115/-1/2014/ServiceMetadataInformation#> . 
@prefix sr:    <http://def.isotc211.org/iso19115/-1/2014/SpatialRepresentationInformation#> .

@prefix iso00639_65: <http://def.isotc211.org/iso00639/-2/LanguageCodes#> .
@prefix iso19110_2259: <http://def.isotc211.org/iso19110/2005/MethodologyForFeatureCataloguing#> .
@prefix iso19107_2211: <http://def.isotc211.org/iso19107/2003/GeometryRoot#> .
@prefix iso19107_2210: <http://def.isotc211.org/iso19107/2003/GeometricPrimitive#> .
@prefix iso19115-1Code: <http://def.isotc211.org/iso19115/-1/2014/CitationAndResponsiblePartyInformation/code/> .
@prefix iso19108_891: <http://def.isotc211.org/iso19108/2006/TemporalObjects#> .
@prefix iso19139_709: <http://def.isotc211.org/iso19139/2007/CulturalAndLinguisticAdapdability#> .
@prefix iso19115-1: <http://def.isotc211.org/iso19115/-1/2014/CitationAndResponsiblePartyInformation#> .
@prefix iso19111_1300: <http://def.isotc211.org/iso19111/2007/CoordinateReferenceSystems#> .
@prefix iso19103_2176: <http://def.isotc211.org/iso19103/2015/RecordTypes#> .
@prefix iso19103_2174: <http://def.isotc211.org/iso19103/2015/NameTypes#> .
@prefix iso03166_66: <http://def.isotc211.org/iso03166/-1/CountryCodes#> .
@prefix iso19115-1_2364: <http://def.isotc211.org/iso19115/-1/2014/ConstraintInformation#> .
@prefix iso19115-1_2376: <http://def.isotc211.org/iso19115/-1/2014/SpatialRepresentationInformation#> .
@prefix iso19115-1_2375: <http://def.isotc211.org/iso19115/-1/2014/ReferenceSystemInformation#> .
@prefix iso19115-1_2365: <http://def.isotc211.org/iso19115/-1/2014/ContentInformation#> .
@prefix iso19115-1_2374: <http://def.isotc211.org/iso19115/-1/2014/PortrayalCatalogueInformation#> .
@prefix iso19115-1_2362: <http://def.isotc211.org/iso19115/-1/2014/ApplicationSchemaInformation#> .
@prefix iso19115-1_2363: <http://def.isotc211.org/iso19115/-1/2014/CitationAndResponsiblePartyInformation#> .
@prefix iso19115-1_2373: <http://def.isotc211.org/iso19115/-1/2014/MetadataExtensionInformation#> .
@prefix iso19115-1_2368: <http://def.isotc211.org/iso19115/-1/2014/ExtentInformation#> .
@prefix iso19115-1_2369: <http://def.isotc211.org/iso19115/-1/2014/IdentificationInformation#> .
@prefix iso19115-1_2366: <http://def.isotc211.org/iso19115/-1/2014/LineageInformation#> .
@prefix iso19103_2178: <http://def.isotc211.org/iso19103/2015/WebEnvironment#> .
@prefix iso19115-1_2367: <http://def.isotc211.org/iso19115/-1/2014/DistributionInformation#> .
@prefix iso19103_2179: <http://def.isotc211.org/iso19103/2015/MeasureTypes#> .
@prefix iso19157_1164: <http://def.isotc211.org/iso19157/2013/DataQuality#> .
@prefix iso19115-1_2371: <http://def.isotc211.org/iso19115/-1/2014/MetadataApplicationInformation#> .
@prefix iso19115-1_2360: <http://def.isotc211.org/iso19115/-1/2014/Language-CharactersetLocalizationInformation#> .
@prefix iso19115-1_2372: <http://def.isotc211.org/iso19115/-1/2014/MetadataInformation#> .
@prefix iso19115-1_2370: <http://def.isotc211.org/iso19115/-1/2014/MaintenanceInformation#> .
@prefix iso19150-2: <http://def.isotc211.org/iso19150/-2/2012/base#> .
@prefix iso19115-1_2358: <http://def.isotc211.org/iso19115/-1/2014/CommonClasses#> .


<IdentificationInformation/code/MD_KeywordTypeCode/taxon>
        a                 iso19115-1_2369:MD_KeywordTypeCode , skos:Concept ;
        rdfs:isDefinedBy  <http://standards.iso.org/iso/19115/-1/ed-1/en/> ;
        rdfs:label        "taxon" ;
        dct:description   "keyword identifies a taxonomy of the resource"^^xsd:string ;
        skos:definition   "keyword identifies a taxonomy of the resource"^^xsd:string ;
        skos:inScheme     <IdentificationInformation/code/MD_KeywordTypeCode> ;
        skos:prefLabel    "taxon" .

<IdentificationInformation/code/MD_KeywordTypeCode/dataCentre>
        a                 iso19115-1_2369:MD_KeywordTypeCode , skos:Concept ;
        rdfs:isDefinedBy  <http://standards.iso.org/iso/19115/-1/ed-1/en/> ;
        rdfs:label        "data Centre" ;
        dct:description   "keyword identifies a repository or archive that manages and distributes data"^^xsd:string ;
        skos:definition   "keyword identifies a repository or archive that manages and distributes data"^^xsd:string ;
        skos:inScheme     <IdentificationInformation/code/MD_KeywordTypeCode> ;
        skos:prefLabel    "dataCentre" .

<IdentificationInformation/code/MD_KeywordTypeCode/project>
        a                 iso19115-1_2369:MD_KeywordTypeCode , skos:Concept ;
        rdfs:isDefinedBy  <http://standards.iso.org/iso/19115/-1/ed-1/en/> ;
        rdfs:label        "project" ;
        dct:description   "keyword identifies an endeavour undertaken to create or modify a product or service"^^xsd:string ;
        skos:definition   "keyword identifies an endeavour undertaken to create or modify a product or service"^^xsd:string ;
        skos:inScheme     <IdentificationInformation/code/MD_KeywordTypeCode> ;
        skos:prefLabel    "project" .

<IdentificationInformation/code/MD_KeywordTypeCode/instrument>
        a                 iso19115-1_2369:MD_KeywordTypeCode , skos:Concept ;
        rdfs:isDefinedBy  <http://standards.iso.org/iso/19115/-1/ed-1/en/> ;
        rdfs:label        "instrument" ;
        dct:description   "keyword identifies a device used to measure or compare physical properties"^^xsd:string ;
        skos:definition   "keyword identifies a device used to measure or compare physical properties"^^xsd:string ;
        skos:inScheme     <IdentificationInformation/code/MD_KeywordTypeCode> ;
        skos:prefLabel    "instrument" .

<IdentificationInformation/code/MD_KeywordTypeCode/process>
        a                 iso19115-1_2369:MD_KeywordTypeCode , skos:Concept ;
        rdfs:isDefinedBy  <http://standards.iso.org/iso/19115/-1/ed-1/en/> ;
        rdfs:label        "process" ;
        dct:description   "keyword identifies a series of actions or natural occurrences"^^xsd:string ;
        skos:definition   "keyword identifies a series of actions or natural occurrences"^^xsd:string ;
        skos:inScheme     <IdentificationInformation/code/MD_KeywordTypeCode> ;
        skos:prefLabel    "process" .

<IdentificationInformation/code/MD_KeywordTypeCode/platform>
        a                 iso19115-1_2369:MD_KeywordTypeCode , skos:Concept ;
        rdfs:isDefinedBy  <http://standards.iso.org/iso/19115/-1/ed-1/en/> ;
        rdfs:label        "platform" ;
        dct:description   "keyword identifies a structure upon which an instrument is mounted"^^xsd:string ;
        skos:definition   "keyword identifies a structure upon which an instrument is mounted"^^xsd:string ;
        skos:inScheme     <IdentificationInformation/code/MD_KeywordTypeCode> ;
        skos:prefLabel    "platform" .

<IdentificationInformation/code/MD_KeywordTypeCode/subTopicCategory>
        a                 iso19115-1_2369:MD_KeywordTypeCode , skos:Concept ;
        rdfs:isDefinedBy  <http://standards.iso.org/iso/19115/-1/ed-1/en/> ;
        rdfs:label        "sub Topic Category" ;
        dct:description   "refinement of a topic category for the purpose of geographic data classification"^^xsd:string ;
        skos:definition   "refinement of a topic category for the purpose of geographic data classification"^^xsd:string ;
        skos:inScheme     <IdentificationInformation/code/MD_KeywordTypeCode> ;
        skos:prefLabel    "subTopicCategory" .

<IdentificationInformation/code/MD_KeywordTypeCode/place>
        a                 iso19115-1_2369:MD_KeywordTypeCode , skos:Concept ;
        rdfs:isDefinedBy  <http://standards.iso.org/iso/19115/-1/ed-1/en/> ;
        rdfs:label        "place" ;
        dct:description   "keyword identifies a location"^^xsd:string ;
        skos:definition   "keyword identifies a location"^^xsd:string ;
        skos:inScheme     <IdentificationInformation/code/MD_KeywordTypeCode> ;
        skos:prefLabel    "place" .

<IdentificationInformation/code/MD_KeywordTypeCode/featureType>
        a                 iso19115-1_2369:MD_KeywordTypeCode , skos:Concept ;
        rdfs:isDefinedBy  <http://standards.iso.org/iso/19115/-1/ed-1/en/> ;
        rdfs:label        "feature Type" ;
        dct:description   "keyword identifies a resource containing or about a collection of feature instances with common characteristics"^^xsd:string ;
        skos:definition   "keyword identifies a resource containing or about a collection of feature instances with common characteristics"^^xsd:string ;
        skos:inScheme     <IdentificationInformation/code/MD_KeywordTypeCode> ;
        skos:prefLabel    "featureType" .

<IdentificationInformation/code/MD_KeywordTypeCode/temporal>
        a                 iso19115-1_2369:MD_KeywordTypeCode , skos:Concept ;
        rdfs:isDefinedBy  <http://standards.iso.org/iso/19115/-1/ed-1/en/> ;
        rdfs:label        "temporal" ;
        dct:description   "keyword identifies a time period related to the resource"^^xsd:string ;
        skos:definition   "keyword identifies a time period related to the resource"^^xsd:string ;
        skos:inScheme     <IdentificationInformation/code/MD_KeywordTypeCode> ;
        skos:prefLabel    "temporal" .

<IdentificationInformation/code/MD_KeywordTypeCode/service>
        a                 iso19115-1_2369:MD_KeywordTypeCode , skos:Concept ;
        rdfs:isDefinedBy  <http://standards.iso.org/iso/19115/-1/ed-1/en/> ;
        rdfs:label        "service" ;
        dct:description   "keyword identifies an activity carried out by one party for the benefit of another"^^xsd:string ;
        skos:definition   "keyword identifies an activity carried out by one party for the benefit of another"^^xsd:string ;
        skos:inScheme     <IdentificationInformation/code/MD_KeywordTypeCode> ;
        skos:prefLabel    "service" .

<IdentificationInformation/code/MD_KeywordTypeCode/product>
        a                 iso19115-1_2369:MD_KeywordTypeCode , skos:Concept ;
        rdfs:isDefinedBy  <http://standards.iso.org/iso/19115/-1/ed-1/en/> ;
        rdfs:label        "product" ;
        dct:description   "keyword identifies a type of product"^^xsd:string ;
        skos:definition   "keyword identifies a type of product"^^xsd:string ;
        skos:inScheme     <IdentificationInformation/code/MD_KeywordTypeCode> ;
        skos:prefLabel    "product" .

<IdentificationInformation/code/MD_KeywordTypeCode/stratum>
        a                 iso19115-1_2369:MD_KeywordTypeCode , skos:Concept ;
        rdfs:isDefinedBy  <http://standards.iso.org/iso/19115/-1/ed-1/en/> ;
        rdfs:label        "stratum" ;
        dct:description   "keyword identifies the layer(s) of any deposited substance or levels within an ordered system"^^xsd:string ;
        skos:definition   "keyword identifies the layer(s) of any deposited substance or levels within an ordered system"^^xsd:string ;
        skos:inScheme     <IdentificationInformation/code/MD_KeywordTypeCode> ;
        skos:prefLabel    "stratum" .

<IdentificationInformation/code/MD_KeywordTypeCode/discipline>
        a                 iso19115-1_2369:MD_KeywordTypeCode , skos:Concept ;
        rdfs:isDefinedBy  <http://standards.iso.org/iso/19115/-1/ed-1/en/> ;
        rdfs:label        "discipline" ;
        dct:description   "keyword identifies a branch of instruction or specialized learning"^^xsd:string ;
        skos:definition   "keyword identifies a branch of instruction or specialized learning"^^xsd:string ;
        skos:inScheme     <IdentificationInformation/code/MD_KeywordTypeCode> ;
        skos:prefLabel    "discipline" .

<IdentificationInformation/code/MD_KeywordTypeCode/theme>
        a                 iso19115-1_2369:MD_KeywordTypeCode , skos:Concept ;
        rdfs:isDefinedBy  <http://standards.iso.org/iso/19115/-1/ed-1/en/> ;
        rdfs:label        "theme" ;
        dct:description   "keyword identifies a particular subject or topic"^^xsd:string ;
        skos:definition   "keyword identifies a particular subject or topic"^^xsd:string ;
        skos:inScheme     <IdentificationInformation/code/MD_KeywordTypeCode> ;
        skos:prefLabel    "theme" .
