@base          <http://def.isotc211.org/iso19115/-1/2014/Metadata-Fundamentals> .
@prefix dc:    <http://purl.org/dc/elements/1.1/> .
@prefix dct:   <http://purl.org/dc/terms/> .
@prefix owl:   <http://www.w3.org/2002/07/owl#> .
@prefix rdf:   <http://www.w3.org/1999/02/22-rdf-syntax-ns#> .
@prefix rdfs:  <http://www.w3.org/2000/01/rdf-schema#> .
@prefix reg:    <http://purl.org/linked-data/registry#>.
@prefix skos:  <http://www.w3.org/2004/02/skos/core#> .

@prefix application: <http://def.isotc211.org/iso19115/-1/2014/ApplicationSchemaInformation#> .
@prefix citation: <http://def.isotc211.org/iso19115/-1/2014/CitationAndResponsiblePartyInformation#> .
@prefix common: <http://def.isotc211.org/iso19115/-1/2014/CommonClasses#> .
@prefix constraint: <http://def.isotc211.org/iso19115/-1/2014/ConstraintInformation#> .
@prefix content: <http://def.isotc211.org/iso19115/-1/2014/ContentInformation#> .
@prefix crs:   <http://def.isotc211.org/iso19111/2007/CoordinateReferenceSystems#> .
@prefix distribution: <http://def.isotc211.org/iso19115/-1/2014/DistributionInformation#> .
@prefix extended: <http://def.isotc211.org/iso19115/-1/2014/ExampleOfExtendedMatadata#> .
@prefix extent: <http://def.isotc211.org/iso19115/-1/2014/ExtentInformation#> .
@prefix fc:    <http://def.isotc211.org/iso19110/2005/MethodologyForFeatureCataloguing#> .
@prefix fundamentals: <http://def.isotc211.org/iso19115/-1/2014/Metadata-Fundamentals#> .
@prefix identification: <http://def.isotc211.org/iso19115/-1/2014/IdentificationInformation#> .
@prefix lineage: <http://def.isotc211.org/iso19115/-1/2014/LineageInformation#> .
@prefix localization: <http://def.isotc211.org/iso19115/-1/2014/Language-CharactersetLocalizationInformation#> .
@prefix maintenance: <http://def.isotc211.org/iso19115/-1/2014/MaintenanceInformation#> .
@prefix metapp: <http://def.isotc211.org/iso19115/-1/2014/MetadataApplicationInformation#> .
@prefix metext: <http://def.isotc211.org/iso19115/-1/2014/MetadataExtensionInformation#> .
@prefix metinf: <http://def.isotc211.org/iso19115/-1/2014/MetadataInformation#> .
@prefix portrayal: <http://def.isotc211.org/iso19115/-1/2014/PortrayalCatalogueInformation#> .
@prefix rs:    <http://def.isotc211.org/iso19115/-1/2014/ReferenceSystemInformation#> .
@prefix service: <http://def.isotc211.org/iso19115/-1/2014/ServiceMetadataInformation#> . 
@prefix sr:    <http://def.isotc211.org/iso19115/-1/2014/SpatialRepresentationInformation#> .

@prefix iso00639_65: <http://def.isotc211.org/iso00639/-2/LanguageCodes#> .
@prefix iso19110_2259: <http://def.isotc211.org/iso19110/2005/MethodologyForFeatureCataloguing#> .
@prefix iso19107_2211: <http://def.isotc211.org/iso19107/2003/GeometryRoot#> .
@prefix iso19107_2210: <http://def.isotc211.org/iso19107/2003/GeometricPrimitive#> .
@prefix iso19115-1Code: <http://def.isotc211.org/iso19115/-1/2014/CitationAndResponsiblePartyInformation/code/> .
@prefix iso19108_891: <http://def.isotc211.org/iso19108/2006/TemporalObjects#> .
@prefix iso19139_709: <http://def.isotc211.org/iso19139/2007/CulturalAndLinguisticAdapdability#> .
@prefix iso19115-1: <http://def.isotc211.org/iso19115/-1/2014/CitationAndResponsiblePartyInformation#> .
@prefix iso19111_1300: <http://def.isotc211.org/iso19111/2007/CoordinateReferenceSystems#> .
@prefix iso19103_2176: <http://def.isotc211.org/iso19103/2015/RecordTypes#> .
@prefix iso19103_2174: <http://def.isotc211.org/iso19103/2015/NameTypes#> .
@prefix iso03166_66: <http://def.isotc211.org/iso03166/-1/CountryCodes#> .
@prefix iso19115-1_2364: <http://def.isotc211.org/iso19115/-1/2014/ConstraintInformation#> .
@prefix iso19115-1_2376: <http://def.isotc211.org/iso19115/-1/2014/SpatialRepresentationInformation#> .
@prefix iso19115-1_2375: <http://def.isotc211.org/iso19115/-1/2014/ReferenceSystemInformation#> .
@prefix iso19115-1_2365: <http://def.isotc211.org/iso19115/-1/2014/ContentInformation#> .
@prefix iso19115-1_2374: <http://def.isotc211.org/iso19115/-1/2014/PortrayalCatalogueInformation#> .
@prefix iso19115-1_2362: <http://def.isotc211.org/iso19115/-1/2014/ApplicationSchemaInformation#> .
@prefix iso19115-1_2363: <http://def.isotc211.org/iso19115/-1/2014/CitationAndResponsiblePartyInformation#> .
@prefix iso19115-1_2373: <http://def.isotc211.org/iso19115/-1/2014/MetadataExtensionInformation#> .
@prefix iso19115-1_2368: <http://def.isotc211.org/iso19115/-1/2014/ExtentInformation#> .
@prefix iso19115-1_2369: <http://def.isotc211.org/iso19115/-1/2014/IdentificationInformation#> .
@prefix iso19115-1_2366: <http://def.isotc211.org/iso19115/-1/2014/LineageInformation#> .
@prefix iso19103_2178: <http://def.isotc211.org/iso19103/2015/WebEnvironment#> .
@prefix iso19115-1_2367: <http://def.isotc211.org/iso19115/-1/2014/DistributionInformation#> .
@prefix iso19103_2179: <http://def.isotc211.org/iso19103/2015/MeasureTypes#> .
@prefix iso19157_1164: <http://def.isotc211.org/iso19157/2013/DataQuality#> .
@prefix iso19115-1_2371: <http://def.isotc211.org/iso19115/-1/2014/MetadataApplicationInformation#> .
@prefix iso19115-1_2360: <http://def.isotc211.org/iso19115/-1/2014/Language-CharactersetLocalizationInformation#> .
@prefix iso19115-1_2372: <http://def.isotc211.org/iso19115/-1/2014/MetadataInformation#> .
@prefix iso19115-1_2370: <http://def.isotc211.org/iso19115/-1/2014/MaintenanceInformation#> .
@prefix iso19150-2: <http://def.isotc211.org/iso19150/-2/2012/base#> .
@prefix iso19115-1_2358: <http://def.isotc211.org/iso19115/-1/2014/CommonClasses#> .


<ReferenceSystemInformation/code/MD_ReferenceSystemTypeCode/parametric>
        a                 iso19115-1_2375:MD_ReferenceSystemTypeCode , skos:Concept ;
        rdfs:isDefinedBy  <http://standards.iso.org/iso/19115/-1/ed-1/en/> ;
        rdfs:label        "parametric" ;
        dct:description   "coordinate reference system based on a parametric datum (datum describing the relationship of a parametric coordinate system to an object) \r\n\r\nEXAMPLE pressure"^^xsd:string ;
        skos:definition   "coordinate reference system based on a parametric datum (datum describing the relationship of a parametric coordinate system to an object) \r\n\r\nEXAMPLE pressure"^^xsd:string ;
        skos:inScheme     <ReferenceSystemInformation/code/MD_ReferenceSystemTypeCode> ;
        skos:prefLabel    "parametric" .

<ReferenceSystemInformation/code/MD_ReferenceSystemTypeCode/vertical>
        a                 iso19115-1_2375:MD_ReferenceSystemTypeCode , skos:Concept ;
        rdfs:isDefinedBy  <http://standards.iso.org/iso/19115/-1/ed-1/en/> ;
        rdfs:label        "vertical" ;
        dct:description   "one-dimensional coordinate reference system based on a vertical datum (datum describing the relation of gravity-related heights or depths to the Earth) \r\n\r\nEXAMPLE [gravity-related] height or depth"^^xsd:string ;
        skos:definition   "one-dimensional coordinate reference system based on a vertical datum (datum describing the relation of gravity-related heights or depths to the Earth) \r\n\r\nEXAMPLE [gravity-related] height or depth"^^xsd:string ;
        skos:inScheme     <ReferenceSystemInformation/code/MD_ReferenceSystemTypeCode> ;
        skos:prefLabel    "vertical" .

<ReferenceSystemInformation/code/MD_ReferenceSystemTypeCode/geodeticGeographic3D>
        a                 iso19115-1_2375:MD_ReferenceSystemTypeCode , skos:Concept ;
        rdfs:isDefinedBy  <http://standards.iso.org/iso/19115/-1/ed-1/en/> ;
        rdfs:label        "geodetic Geographic 3D" ;
        dct:description   "geodetic CRS having an ellipsoidal 3D coordinate system \r\n\r\nEXAMPLE latitude, longitude, ellipsoidal height"^^xsd:string ;
        skos:definition   "geodetic CRS having an ellipsoidal 3D coordinate system \r\n\r\nEXAMPLE latitude, longitude, ellipsoidal height"^^xsd:string ;
        skos:inScheme     <ReferenceSystemInformation/code/MD_ReferenceSystemTypeCode> ;
        skos:prefLabel    "geodeticGeographic3D" .

<ReferenceSystemInformation/code/MD_ReferenceSystemTypeCode/compoundGeographic3DTemporal>
        a                 iso19115-1_2375:MD_ReferenceSystemTypeCode , skos:Concept ;
        rdfs:isDefinedBy  <http://standards.iso.org/iso/19115/-1/ed-1/en/> ;
        rdfs:label        "compound Geographic 3D Temporal" ;
        dct:description   "compound spatio-temporal coordinate reference system containing a 3 dimensional geographic and a temporal coordinate reference system \r\n\r\nEXAMPLE latitude, longitude, ellipsoidal height, time"^^xsd:string ;
        skos:definition   "compound spatio-temporal coordinate reference system containing a 3 dimensional geographic and a temporal coordinate reference system \r\n\r\nEXAMPLE latitude, longitude, ellipsoidal height, time"^^xsd:string ;
        skos:inScheme     <ReferenceSystemInformation/code/MD_ReferenceSystemTypeCode> ;
        skos:prefLabel    "compoundGeographic3DTemporal" .

<ReferenceSystemInformation/code/MD_ReferenceSystemTypeCode/compoundProjectedVertical>
        a                 iso19115-1_2375:MD_ReferenceSystemTypeCode , skos:Concept ;
        rdfs:isDefinedBy  <http://standards.iso.org/iso/19115/-1/ed-1/en/> ;
        rdfs:label        "compound Projected Vertical" ;
        dct:description   "compound spatial reference system containing a horizontal projected coordinate reference system and a vertical coordinate reference system \r\n\r\nEXAMPLE easting, northing, [gravity-related] height or depth"^^xsd:string ;
        skos:definition   "compound spatial reference system containing a horizontal projected coordinate reference system and a vertical coordinate reference system \r\n\r\nEXAMPLE easting, northing, [gravity-related] height or depth"^^xsd:string ;
        skos:inScheme     <ReferenceSystemInformation/code/MD_ReferenceSystemTypeCode> ;
        skos:prefLabel    "compoundProjectedVertical" .

<ReferenceSystemInformation/code/MD_ReferenceSystemTypeCode/compoundEngineeringVertical>
        a                 iso19115-1_2375:MD_ReferenceSystemTypeCode , skos:Concept ;
        rdfs:isDefinedBy  <http://standards.iso.org/iso/19115/-1/ed-1/en/> ;
        rdfs:label        "compound Engineering Vertical" ;
        dct:description   "compound spatial reference system containing a horizontal engineering coordinate reference system and a vertical coordinate reference system \r\n\r\nEXAMPLE [local] x, y, height"^^xsd:string ;
        skos:definition   "compound spatial reference system containing a horizontal engineering coordinate reference system and a vertical coordinate reference system \r\n\r\nEXAMPLE [local] x, y, height"^^xsd:string ;
        skos:inScheme     <ReferenceSystemInformation/code/MD_ReferenceSystemTypeCode> ;
        skos:prefLabel    "compoundEngineeringVertical" .

<ReferenceSystemInformation/code/MD_ReferenceSystemTypeCode/linear>
        a                 iso19115-1_2375:MD_ReferenceSystemTypeCode , skos:Concept ;
        rdfs:isDefinedBy  <http://standards.iso.org/iso/19115/-1/ed-1/en/> ;
        rdfs:label        "linear" ;
        dct:description   "reference system that identifies a location by reference to a segment of a linear geographic feature and distance along that segment from a given point \r\n\r\nEXAMPLE x km along road"^^xsd:string ;
        skos:definition   "reference system that identifies a location by reference to a segment of a linear geographic feature and distance along that segment from a given point \r\n\r\nEXAMPLE x km along road"^^xsd:string ;
        skos:inScheme     <ReferenceSystemInformation/code/MD_ReferenceSystemTypeCode> ;
        skos:prefLabel    "linear" .

<ReferenceSystemInformation/code/MD_ReferenceSystemTypeCode/compoundEngineeringParametric>
        a                 iso19115-1_2375:MD_ReferenceSystemTypeCode , skos:Concept ;
        rdfs:isDefinedBy  <http://standards.iso.org/iso/19115/-1/ed-1/en/> ;
        rdfs:label        "compound Engineering Parametric" ;
        dct:description   "compound spatio-parametric coordinate reference system containing an engineering coordinate reference system and a parametric reference system \r\n\r\nEXAMPLE [local] x, y, pressure"^^xsd:string ;
        skos:definition   "compound spatio-parametric coordinate reference system containing an engineering coordinate reference system and a parametric reference system \r\n\r\nEXAMPLE [local] x, y, pressure"^^xsd:string ;
        skos:inScheme     <ReferenceSystemInformation/code/MD_ReferenceSystemTypeCode> ;
        skos:prefLabel    "compoundEngineeringParametric" .

<ReferenceSystemInformation/code/MD_ReferenceSystemTypeCode/geodeticGeographic2D>
        a                 iso19115-1_2375:MD_ReferenceSystemTypeCode , skos:Concept ;
        rdfs:isDefinedBy  <http://standards.iso.org/iso/19115/-1/ed-1/en/> ;
        rdfs:label        "geodetic Geographic 2D" ;
        dct:description   "geodetic CRS having an ellipsoidal 2D coordinate system \r\n\r\nEXAMPLE latitude, longitude"^^xsd:string ;
        skos:definition   "geodetic CRS having an ellipsoidal 2D coordinate system \r\n\r\nEXAMPLE latitude, longitude"^^xsd:string ;
        skos:inScheme     <ReferenceSystemInformation/code/MD_ReferenceSystemTypeCode> ;
        skos:prefLabel    "geodeticGeographic2D" .

<ReferenceSystemInformation/code/MD_ReferenceSystemTypeCode/compoundGeographic2DVerticalTemporal>
        a                 iso19115-1_2375:MD_ReferenceSystemTypeCode , skos:Concept ;
        rdfs:isDefinedBy  <http://standards.iso.org/iso/19115/-1/ed-1/en/> ;
        rdfs:label        "compound Geographic 2D Vertical Temporal" ;
        dct:description   "compound spatio-temporal coordinate reference system containing a 2 dimensional geographic horizontal, a vertical, and a temporal coordinate reference system \r\n\r\nEXAMPLE latitude, longitude, height, time"^^xsd:string ;
        skos:definition   "compound spatio-temporal coordinate reference system containing a 2 dimensional geographic horizontal, a vertical, and a temporal coordinate reference system \r\n\r\nEXAMPLE latitude, longitude, height, time"^^xsd:string ;
        skos:inScheme     <ReferenceSystemInformation/code/MD_ReferenceSystemTypeCode> ;
        skos:prefLabel    "compoundGeographic2DVerticalTemporal" .

<ReferenceSystemInformation/code/MD_ReferenceSystemTypeCode/engineeringDesign>
        a                 iso19115-1_2375:MD_ReferenceSystemTypeCode , skos:Concept ;
        rdfs:isDefinedBy  <http://standards.iso.org/iso/19115/-1/ed-1/en/> ;
        rdfs:label        "engineering Design" ;
        dct:description   "engineering coordinate reference system in which the base representation of a moving object is specified \r\n\r\nEXAMPLE [local] x,y"^^xsd:string ;
        skos:definition   "engineering coordinate reference system in which the base representation of a moving object is specified \r\n\r\nEXAMPLE [local] x,y"^^xsd:string ;
        skos:inScheme     <ReferenceSystemInformation/code/MD_ReferenceSystemTypeCode> ;
        skos:prefLabel    "engineeringDesign" .

<ReferenceSystemInformation/code/MD_ReferenceSystemTypeCode/compoundEngineeringParametricTemporal>
        a                 iso19115-1_2375:MD_ReferenceSystemTypeCode , skos:Concept ;
        rdfs:isDefinedBy  <http://standards.iso.org/iso/19115/-1/ed-1/en/> ;
        rdfs:label        "compound Engineering Parametric Temporal" ;
        dct:description   "compound spatio-parametric-temporal coordinate reference system containing an engineering, a parametric, and a temporal coordinate reference system \r\n\r\nEXAMPLE [local] x, y, pressure, time"^^xsd:string ;
        skos:definition   "compound spatio-parametric-temporal coordinate reference system containing an engineering, a parametric, and a temporal coordinate reference system \r\n\r\nEXAMPLE [local] x, y, pressure, time"^^xsd:string ;
        skos:inScheme     <ReferenceSystemInformation/code/MD_ReferenceSystemTypeCode> ;
        skos:prefLabel    "compoundEngineeringParametricTemporal" .

<ReferenceSystemInformation/code/MD_ReferenceSystemTypeCode/engineering>
        a                 iso19115-1_2375:MD_ReferenceSystemTypeCode , skos:Concept ;
        rdfs:isDefinedBy  <http://standards.iso.org/iso/19115/-1/ed-1/en/> ;
        rdfs:label        "engineering" ;
        dct:description   "coordinate reference system based on an engineering datum (datum describing the relationship of a coordinate system to a local reference) \r\n\r\nEXAMPLE [local] x,y"^^xsd:string ;
        skos:definition   "coordinate reference system based on an engineering datum (datum describing the relationship of a coordinate system to a local reference) \r\n\r\nEXAMPLE [local] x,y"^^xsd:string ;
        skos:inScheme     <ReferenceSystemInformation/code/MD_ReferenceSystemTypeCode> ;
        skos:prefLabel    "engineering" .

<ReferenceSystemInformation/code/MD_ReferenceSystemTypeCode/compoundProjected2DParametric>
        a                 iso19115-1_2375:MD_ReferenceSystemTypeCode , skos:Concept ;
        rdfs:isDefinedBy  <http://standards.iso.org/iso/19115/-1/ed-1/en/> ;
        rdfs:label        "compound Projected 2D Parametric" ;
        dct:description   "compound spatio-parametric coordinate reference system containing a projected horizontal coordinate reference system and a parametric reference system \r\n\r\nEXAMPLE easting, northing, density"^^xsd:string ;
        skos:definition   "compound spatio-parametric coordinate reference system containing a projected horizontal coordinate reference system and a parametric reference system \r\n\r\nEXAMPLE easting, northing, density"^^xsd:string ;
        skos:inScheme     <ReferenceSystemInformation/code/MD_ReferenceSystemTypeCode> ;
        skos:prefLabel    "compoundProjected2DParametric" .

<ReferenceSystemInformation/code/MD_ReferenceSystemTypeCode/geographicIdentifier>
        a                 iso19115-1_2375:MD_ReferenceSystemTypeCode , skos:Concept ;
        rdfs:isDefinedBy  <http://standards.iso.org/iso/19115/-1/ed-1/en/> ;
        rdfs:label        "geographic Identifier" ;
        dct:description   "spatial reference in the form of a label or code that identifies a location \r\n\r\nEXAMPLE post code"^^xsd:string ;
        skos:definition   "spatial reference in the form of a label or code that identifies a location \r\n\r\nEXAMPLE post code"^^xsd:string ;
        skos:inScheme     <ReferenceSystemInformation/code/MD_ReferenceSystemTypeCode> ;
        skos:prefLabel    "geographicIdentifier" .

<ReferenceSystemInformation/code/MD_ReferenceSystemTypeCode/temporal>
        a                 iso19115-1_2375:MD_ReferenceSystemTypeCode , skos:Concept ;
        rdfs:isDefinedBy  <http://standards.iso.org/iso/19115/-1/ed-1/en/> ;
        rdfs:label        "temporal" ;
        dct:description   "reference system against which time is measured \r\n\r\nEXAMPLE time"^^xsd:string ;
        skos:definition   "reference system against which time is measured \r\n\r\nEXAMPLE time"^^xsd:string ;
        skos:inScheme     <ReferenceSystemInformation/code/MD_ReferenceSystemTypeCode> ;
        skos:prefLabel    "temporal" .

<ReferenceSystemInformation/code/MD_ReferenceSystemTypeCode/compoundProjectedTemporal>
        a                 iso19115-1_2375:MD_ReferenceSystemTypeCode , skos:Concept ;
        rdfs:isDefinedBy  <http://standards.iso.org/iso/19115/-1/ed-1/en/> ;
        rdfs:label        "compound Projected Temporal" ;
        dct:description   "compound spatio-temporal coordinate reference system containing a projected horizontal and a temporal coordinate reference system \r\n\r\nEXAMPLE easting, northing, time"^^xsd:string ;
        skos:definition   "compound spatio-temporal coordinate reference system containing a projected horizontal and a temporal coordinate reference system \r\n\r\nEXAMPLE easting, northing, time"^^xsd:string ;
        skos:inScheme     <ReferenceSystemInformation/code/MD_ReferenceSystemTypeCode> ;
        skos:prefLabel    "compoundProjectedTemporal" .

<ReferenceSystemInformation/code/MD_ReferenceSystemTypeCode/compoundGeographic2DParametricTemporal>
        a                 iso19115-1_2375:MD_ReferenceSystemTypeCode , skos:Concept ;
        rdfs:isDefinedBy  <http://standards.iso.org/iso/19115/-1/ed-1/en/> ;
        rdfs:label        "compound Geographic 2D Parametric Temporal" ;
        dct:description   "compound spatio-parametric-temporal coordinate reference system containing a 2 dimensional geographic horizontal, a parametric and a temporal coordinate reference system \r\n\r\nEXAMPLE latitude, longitude, pressure, time"^^xsd:string ;
        skos:definition   "compound spatio-parametric-temporal coordinate reference system containing a 2 dimensional geographic horizontal, a parametric and a temporal coordinate reference system \r\n\r\nEXAMPLE latitude, longitude, pressure, time"^^xsd:string ;
        skos:inScheme     <ReferenceSystemInformation/code/MD_ReferenceSystemTypeCode> ;
        skos:prefLabel    "compoundGeographic2DParametricTemporal" .

<ReferenceSystemInformation/code/MD_ReferenceSystemTypeCode/compoundEngineeringTemporal>
        a                 iso19115-1_2375:MD_ReferenceSystemTypeCode , skos:Concept ;
        rdfs:isDefinedBy  <http://standards.iso.org/iso/19115/-1/ed-1/en/> ;
        rdfs:label        "compound Engineering Temporal" ;
        dct:description   "compound spatio-temporal coordinate reference system containing an engineering and a temporal coordinate reference system \r\n\r\nEXAMPLE [local] x, y, time"^^xsd:string ;
        skos:definition   "compound spatio-temporal coordinate reference system containing an engineering and a temporal coordinate reference system \r\n\r\nEXAMPLE [local] x, y, time"^^xsd:string ;
        skos:inScheme     <ReferenceSystemInformation/code/MD_ReferenceSystemTypeCode> ;
        skos:prefLabel    "compoundEngineeringTemporal" .

<ReferenceSystemInformation/code/MD_ReferenceSystemTypeCode/compoundGeographic2DVertical>
        a                 iso19115-1_2375:MD_ReferenceSystemTypeCode , skos:Concept ;
        rdfs:isDefinedBy  <http://standards.iso.org/iso/19115/-1/ed-1/en/> ;
        rdfs:label        "compound Geographic 2D Vertical" ;
        dct:description   "compound coordinate reference system in which one constituent coordinate reference system is a horizontal geodetic coordinate reference system and one is a vertical coordinate reference system \r\n\r\nEXAMPLE latitude, longitude, [gravity-related] height or depth"^^xsd:string ;
        skos:definition   "compound coordinate reference system in which one constituent coordinate reference system is a horizontal geodetic coordinate reference system and one is a vertical coordinate reference system \r\n\r\nEXAMPLE latitude, longitude, [gravity-related] height or depth"^^xsd:string ;
        skos:inScheme     <ReferenceSystemInformation/code/MD_ReferenceSystemTypeCode> ;
        skos:prefLabel    "compoundGeographic2DVertical" .

<ReferenceSystemInformation/code/MD_ReferenceSystemTypeCode/projected>
        a                 iso19115-1_2375:MD_ReferenceSystemTypeCode , skos:Concept ;
        rdfs:isDefinedBy  <http://standards.iso.org/iso/19115/-1/ed-1/en/> ;
        rdfs:label        "projected" ;
        dct:description   "coordinate reference system derived from a two-dimensional geodetic coordinate reference system by applying a map projection \r\n\r\nEXAMPLE easting, northing"^^xsd:string ;
        skos:definition   "coordinate reference system derived from a two-dimensional geodetic coordinate reference system by applying a map projection \r\n\r\nEXAMPLE easting, northing"^^xsd:string ;
        skos:inScheme     <ReferenceSystemInformation/code/MD_ReferenceSystemTypeCode> ;
        skos:prefLabel    "projected" .

<ReferenceSystemInformation/code/MD_ReferenceSystemTypeCode/compoundEngineeringVerticalTemporal>
        a                 iso19115-1_2375:MD_ReferenceSystemTypeCode , skos:Concept ;
        rdfs:isDefinedBy  <http://standards.iso.org/iso/19115/-1/ed-1/en/> ;
        rdfs:label        "compound Engineering Vertical Temporal" ;
        dct:description   "compound spatio-temporal coordinate reference system containing an engineering, a vertical, and a temporal coordinate reference system \r\n\r\nEXAMPLE [local] x, y, height, time"^^xsd:string ;
        skos:definition   "compound spatio-temporal coordinate reference system containing an engineering, a vertical, and a temporal coordinate reference system \r\n\r\nEXAMPLE [local] x, y, height, time"^^xsd:string ;
        skos:inScheme     <ReferenceSystemInformation/code/MD_ReferenceSystemTypeCode> ;
        skos:prefLabel    "compoundEngineeringVerticalTemporal" .

<ReferenceSystemInformation/code/MD_ReferenceSystemTypeCode/compoundProjectedVerticalTemporal>
        a                 iso19115-1_2375:MD_ReferenceSystemTypeCode , skos:Concept ;
        rdfs:isDefinedBy  <http://standards.iso.org/iso/19115/-1/ed-1/en/> ;
        rdfs:label        "compound Projected Vertical Temporal" ;
        dct:description   "compound spatio-temporal coordinate reference system containing a projected horizontal, a vertical, and a temporal coordinate reference system \r\n\r\nEXAMPLE easting, northing, height, time"^^xsd:string ;
        skos:definition   "compound spatio-temporal coordinate reference system containing a projected horizontal, a vertical, and a temporal coordinate reference system \r\n\r\nEXAMPLE easting, northing, height, time"^^xsd:string ;
        skos:inScheme     <ReferenceSystemInformation/code/MD_ReferenceSystemTypeCode> ;
        skos:prefLabel    "compoundProjectedVerticalTemporal" .

<ReferenceSystemInformation/code/MD_ReferenceSystemTypeCode/compoundGeographic2DTemporal>
        a                 iso19115-1_2375:MD_ReferenceSystemTypeCode , skos:Concept ;
        rdfs:isDefinedBy  <http://standards.iso.org/iso/19115/-1/ed-1/en/> ;
        rdfs:label        "compound Geographic 2D Temporal" ;
        dct:description   "compound spatio-temporal coordinate reference system containing a 2 dimensional geographic horizontal coordinate reference system and a temporal reference system \r\n\r\nEXAMPLE latitude, longitude, time"^^xsd:string ;
        skos:definition   "compound spatio-temporal coordinate reference system containing a 2 dimensional geographic horizontal coordinate reference system and a temporal reference system \r\n\r\nEXAMPLE latitude, longitude, time"^^xsd:string ;
        skos:inScheme     <ReferenceSystemInformation/code/MD_ReferenceSystemTypeCode> ;
        skos:prefLabel    "compoundGeographic2DTemporal" .

<ReferenceSystemInformation/code/MD_ReferenceSystemTypeCode/geodeticGeocentric>
        a                 iso19115-1_2375:MD_ReferenceSystemTypeCode , skos:Concept ;
        rdfs:isDefinedBy  <http://standards.iso.org/iso/19115/-1/ed-1/en/> ;
        rdfs:label        "geodetic Geocentric" ;
        dct:description   "geodetic CRS having a Cartesian 3D coordinate system \r\n\r\nEXAMPLE [geocentric] X,Y,Z"^^xsd:string ;
        skos:definition   "geodetic CRS having a Cartesian 3D coordinate system \r\n\r\nEXAMPLE [geocentric] X,Y,Z"^^xsd:string ;
        skos:inScheme     <ReferenceSystemInformation/code/MD_ReferenceSystemTypeCode> ;
        skos:prefLabel    "geodeticGeocentric" .

<ReferenceSystemInformation/code/MD_ReferenceSystemTypeCode/compoundGeographic2DParametric>
        a                 iso19115-1_2375:MD_ReferenceSystemTypeCode , skos:Concept ;
        rdfs:isDefinedBy  <http://standards.iso.org/iso/19115/-1/ed-1/en/> ;
        rdfs:label        "compound Geographic 2D Parametric" ;
        dct:description   "compound spatio-parametric coordinate reference system containing a 2 dimensional geographic horizontal coordinate reference system and a parametric reference system \r\n\r\nEXAMPLE latitude, longitude, pressure"^^xsd:string ;
        skos:definition   "compound spatio-parametric coordinate reference system containing a 2 dimensional geographic horizontal coordinate reference system and a parametric reference system \r\n\r\nEXAMPLE latitude, longitude, pressure"^^xsd:string ;
        skos:inScheme     <ReferenceSystemInformation/code/MD_ReferenceSystemTypeCode> ;
        skos:prefLabel    "compoundGeographic2DParametric" .

<ReferenceSystemInformation/code/MD_ReferenceSystemTypeCode/compoundProjected2DParametricTemporal>
        a                 iso19115-1_2375:MD_ReferenceSystemTypeCode , skos:Concept ;
        rdfs:isDefinedBy  <http://standards.iso.org/iso/19115/-1/ed-1/en/> ;
        rdfs:label        "compound Projected 2D Parametric Temporal" ;
        dct:description   "compound spatio-parametric-temporal coordinate reference system containing a projected horizontal, a parametric, and a temporal coordinate reference system \r\n\r\nEXAMPLE easting, northing, density, time"^^xsd:string ;
        skos:definition   "compound spatio-parametric-temporal coordinate reference system containing a projected horizontal, a parametric, and a temporal coordinate reference system \r\n\r\nEXAMPLE easting, northing, density, time"^^xsd:string ;
        skos:inScheme     <ReferenceSystemInformation/code/MD_ReferenceSystemTypeCode> ;
        skos:prefLabel    "compoundProjected2DParametricTemporal" .

<ReferenceSystemInformation/code/MD_ReferenceSystemTypeCode/engineeringImage>
        a                 iso19115-1_2375:MD_ReferenceSystemTypeCode , skos:Concept ;
        rdfs:isDefinedBy  <http://standards.iso.org/iso/19115/-1/ed-1/en/> ;
        rdfs:label        "engineering Image" ;
        dct:description   "coordinate reference system based on an image datum (engineering datum which defines the relationship of a coordinate system to an image) \r\n\r\nEXAMPLE row, column"^^xsd:string ;
        skos:definition   "coordinate reference system based on an image datum (engineering datum which defines the relationship of a coordinate system to an image) \r\n\r\nEXAMPLE row, column"^^xsd:string ;
        skos:inScheme     <ReferenceSystemInformation/code/MD_ReferenceSystemTypeCode> ;
        skos:prefLabel    "engineeringImage" .
