@base          <http://def.isotc211.org/iso19115/-1/2014/Metadata-Fundamentals> .
@prefix dc:    <http://purl.org/dc/elements/1.1/> .
@prefix dct:   <http://purl.org/dc/terms/> .
@prefix owl:   <http://www.w3.org/2002/07/owl#> .
@prefix rdf:   <http://www.w3.org/1999/02/22-rdf-syntax-ns#> .
@prefix rdfs:  <http://www.w3.org/2000/01/rdf-schema#> .
@prefix reg:    <http://purl.org/linked-data/registry#>.
@prefix skos:  <http://www.w3.org/2004/02/skos/core#> .

@prefix application: <http://def.isotc211.org/iso19115/-1/2014/ApplicationSchemaInformation#> .
@prefix citation: <http://def.isotc211.org/iso19115/-1/2014/CitationAndResponsiblePartyInformation#> .
@prefix common: <http://def.isotc211.org/iso19115/-1/2014/CommonClasses#> .
@prefix constraint: <http://def.isotc211.org/iso19115/-1/2014/ConstraintInformation#> .
@prefix content: <http://def.isotc211.org/iso19115/-1/2014/ContentInformation#> .
@prefix crs:   <http://def.isotc211.org/iso19111/2007/CoordinateReferenceSystems#> .
@prefix distribution: <http://def.isotc211.org/iso19115/-1/2014/DistributionInformation#> .
@prefix extended: <http://def.isotc211.org/iso19115/-1/2014/ExampleOfExtendedMatadata#> .
@prefix extent: <http://def.isotc211.org/iso19115/-1/2014/ExtentInformation#> .
@prefix fc:    <http://def.isotc211.org/iso19110/2005/MethodologyForFeatureCataloguing#> .
@prefix fundamentals: <http://def.isotc211.org/iso19115/-1/2014/Metadata-Fundamentals#> .
@prefix identification: <http://def.isotc211.org/iso19115/-1/2014/IdentificationInformation#> .
@prefix lineage: <http://def.isotc211.org/iso19115/-1/2014/LineageInformation#> .
@prefix localization: <http://def.isotc211.org/iso19115/-1/2014/Language-CharactersetLocalizationInformation#> .
@prefix maintenance: <http://def.isotc211.org/iso19115/-1/2014/MaintenanceInformation#> .
@prefix metapp: <http://def.isotc211.org/iso19115/-1/2014/MetadataApplicationInformation#> .
@prefix metext: <http://def.isotc211.org/iso19115/-1/2014/MetadataExtensionInformation#> .
@prefix metinf: <http://def.isotc211.org/iso19115/-1/2014/MetadataInformation#> .
@prefix portrayal: <http://def.isotc211.org/iso19115/-1/2014/PortrayalCatalogueInformation#> .
@prefix rs:    <http://def.isotc211.org/iso19115/-1/2014/ReferenceSystemInformation#> .
@prefix service: <http://def.isotc211.org/iso19115/-1/2014/ServiceMetadataInformation#> . 
@prefix sr:    <http://def.isotc211.org/iso19115/-1/2014/SpatialRepresentationInformation#> .

@prefix iso00639_65: <http://def.isotc211.org/iso00639/-2/LanguageCodes#> .
@prefix iso19110_2259: <http://def.isotc211.org/iso19110/2005/MethodologyForFeatureCataloguing#> .
@prefix iso19107_2211: <http://def.isotc211.org/iso19107/2003/GeometryRoot#> .
@prefix iso19107_2210: <http://def.isotc211.org/iso19107/2003/GeometricPrimitive#> .
@prefix iso19115-1Code: <http://def.isotc211.org/iso19115/-1/2014/CitationAndResponsiblePartyInformation/code/> .
@prefix iso19108_891: <http://def.isotc211.org/iso19108/2006/TemporalObjects#> .
@prefix iso19139_709: <http://def.isotc211.org/iso19139/2007/CulturalAndLinguisticAdapdability#> .
@prefix iso19115-1: <http://def.isotc211.org/iso19115/-1/2014/CitationAndResponsiblePartyInformation#> .
@prefix iso19111_1300: <http://def.isotc211.org/iso19111/2007/CoordinateReferenceSystems#> .
@prefix iso19103_2176: <http://def.isotc211.org/iso19103/2015/RecordTypes#> .
@prefix iso19103_2174: <http://def.isotc211.org/iso19103/2015/NameTypes#> .
@prefix iso03166_66: <http://def.isotc211.org/iso03166/-1/CountryCodes#> .
@prefix iso19115-1_2364: <http://def.isotc211.org/iso19115/-1/2014/ConstraintInformation#> .
@prefix iso19115-1_2376: <http://def.isotc211.org/iso19115/-1/2014/SpatialRepresentationInformation#> .
@prefix iso19115-1_2375: <http://def.isotc211.org/iso19115/-1/2014/ReferenceSystemInformation#> .
@prefix iso19115-1_2365: <http://def.isotc211.org/iso19115/-1/2014/ContentInformation#> .
@prefix iso19115-1_2374: <http://def.isotc211.org/iso19115/-1/2014/PortrayalCatalogueInformation#> .
@prefix iso19115-1_2362: <http://def.isotc211.org/iso19115/-1/2014/ApplicationSchemaInformation#> .
@prefix iso19115-1_2363: <http://def.isotc211.org/iso19115/-1/2014/CitationAndResponsiblePartyInformation#> .
@prefix iso19115-1_2373: <http://def.isotc211.org/iso19115/-1/2014/MetadataExtensionInformation#> .
@prefix iso19115-1_2368: <http://def.isotc211.org/iso19115/-1/2014/ExtentInformation#> .
@prefix iso19115-1_2369: <http://def.isotc211.org/iso19115/-1/2014/IdentificationInformation#> .
@prefix iso19115-1_2366: <http://def.isotc211.org/iso19115/-1/2014/LineageInformation#> .
@prefix iso19103_2178: <http://def.isotc211.org/iso19103/2015/WebEnvironment#> .
@prefix iso19115-1_2367: <http://def.isotc211.org/iso19115/-1/2014/DistributionInformation#> .
@prefix iso19103_2179: <http://def.isotc211.org/iso19103/2015/MeasureTypes#> .
@prefix iso19157_1164: <http://def.isotc211.org/iso19157/2013/DataQuality#> .
@prefix iso19115-1_2371: <http://def.isotc211.org/iso19115/-1/2014/MetadataApplicationInformation#> .
@prefix iso19115-1_2360: <http://def.isotc211.org/iso19115/-1/2014/Language-CharactersetLocalizationInformation#> .
@prefix iso19115-1_2372: <http://def.isotc211.org/iso19115/-1/2014/MetadataInformation#> .
@prefix iso19115-1_2370: <http://def.isotc211.org/iso19115/-1/2014/MaintenanceInformation#> .
@prefix iso19150-2: <http://def.isotc211.org/iso19150/-2/2012/base#> .
@prefix iso19115-1_2358: <http://def.isotc211.org/iso19115/-1/2014/CommonClasses#> .



<SpatialRepresentationInformation/code/MD_TopologyLevelCode/fullPlanarGraph>
        a                 iso19115-1_2376:MD_TopologyLevelCode , skos:Concept ;
        rdfs:isDefinedBy  <http://standards.iso.org/iso/19115/-1/ed-1/en/> ;
        rdfs:label        "full Planar Graph" ;
        dct:description   "2-dimensional topological complex that is planar \r\nNOTE A 2-dimensional topological complex is commonly called “full topology” in a cartographic 2D environment."^^xsd:string ;
        skos:definition   "2-dimensional topological complex that is planar \r\nNOTE A 2-dimensional topological complex is commonly called “full topology” in a cartographic 2D environment."^^xsd:string ;
        skos:inScheme     <SpatialRepresentationInformation/code/MD_TopologyLevelCode> ;
        skos:prefLabel    "fullPlanarGraph" .

<SpatialRepresentationInformation/code/MD_TopologyLevelCode/planarGraph>
        a                 iso19115-1_2376:MD_TopologyLevelCode , skos:Concept ;
        rdfs:isDefinedBy  <http://standards.iso.org/iso/19115/-1/ed-1/en/> ;
        rdfs:label        "planar Graph" ;
        dct:description   "1-dimensional topological complex that is planar \r\nNOTE A planar graph is a graph that can be drawn in a plane in such a way that no two edges intersect except at a vertex."^^xsd:string ;
        skos:definition   "1-dimensional topological complex that is planar \r\nNOTE A planar graph is a graph that can be drawn in a plane in such a way that no two edges intersect except at a vertex."^^xsd:string ;
        skos:inScheme     <SpatialRepresentationInformation/code/MD_TopologyLevelCode> ;
        skos:prefLabel    "planarGraph" .

<SpatialRepresentationInformation/code/MD_TopologyLevelCode/geometryOnly>
        a                 iso19115-1_2376:MD_TopologyLevelCode , skos:Concept ;
        rdfs:isDefinedBy  <http://standards.iso.org/iso/19115/-1/ed-1/en/> ;
        rdfs:label        "geometry Only" ;
        dct:description   "geometry objects without any additional structure which describes topology"^^xsd:string ;
        skos:definition   "geometry objects without any additional structure which describes topology"^^xsd:string ;
        skos:inScheme     <SpatialRepresentationInformation/code/MD_TopologyLevelCode> ;
        skos:prefLabel    "geometryOnly" .

<SpatialRepresentationInformation/code/MD_TopologyLevelCode/abstract>
        a                 iso19115-1_2376:MD_TopologyLevelCode , skos:Concept ;
        rdfs:isDefinedBy  <http://standards.iso.org/iso/19115/-1/ed-1/en/> ;
        rdfs:label        "abstract" ;
        dct:description   "topological complex without any specified geometric realisation"^^xsd:string ;
        skos:definition   "topological complex without any specified geometric realisation"^^xsd:string ;
        skos:inScheme     <SpatialRepresentationInformation/code/MD_TopologyLevelCode> ;
        skos:prefLabel    "abstract" .

<SpatialRepresentationInformation/code/MD_TopologyLevelCode/surfaceGraph>
        a                 iso19115-1_2376:MD_TopologyLevelCode , skos:Concept ;
        rdfs:isDefinedBy  <http://standards.iso.org/iso/19115/-1/ed-1/en/> ;
        rdfs:label        "surface Graph" ;
        dct:description   "1-dimensional topological complex that is isomorphic to a subset of a surface \r\nNOTE A geometric complex is isomorphic to a topological complex if their elements are in a one-to-one, dimensional-and boundary-preserving correspondence to one another."^^xsd:string ;
        skos:definition   "1-dimensional topological complex that is isomorphic to a subset of a surface \r\nNOTE A geometric complex is isomorphic to a topological complex if their elements are in a one-to-one, dimensional-and boundary-preserving correspondence to one another."^^xsd:string ;
        skos:inScheme     <SpatialRepresentationInformation/code/MD_TopologyLevelCode> ;
        skos:prefLabel    "surfaceGraph" .

<SpatialRepresentationInformation/code/MD_TopologyLevelCode/topology1D>
        a                 iso19115-1_2376:MD_TopologyLevelCode , skos:Concept ;
        rdfs:isDefinedBy  <http://standards.iso.org/iso/19115/-1/ed-1/en/> ;
        rdfs:label        "topology 1D" ;
        dct:description   "1-dimensional topological complex – commonly called “chain-node” topology"^^xsd:string ;
        skos:definition   "1-dimensional topological complex – commonly called “chain-node” topology"^^xsd:string ;
        skos:inScheme     <SpatialRepresentationInformation/code/MD_TopologyLevelCode> ;
        skos:prefLabel    "topology1D" .

<SpatialRepresentationInformation/code/MD_TopologyLevelCode/fullTopology3D>
        a                 iso19115-1_2376:MD_TopologyLevelCode , skos:Concept ;
        rdfs:isDefinedBy  <http://standards.iso.org/iso/19115/-1/ed-1/en/> ;
        rdfs:label        "full Topology 3D" ;
        dct:description   "complete coverage of a 3D Euclidean coordinate space"^^xsd:string ;
        skos:definition   "complete coverage of a 3D Euclidean coordinate space"^^xsd:string ;
        skos:inScheme     <SpatialRepresentationInformation/code/MD_TopologyLevelCode> ;
        skos:prefLabel    "fullTopology3D" .

<SpatialRepresentationInformation/code/MD_TopologyLevelCode/topology3D>
        a                 iso19115-1_2376:MD_TopologyLevelCode , skos:Concept ;
        rdfs:isDefinedBy  <http://standards.iso.org/iso/19115/-1/ed-1/en/> ;
        rdfs:label        "topology 3D" ;
        dct:description   "3-dimensional topological complex \r\nNOTE A topological complex is a collection of topological primitives that are closed under the boundary operations."^^xsd:string ;
        skos:definition   "3-dimensional topological complex \r\nNOTE A topological complex is a collection of topological primitives that are closed under the boundary operations."^^xsd:string ;
        skos:inScheme     <SpatialRepresentationInformation/code/MD_TopologyLevelCode> ;
        skos:prefLabel    "topology3D" .

<SpatialRepresentationInformation/code/MD_TopologyLevelCode/fullSurfaceGraph>
        a                 iso19115-1_2376:MD_TopologyLevelCode , skos:Concept ;
        rdfs:isDefinedBy  <http://standards.iso.org/iso/19115/-1/ed-1/en/> ;
        rdfs:label        "full Surface Graph" ;
        dct:description   "1-dimensional topological complex that is isomorphic to a subset of a surface \r\nNOTE A geometric complex is isomorphic to a topological complex if their elements are in a one-to-one, dimensional-and boundary-preserving correspondence to one another."^^xsd:string ;
        skos:definition   "1-dimensional topological complex that is isomorphic to a subset of a surface \r\nNOTE A geometric complex is isomorphic to a topological complex if their elements are in a one-to-one, dimensional-and boundary-preserving correspondence to one another."^^xsd:string ;
        skos:inScheme     <SpatialRepresentationInformation/code/MD_TopologyLevelCode> ;
        skos:prefLabel    "fullSurfaceGraph" .
