# baseURI: http://def.isotc211.org/iso19115/-1/2014/IdentificationInformation/code/MD_TopicCategoryCode
# imports: http://www.w3.org/2004/02/skos/core

@prefix application: <http://def.isotc211.org/iso19115/-1/2014/ApplicationSchemaInformation#> .
@prefix citation: <http://def.isotc211.org/iso19115/-1/2014/CitationAndResponsiblePartyInformation#> .
@prefix common: <http://def.isotc211.org/iso19115/-1/2014/CommonClasses#> .
@prefix constraint: <http://def.isotc211.org/iso19115/-1/2014/ConstraintInformation#> .
@prefix content: <http://def.isotc211.org/iso19115/-1/2014/ContentInformation#> .
@prefix crs: <http://def.isotc211.org/iso19111/2007/CoordinateReferenceSystems#> .
@prefix dc: <http://purl.org/dc/elements/1.1/> .
@prefix dct: <http://purl.org/dc/terms/> .
@prefix distribution: <http://def.isotc211.org/iso19115/-1/2014/DistributionInformation#> .
@prefix extended: <http://def.isotc211.org/iso19115/-1/2014/ExampleOfExtendedMatadata#> .
@prefix extent: <http://def.isotc211.org/iso19115/-1/2014/ExtentInformation#> .
@prefix fc: <http://def.isotc211.org/iso19110/2005/MethodologyForFeatureCataloguing#> .
@prefix fundamentals: <http://def.isotc211.org/iso19115/-1/2014/Metadata-Fundamentals#> .
@prefix identification: <http://def.isotc211.org/iso19115/-1/2014/IdentificationInformation#> .
@prefix lineage: <http://def.isotc211.org/iso19115/-1/2014/LineageInformation#> .
@prefix localization: <http://def.isotc211.org/iso19115/-1/2014/Language-CharactersetLocalizationInformation#> .
@prefix maintenance: <http://def.isotc211.org/iso19115/-1/2014/MaintenanceInformation#> .
@prefix metapp: <http://def.isotc211.org/iso19115/-1/2014/MetadataApplicationInformation#> .
@prefix metext: <http://def.isotc211.org/iso19115/-1/2014/MetadataExtensionInformation#> .
@prefix metinf: <http://def.isotc211.org/iso19115/-1/2014/MetadataInformation#> .
@prefix owl: <http://www.w3.org/2002/07/owl#> .
@prefix portrayal: <http://def.isotc211.org/iso19115/-1/2014/PortrayalCatalogueInformation#> .
@prefix rdf: <http://www.w3.org/1999/02/22-rdf-syntax-ns#> .
@prefix rdfs: <http://www.w3.org/2000/01/rdf-schema#> .
@prefix rs: <http://def.isotc211.org/iso19115/-1/2014/ReferenceSystemInformation#> .
@prefix service: <http://def.isotc211.org/iso19115/-1/2014/ServiceMetadataInformation#> .
@prefix skos: <http://www.w3.org/2004/02/skos/core#> .
@prefix sr: <http://def.isotc211.org/iso19115/-1/2014/SpatialRepresentationInformation#> .
@prefix topic: <http://def.isotc211.org/iso19115/-1/2014/IdentificationInformation/code/MD_TopicCategoryCode/> .
@prefix xsd: <http://www.w3.org/2001/XMLSchema#> .

<http://def.isotc211.org/iso19115/-1/2014/IdentificationInformation/code/MD_TopicCategoryCode>
  rdf:type skos:ConceptScheme ;
  dct:description "high-level geographic data thematic classification to assist in the grouping and search of available geographic data sets NOTE 1 Can be used to group keywords as well. Listed examples are not exhaustive. NOTE 2 It is understood there are overlaps between general categories and the user is encouraged to select the one most appropriate." ;
  rdfs:isDefinedBy <http://standards.iso.org/iso/19115/-1/ed-1/en/> ;
  rdfs:label "MD Topic Category Code" ;
  owl:imports <http://www.w3.org/2004/02/skos/core> ;
  skos:definition "high-level geographic data thematic classification to assist in the grouping and search of available geographic data sets NOTE 1 Can be used to group keywords as well. Listed examples are not exhaustive. NOTE 2 It is understood there are overlaps between general categories and the user is encouraged to select the one most appropriate." ;
  skos:prefLabel "MD_TopicCategoryCode" ;
.
topic:biota
  rdf:type skos:Concept ;
  dct:description """flora and/or fauna in natural environment 

EXAMPLES Wildlife, vegetation, biological sciences, ecology, wilderness, sealife, wetlands, habitat."""^^xsd:string ;
  rdfs:isDefinedBy <http://standards.iso.org/iso/19115/-1/ed-1/en/> ;
  rdfs:label "biota" ;
  skos:definition """flora and/or fauna in natural environment 

EXAMPLES Wildlife, vegetation, biological sciences, ecology, wilderness, sealife, wetlands, habitat."""^^xsd:string ;
  skos:example "biological sciences"^^xsd:string ;
  skos:example "ecology"^^xsd:string ;
  skos:example "habitat"^^xsd:string ;
  skos:example "sealife"^^xsd:string ;
  skos:example "vegetation"^^xsd:string ;
  skos:example "wetlands"^^xsd:string ;
  skos:example "wilderness"^^xsd:string ;
  skos:example "wildlife"^^xsd:string ;
  skos:inScheme <file:///C:/Users/cox075/dev/isotc211-owl/isotc211_GOM_harmonizedOntology/19115-1/2014/codes/IdentificationInformation/code/MD_TopicCategoryCode> ;
  skos:prefLabel "biota" ;
.
topic:boundaries
  rdf:type skos:Concept ;
  dct:description """legal land descriptions, maritime boundaries 

EXAMPLES Political and administrative boundaries, territorial seas, EEZ, port security zones."""^^xsd:string ;
  rdfs:isDefinedBy <http://standards.iso.org/iso/19115/-1/ed-1/en/> ;
  rdfs:label "boundaries" ;
  skos:definition """legal land descriptions, maritime boundaries 

EXAMPLES Political and administrative boundaries, territorial seas, EEZ, port security zones."""^^xsd:string ;
  skos:example "Political and administrative boundaries, territorial seas, EEZ, port security zones."^^xsd:string ;
  skos:inScheme <file:///C:/Users/cox075/dev/isotc211-owl/isotc211_GOM_harmonizedOntology/19115-1/2014/codes/IdentificationInformation/code/MD_TopicCategoryCode> ;
  skos:prefLabel "boundaries" ;
.
topic:climatologyMeteorologyAtmosphere
  rdf:type skos:Concept ;
  dct:description """processes and phenomena of the atmosphere 

EXAMPLES Cloud cover, weather, climate, atmospheric conditions, climate change, precipitation."""^^xsd:string ;
  rdfs:isDefinedBy <http://standards.iso.org/iso/19115/-1/ed-1/en/> ;
  rdfs:label "climatology Meteorology Atmosphere" ;
  skos:definition """processes and phenomena of the atmosphere 

EXAMPLES Cloud cover, weather, climate, atmospheric conditions, climate change, precipitation."""^^xsd:string ;
  skos:example "Cloud cover, weather, climate, atmospheric conditions, climate change, precipitation."^^xsd:string ;
  skos:inScheme <file:///C:/Users/cox075/dev/isotc211-owl/isotc211_GOM_harmonizedOntology/19115-1/2014/codes/IdentificationInformation/code/MD_TopicCategoryCode> ;
  skos:prefLabel "climatologyMeteorologyAtmosphere" ;
.
topic:disaster
  rdf:type skos:Concept ;
  dct:description """information related to disasters 

EXAMPLES Site of the disaster, evacuation zone, disaster-prevention facility, disaster relief activities."""^^xsd:string ;
  rdfs:isDefinedBy <http://standards.iso.org/iso/19115/-1/ed-1/en/> ;
  rdfs:label "disaster" ;
  skos:definition """information related to disasters 

EXAMPLES Site of the disaster, evacuation zone, disaster-prevention facility, disaster relief activities."""^^xsd:string ;
  skos:example "Site of the disaster, evacuation zone, disaster-prevention facility, disaster relief activities."^^xsd:string ;
  skos:inScheme <file:///C:/Users/cox075/dev/isotc211-owl/isotc211_GOM_harmonizedOntology/19115-1/2014/codes/IdentificationInformation/code/MD_TopicCategoryCode> ;
  skos:prefLabel "disaster" ;
.
topic:economy
  rdf:type skos:Concept ;
  dct:description """economic activities, conditions and employment 

EXAMPLES Production, labour, revenue, commerce, industry, tourism and ecotourism, forestry, fisheries, commercial or subsistence hunting, exploration and exploitation of resources such as minerals, oil and gas."""^^xsd:string ;
  rdfs:isDefinedBy <http://standards.iso.org/iso/19115/-1/ed-1/en/> ;
  rdfs:label "economy" ;
  skos:definition """economic activities, conditions and employment 

EXAMPLES Production, labour, revenue, commerce, industry, tourism and ecotourism, forestry, fisheries, commercial or subsistence hunting, exploration and exploitation of resources such as minerals, oil and gas."""^^xsd:string ;
  skos:example "Production, labour, revenue, commerce, industry, tourism and ecotourism, forestry, fisheries, commercial or subsistence hunting, exploration and exploitation of resources such as minerals, oil and gas."^^xsd:string ;
  skos:inScheme <file:///C:/Users/cox075/dev/isotc211-owl/isotc211_GOM_harmonizedOntology/19115-1/2014/codes/IdentificationInformation/code/MD_TopicCategoryCode> ;
  skos:prefLabel "economy" ;
.
topic:elevation
  rdf:type skos:Concept ;
  dct:description """height above or below a vertical datum 

EXAMPLES Altitude, bathymetry, digital elevation models, slope, derived products."""^^xsd:string ;
  rdfs:isDefinedBy <http://standards.iso.org/iso/19115/-1/ed-1/en/> ;
  rdfs:label "elevation" ;
  skos:definition """height above or below a vertical datum 

EXAMPLES Altitude, bathymetry, digital elevation models, slope, derived products."""^^xsd:string ;
  skos:example "Altitude, bathymetry, digital elevation models, slope, derived products."^^xsd:string ;
  skos:inScheme <file:///C:/Users/cox075/dev/isotc211-owl/isotc211_GOM_harmonizedOntology/19115-1/2014/codes/IdentificationInformation/code/MD_TopicCategoryCode> ;
  skos:prefLabel "elevation" ;
.
topic:environment
  rdf:type skos:Concept ;
  dct:description """environmental resources, protection and conservation 

EXAMPLES Environmental pollution, waste storage and treatment, environmental impact assessment, monitoring environmental risk, nature reserves, landscape."""^^xsd:string ;
  rdfs:isDefinedBy <http://standards.iso.org/iso/19115/-1/ed-1/en/> ;
  rdfs:label "environment" ;
  skos:definition """environmental resources, protection and conservation 

EXAMPLES Environmental pollution, waste storage and treatment, environmental impact assessment, monitoring environmental risk, nature reserves, landscape."""^^xsd:string ;
  skos:example "Environmental pollution, waste storage and treatment, environmental impact assessment, monitoring environmental risk, nature reserves, landscape."^^xsd:string ;
  skos:inScheme <file:///C:/Users/cox075/dev/isotc211-owl/isotc211_GOM_harmonizedOntology/19115-1/2014/codes/IdentificationInformation/code/MD_TopicCategoryCode> ;
  skos:prefLabel "environment" ;
.
topic:extraTerrestrial
  rdf:type skos:Concept ;
  dct:description "region more than 100 km above the surface of the Earth." ;
  rdfs:isDefinedBy <http://standards.iso.org/iso/19115/-1/ed-1/en/> ;
  rdfs:label "extra Terrestrial" ;
  skos:definition "region more than 100 km above the surface of the Earth." ;
  skos:inScheme <file:///C:/Users/cox075/dev/isotc211-owl/isotc211_GOM_harmonizedOntology/19115-1/2014/codes/IdentificationInformation/code/MD_TopicCategoryCode> ;
  skos:prefLabel "extraTerrestrial" ;
.
topic:farming
  rdf:type skos:Concept ;
  dct:description """rearing of animals and/or cultivation of plants 

EXAMPLES Agriculture, irrigation, aquaculture, plantations, herding, pests and diseases affecting crops and livestock."""^^xsd:string ;
  rdfs:isDefinedBy <http://standards.iso.org/iso/19115/-1/ed-1/en/> ;
  rdfs:label "farming" ;
  skos:definition """rearing of animals and/or cultivation of plants 

EXAMPLES Agriculture, irrigation, aquaculture, plantations, herding, pests and diseases affecting crops and livestock."""^^xsd:string ;
  skos:example "Agriculture, irrigation, aquaculture, plantations, herding, pests and diseases affecting crops and livestock."^^xsd:string ;
  skos:inScheme <file:///C:/Users/cox075/dev/isotc211-owl/isotc211_GOM_harmonizedOntology/19115-1/2014/codes/IdentificationInformation/code/MD_TopicCategoryCode> ;
  skos:prefLabel "farming" ;
.
topic:geoscientificInformation
  rdf:type skos:Concept ;
  dct:description """information pertaining to earth sciences 

EXAMPLES Geophysical features and processes, geology, minerals, sciences dealing with the composition, structure and origin of the earth’s rocks, risks of earthquakes, volcanic activity, landslides, gravity information, soils, permafrost, hydrogeology, erosion."""^^xsd:string ;
  rdfs:isDefinedBy <http://standards.iso.org/iso/19115/-1/ed-1/en/> ;
  rdfs:label "geoscientific Information" ;
  skos:definition """information pertaining to earth sciences 

EXAMPLES Geophysical features and processes, geology, minerals, sciences dealing with the composition, structure and origin of the earth’s rocks, risks of earthquakes, volcanic activity, landslides, gravity information, soils, permafrost, hydrogeology, erosion."""^^xsd:string ;
  skos:example "Geophysical features and processes, geology, minerals, sciences dealing with the composition, structure and origin of the earth’s rocks, risks of earthquakes, volcanic activity, landslides, gravity information, soils, permafrost, hydrogeology, erosion."^^xsd:string ;
  skos:inScheme <file:///C:/Users/cox075/dev/isotc211-owl/isotc211_GOM_harmonizedOntology/19115-1/2014/codes/IdentificationInformation/code/MD_TopicCategoryCode> ;
  skos:prefLabel "geoscientificInformation" ;
.
topic:health
  rdf:type skos:Concept ;
  dct:description """health, health services, human ecology, and safety 

EXAMPLES Disease and illness, factors affecting health, hygiene, substance abuse, mental and physical health, health services."""^^xsd:string ;
  rdfs:isDefinedBy <http://standards.iso.org/iso/19115/-1/ed-1/en/> ;
  rdfs:label "health" ;
  skos:definition """health, health services, human ecology, and safety 

EXAMPLES Disease and illness, factors affecting health, hygiene, substance abuse, mental and physical health, health services."""^^xsd:string ;
  skos:example "Disease and illness, factors affecting health, hygiene, substance abuse, mental and physical health, health services."^^xsd:string ;
  skos:inScheme <file:///C:/Users/cox075/dev/isotc211-owl/isotc211_GOM_harmonizedOntology/19115-1/2014/codes/IdentificationInformation/code/MD_TopicCategoryCode> ;
  skos:prefLabel "health" ;
.
topic:imageryBaseMapsEarthCover
  rdf:type skos:Concept ;
  dct:description """base maps 

EXAMPLES Land cover, topographic maps, imagery, unclassified images, annotations."""^^xsd:string ;
  rdfs:isDefinedBy <http://standards.iso.org/iso/19115/-1/ed-1/en/> ;
  rdfs:label "imagery Base Maps Earth Cover" ;
  skos:definition """base maps 

EXAMPLES Land cover, topographic maps, imagery, unclassified images, annotations."""^^xsd:string ;
  skos:example "Land cover, topographic maps, imagery, unclassified images, annotations."^^xsd:string ;
  skos:inScheme <file:///C:/Users/cox075/dev/isotc211-owl/isotc211_GOM_harmonizedOntology/19115-1/2014/codes/IdentificationInformation/code/MD_TopicCategoryCode> ;
  skos:prefLabel "imageryBaseMapsEarthCover" ;
.
topic:inlandWaters
  rdf:type skos:Concept ;
  dct:description """inland water features, drainage systems and their characteristics 

EXAMPLES Rivers and glaciers, salt lakes, water utilization plans, dams, currents, floods, water quality, hydrologic information."""^^xsd:string ;
  rdfs:isDefinedBy <http://standards.iso.org/iso/19115/-1/ed-1/en/> ;
  rdfs:label "inland Waters" ;
  skos:definition """inland water features, drainage systems and their characteristics 

EXAMPLES Rivers and glaciers, salt lakes, water utilization plans, dams, currents, floods, water quality, hydrologic information."""^^xsd:string ;
  skos:example "Rivers and glaciers, salt lakes, water utilization plans, dams, currents, floods, water quality, hydrologic information."^^xsd:string ;
  skos:inScheme <file:///C:/Users/cox075/dev/isotc211-owl/isotc211_GOM_harmonizedOntology/19115-1/2014/codes/IdentificationInformation/code/MD_TopicCategoryCode> ;
  skos:prefLabel "inlandWaters" ;
.
topic:intelligenceMilitary
  rdf:type skos:Concept ;
  dct:description """military bases, structures, activities 

EXAMPLES Barracks, training grounds, military transportation, information collection."""^^xsd:string ;
  rdfs:isDefinedBy <http://standards.iso.org/iso/19115/-1/ed-1/en/> ;
  rdfs:label "intelligence Military" ;
  skos:definition """military bases, structures, activities 

EXAMPLES Barracks, training grounds, military transportation, information collection."""^^xsd:string ;
  skos:example "Barracks, training grounds, military transportation, information collection."^^xsd:string ;
  skos:inScheme <file:///C:/Users/cox075/dev/isotc211-owl/isotc211_GOM_harmonizedOntology/19115-1/2014/codes/IdentificationInformation/code/MD_TopicCategoryCode> ;
  skos:prefLabel "intelligenceMilitary" ;
.
topic:location
  rdf:type skos:Concept ;
  dct:description """positional information and services 

EXAMPLES Addresses, geodetic networks, control points, postal zones and services, place names."""^^xsd:string ;
  rdfs:isDefinedBy <http://standards.iso.org/iso/19115/-1/ed-1/en/> ;
  rdfs:label "location" ;
  skos:definition """positional information and services 

EXAMPLES Addresses, geodetic networks, control points, postal zones and services, place names."""^^xsd:string ;
  skos:example "Addresses, geodetic networks, control points, postal zones and services, place names."^^xsd:string ;
  skos:inScheme <file:///C:/Users/cox075/dev/isotc211-owl/isotc211_GOM_harmonizedOntology/19115-1/2014/codes/IdentificationInformation/code/MD_TopicCategoryCode> ;
  skos:prefLabel "location" ;
.
topic:oceans
  rdf:type skos:Concept ;
  dct:description """features and characteristics of salt water bodies (excluding inland waters) 

EXAMPLES Tides, tsunamis, coastal information, reefs."""^^xsd:string ;
  rdfs:isDefinedBy <http://standards.iso.org/iso/19115/-1/ed-1/en/> ;
  rdfs:label "oceans" ;
  skos:definition """features and characteristics of salt water bodies (excluding inland waters) 

EXAMPLES Tides, tsunamis, coastal information, reefs."""^^xsd:string ;
  skos:example "Tides, tsunamis, coastal information, reefs."^^xsd:string ;
  skos:inScheme <file:///C:/Users/cox075/dev/isotc211-owl/isotc211_GOM_harmonizedOntology/19115-1/2014/codes/IdentificationInformation/code/MD_TopicCategoryCode> ;
  skos:prefLabel "oceans" ;
.
topic:planningCadastre
  rdf:type skos:Concept ;
  dct:description """information used for appropriate actions for future use of the land 

EXAMPLES Land use maps, zoning maps, cadastral surveys, land ownership."""^^xsd:string ;
  rdfs:isDefinedBy <http://standards.iso.org/iso/19115/-1/ed-1/en/> ;
  rdfs:label "planning Cadastre" ;
  skos:definition """information used for appropriate actions for future use of the land 

EXAMPLES Land use maps, zoning maps, cadastral surveys, land ownership."""^^xsd:string ;
  skos:example "Land use maps, zoning maps, cadastral surveys, land ownership."^^xsd:string ;
  skos:inScheme <file:///C:/Users/cox075/dev/isotc211-owl/isotc211_GOM_harmonizedOntology/19115-1/2014/codes/IdentificationInformation/code/MD_TopicCategoryCode> ;
  skos:prefLabel "planningCadastre" ;
.
topic:society
  rdf:type skos:Concept ;
  dct:description """characteristics of society and cultures 

EXAMPLES Settlements, anthropology, archaeology, education, traditional beliefs, manners and customs, demographic data, recreational areas and activities, social impact assessments, crime and justice, census information."""^^xsd:string ;
  rdfs:isDefinedBy <http://standards.iso.org/iso/19115/-1/ed-1/en/> ;
  rdfs:label "society" ;
  skos:definition """characteristics of society and cultures 

EXAMPLES Settlements, anthropology, archaeology, education, traditional beliefs, manners and customs, demographic data, recreational areas and activities, social impact assessments, crime and justice, census information."""^^xsd:string ;
  skos:example "Settlements, anthropology, archaeology, education, traditional beliefs, manners and customs, demographic data, recreational areas and activities, social impact assessments, crime and justice, census information."^^xsd:string ;
  skos:inScheme <file:///C:/Users/cox075/dev/isotc211-owl/isotc211_GOM_harmonizedOntology/19115-1/2014/codes/IdentificationInformation/code/MD_TopicCategoryCode> ;
  skos:prefLabel "society" ;
.
topic:structure
  rdf:type skos:Concept ;
  dct:description """man-made construction 

EXAMPLES Buildings, museums, churches, factories, housing, monuments, shops, towers."""^^xsd:string ;
  rdfs:isDefinedBy <http://standards.iso.org/iso/19115/-1/ed-1/en/> ;
  rdfs:label "structure" ;
  skos:definition """man-made construction 

EXAMPLES Buildings, museums, churches, factories, housing, monuments, shops, towers."""^^xsd:string ;
  skos:example "Buildings, museums, churches, factories, housing, monuments, shops, towers."^^xsd:string ;
  skos:inScheme <file:///C:/Users/cox075/dev/isotc211-owl/isotc211_GOM_harmonizedOntology/19115-1/2014/codes/IdentificationInformation/code/MD_TopicCategoryCode> ;
  skos:prefLabel "structure" ;
.
topic:transportation
  rdf:type skos:Concept ;
  dct:description """means and aids for conveying persons and/or goods 

EXAMPLES Roads, airports/airstrips, shipping routes, tunnels, nautical charts, vehicle or vessel location, aeronautical charts, railways."""^^xsd:string ;
  rdfs:isDefinedBy <http://standards.iso.org/iso/19115/-1/ed-1/en/> ;
  rdfs:label "transportation" ;
  skos:definition """means and aids for conveying persons and/or goods 

EXAMPLES Roads, airports/airstrips, shipping routes, tunnels, nautical charts, vehicle or vessel location, aeronautical charts, railways."""^^xsd:string ;
  skos:example "Roads, airports/airstrips, shipping routes, tunnels, nautical charts, vehicle or vessel location, aeronautical charts, railways."^^xsd:string ;
  skos:inScheme <file:///C:/Users/cox075/dev/isotc211-owl/isotc211_GOM_harmonizedOntology/19115-1/2014/codes/IdentificationInformation/code/MD_TopicCategoryCode> ;
  skos:prefLabel "transportation" ;
.
topic:utilitiesCommunication
  rdf:type skos:Concept ;
  dct:description """energy, water and waste systems and communications infrastructure and services 

EXAMPLES Hydroelectricity, geothermal, solar and nuclear sources of energy, water purification and distribution, sewage collection and disposal, electricity and gas distribution, data communication, telecommunication, radio, communication networks."""^^xsd:string ;
  rdfs:isDefinedBy <http://standards.iso.org/iso/19115/-1/ed-1/en/> ;
  rdfs:label "utilities Communication" ;
  skos:definition """energy, water and waste systems and communications infrastructure and services 

EXAMPLES Hydroelectricity, geothermal, solar and nuclear sources of energy, water purification and distribution, sewage collection and disposal, electricity and gas distribution, data communication, telecommunication, radio, communication networks."""^^xsd:string ;
  skos:example "Hydroelectricity, geothermal, solar and nuclear sources of energy, water purification and distribution, sewage collection and disposal, electricity and gas distribution, data communication, telecommunication, radio, communication networks."^^xsd:string ;
  skos:inScheme <file:///C:/Users/cox075/dev/isotc211-owl/isotc211_GOM_harmonizedOntology/19115-1/2014/codes/IdentificationInformation/code/MD_TopicCategoryCode> ;
  skos:prefLabel "utilitiesCommunication" ;
.
