@prefix dcterms: <http://purl.org/dc/terms/> .
@prefix owl: <http://www.w3.org/2002/07/owl#> .
@prefix rdfs: <http://www.w3.org/2000/01/rdf-schema#> .
@prefix sdo: <https://schema.org/> .
@prefix skos: <http://www.w3.org/2004/02/skos/core#> .
@prefix xsd: <http://www.w3.org/2001/XMLSchema#> .

@prefix rr: <https://example.com/roles-responsibilities/> .

<https://example.com/roles-responsibilities> 
    a owl:Ontology , skos:ConceptScheme ;
    skos:prefLabel "19135-1 Roles for the management of registers"@en ;
    skos:definition "Roles defined by the standard ISO/DIS 19135-1 _Geographic information â€” Procedures for item registration_, Section 5 \"Roles and responsibilities in the management of registers\""@en ;
    dcterms:source "https://www.iso.org/standard/54721.html"^^xsd:anyURI ;
    dcterms:creator <https://committee.iso.org/home/tc211> ;
    dcterms:created "2021-03-23"^^xsd:date ;
    dcterms:modified "2021-03-23"^^xsd:date ;
    dcterms:provenance "This vocabulary was generated manually from content within ISO/DIS 19135-1, rather than automaticallygenerated from UML versions of that document. This was done to ensure that role definitions were presented in a consistent manner, which may not have been possible with a direct UML translation." ;
    dcterms:publisher <https://example.com/unofficial> ;
    skos:hasTopConcept 
        rr:register-owner ,
        rr:register-manager ,
        rr:submitting-organization ,
        rr:control-body ,
        rr:registry-manager ,
        rr:register-user ;
.

<https://committee.iso.org/home/tc211>
    a sdo:Organization ;
    sdo:name "ISO Technical Committee 211 Geographic information/Geomatics" ;
    sdo:url "https://committee.iso.org/home/tc211"^^xsd:anyURI ;
.

<https://example.com/unofficial>
    a sdo:Organization ;
    sdo:name "Unofficial - no publisher" ;
    sdo:url "https://example.com/unofficial"^^xsd:anyURI ;
.

rr:register-owner
    a skos:Concept ;
    rdfs:isDefinedBy <https://example.com/roles-responsibilities> ;
    skos:prefLabel "Register owner"@en ;
    skos:definition "A register owner is an organization that: a) has established one or more registers; and b) has primary responsibility for the management, dissemination and intellectual content of those registers."@en ;
    skos:inScheme <https://example.com/roles-responsibilities> ;
    skos:topConceptOf <https://example.com/roles-responsibilities> ;
.

rr:register-manager
    a skos:Concept ;
    rdfs:isDefinedBy <https://example.com/roles-responsibilities> ;
    skos:prefLabel "Register manager"@en ;
    skos:definition "A register manager is an organization that delegated by a register owner to manage a register."@en ;
    skos:inScheme <https://example.com/roles-responsibilities> ;
    skos:topConceptOf <https://example.com/roles-responsibilities> ;
.

rr:submitting-organization
    a skos:Concept ;
    rdfs:isDefinedBy <https://example.com/roles-responsibilities> ;
    skos:prefLabel "Submitting organization"@en ;
    skos:definition "A submitting organization is an organization that is qualified under criteria determined by the register owner to propose changes to the content of a register."@en ;
    skos:inScheme <https://example.com/roles-responsibilities> ;
    skos:topConceptOf <https://example.com/roles-responsibilities> ;
.

rr:control-body
    a skos:Concept ;
    rdfs:isDefinedBy <https://example.com/roles-responsibilities> ;
    skos:prefLabel "Control body"@en ;
    skos:definition "A control body is a group of technical experts appointed by a register owner to decide on the acceptability of proposals for changes to the content of a register."@en ;
    skos:inScheme <https://example.com/roles-responsibilities> ;
    skos:topConceptOf <https://example.com/roles-responsibilities> ;
.

rr:registry-manager
    a skos:Concept ;
    rdfs:isDefinedBy <https://example.com/roles-responsibilities> ;
    skos:prefLabel "Registry manager"@en ;
    skos:definition "A registry manager is a person or an organization responsible for the day-to-day management of a registry."@en ;
    skos:inScheme <https://example.com/roles-responsibilities> ;
    skos:topConceptOf <https://example.com/roles-responsibilities> ;
.

rr:register-user
    a skos:Concept ;
    rdfs:isDefinedBy <https://example.com/roles-responsibilities> ;
    skos:prefLabel "Register user"@en ;
    skos:definition "Register users access a registry in order to use one or more of the registers held in that registry. Register users include any person or organization interested in accessing or influencing the content of a register."@en ;
    skos:inScheme <https://example.com/roles-responsibilities> ;
    skos:topConceptOf <https://example.com/roles-responsibilities> ;
.