PREFIX : <http://def.isotc211.org/iso19135/-1/2015/CoreModel/code/RE_SimilarityToSource/>
PREFIX cs: <http://def.isotc211.org/iso19135/-1/2015/CoreModel/code/RE_SimilarityToSource>
PREFIX prov: <http://www.w3.org/ns/prov#>
PREFIX rdfs: <http://www.w3.org/2000/01/rdf-schema#>
PREFIX reg: <http://purl.org/linked-data/registry#>
PREFIX schema: <https://schema.org/>
PREFIX status: <http://def.isotc211.org/iso19135/-1/2015/CoreModel/code/RE_ItemStatus/>
PREFIX skos: <http://www.w3.org/2004/02/skos/core#>
PREFIX xsd: <http://www.w3.org/2001/XMLSchema#>

:1
    a skos:Concept ;
    reg:status status:original ;
    rdfs:isDefinedBy cs: ;
    skos:definition "No change has been made to the specification"@en ;
    skos:inScheme cs: ;
    skos:prefLabel "No change"@en ;
    skos:historyNote "From page 52, ISO19135-1:2014"@en ;
.

:2
    a skos:Concept ;
    reg:status status:original ;
    rdfs:isDefinedBy cs: ;
    skos:definition "The style of the specification has been changed to match the style and structure of other specifications in the register that has imported the specification"@en ;
    skos:inScheme cs: ;
    skos:prefLabel "Style"@en ;
    skos:historyNote "From page 52, ISO19135-1:2014"@en ;
.

:3
    a skos:Concept ;
    reg:status status:original ;
    rdfs:isDefinedBy cs: ;
    skos:definition "The specification includes information about its context that is not explicit in the specification in the external source"@en ;
    skos:inScheme cs: ;
    skos:prefLabel "Extra not explict"@en ;
    skos:historyNote "From page 52, ISO19135-1:2014"@en ;
.

:4
    a skos:Concept ;
    reg:status status:original ;
    rdfs:isDefinedBy cs: ;
    skos:definition "The specification of the register item has been generalized to have a broader meaning than the item specified in the external source"@en ;
    skos:inScheme cs: ;
    skos:prefLabel "Generalized"@en ;
    skos:historyNote "From page 52, ISO19135-1:2014"@en ;
.

:5
    a skos:Concept ;
    reg:status status:original ;
    rdfs:isDefinedBy cs: ;
    skos:definition "The specification of the register item has been specialized to have a narrower meaning than the item specified in the external source"@en ;
    skos:inScheme cs: ;
    skos:prefLabel "Narrower"@en ;
    skos:historyNote "From page 52, ISO19135-1:2014"@en ;
.

:6
    a skos:Concept ;
    reg:status status:original ;
    rdfs:isDefinedBy cs: ;
    skos:definition "The nature of the differences between the register item and the similar item in the external source is unspecified"@en ;
    skos:inScheme cs: ;
    skos:prefLabel "Unspecified"@en ;
    skos:historyNote "From page 52, ISO19135-1:2014"@en ;
.


cs:
    a skos:ConceptScheme ;
    reg:status status:experimental ;
    skos:definition "Instances of RE_SimilarityToSource that specifiy the type of change that has been made to the item specification relative to the item specification in the external source"@en ;
    skos:hasTopConcept
        :1 ,
        :2 ,
        :3 ,
        :4 ,
        :5 ,
        :6 ;
    skos:prefLabel "Similarity To Source Codes"@en ;
    prov:qualifiedDerivation
        [
            prov:entity <http://example.com/none> ;
            prov:hadRole <https://linked.data.gov.au/def/vocab-derivation-modes/none> ;
        ] ;
    schema:citation "http://standards.iso.org/iso/19135/-1/ed-1/en/"^^xsd:anyURI ;
    schema:creator <https://committee.iso.org/home/tc211> ;
    schema:dateCreated "2014-09-18"^^xsd:date ;
    schema:dateModified "2024-10-02"^^xsd:date ;
    schema:identifier "RE_SimilarityToSource"^^xsd:token ;
    skos:historyNote "Created manually by GOM staff directly from the ISO19135-1:2014 document"@en ;
    schema:publisher <https://committee.iso.org/home/tc211> ;
.
