<?xml version="1.0"?>

<!DOCTYPE rdf:RDF [
  <!ENTITY owl "http://www.w3.org/2002/07/owl#" >
  <!ENTITY xsd "http://www.w3.org/2001/XMLSchema#" >
  <!ENTITY rdfs "http://www.w3.org/2000/01/rdf-schema#" >
  <!ENTITY rdf "http://www.w3.org/1999/02/22-rdf-syntax-ns#" >
  <!ENTITY dc "http://purl.org/dc/elements/1.1/" >
  <!ENTITY dct "http://purl.org/dc/terms/" >
  <!ENTITY skos "http://www.w3.org/2004/02/skos/core#" >
  <!ENTITY iso19150-2 "http://def.isotc211.org/iso19150/-2/2012/base#" >
  <!ENTITY iso19144-2 "http://def.isotc211.org/iso19144/-2/2012/LC_ValueObjectTypes#" >

]>

  <!--++++++++++++++++++++++++++++++++++++++++++++++++++++++-->
  <!-- File name:         iso19144-2LC_ValueObjectTypes.rdf -->
  <!-- Generator:         GOM_Technologies::UML2OWL         -->
  <!-- Generator version: 2.5                               -->
  <!-- File date:         12-4-2016                         -->
  <!--++++++++++++++++++++++++++++++++++++++++++++++++++++++-->

<rdf:RDF xmlns="http://def.isotc211.org/iso19144/-2/2012/LC_ValueObjectTypes#"
  xml:base="http://def.isotc211.org/iso19144/-2/2012/LC_ValueObjectTypes"
  xmlns:owl="http://www.w3.org/2002/07/owl#"
  xmlns:xsd="http://www.w3.org/2001/XMLSchema#"
  xmlns:rdfs="http://www.w3.org/2000/01/rdf-schema#"
  xmlns:rdf="http://www.w3.org/1999/02/22-rdf-syntax-ns#"
  xmlns:dc="http://purl.org/dc/elements/1.1/"
  xmlns:dct="http://purl.org/dc/terms/"
  xmlns:skos="http://www.w3.org/2004/02/skos/core#"
  xmlns:iso19150-2="http://def.isotc211.org/iso19150/-2/2012/base#"
  xmlns:iso19144-2="http://def.isotc211.org/iso19144/-2/2012/LC_ValueObjectTypes#">

  <!--++++++++++++++++++++++++++++++++++++++++++++++++-->
  <!-- Ontology: ISO 19144-2:2012 LC_ValueObjectTypes -->
  <!--++++++++++++++++++++++++++++++++++++++++++++++++-->
  <owl:Ontology rdf:about="http://def.isotc211.org/iso19144/-2/2012/LC_ValueObjectTypes">
    <rdfs:label>ISO 19144-2:2012 LC_ValueObjectTypes</rdfs:label>
    <dct:source>http://standards.iso.org/iso/19144/-2/ed-1/en/</dct:source>
    <owl:versionInfo>2012-07-01</owl:versionInfo>
    <owl:imports rdf:resource="http://def.isotc211.org/iso19150/-2/2012/base"/>
  </owl:Ontology>

  <!--+++++++++++++++++++++++++++++++++++++-->
  <!-- Class: LC_PermittedIntegerValueType -->
  <!--+++++++++++++++++++++++++++++++++++++-->
  <owl:Class rdf:about="&iso19144-2;LC_PermittedIntegerValueType">
    <rdfs:label>LC_PermittedIntegerValueType</rdfs:label>
    <skos:definition>The LC_PermittedIntegerValueType metalanguage object is a subtype of LC_ValueClass. It is an abstract metaclass for the various integer number values permitted in the metalanguage whose subtypes which may be instantiated as an integer number type using the Integer type from the basic Primitive Types package in ISO.sl.TS 19103, with constraints. It has two subtypes LC_PermittedPosIntegerValueType, and LC_PermittedPosIntegerRange.</skos:definition>
    <rdfs:isDefinedBy>http://standards.iso.org/iso/19144/-2/ed-1/en/</rdfs:isDefinedBy>
    <iso19150-2:isAbstract rdf:datatype="&xsd;boolean">true</iso19150-2:isAbstract>
    <rdfs:subClassOf rdf:resource="&iso19144-2;LC_ValueObject"/>
  </owl:Class>

  <!--++++++++++++++++++++++++++++++++++++-->
  <!-- Class: LC_PermittedPercentageRange -->
  <!--++++++++++++++++++++++++++++++++++++-->
  <owl:Class rdf:about="&iso19144-2;LC_PermittedPercentageRange">
    <rdfs:label>LC_PermittedPercentageRange</rdfs:label>
    <skos:definition>The LC_PermittedPercentageRange metalanguage object is a subtype of LC_PermittedPercentageValue and indirectly of LC_PermittedPercentageValueType. It is a metalanguage object for a positive percentage number value range permitted in the metalanguage. The inherited attribute baseV.lt.i.gt.alue .lt..sl.i.gt.becomes the minimum value of the range and a new attribute .lt.i.gt.maxValue.lt..sl.i.gt. describes the maximum value of the range,  where the attribute baseV.lt.i.gt.alue .lt..sl.i.gt.and .lt.i.gt.maxValue .lt..sl.i.gt.may be instantiated as a pair of real number types using the Real type from the basic Primitive Types package in ISO.sl.TS 19103, with the constraints:    {.lt.i.gt.maxValue.lt..sl.i.gt. .gt. .lt.i.gt.baseValu.lt..sl.i.gt.e  and    maxValue .gt..eq. 0   and   maxValue .lt..eq. 100.0}</skos:definition>
    <rdfs:isDefinedBy>http://standards.iso.org/iso/19144/-2/ed-1/en/</rdfs:isDefinedBy>
    <iso19150-2:constraint>maxValue .gt. baseValue</iso19150-2:constraint>
    <iso19150-2:constraint>maxValue .gt. baseValue</iso19150-2:constraint>
    <iso19150-2:constraint>maxValue .gt. baseValue</iso19150-2:constraint>
    <rdfs:subClassOf rdf:resource="&iso19144-2;LC_PermittedPercentageValue"/>
    <rdfs:subClassOf>
      <owl:Restriction>
        <owl:onProperty rdf:resource="&iso19144-2;LC_PermittedPercentageRange.maxValue"/>
        <owl:cardinality rdf:datatype="&xsd;nonNegativeInteger">1</owl:cardinality>
      </owl:Restriction>
    </rdfs:subClassOf>
    <rdfs:subClassOf>
      <owl:Restriction>
        <owl:onProperty rdf:resource="&iso19144-2;LC_PermittedPercentageRange.maxValue"/>
        <owl:allValuesFrom rdf:resource="&xsd;double"/>
      </owl:Restriction>
    </rdfs:subClassOf>
  </owl:Class>

  <!--++++++++++++++++++++++++++++++++++++-->
  <!-- Class: LC_PermittedPercentageValue -->
  <!--++++++++++++++++++++++++++++++++++++-->
  <owl:Class rdf:about="&iso19144-2;LC_PermittedPercentageValue">
    <rdfs:label>LC_PermittedPercentageValue</rdfs:label>
    <skos:definition>The LC_PermittedPercentageValue metalanguage object is a subtype of LC_PermittedPergentageValueType. It is a metalanguage object for a positive percentage value permitted in the metalanguage where the attribute .lt.i.gt.baseValue.lt..sl.i.gt. may be instantiated as a real number type using the Real type from the basic Primitive Types package in ISO.sl.TS 19103, with the constraint:   {.lt.i.gt.baseValue.lt..sl.i.gt. .gt..eq. 0.0} and      ba.lt.i.gt.seValue.lt..sl.i.gt. .lt..eq. 100.0}.</skos:definition>
    <rdfs:isDefinedBy>http://standards.iso.org/iso/19144/-2/ed-1/en/</rdfs:isDefinedBy>
    <iso19150-2:constraint>baseValue .gt..eq. 0.0</iso19150-2:constraint>
    <iso19150-2:constraint>baseValue .gt..eq. 0.0</iso19150-2:constraint>
    <rdfs:subClassOf rdf:resource="&iso19144-2;LC_PermittedPercentageValueType"/>
    <rdfs:subClassOf>
      <owl:Restriction>
        <owl:onProperty rdf:resource="&iso19144-2;LC_PermittedPercentageValue.baseValue"/>
        <owl:cardinality rdf:datatype="&xsd;nonNegativeInteger">1</owl:cardinality>
      </owl:Restriction>
    </rdfs:subClassOf>
    <rdfs:subClassOf>
      <owl:Restriction>
        <owl:onProperty rdf:resource="&iso19144-2;LC_PermittedPercentageValue.baseValue"/>
        <owl:allValuesFrom rdf:resource="&xsd;double"/>
      </owl:Restriction>
    </rdfs:subClassOf>
  </owl:Class>

  <!--++++++++++++++++++++++++++++++++++++++++-->
  <!-- Class: LC_PermittedPercentageValueType -->
  <!--++++++++++++++++++++++++++++++++++++++++-->
  <owl:Class rdf:about="&iso19144-2;LC_PermittedPercentageValueType">
    <rdfs:label>LC_PermittedPercentageValueType</rdfs:label>
    <skos:definition>The LC_PermittedPercentageValueType metalanguage object is a subtype of LC_ValueObject. It is a metalanguage object for the various types of percentage values permitted in the metalanguage whose subtypes may be instantiated as a real number types using the Real type from the basic Primitive Types package in ISO.sl.TS 19103, with constraints. It has two subtypes LC_PermittedPercentageValueType, and LC_PermittedPercentageRange.</skos:definition>
    <rdfs:isDefinedBy>http://standards.iso.org/iso/19144/-2/ed-1/en/</rdfs:isDefinedBy>
    <iso19150-2:isAbstract rdf:datatype="&xsd;boolean">true</iso19150-2:isAbstract>
    <rdfs:subClassOf rdf:resource="&iso19144-2;LC_ValueObject"/>
  </owl:Class>

  <!--++++++++++++++++++++++++++++++++++++-->
  <!-- Class: LC_PermittedPosIntegerRange -->
  <!--++++++++++++++++++++++++++++++++++++-->
  <owl:Class rdf:about="&iso19144-2;LC_PermittedPosIntegerRange">
    <rdfs:label>LC_PermittedPosIntegerRange</rdfs:label>
    <skos:definition>The LC_PermittedPosIntegerRange metalanguage object is a subtype of LC_PermittedPosIntegerValue and indirectly of LC_PermittedPosIntegerValueType. It is a metalanguage object for a positive integer number value range permitted in the metalanguage. The inherited attribute .lt.i.gt.baseValue .lt..sl.i.gt.becomes the minimum value of the range and a new attribute .lt.i.gt.maxValue.lt..sl.i.gt. describes the maximum value of the rangeThe attributes .lt.i.gt.baseValue.lt..sl.i.gt. and .lt.i.gt.maxValue.lt..sl.i.gt. may be instantiated as a pair of integer number types using the Integer type from the basic Primitive Types package in ISO.sl.TS 19103, with the constraints:    {.lt.i.gt.maxValue.lt..sl.i.gt. .gt. .lt.i.gt.baseValue .lt..sl.i.gt. and    .lt.i.gt.maxValue.lt..sl.i.gt. .gt..eq. 0}.</skos:definition>
    <rdfs:isDefinedBy>http://standards.iso.org/iso/19144/-2/ed-1/en/</rdfs:isDefinedBy>
    <iso19150-2:constraint>maxValue .gt..eq. 0</iso19150-2:constraint>
    <iso19150-2:constraint>maxValue .gt..eq. 0</iso19150-2:constraint>
    <rdfs:subClassOf rdf:resource="&iso19144-2;LC_PermittedPosIntegerValue"/>
    <rdfs:subClassOf>
      <owl:Restriction>
        <owl:onProperty rdf:resource="&iso19144-2;LC_PermittedPosIntegerRange.maxValue"/>
        <owl:cardinality rdf:datatype="&xsd;nonNegativeInteger">1</owl:cardinality>
      </owl:Restriction>
    </rdfs:subClassOf>
    <rdfs:subClassOf>
      <owl:Restriction>
        <owl:onProperty rdf:resource="&iso19144-2;LC_PermittedPosIntegerRange.maxValue"/>
        <owl:allValuesFrom rdf:resource="&xsd;integer"/>
      </owl:Restriction>
    </rdfs:subClassOf>
  </owl:Class>

  <!--++++++++++++++++++++++++++++++++++++-->
  <!-- Class: LC_PermittedPosIntegerValue -->
  <!--++++++++++++++++++++++++++++++++++++-->
  <owl:Class rdf:about="&iso19144-2;LC_PermittedPosIntegerValue">
    <rdfs:label>LC_PermittedPosIntegerValue</rdfs:label>
    <skos:definition>The LC_PermittedPosIntegerValue metalanguage object is a subtype of LC_PermittedPosIntegerValueType. It is a metalanguage object for a positive integer number value permitted in the metalanguage where the attribute .lt.i.gt.baseValue.lt..sl.i.gt. may be instantiated as a integer number type using the Integer type from the basic Primitive Types package in ISO.sl.TS 19103, with the constraint: {baseValue .gt..eq. 0}.</skos:definition>
    <rdfs:isDefinedBy>http://standards.iso.org/iso/19144/-2/ed-1/en/</rdfs:isDefinedBy>
    <iso19150-2:isAbstract rdf:datatype="&xsd;boolean">true</iso19150-2:isAbstract>
    <iso19150-2:constraint>baseValue .gt..eq. 0</iso19150-2:constraint>
    <rdfs:subClassOf rdf:resource="&iso19144-2;LC_PermittedIntegerValueType"/>
    <rdfs:subClassOf>
      <owl:Restriction>
        <owl:onProperty rdf:resource="&iso19144-2;LC_PermittedPosIntegerValue.baseValue"/>
        <owl:cardinality rdf:datatype="&xsd;nonNegativeInteger">1</owl:cardinality>
      </owl:Restriction>
    </rdfs:subClassOf>
    <rdfs:subClassOf>
      <owl:Restriction>
        <owl:onProperty rdf:resource="&iso19144-2;LC_PermittedPosIntegerValue.baseValue"/>
        <owl:allValuesFrom rdf:resource="&xsd;integer"/>
      </owl:Restriction>
    </rdfs:subClassOf>
  </owl:Class>

  <!--+++++++++++++++++++++++++++++++++-->
  <!-- Class: LC_PermittedPosRealRange -->
  <!--+++++++++++++++++++++++++++++++++-->
  <owl:Class rdf:about="&iso19144-2;LC_PermittedPosRealRange">
    <rdfs:label>LC_PermittedPosRealRange</rdfs:label>
    <skos:definition>The LC_PermittedPosRealRange metalanguage object is a subtype of LC_PermittedPosRealValue and indirectly of  LC_PermittedRealValueType. It is a metalanguage object for a positive real number value range permitted in the metalanguage.  The inherited attribute .lt.i.gt.baseValue .lt..sl.i.gt.becomes the minimum value of the range and a new attribute .lt.i.gt.maxValue.lt..sl.i.gt. describes the maximum value of the range, .where the attribute .lt.i.gt.baseValue .lt..sl.i.gt.and .lt.i.gt.maxValue.lt..sl.i.gt. may be instantiated as a pair of real number types using the Real type from the basic Primitive Types package in ISO.sl.TS 19103, with the constraints:   {maxValue .gt. baseValue  and   baseValue .gt..eq. 0.0and    maxValue .gt..eq. 0.0}.</skos:definition>
    <rdfs:isDefinedBy>http://standards.iso.org/iso/19144/-2/ed-1/en/</rdfs:isDefinedBy>
    <iso19150-2:constraint>maxValue .gt..eq. 0.0</iso19150-2:constraint>
    <iso19150-2:constraint>maxValue .gt..eq. 0.0</iso19150-2:constraint>
    <iso19150-2:constraint>maxValue .gt..eq. 0.0</iso19150-2:constraint>
    <rdfs:subClassOf rdf:resource="&iso19144-2;LC_PermittedPosRealValue"/>
    <rdfs:subClassOf>
      <owl:Restriction>
        <owl:onProperty rdf:resource="&iso19144-2;LC_PermittedPosRealRange.maxValue"/>
        <owl:cardinality rdf:datatype="&xsd;nonNegativeInteger">1</owl:cardinality>
      </owl:Restriction>
    </rdfs:subClassOf>
    <rdfs:subClassOf>
      <owl:Restriction>
        <owl:onProperty rdf:resource="&iso19144-2;LC_PermittedPosRealRange.maxValue"/>
        <owl:allValuesFrom rdf:resource="&xsd;double"/>
      </owl:Restriction>
    </rdfs:subClassOf>
  </owl:Class>

  <!--+++++++++++++++++++++++++++++++++-->
  <!-- Class: LC_PermittedPosRealValue -->
  <!--+++++++++++++++++++++++++++++++++-->
  <owl:Class rdf:about="&iso19144-2;LC_PermittedPosRealValue">
    <rdfs:label>LC_PermittedPosRealValue</rdfs:label>
    <skos:definition>The LC_PermittedPosRealValue metalanguage object is a subtype of LC_PermittedRealValueType. It is a metalanguage object for a positive real number value permitted in the metalanguage where the attribute value may be instantiated as a real number type using the Real type from the basic Primitive Types package in ISO.sl.TS 19103, with the constraint: {Value .gt..eq. 0.0}.</skos:definition>
    <rdfs:isDefinedBy>http://standards.iso.org/iso/19144/-2/ed-1/en/</rdfs:isDefinedBy>
    <iso19150-2:constraint>baseValue .gt..eq. 0.0</iso19150-2:constraint>
    <rdfs:subClassOf rdf:resource="&iso19144-2;LC_PermittedRealValueType"/>
    <rdfs:subClassOf>
      <owl:Restriction>
        <owl:onProperty rdf:resource="&iso19144-2;LC_PermittedPosRealValue.baseValue"/>
        <owl:cardinality rdf:datatype="&xsd;nonNegativeInteger">1</owl:cardinality>
      </owl:Restriction>
    </rdfs:subClassOf>
    <rdfs:subClassOf>
      <owl:Restriction>
        <owl:onProperty rdf:resource="&iso19144-2;LC_PermittedPosRealValue.baseValue"/>
        <owl:allValuesFrom rdf:resource="&xsd;double"/>
      </owl:Restriction>
    </rdfs:subClassOf>
  </owl:Class>

  <!--++++++++++++++++++++++++++++++-->
  <!-- Class: LC_PermittedRealValue -->
  <!--++++++++++++++++++++++++++++++-->
  <owl:Class rdf:about="&iso19144-2;LC_PermittedRealValue">
    <rdfs:label>LC_PermittedRealValue</rdfs:label>
    <skos:definition>The LC_PermittedRealValue metalanguage object is a subtype of LC_PermittedRealValueType. It is a metalanguage object for a real number value permitted in the metalanguage where the attribute value may be instantiated as a real number type using the Real type from the basic Primitive Types package in ISO.sl.TS 19103, where the value may be positive or negative. The sign convention is that negative values are depths and positive values are heights.</skos:definition>
    <rdfs:isDefinedBy>http://standards.iso.org/iso/19144/-2/ed-1/en/</rdfs:isDefinedBy>
    <rdfs:subClassOf rdf:resource="&iso19144-2;LC_PermittedRealValueType"/>
    <rdfs:subClassOf>
      <owl:Restriction>
        <owl:onProperty rdf:resource="&iso19144-2;LC_PermittedRealValue.value"/>
        <owl:cardinality rdf:datatype="&xsd;nonNegativeInteger">1</owl:cardinality>
      </owl:Restriction>
    </rdfs:subClassOf>
    <rdfs:subClassOf>
      <owl:Restriction>
        <owl:onProperty rdf:resource="&iso19144-2;LC_PermittedRealValue.value"/>
        <owl:allValuesFrom rdf:resource="&xsd;double"/>
      </owl:Restriction>
    </rdfs:subClassOf>
  </owl:Class>

  <!--++++++++++++++++++++++++++++++++++-->
  <!-- Class: LC_PermittedRealValueType -->
  <!--++++++++++++++++++++++++++++++++++-->
  <owl:Class rdf:about="&iso19144-2;LC_PermittedRealValueType">
    <rdfs:label>LC_PermittedRealValueType</rdfs:label>
    <skos:definition>The LC_PermittedRealValueType metalanguage object is a subtype of LC_ValueObject. It is an abstract metalanguage object for the various types of real number values permitted in the metalanguage whose subtypes may be instantiated as a real number types using the Real type from the basic Primitive Types package in ISO.sl.TS 19103, with constraints.It has three subtypes LC_PermittedRealValue, LC_PermittedPosRealValue and LC_PermittedPosRealRange.</skos:definition>
    <rdfs:isDefinedBy>http://standards.iso.org/iso/19144/-2/ed-1/en/</rdfs:isDefinedBy>
    <iso19150-2:isAbstract rdf:datatype="&xsd;boolean">true</iso19150-2:isAbstract>
    <rdfs:subClassOf rdf:resource="&iso19144-2;LC_ValueObject"/>
  </owl:Class>

  <!--+++++++++++++++++++++++-->
  <!-- Class: LC_ValueObject -->
  <!--+++++++++++++++++++++++-->
  <owl:Class rdf:about="&iso19144-2;LC_ValueObject">
    <rdfs:label>LC_ValueObject</rdfs:label>
    <skos:definition>The LC_ValueObject is a metalanguage object that describes how permitted numeric values at the metalanguage level maybe instantiated to the basic number types form ISO.sl.TS 19103 at the type level. The LC_ValueClass metalanguage object is a supertype of the three value metalanguage value objects LC_PermittedRealValueType, LC_PermittedPercentageValueType and LC_PermittedIntegerValueType. Each of these value objects has subtypes that describe a number and a range. Each of the value objects is described by a constraint that characterises the type of numerical entity that may be represented by the value object. These value objects are generators for the actual value objects that will appear in instances of a classification system generated using the LCML. The result of instantiating these objects are value classes taken from the basic types provided in ISO.sl.TS 19103. The results of instantiating a classification system are objects that carry actual values. In the various examples given in this international standard value objects have been instantiated from the metalanguage level to the type level and then to the instance level, to produce real objects as needed in an example.It has three subtypes: LC_PermittedRealValueType, LC_PermittedPercentageValueType, and LC_PermittedIntegerValueType.</skos:definition>
    <rdfs:isDefinedBy>http://standards.iso.org/iso/19144/-2/ed-1/en/</rdfs:isDefinedBy>
    <iso19150-2:isAbstract rdf:datatype="&xsd;boolean">true</iso19150-2:isAbstract>
  </owl:Class>

  <!--++++++++++++++++++++++++++++++++++++++++++++++++++++++++-->
  <!-- DatatypeProperty: LC_PermittedPercentageRange.maxValue -->
  <!--++++++++++++++++++++++++++++++++++++++++++++++++++++++++-->
  <owl:DatatypeProperty rdf:about="&iso19144-2;LC_PermittedPercentageRange.maxValue">
    <rdfs:label>maxValue</rdfs:label>
    <rdfs:isDefinedBy>http://standards.iso.org/iso/19144/-2/ed-1/en/</rdfs:isDefinedBy>
    <rdfs:domain rdf:resource="&iso19144-2;LC_PermittedPercentageRange"/>
    <rdfs:range rdf:resource="&xsd;double"/>
  </owl:DatatypeProperty>

  <!--+++++++++++++++++++++++++++++++++++++++++++++++++++++++++-->
  <!-- DatatypeProperty: LC_PermittedPercentageValue.baseValue -->
  <!--+++++++++++++++++++++++++++++++++++++++++++++++++++++++++-->
  <owl:DatatypeProperty rdf:about="&iso19144-2;LC_PermittedPercentageValue.baseValue">
    <rdfs:label>baseValue</rdfs:label>
    <rdfs:isDefinedBy>http://standards.iso.org/iso/19144/-2/ed-1/en/</rdfs:isDefinedBy>
    <rdfs:domain rdf:resource="&iso19144-2;LC_PermittedPercentageValue"/>
    <rdfs:range rdf:resource="&xsd;double"/>
  </owl:DatatypeProperty>

   <!--+++++++++++++++++++++++++++++++++++++++++++++++++++++++-->
  <!-- DatatypeProperty: LC_PermittedPosIntegerRange.maxValue -->
  <!--++++++++++++++++++++++++++++++++++++++++++++++++++++++++-->
  <owl:DatatypeProperty rdf:about="&iso19144-2;LC_PermittedPosIntegerRange.maxValue">
    <rdfs:label>maxValue</rdfs:label>
    <rdfs:isDefinedBy>http://standards.iso.org/iso/19144/-2/ed-1/en/</rdfs:isDefinedBy>
    <rdfs:domain rdf:resource="&iso19144-2;LC_PermittedPosRealRange"/>
    <rdfs:range rdf:resource="&xsd;integer"/>
  </owl:DatatypeProperty>

  <!--+++++++++++++++++++++++++++++++++++++++++++++++++++++++++-->
  <!-- DatatypeProperty: LC_PermittedPosIntegerValue.baseValue -->
  <!--+++++++++++++++++++++++++++++++++++++++++++++++++++++++++-->
  <owl:DatatypeProperty rdf:about="&iso19144-2;LC_PermittedPosIntegerValue.baseValue">
    <rdfs:label>baseValue</rdfs:label>
    <rdfs:isDefinedBy>http://standards.iso.org/iso/19144/-2/ed-1/en/</rdfs:isDefinedBy>
    <rdfs:domain rdf:resource="&iso19144-2;LC_PermittedPosIntegerValue"/>
    <rdfs:range rdf:resource="&xsd;integer"/>
  </owl:DatatypeProperty>

  <!--+++++++++++++++++++++++++++++++++++++++++++++++++++++-->
  <!-- DatatypeProperty: LC_PermittedPosRealRange.maxValue -->
  <!--+++++++++++++++++++++++++++++++++++++++++++++++++++++-->
  <owl:DatatypeProperty rdf:about="&iso19144-2;LC_PermittedPosRealRange.maxValue">
    <rdfs:label>maxValue</rdfs:label>
    <rdfs:isDefinedBy>http://standards.iso.org/iso/19144/-2/ed-1/en/</rdfs:isDefinedBy>
    <rdfs:domain rdf:resource="&iso19144-2;LC_PermittedPosRealRange"/>
    <rdfs:range rdf:resource="&xsd;double"/>
  </owl:DatatypeProperty>

  <!--++++++++++++++++++++++++++++++++++++++++++++++++++++++-->
  <!-- DatatypeProperty: LC_PermittedPosRealValue.baseValue -->
  <!--++++++++++++++++++++++++++++++++++++++++++++++++++++++-->
  <owl:DatatypeProperty rdf:about="&iso19144-2;LC_PermittedPosRealValue.baseValue">
    <rdfs:label>baseValue</rdfs:label>
    <rdfs:isDefinedBy>http://standards.iso.org/iso/19144/-2/ed-1/en/</rdfs:isDefinedBy>
    <rdfs:domain rdf:resource="&iso19144-2;LC_PermittedPosRealValue"/>
    <rdfs:range rdf:resource="&xsd;double"/>
  </owl:DatatypeProperty>

  <!--+++++++++++++++++++++++++++++++++++++++++++++++-->
  <!-- DatatypeProperty: LC_PermittedRealValue.value -->
  <!--+++++++++++++++++++++++++++++++++++++++++++++++-->
  <owl:DatatypeProperty rdf:about="&iso19144-2;LC_PermittedRealValue.value">
    <rdfs:label>value</rdfs:label>
    <rdfs:isDefinedBy>http://standards.iso.org/iso/19144/-2/ed-1/en/</rdfs:isDefinedBy>
    <rdfs:domain rdf:resource="&iso19144-2;LC_PermittedRealValue"/>
    <rdfs:range rdf:resource="&xsd;double"/>
  </owl:DatatypeProperty>

</rdf:RDF>

