PREFIX cs: <http://def.isotc211.org/iso19157/-1/20yy/DataQualityEvaluation/code/EvaluationMethodTypeCode/>
PREFIX dcterms: <http://purl.org/dc/terms/>
PREFIX rdfs: <http://www.w3.org/2000/01/rdf-schema#>
PREFIX reg: <http://purl.org/linked-data/registry#>
PREFIX schema: <https://schema.org/>
PREFIX skos: <http://www.w3.org/2004/02/skos/core#>
PREFIX status: <http://def.isotc211.org/iso19135/-1/2015/CoreModel/code/RE_ItemStatus/>
PREFIX xsd: <http://www.w3.org/2001/XMLSchema#>

cs:directExternal
    a skos:Concept ;
    dcterms:identifier "directExternal"^^xsd:token ;
    dcterms:provenance "Presented in the original standard's codelist"@en ;
    reg:status status:original ;
    rdfs:isDefinedBy cs: ;
    skos:definition "method of evaluating the quality of a dataset based on inspection of items within the dataset, where reference data external to the dataset being evaluated is required" ;
    skos:inScheme cs: ;
    skos:prefLabel "directExternal" ;
    skos:topConceptOf cs: ;
.

cs:directInternal
    a skos:Concept ;
    dcterms:identifier "directInternal"^^xsd:token ;
    dcterms:provenance "Presented in the original standard's codelist"@en ;
    reg:status status:original ;
    rdfs:isDefinedBy cs: ;
    skos:definition "method of evaluating the quality of a dataset based on inspection of items within the dataset, where all data required is internal to the dataset being evaluated" ;
    skos:inScheme cs: ;
    skos:prefLabel "directInternal" ;
    skos:topConceptOf cs: ;
.

cs:indirect
    a skos:Concept ;
    dcterms:identifier "indirect"^^xsd:token ;
    dcterms:provenance "Presented in the original standard's codelist"@en ;
    reg:status status:original ;
    rdfs:isDefinedBy cs: ;
    skos:definition "method of evaluating the quality of a dataset based on external knowledge" ;
    skos:inScheme cs: ;
    skos:prefLabel "indirect" ;
    skos:topConceptOf cs: ;
.

<http://def.isotc211.org/org/tc211>
    a schema:Organization ;
    schema:description "The International Organization for Standardization's Technical Committee on \"Geographic information/Geomatics\", charged with standardization in the field of digital geographic information"@en ;
    schema:name "ISO's Technical Committee 211" ;
    schema:url "https://www.iso.org/committee/54904.html"^^xsd:anyURI ;
.

<http://def.isotc211.org/iso19157/-1/20yy/DataQualityEvaluation/code/EvaluationMethodTypeCode>
    a skos:ConceptScheme ;
    dcterms:created "2000-01-01"^^xsd:date ;
    dcterms:creator <http://def.isotc211.org/org/tc211> ;
    dcterms:identifier "EvaluationMethodTypeCode"^^xsd:token ;
    dcterms:isFormatOf <http://def.isotc211.org/iso19115/-1/2018/CitationAndResponsiblePartyInformation#CI_DateTypeCode> ;
    dcterms:issued "2000-01-01"^^xsd:date ;
    dcterms:modified "2000-01-01"^^xsd:date ;
    dcterms:provenance "Derived from TC211-produced RDF versions of the standard's UML"@en ;
    dcterms:publisher <http://def.isotc211.org/org/tc211> ;
    dcterms:source "http://standards.iso.org/iso/19157/-1/ed-1/en/"^^xsd:anyURI ;
    skos:definition "An ISO standard's ConceptScheme"@en ;
    skos:hasTopConcept
        cs:directExternal ,
        cs:directInternal ,
        cs:indirect ;
    skos:prefLabel "Evaluation Method Type Code"@en ;
.
