PREFIX : <http://def.isotc211.org/iso19115/-1/2018/CitationAndResponsiblePartyInformation/code/CI_PresentationFormCode/>
PREFIX cs: <http://def.isotc211.org/iso19115/-1/2018/CitationAndResponsiblePartyInformation/code/CI_PresentationFormCode>
PREFIX dcterms: <http://purl.org/dc/terms/>
PREFIX rdfs: <http://www.w3.org/2000/01/rdf-schema#>
PREFIX schema: <https://schema.org/>
PREFIX skos: <http://www.w3.org/2004/02/skos/core#>
PREFIX xsd: <http://www.w3.org/2001/XMLSchema#>

:audioDigital
    a skos:Concept ;
    dcterms:identifier "audioDigital"^^xsd:token ;
    dcterms:provenance "Code originally presented in the standard"@en ;
    rdfs:isDefinedBy cs: ;
    skos:definition "digital audio recording" ;
    skos:inScheme cs: ;
    skos:prefLabel "audioDigital" ;
    skos:topConceptOf cs: ;
.

:audioHardcopy
    a skos:Concept ;
    dcterms:identifier "audioHardcopy"^^xsd:token ;
    dcterms:provenance "Code originally presented in the standard"@en ;
    rdfs:isDefinedBy cs: ;
    skos:definition "audio recording delivered by analog media, such as a magnetic tape" ;
    skos:inScheme cs: ;
    skos:prefLabel "audioHardcopy" ;
    skos:topConceptOf cs: ;
.

:diagramDigital
    a skos:Concept ;
    dcterms:identifier "diagramDigital"^^xsd:token ;
    dcterms:provenance "Code originally presented in the standard"@en ;
    rdfs:isDefinedBy cs: ;
    skos:definition "information represented graphically by charts such as pie chart, bar chart, and other type of diagrams and recorded in digital format" ;
    skos:inScheme cs: ;
    skos:prefLabel "diagramDigital" ;
    skos:topConceptOf cs: ;
.

:diagramHardcopy
    a skos:Concept ;
    dcterms:identifier "diagramHardcopy"^^xsd:token ;
    dcterms:provenance "Code originally presented in the standard"@en ;
    rdfs:isDefinedBy cs: ;
    skos:definition "information represented graphically by charts such as pie chart, bar chart, and other type of diagrams and printed on paper, photographic material, or other media" ;
    skos:inScheme cs: ;
    skos:prefLabel "diagramHardcopy" ;
    skos:topConceptOf cs: ;
.

:documentDigital
    a skos:Concept ;
    dcterms:identifier "documentDigital"^^xsd:token ;
    dcterms:provenance "Code originally presented in the standard"@en ;
    rdfs:isDefinedBy cs: ;
    skos:definition "digital representation of a primarily textual item (can contain illustrations also)" ;
    skos:inScheme cs: ;
    skos:prefLabel "documentDigital" ;
    skos:topConceptOf cs: ;
.

:documentHardcopy
    a skos:Concept ;
    dcterms:identifier "documentHardcopy"^^xsd:token ;
    dcterms:provenance "Code originally presented in the standard"@en ;
    rdfs:isDefinedBy cs: ;
    skos:definition "representation of a primarily textual item (can contain illustrations also) on paper, photographic material, or other media" ;
    skos:inScheme cs: ;
    skos:prefLabel "documentHardcopy" ;
    skos:topConceptOf cs: ;
.

:imageDigital
    a skos:Concept ;
    dcterms:identifier "imageDigital"^^xsd:token ;
    dcterms:provenance "Code originally presented in the standard"@en ;
    rdfs:isDefinedBy cs: ;
    skos:definition "likeness of natural or man-made features, objects, and activities acquired through the sensing of visual or any other segment of the electromagnetic spectrum by sensors, such as thermal infrared, and high resolution radar and stored in digital format" ;
    skos:inScheme cs: ;
    skos:prefLabel "imageDigital" ;
    skos:topConceptOf cs: ;
.

:imageHardcopy
    a skos:Concept ;
    dcterms:identifier "imageHardcopy"^^xsd:token ;
    dcterms:provenance "Code originally presented in the standard"@en ;
    rdfs:isDefinedBy cs: ;
    skos:definition "likeness of natural or man-made features, objects, and activities acquired through the sensing of visual or any other segment of the electromagnetic spectrum by sensors, such as thermal infrared, and high resolution radar and reproduced on paper, photographic material, or other media for use directly by the human user" ;
    skos:inScheme cs: ;
    skos:prefLabel "imageHardcopy" ;
    skos:topConceptOf cs: ;
.

:mapDigital
    a skos:Concept ;
    dcterms:identifier "mapDigital"^^xsd:token ;
    dcterms:provenance "Code originally presented in the standard"@en ;
    rdfs:isDefinedBy cs: ;
    skos:definition "map represented in raster or vector form" ;
    skos:inScheme cs: ;
    skos:prefLabel "mapDigital" ;
    skos:topConceptOf cs: ;
.

:mapHardcopy
    a skos:Concept ;
    dcterms:identifier "mapHardcopy"^^xsd:token ;
    dcterms:provenance "Code originally presented in the standard"@en ;
    rdfs:isDefinedBy cs: ;
    skos:definition "map printed on paper, photographic material, or other media for use directly by the human user" ;
    skos:inScheme cs: ;
    skos:prefLabel "mapHardcopy" ;
    skos:topConceptOf cs: ;
.

:modelDigital
    a skos:Concept ;
    dcterms:identifier "modelDigital"^^xsd:token ;
    dcterms:provenance "Code originally presented in the standard"@en ;
    rdfs:isDefinedBy cs: ;
    skos:definition "multi-dimensional digital representation of a feature, process, etc." ;
    skos:inScheme cs: ;
    skos:prefLabel "modelDigital" ;
    skos:topConceptOf cs: ;
.

:modelHardcopy
    a skos:Concept ;
    dcterms:identifier "modelHardcopy"^^xsd:token ;
    dcterms:provenance "Code originally presented in the standard"@en ;
    rdfs:isDefinedBy cs: ;
    skos:definition "3-dimensional, physical model" ;
    skos:inScheme cs: ;
    skos:prefLabel "modelHardcopy" ;
    skos:topConceptOf cs: ;
.

:multimediaDigital
    a skos:Concept ;
    dcterms:identifier "multimediaDigital"^^xsd:token ;
    dcterms:provenance "Code originally presented in the standard"@en ;
    rdfs:isDefinedBy cs: ;
    skos:definition "information representation using simultaneously various digital modes for text, sound, image" ;
    skos:inScheme cs: ;
    skos:prefLabel "multimediaDigital" ;
    skos:topConceptOf cs: ;
.

:multimediaHardcopy
    a skos:Concept ;
    dcterms:identifier "multimediaHardcopy"^^xsd:token ;
    dcterms:provenance "Code originally presented in the standard"@en ;
    rdfs:isDefinedBy cs: ;
    skos:definition "information representation using simultaneously various analog modes for text, sound, image" ;
    skos:inScheme cs: ;
    skos:prefLabel "multimediaHardcopy" ;
    skos:topConceptOf cs: ;
.

:physicalObject
    a skos:Concept ;
    dcterms:identifier "physicalObject"^^xsd:token ;
    dcterms:provenance "Code originally presented in the standard"@en ;
    rdfs:isDefinedBy cs: ;
    skos:definition "a physical object. Eg. Rock or mineral sample, microscope slide" ;
    skos:inScheme cs: ;
    skos:prefLabel "physicalObject" ;
    skos:topConceptOf cs: ;
.

:profileDigital
    a skos:Concept ;
    dcterms:identifier "profileDigital"^^xsd:token ;
    dcterms:provenance "Code originally presented in the standard"@en ;
    rdfs:isDefinedBy cs: ;
    skos:definition "vertical cross-section in digital form" ;
    skos:inScheme cs: ;
    skos:prefLabel "profileDigital" ;
    skos:topConceptOf cs: ;
.

:profileHardcopy
    a skos:Concept ;
    dcterms:identifier "profileHardcopy"^^xsd:token ;
    dcterms:provenance "Code originally presented in the standard"@en ;
    rdfs:isDefinedBy cs: ;
    skos:definition "vertical cross-section printed on paper, etc." ;
    skos:inScheme cs: ;
    skos:prefLabel "profileHardcopy" ;
    skos:topConceptOf cs: ;
.

:tableDigital
    a skos:Concept ;
    dcterms:identifier "tableDigital"^^xsd:token ;
    dcterms:provenance "Code originally presented in the standard"@en ;
    rdfs:isDefinedBy cs: ;
    skos:definition "digital representation of facts or figures systematically displayed, especially in columns" ;
    skos:inScheme cs: ;
    skos:prefLabel "tableDigital" ;
    skos:topConceptOf cs: ;
.

:tableHardcopy
    a skos:Concept ;
    dcterms:identifier "tableHardcopy"^^xsd:token ;
    dcterms:provenance "Code originally presented in the standard"@en ;
    rdfs:isDefinedBy cs: ;
    skos:definition "representation of facts or figures systematically displayed, especially in columns, printed on paper, photographic material, or other media" ;
    skos:inScheme cs: ;
    skos:prefLabel "tableHardcopy" ;
    skos:topConceptOf cs: ;
.

:videoDigital
    a skos:Concept ;
    dcterms:identifier "videoDigital"^^xsd:token ;
    dcterms:provenance "Code originally presented in the standard"@en ;
    rdfs:isDefinedBy cs: ;
    skos:definition "digital video recording" ;
    skos:inScheme cs: ;
    skos:prefLabel "videoDigital" ;
    skos:topConceptOf cs: ;
.

:videoHardcopy
    a skos:Concept ;
    dcterms:identifier "videoHardcopy"^^xsd:token ;
    dcterms:provenance "Code originally presented in the standard"@en ;
    rdfs:isDefinedBy cs: ;
    skos:definition "video recording on film" ;
    skos:inScheme cs: ;
    skos:prefLabel "videoHardcopy" ;
    skos:topConceptOf cs: ;
.

<http://def.isotc211.org/org/tc211>
    a schema:Organization ;
    schema:description "The International Organization for Standardization's Technical Committee on \"Geographic information/Geomatics\", charged with standardization in the field of digital geographic information"@en ;
    schema:name "ISO's Technical Committee 211" ;
    schema:url "https://www.iso.org/committee/54904.html"^^xsd:anyURI ;
.

cs:
    a skos:ConceptScheme ;
    dcterms:created "2000-01-01"^^xsd:date ;
    dcterms:creator <http://def.isotc211.org/org/tc211> ;
    dcterms:identifier "CI_PresentationFormCode"^^xsd:token ;
    dcterms:isFormatOf <http://def.isotc211.org/iso19115/-1/2018/CitationAndResponsiblePartyInformation#CI_PresentationFormCode> ;
    dcterms:issued "2000-01-01"^^xsd:date ;
    dcterms:modified "2000-01-01"^^xsd:date ;
    dcterms:provenance "Derived from TC211-produced RDF versions of the standard's UML"@en ;
    dcterms:publisher <http://def.isotc211.org/org/tc211> ;
    dcterms:source "http://standards.iso.org/iso/19115/-1/ed-1/en/"^^xsd:anyURI ;
    skos:definition "An ISO standard's ConceptScheme"@en ;
    skos:hasTopConcept
        :audioDigital ,
        :audioHardcopy ,
        :diagramDigital ,
        :diagramHardcopy ,
        :documentDigital ,
        :documentHardcopy ,
        :imageDigital ,
        :imageHardcopy ,
        :mapDigital ,
        :mapHardcopy ,
        :modelDigital ,
        :modelHardcopy ,
        :multimediaDigital ,
        :multimediaHardcopy ,
        :physicalObject ,
        :profileDigital ,
        :profileHardcopy ,
        :tableDigital ,
        :tableHardcopy ,
        :videoDigital ,
        :videoHardcopy ;
    skos:prefLabel "CI_PresentationFormCode"@en ;
.

