PREFIX : <http://def.isotc211.org/iso19115/-1/2018/SpatialRepresentationInformation/code/MD_TopologyLevelCode/>
PREFIX cs: <http://def.isotc211.org/iso19115/-1/2018/SpatialRepresentationInformation/code/MD_TopologyLevelCode>
PREFIX dcterms: <http://purl.org/dc/terms/>
PREFIX rdfs: <http://www.w3.org/2000/01/rdf-schema#>
PREFIX schema: <https://schema.org/>
PREFIX skos: <http://www.w3.org/2004/02/skos/core#>
PREFIX xsd: <http://www.w3.org/2001/XMLSchema#>

:abstract
    a skos:Concept ;
    dcterms:identifier "abstract"^^xsd:token ;
    dcterms:provenance "Code originally presented in the standard"@en ;
    rdfs:isDefinedBy cs: ;
    skos:definition "topological complex without any specified geometric realisation" ;
    skos:inScheme cs: ;
    skos:prefLabel "abstract" ;
    skos:topConceptOf cs: ;
.

:fullPlanarGraph
    a skos:Concept ;
    dcterms:identifier "fullPlanarGraph"^^xsd:token ;
    dcterms:provenance "Code originally presented in the standard"@en ;
    rdfs:isDefinedBy cs: ;
    skos:definition "2-dimensional topological complex that is planar. (A 2-dimensional topological complex is commonly called 'full topology' in a cartographic 2D environment.)" ;
    skos:inScheme cs: ;
    skos:prefLabel "fullPlanarGraph" ;
    skos:topConceptOf cs: ;
.

:fullSurfaceGraph
    a skos:Concept ;
    dcterms:identifier "fullSurfaceGraph"^^xsd:token ;
    dcterms:provenance "Code originally presented in the standard"@en ;
    rdfs:isDefinedBy cs: ;
    skos:definition "2-dimensional topological complex that is isomorphic to a subset of a surface" ;
    skos:inScheme cs: ;
    skos:prefLabel "fullSurfaceGraph" ;
    skos:topConceptOf cs: ;
.

:fullTopology3D
    a skos:Concept ;
    dcterms:identifier "fullTopology3D"^^xsd:token ;
    dcterms:provenance "Code originally presented in the standard"@en ;
    rdfs:isDefinedBy cs: ;
    skos:definition "complete coverage of a 3D Euclidean coordinate space" ;
    skos:inScheme cs: ;
    skos:prefLabel "fullTopology3D" ;
    skos:topConceptOf cs: ;
.

:geometryOnly
    a skos:Concept ;
    dcterms:identifier "geometryOnly"^^xsd:token ;
    dcterms:provenance "Code originally presented in the standard"@en ;
    rdfs:isDefinedBy cs: ;
    skos:definition "geometry objects without any additional structure which describes topology" ;
    skos:inScheme cs: ;
    skos:prefLabel "geometryOnly" ;
    skos:topConceptOf cs: ;
.

:planarGraph
    a skos:Concept ;
    dcterms:identifier "planarGraph"^^xsd:token ;
    dcterms:provenance "Code originally presented in the standard"@en ;
    rdfs:isDefinedBy cs: ;
    skos:definition "1-dimensional topological complex that is planar. (A planar graph is a graph that can be drawn in a plane in such a way that no two edges intersect except at a vertex.)" ;
    skos:inScheme cs: ;
    skos:prefLabel "planarGraph" ;
    skos:topConceptOf cs: ;
.

:surfaceGraph
    a skos:Concept ;
    dcterms:identifier "surfaceGraph"^^xsd:token ;
    dcterms:provenance "Code originally presented in the standard"@en ;
    rdfs:isDefinedBy cs: ;
    skos:definition "1-dimensional topological complex that is isomorphic to a subset of a surface. (A geometric complex is isomorphic to a topological complex if their elements are in a one-to-one, dimensional-and boundary-preserving correspondence to one another.)" ;
    skos:inScheme cs: ;
    skos:prefLabel "surfaceGraph" ;
    skos:topConceptOf cs: ;
.

:topology1D
    a skos:Concept ;
    dcterms:identifier "topology1D"^^xsd:token ;
    dcterms:provenance "Code originally presented in the standard"@en ;
    rdfs:isDefinedBy cs: ;
    skos:definition "1-dimensional topological complex - commonly called 'chain-node' topology" ;
    skos:inScheme cs: ;
    skos:prefLabel "topology1D" ;
    skos:topConceptOf cs: ;
.

:topology3D
    a skos:Concept ;
    dcterms:identifier "topology3D"^^xsd:token ;
    dcterms:provenance "Code originally presented in the standard"@en ;
    rdfs:isDefinedBy cs: ;
    skos:definition "3-dimensional topological complex. (A topological complex is a collection of topological primitives that are closed under the boundary operations.)" ;
    skos:inScheme cs: ;
    skos:prefLabel "topology3D" ;
    skos:topConceptOf cs: ;
.

<http://def.isotc211.org/org/tc211>
    a schema:Organization ;
    schema:description "The International Organization for Standardization's Technical Committee on \"Geographic information/Geomatics\", charged with standardization in the field of digital geographic information"@en ;
    schema:name "ISO's Technical Committee 211" ;
    schema:url "https://www.iso.org/committee/54904.html"^^xsd:anyURI ;
.

cs:
    a skos:ConceptScheme ;
    dcterms:created "2000-01-01"^^xsd:date ;
    dcterms:creator <http://def.isotc211.org/org/tc211> ;
    dcterms:identifier "MD_TopologyLevelCode"^^xsd:token ;
    dcterms:isFormatOf <http://def.isotc211.org/iso19115/-1/2018/SpatialRepresentationInformation#MD_TopologyLevelCode> ;
    dcterms:issued "2000-01-01"^^xsd:date ;
    dcterms:modified "2000-01-01"^^xsd:date ;
    dcterms:provenance "Derived from TC211-produced RDF versions of the standard's UML"@en ;
    dcterms:publisher <http://def.isotc211.org/org/tc211> ;
    dcterms:source "http://standards.iso.org/iso/19115/-1/ed-1/en/"^^xsd:anyURI ;
    skos:definition "An ISO standard's ConceptScheme"@en ;
    skos:hasTopConcept
        :abstract ,
        :fullPlanarGraph ,
        :fullSurfaceGraph ,
        :fullTopology3D ,
        :geometryOnly ,
        :planarGraph ,
        :surfaceGraph ,
        :topology1D ,
        :topology3D ;
    skos:prefLabel "MD_TopologyLevelCode"@en ;
.

