<?xml version="1.0"?>

<!DOCTYPE rdf:RDF [
  <!ENTITY owl "http://www.w3.org/2002/07/owl#" >
  <!ENTITY xsd "http://www.w3.org/2001/XMLSchema#" >
  <!ENTITY rdfs "http://www.w3.org/2000/01/rdf-schema#" >
  <!ENTITY rdf "http://www.w3.org/1999/02/22-rdf-syntax-ns#" >
  <!ENTITY dc "http://purl.org/dc/elements/1.1/" >
  <!ENTITY dct "http://purl.org/dc/terms/" >
  <!ENTITY skos "http://www.w3.org/2004/02/skos/core#" >
  <!ENTITY iso19150-2 "http://def.isotc211.org/iso19150/-2/2012/base#" >
  <!ENTITY iso19103 "http://def.isotc211.org/iso19103/2005/Numerics#" >

]>

<rdf:RDF xmlns="http://def.isotc211.org/iso19103/2005/Numerics#"
  xml:base="http://def.isotc211.org/iso19103/2005/Numerics"
  xmlns:owl="http://www.w3.org/2002/07/owl#"
  xmlns:xsd="http://www.w3.org/2001/XMLSchema#"
  xmlns:rdfs="http://www.w3.org/2000/01/rdf-schema#"
  xmlns:rdf="http://www.w3.org/1999/02/22-rdf-syntax-ns#"
  xmlns:dc="http://purl.org/dc/elements/1.1/"
  xmlns:dct="http://purl.org/dc/terms/"
  xmlns:skos="http://www.w3.org/2004/02/skos/core#"
  xmlns:iso19150-2="http://def.isotc211.org/iso19150/-2/2012/base#"
  xmlns:iso19103="http://def.isotc211.org/iso19103/2005/Numerics#">
  <owl:Ontology rdf:about="http://def.isotc211.org/iso19103/2005/Numerics">
    <rdfs:label>ISO 19103:2005 Numerics</rdfs:label>
    <dct:source>http://standards.iso.org/iso/19103/ed-1/en/</dct:source>
    <owl:versionInfo>2005-07-15</owl:versionInfo>
    <owl:imports rdf:resource="http://def.isotc211.org/iso19150/-2/2012/base"/>
  </owl:Ontology>
  <owl:Class rdf:about="&iso19103;Decimal">
    <rdfs:label>Decimal</rdfs:label>
    <skos:definition>The usually finite representation of a decimal number. It differs from the common binary Real implementation in that it can represent 1.sl.10 (one-tenth) without error, while binary real representation can only represent powers of 1.sl.2 (one-half) exactly. Since many currencies are decimal, these representations are preferred in dealing with such moneys. This is also true for mile markers, which are often given in decimals.Can be thought of as an integer part followed by a fractional part given in multiples of powers of 1.sl.10 (tenths).</skos:definition>
    <rdfs:isDefinedBy>http://standards.iso.org/iso/19103/ed-1/en/</rdfs:isDefinedBy>
    <rdfs:subClassOf rdf:resource="&iso19103;Number"/>
  </owl:Class>
  <owl:Class rdf:about="&iso19103;Integer">
    <rdfs:label>Integer</rdfs:label>
    <skos:definition>An exact integer value, with no fractional part. </skos:definition>
    <rdfs:isDefinedBy>http://standards.iso.org/iso/19103/ed-1/en/</rdfs:isDefinedBy>
    <rdfs:subClassOf rdf:resource="&iso19103;Number"/>
  </owl:Class>
  <owl:Class rdf:about="&iso19103;Number">
    <rdfs:label>Number</rdfs:label>
    <skos:definition>The base type for all number data, giving the basic algebraic operations. Since all concrete types have finite representations, some part of this algebra for most types exhibit some inaccuracy. For example, Integers cannot divide very well, and reals and decimals cannot avoid certain types of inaccuracies that depend on their representation semantics. </skos:definition>
    <rdfs:isDefinedBy>http://standards.iso.org/iso/19103/ed-1/en/</rdfs:isDefinedBy>
    <iso19150-2:isAbstract rdf:datatype="&xsd;boolean">true</iso19150-2:isAbstract>
  </owl:Class>
  <owl:Class rdf:about="&iso19103;Real">
    <rdfs:label>Real</rdfs:label>
    <skos:definition>The common binary Real finite implementation using base 2. Since such reals can approximate any measure where absolute accuracy is not possible, this form of numeric is most often used for measures. In cases were absolute accuracy is needed, such as currencies, then a decimal representation may be preferred (assuming the currency is decimal, such as the US dollar, British pound, etc.). Where there are no subunits possible, Integer numbers may be preferred.  Can be thought of as an integer part followed by a fractional part given in multiples of powers of 1.sl.2 (halves).</skos:definition>
    <rdfs:isDefinedBy>http://standards.iso.org/iso/19103/ed-1/en/</rdfs:isDefinedBy>
    <rdfs:subClassOf rdf:resource="&iso19103;Number"/>
  </owl:Class>
  <owl:Class rdf:about="&iso19103;UnlimitedInteger">
    <rdfs:label>UnlimitedInteger</rdfs:label>
    <skos:definition>-- Infinite if and only if value is not specified{[ isInfinte .eq. True ] .eq. [ value .eq. Null ]}-- value is either infinite or non-negative{value .lt..gt. Null implies value .gt..eq. 0}</skos:definition>
    <rdfs:isDefinedBy>http://standards.iso.org/iso/19103/ed-1/en/</rdfs:isDefinedBy>
    <rdfs:subClassOf>
      <owl:Restriction>
        <owl:onProperty rdf:resource="&iso19103;UnlimitedInteger.isInfinite"/>
        <owl:cardinality rdf:datatype="&xsd;nonNegativeInteger">1</owl:cardinality>
      </owl:Restriction>
    </rdfs:subClassOf>
    <rdfs:subClassOf>
      <owl:Restriction>
        <owl:onProperty rdf:resource="&iso19103;UnlimitedInteger.isInfinite"/>
        <owl:allValuesFrom rdf:resource="&xsd;boolean"/>
      </owl:Restriction>
    </rdfs:subClassOf>
    <rdfs:subClassOf>
      <owl:Restriction>
        <owl:onProperty rdf:resource="&iso19103;UnlimitedInteger.value"/>
        <owl:maxCardinality rdf:datatype="&xsd;nonNegativeInteger">1</owl:maxCardinality>
      </owl:Restriction>
    </rdfs:subClassOf>
    <rdfs:subClassOf>
      <owl:Restriction>
        <owl:onProperty rdf:resource="&iso19103;UnlimitedInteger.value"/>
        <owl:allValuesFrom rdf:resource="&xsd;integer"/>
      </owl:Restriction>
    </rdfs:subClassOf>
  </owl:Class>
  <owl:Class rdf:about="&iso19103;Vector">
    <rdfs:label>Vector</rdfs:label>
    <skos:definition>A vector is a sequence of a fixed length of Numbers. Normally, the numbers represent some measures, and thus vectors are often used where records of Numbers would be more appropriate. In geometry for example, direct positions are given by undistinguished coordinate vectors, which can be interpreted through the use of coordinate reference systems. </skos:definition>
    <rdfs:isDefinedBy>http://standards.iso.org/iso/19103/ed-1/en/</rdfs:isDefinedBy>
    <rdfs:subClassOf>
      <owl:Restriction>
        <owl:onProperty rdf:resource="&iso19103;Vector.dimension"/>
        <owl:cardinality rdf:datatype="&xsd;nonNegativeInteger">1</owl:cardinality>
      </owl:Restriction>
    </rdfs:subClassOf>
    <rdfs:subClassOf>
      <owl:Restriction>
        <owl:onProperty rdf:resource="&iso19103;Vector.dimension"/>
        <owl:allValuesFrom rdf:resource="&xsd;integer"/>
      </owl:Restriction>
    </rdfs:subClassOf>
    <rdfs:subClassOf>
      <owl:Restriction>
        <owl:onProperty rdf:resource="&iso19103;Vector.ordinates"/>
        <owl:minCardinality rdf:datatype="&xsd;nonNegativeInteger">1</owl:minCardinality>
      </owl:Restriction>
    </rdfs:subClassOf>
    <rdfs:subClassOf>
      <owl:Restriction>
        <owl:onProperty rdf:resource="&iso19103;Vector.ordinates"/>
        <owl:allValuesFrom rdf:resource="&iso19103;Number"/>
      </owl:Restriction>
    </rdfs:subClassOf>
  </owl:Class>
  <owl:DatatypeProperty rdf:about="&iso19103;UnlimitedInteger.isInfinite">
    <rdfs:label>isInfinite</rdfs:label>
    <rdfs:isDefinedBy>http://standards.iso.org/iso/19103/ed-1/en/</rdfs:isDefinedBy>
    <rdfs:domain rdf:resource="&iso19103;UnlimitedInteger"/>
    <rdfs:range rdf:resource="&xsd;boolean"/>
  </owl:DatatypeProperty>
  <owl:DatatypeProperty rdf:about="&iso19103;UnlimitedInteger.value">
    <rdfs:label>value</rdfs:label>
    <rdfs:isDefinedBy>http://standards.iso.org/iso/19103/ed-1/en/</rdfs:isDefinedBy>
    <rdfs:domain rdf:resource="&iso19103;UnlimitedInteger"/>
    <rdfs:range rdf:resource="&xsd;integer"/>
  </owl:DatatypeProperty>
  <owl:DatatypeProperty rdf:about="&iso19103;Vector.dimension">
    <rdfs:label>dimension</rdfs:label>
    <rdfs:isDefinedBy>http://standards.iso.org/iso/19103/ed-1/en/</rdfs:isDefinedBy>
    <rdfs:domain rdf:resource="&iso19103;Vector"/>
    <rdfs:range rdf:resource="&xsd;integer"/>
  </owl:DatatypeProperty>
  <owl:ObjectProperty rdf:about="&iso19103;Vector.ordinates">
    <rdfs:label>ordinates</rdfs:label>
    <rdfs:isDefinedBy>http://standards.iso.org/iso/19103/ed-1/en/</rdfs:isDefinedBy>
    <rdfs:domain rdf:resource="&iso19103;Vector"/>
    <rdfs:range rdf:resource="&iso19103;Number"/>
  </owl:ObjectProperty>
</rdf:RDF>

