<?xml version="1.0"?>

<!DOCTYPE rdf:RDF [
  <!ENTITY owl "http://www.w3.org/2002/07/owl#" >
  <!ENTITY xsd "http://www.w3.org/2001/XMLSchema#" >
  <!ENTITY rdfs "http://www.w3.org/2000/01/rdf-schema#" >
  <!ENTITY rdf "http://www.w3.org/1999/02/22-rdf-syntax-ns#" >
  <!ENTITY dc "http://purl.org/dc/elements/1.1/" >
  <!ENTITY dct "http://purl.org/dc/terms/" >
  <!ENTITY skos "http://www.w3.org/2004/02/skos/core#" >
  <!ENTITY iso19150-2 "http://def.isotc211.org/iso19150/-2/2012/base#" >
  <!ENTITY iso19111_7020 "http://def.isotc211.org/iso19111/2019/CommonClasses#" >
  <!ENTITY iso19103_5905 "http://def.isotc211.org/iso19103/2015/MeasureTypes#" >
  <!ENTITY iso19111_7025 "http://def.isotc211.org/iso19111/2019/CoordinateOperations#" >
  <!ENTITY iso19157_4482 "http://def.isotc211.org/iso19157/2013/DataQuality#" >
  <!ENTITY iso19111_4044 "http://def.isotc211.org/iso19111/2007/Datums#" >
  <!ENTITY iso19111 "http://def.isotc211.org/iso19111/2019/Datums#" >
  <!ENTITY iso19111Code "http://def.isotc211.org/iso19111/2019/Datums/code/">

]>

  <!--++++++++++++++++++++++++++++++++++++++++++++++-->
  <!-- File name:         Datums.rdf                -->
  <!-- Generator:         GOM_Technologies::UML2OWL -->
  <!-- Generator version: 2.6                       -->
  <!-- File date:         5-11-2019                 -->
  <!--++++++++++++++++++++++++++++++++++++++++++++++-->

<rdf:RDF xmlns="http://def.isotc211.org/iso19111/2019/Datums#"
  xml:base="http://def.isotc211.org/iso19111/2019/Datums"
  xmlns:owl="http://www.w3.org/2002/07/owl#"
  xmlns:xsd="http://www.w3.org/2001/XMLSchema#"
  xmlns:rdfs="http://www.w3.org/2000/01/rdf-schema#"
  xmlns:rdf="http://www.w3.org/1999/02/22-rdf-syntax-ns#"
  xmlns:dc="http://purl.org/dc/elements/1.1/"
  xmlns:dct="http://purl.org/dc/terms/"
  xmlns:skos="http://www.w3.org/2004/02/skos/core#"
  xmlns:iso19150-2="http://def.isotc211.org/iso19150/-2/2012/base#"
  xmlns:iso19111_7020="http://def.isotc211.org/iso19111/2019/CommonClasses#"
  xmlns:iso19103_5905="http://def.isotc211.org/iso19103/2015/MeasureTypes#"
  xmlns:iso19111_7025="http://def.isotc211.org/iso19111/2019/CoordinateOperations#"
  xmlns:iso19157_4482="http://def.isotc211.org/iso19157/2013/DataQuality#"
  xmlns:iso19111_4044="http://def.isotc211.org/iso19111/2007/Datums#"
  xmlns:iso19111="http://def.isotc211.org/iso19111/2019/Datums#"
  xmlns:iso19111Code="http://def.isotc211.org/iso19111/2019/Datums/code/">

  <!--+++++++++++++++++++++++++++++++++-->
  <!-- Ontology: ISO 19111:2019 Datums -->
  <!--+++++++++++++++++++++++++++++++++-->
  <owl:Ontology rdf:about="http://def.isotc211.org/iso19111/2019/Datums">
    <rdfs:label>ISO 19111:2019 Datums</rdfs:label>
    <dct:source>http://standards.iso.org/iso/19111/ed-3/en/</dct:source>
    <owl:versionInfo>2019-01</owl:versionInfo>
    <owl:imports rdf:resource="http://def.isotc211.org/iso19111/2019/CommonClasses"/>
    <!--owl:imports rdf:resource="http://def.isotc211.org/iso19103/2015/MeasureTypes"/-->
    <owl:imports rdf:resource="http://def.isotc211.org/iso19111/2019/CoordinateOperations"/>
    <!--owl:imports rdf:resource="http://def.isotc211.org/iso19157/2013/DataQuality"/-->
    <owl:imports rdf:resource="http://def.isotc211.org/iso19111/2007/Datums"/>
    <owl:imports rdf:resource="http://def.isotc211.org/iso19150/-2/2012/base"/>
  </owl:Ontology>

  <!--++++++++++++++-->
  <!-- Class: Datum -->
  <!--++++++++++++++-->
  <owl:Class rdf:about="&iso19111;Datum">
    <rdfs:label>Datum</rdfs:label>
    <skos:definition>specification of the relationship of a coordinate system to an object, thus creating a coordinate reference systemNote: For geodetic and vertical coordinate reference systems, it relates a coordinate system to the Earth. With other types of coordinate reference systems, the datum may relate the coordinate system to another physical or virtual object. A datum uses a parameter or set of parameters that determine the location of the origin of the coordinate reference system. Each datum subtype can be associated with only specific types of coordinate reference systems.</skos:definition>
    <rdfs:isDefinedBy>http://standards.iso.org/iso/19111/ed-3/en/</rdfs:isDefinedBy>
    <iso19150-2:isAbstract rdf:datatype="&xsd;boolean">true</iso19150-2:isAbstract>
    <rdfs:subClassOf rdf:resource="&iso19111_7020;ObjectUsage"/>
    <rdfs:subClassOf>
      <owl:Restriction>
        <owl:onProperty rdf:resource="&iso19111;Datum.anchorDefinition"/>
        <owl:maxCardinality rdf:datatype="&xsd;nonNegativeInteger">1</owl:maxCardinality>
      </owl:Restriction>
    </rdfs:subClassOf>
    <rdfs:subClassOf>
      <owl:Restriction>
        <owl:onProperty rdf:resource="&iso19111;Datum.anchorDefinition"/>
        <owl:allValuesFrom rdf:resource="&xsd;string"/>
      </owl:Restriction>
    </rdfs:subClassOf>
    <rdfs:subClassOf>
      <owl:Restriction>
        <owl:onProperty rdf:resource="&iso19111;Datum.publicationDate"/>
        <owl:maxCardinality rdf:datatype="&xsd;nonNegativeInteger">1</owl:maxCardinality>
      </owl:Restriction>
    </rdfs:subClassOf>
    <rdfs:subClassOf>
      <owl:Restriction>
        <owl:onProperty rdf:resource="&iso19111;Datum.publicationDate"/>
        <owl:allValuesFrom rdf:resource="&rdf;XMLLiteral"/>
      </owl:Restriction>
    </rdfs:subClassOf>
    <rdfs:subClassOf>
      <owl:Restriction>
        <owl:onProperty rdf:resource="&iso19111;Datum.conventionalRS"/>
        <owl:maxCardinality rdf:datatype="&xsd;nonNegativeInteger">1</owl:maxCardinality>
      </owl:Restriction>
    </rdfs:subClassOf>
    <rdfs:subClassOf>
      <owl:Restriction>
        <owl:onProperty rdf:resource="&iso19111;Datum.conventionalRS"/>
        <owl:allValuesFrom rdf:resource="&iso19111_7020;IdentifiedObject"/>
      </owl:Restriction>
    </rdfs:subClassOf>
  </owl:Class>

  <!--+++++++++++++++++++++++++++++++-->
  <!-- Class: GeodeticReferenceFrame -->
  <!--+++++++++++++++++++++++++++++++-->
  <owl:Class rdf:about="&iso19111;GeodeticReferenceFrame">
    <rdfs:label>GeodeticReferenceFrame</rdfs:label>
    <skos:definition>definition of the position, scale and orientation of a geocentric Cartesian 3D coordinate system relative to the EarthNote 1: It may also identify a defined ellipsoid (or sphere) that approximates the shape of the Earth and which is centred on and aligned to this geocentric coordinate system. Older geodetic datums define the location and orientation of a defined ellipsoid (or sphere) that approximates the shape of the earth.Note 2: In 19111:2007 this class was called GeodeticDatum.</skos:definition>
    <rdfs:isDefinedBy>http://standards.iso.org/iso/19111/ed-3/en/</rdfs:isDefinedBy>
    <rdfs:subClassOf rdf:resource="&iso19111;Datum"/>
    <rdfs:subClassOf>
      <owl:Restriction>
        <owl:onProperty rdf:resource="&iso19111;GeodeticReferenceFrame.ellipsoid"/>
        <owl:maxCardinality rdf:datatype="&xsd;nonNegativeInteger">1</owl:maxCardinality>
      </owl:Restriction>
    </rdfs:subClassOf>
    <rdfs:subClassOf>
      <owl:Restriction>
        <owl:onProperty rdf:resource="&iso19111;GeodeticReferenceFrame.ellipsoid"/>
        <owl:allValuesFrom rdf:resource="&iso19111;Ellipsoid"/>
      </owl:Restriction>
    </rdfs:subClassOf>
    <rdfs:subClassOf>
      <owl:Restriction>
        <owl:onProperty rdf:resource="&iso19111;GeodeticReferenceFrame.primeMeridian"/>
        <owl:cardinality rdf:datatype="&xsd;nonNegativeInteger">1</owl:cardinality>
      </owl:Restriction>
    </rdfs:subClassOf>
    <rdfs:subClassOf>
      <owl:Restriction>
        <owl:onProperty rdf:resource="&iso19111;GeodeticReferenceFrame.primeMeridian"/>
        <owl:allValuesFrom rdf:resource="&iso19111;PrimeMeridian"/>
      </owl:Restriction>
    </rdfs:subClassOf>
  </owl:Class>

  <!--++++++++++++++++++++++++++++++++++++++-->
  <!-- Class: DynamicGeodeticReferenceFrame -->
  <!--++++++++++++++++++++++++++++++++++++++-->
  <owl:Class rdf:about="&iso19111;DynamicGeodeticReferenceFrame">
    <rdfs:label>DynamicGeodeticReferenceFrame</rdfs:label>
    <skos:definition>geodetic reference frame in which some of the parameters describe time evolution of defining station coordinatesExample: defining station coordinates having linear velocities to account for crustal motion.</skos:definition>
    <rdfs:isDefinedBy>http://standards.iso.org/iso/19111/ed-3/en/</rdfs:isDefinedBy>
    <rdfs:subClassOf rdf:resource="&iso19111;GeodeticReferenceFrame"/>
    <rdfs:subClassOf>
      <owl:Restriction>
        <owl:onProperty rdf:resource="&iso19111;DynamicGeodeticReferenceFrame.frameReferenceEpoch"/>
        <owl:cardinality rdf:datatype="&xsd;nonNegativeInteger">1</owl:cardinality>
      </owl:Restriction>
    </rdfs:subClassOf>
    <rdfs:subClassOf>
      <owl:Restriction>
        <owl:onProperty rdf:resource="&iso19111;DynamicGeodeticReferenceFrame.frameReferenceEpoch"/>
        <owl:allValuesFrom rdf:resource="&iso19103_5905;Measure"/>
      </owl:Restriction>
    </rdfs:subClassOf>
  </owl:Class>

  <!--++++++++++++++++++++++-->
  <!-- Class: PrimeMeridian -->
  <!--++++++++++++++++++++++-->
  <owl:Class rdf:about="&iso19111;PrimeMeridian">
    <rdfs:label>PrimeMeridian</rdfs:label>
    <skos:definition>origin meridian from which longitude values are determined Note: The default value for prime meridian name is “Greenwich”. When the default applies, the value for the greenwichLongitude shall be 0 (degrees).</skos:definition>
    <rdfs:isDefinedBy>http://standards.iso.org/iso/19111/ed-3/en/</rdfs:isDefinedBy>
    <rdfs:subClassOf rdf:resource="&iso19111_7020;IdentifiedObject"/>
    <rdfs:subClassOf>
      <owl:Restriction>
        <owl:onProperty rdf:resource="&iso19111;PrimeMeridian.greenwichLongitude"/>
        <owl:cardinality rdf:datatype="&xsd;nonNegativeInteger">1</owl:cardinality>
      </owl:Restriction>
    </rdfs:subClassOf>
    <rdfs:subClassOf>
      <owl:Restriction>
        <owl:onProperty rdf:resource="&iso19111;PrimeMeridian.greenwichLongitude"/>
        <owl:allValuesFrom rdf:resource="&iso19103_5905;Angle"/>
      </owl:Restriction>
    </rdfs:subClassOf>
  </owl:Class>

  <!--++++++++++++++++++-->
  <!-- Class: Ellipsoid -->
  <!--++++++++++++++++++-->
  <owl:Class rdf:about="&iso19111;Ellipsoid">
    <rdfs:label>Ellipsoid</rdfs:label>
    <skos:definition>geometric reference surface embedded in 3D Euclidean space formed by an ellipse that is rotated about a main axisNote: For the Earth the ellipsoid is bi-axial with rotation about the polar axis. This results in an oblate ellipsoid with the midpoint of the foci located at the nominal centre of the Earth.</skos:definition>
    <rdfs:isDefinedBy>http://standards.iso.org/iso/19111/ed-3/en/</rdfs:isDefinedBy>
    <rdfs:subClassOf rdf:resource="&iso19111_7020;IdentifiedObject"/>
    <rdfs:subClassOf>
      <owl:Restriction>
        <owl:onProperty rdf:resource="&iso19111;Ellipsoid.semiMajorAxis"/>
        <owl:cardinality rdf:datatype="&xsd;nonNegativeInteger">1</owl:cardinality>
      </owl:Restriction>
    </rdfs:subClassOf>
    <rdfs:subClassOf>
      <owl:Restriction>
        <owl:onProperty rdf:resource="&iso19111;Ellipsoid.semiMajorAxis"/>
        <owl:allValuesFrom rdf:resource="&iso19103_5905;Length"/>
      </owl:Restriction>
    </rdfs:subClassOf>
    <rdfs:subClassOf>
      <owl:Restriction>
        <owl:onProperty rdf:resource="&iso19111;Ellipsoid.secondDefiningParameter"/>
        <owl:cardinality rdf:datatype="&xsd;nonNegativeInteger">1</owl:cardinality>
      </owl:Restriction>
    </rdfs:subClassOf>
    <rdfs:subClassOf>
      <owl:Restriction>
        <owl:onProperty rdf:resource="&iso19111;Ellipsoid.secondDefiningParameter"/>
        <owl:allValuesFrom rdf:resource="&iso19111;SecondDefiningParameter"/>
      </owl:Restriction>
    </rdfs:subClassOf>
    <rdfs:subClassOf>
      <owl:Restriction>
        <owl:onProperty rdf:resource="&iso19111;Ellipsoid.semiMedianAxis"/>
        <owl:maxCardinality rdf:datatype="&xsd;nonNegativeInteger">1</owl:maxCardinality>
      </owl:Restriction>
    </rdfs:subClassOf>
    <rdfs:subClassOf>
      <owl:Restriction>
        <owl:onProperty rdf:resource="&iso19111;Ellipsoid.semiMedianAxis"/>
        <owl:allValuesFrom rdf:resource="&iso19103_5905;Length"/>
      </owl:Restriction>
    </rdfs:subClassOf>
  </owl:Class>

  <!--++++++++++++++++++++++++++-->
  <!-- Class: InverseFlattening -->
  <!--++++++++++++++++++++++++++-->
  <owl:Class rdf:about="&iso19111;uInverseFlattening">
    <rdfs:label>InverseFlattening</rdfs:label>
    <skos:definition>inverse flattening value of the ellipsoid</skos:definition>
    <rdfs:isDefinedBy>http://standards.iso.org/iso/19111/ed-3/en/</rdfs:isDefinedBy>
    <rdfs:subClassOf>
      <owl:Restriction>
        <owl:onProperty rdf:resource="&iso19111;uInverseFlattening.inverseFlattening"/>
        <owl:cardinality rdf:datatype="&xsd;nonNegativeInteger">1</owl:cardinality>
      </owl:Restriction>
    </rdfs:subClassOf>
    <rdfs:subClassOf>
      <owl:Restriction>
        <owl:onProperty rdf:resource="&iso19111;uInverseFlattening.inverseFlattening"/>
        <owl:allValuesFrom rdf:resource="&iso19103_5905;Scale"/>
      </owl:Restriction>
    </rdfs:subClassOf>
  </owl:Class>

  <!--++++++++++++++++++++++-->
  <!-- Class: SemiMinorAxis -->
  <!--++++++++++++++++++++++-->
  <owl:Class rdf:about="&iso19111;uSemiMinorAxis">
    <rdfs:label>SemiMinorAxis</rdfs:label>
    <skos:definition>length of the semi-minor axis of the ellipsoid</skos:definition>
    <rdfs:isDefinedBy>http://standards.iso.org/iso/19111/ed-3/en/</rdfs:isDefinedBy>
    <rdfs:subClassOf>
      <owl:Restriction>
        <owl:onProperty rdf:resource="&iso19111;uSemiMinorAxis.semiMinorAxis"/>
        <owl:cardinality rdf:datatype="&xsd;nonNegativeInteger">1</owl:cardinality>
      </owl:Restriction>
    </rdfs:subClassOf>
    <rdfs:subClassOf>
      <owl:Restriction>
        <owl:onProperty rdf:resource="&iso19111;uSemiMinorAxis.semiMinorAxis"/>
        <owl:allValuesFrom rdf:resource="&iso19103_5905;Length"/>
      </owl:Restriction>
    </rdfs:subClassOf>
  </owl:Class>

  <!--+++++++++++++++++-->
  <!-- Class: IsSphere -->
  <!--+++++++++++++++++-->
  <owl:Class rdf:about="&iso19111;uIsSphere">
    <rdfs:label>IsSphere</rdfs:label>
    <skos:definition>ellipsoid is degenerate and is actually a sphereNote: The sphere is completely defined by the semi-major axis, which is the radius of the sphere. This attribute has the value “true” if the figure is a sphere.</skos:definition>
    <rdfs:isDefinedBy>http://standards.iso.org/iso/19111/ed-3/en/</rdfs:isDefinedBy>
    <rdfs:subClassOf>
      <owl:Restriction>
        <owl:onProperty rdf:resource="&iso19111;uIsSphere.isSphere"/>
        <owl:cardinality rdf:datatype="&xsd;nonNegativeInteger">1</owl:cardinality>
      </owl:Restriction>
    </rdfs:subClassOf>
    <rdfs:subClassOf>
      <owl:Restriction>
        <owl:onProperty rdf:resource="&iso19111;uIsSphere.isSphere"/>
        <owl:allValuesFrom rdf:resource="&xsd;boolean"/>
      </owl:Restriction>
    </rdfs:subClassOf>
  </owl:Class>

  <!--+++++++++++++++++++++++++++++++-->
  <!-- Class: VerticalReferenceFrame -->
  <!--+++++++++++++++++++++++++++++++-->
  <owl:Class rdf:about="&iso19111;VerticalReferenceFrame">
    <rdfs:label>VerticalReferenceFrame</rdfs:label>
    <skos:definition>textual description and.sl.or a set of parameters identifying a particular reference level surface used as a zero-height or zero-depth surface, including its position with respect to the EarthNote: In 19111:2007 this class was called VerticalDatum.</skos:definition>
    <rdfs:isDefinedBy>http://standards.iso.org/iso/19111/ed-3/en/</rdfs:isDefinedBy>
    <rdfs:subClassOf rdf:resource="&iso19111;Datum"/>
    <rdfs:subClassOf>
      <owl:Restriction>
        <owl:onProperty rdf:resource="&iso19111;VerticalReferenceFrame.realizationMethod"/>
        <owl:maxCardinality rdf:datatype="&xsd;nonNegativeInteger">1</owl:maxCardinality>
      </owl:Restriction>
    </rdfs:subClassOf>
    <rdfs:subClassOf>
      <owl:Restriction>
        <owl:onProperty rdf:resource="&iso19111;VerticalReferenceFrame.realizationMethod"/>
        <owl:allValuesFrom rdf:resource="&iso19111;RealizationMethod"/>
      </owl:Restriction>
    </rdfs:subClassOf>
  </owl:Class>

  <!--++++++++++++++++++++++++++++++++++++++-->
  <!-- Class: DynamicVerticalReferenceFrame -->
  <!--++++++++++++++++++++++++++++++++++++++-->
  <owl:Class rdf:about="&iso19111;DynamicVerticalReferenceFrame">
    <rdfs:label>DynamicVerticalReferenceFrame</rdfs:label>
    <skos:definition>vertical reference frame in which some of the defining parameters have time dependencyExample: Defining station heights have velocity to account for post-glacial isostatic rebound motion.</skos:definition>
    <rdfs:isDefinedBy>http://standards.iso.org/iso/19111/ed-3/en/</rdfs:isDefinedBy>
    <rdfs:subClassOf rdf:resource="&iso19111;VerticalReferenceFrame"/>
    <rdfs:subClassOf>
      <owl:Restriction>
        <owl:onProperty rdf:resource="&iso19111;DynamicVerticalReferenceFrame.frameReferenceEpoch"/>
        <owl:cardinality rdf:datatype="&xsd;nonNegativeInteger">1</owl:cardinality>
      </owl:Restriction>
    </rdfs:subClassOf>
    <rdfs:subClassOf>
      <owl:Restriction>
        <owl:onProperty rdf:resource="&iso19111;DynamicVerticalReferenceFrame.frameReferenceEpoch"/>
        <owl:allValuesFrom rdf:resource="&iso19103_5905;Measure"/>
      </owl:Restriction>
    </rdfs:subClassOf>
  </owl:Class>

  <!--++++++++++++++++++++++++-->
  <!-- Class: ParametricDatum -->
  <!--++++++++++++++++++++++++-->
  <owl:Class rdf:about="&iso19111;ParametricDatum">
    <rdfs:label>ParametricDatum</rdfs:label>
    <skos:definition>textual description and.sl.or a set of parameters identifying a particular reference surface used as the origin of a parametric coordinate system, including its position with respect to the Earth</skos:definition>
    <rdfs:isDefinedBy>http://standards.iso.org/iso/19111/ed-3/en/</rdfs:isDefinedBy>
    <rdfs:subClassOf rdf:resource="&iso19111_4044;CD_Datum"/>
    <rdfs:subClassOf rdf:resource="&iso19111;Datum"/>
    <rdfs:subClassOf>
      <owl:Restriction>
        <owl:onProperty rdf:resource="&iso19111;ParametricDatum.datumDefiningParameter"/>
        <owl:allValuesFrom rdf:resource="&iso19111;DefiningParameter"/>
      </owl:Restriction>
    </rdfs:subClassOf>
  </owl:Class>

  <!--++++++++++++++++++++++++++-->
  <!-- Class: DefiningParameter -->
  <!--++++++++++++++++++++++++++-->
  <owl:Class rdf:about="&iso19111;DefiningParameter">
    <rdfs:label>DefiningParameter</rdfs:label>
    <skos:definition>parameter value, an ordered sequence of values, or a reference to a file of parameter values that define a paramtric datum</skos:definition>
    <rdfs:isDefinedBy>http://standards.iso.org/iso/19111/ed-3/en/</rdfs:isDefinedBy>
    <rdfs:subClassOf rdf:resource="&iso19111_7020;IdentifiedObject"/>
    <rdfs:subClassOf>
      <owl:Restriction>
        <owl:onProperty rdf:resource="&iso19111;DefiningParameter.parameterValue"/>
        <owl:cardinality rdf:datatype="&xsd;nonNegativeInteger">1</owl:cardinality>
      </owl:Restriction>
    </rdfs:subClassOf>
    <rdfs:subClassOf>
      <owl:Restriction>
        <owl:onProperty rdf:resource="&iso19111;DefiningParameter.parameterValue"/>
        <owl:allValuesFrom rdf:resource="&iso19111_7025;ParameterValue"/>
      </owl:Restriction>
    </rdfs:subClassOf>
  </owl:Class>

  <!--+++++++++++++++++++++++++-->
  <!-- Class: EngineeringDatum -->
  <!--+++++++++++++++++++++++++-->
  <owl:Class rdf:about="&iso19111;EngineeringDatum">
    <rdfs:label>EngineeringDatum</rdfs:label>
    <skos:definition>definition of the origin and orientation of an engineering coordinate reference systemNote: The origin can be fixed with respect to the Earth (such as a defined point at a construction site), or be a defined point on a moving vehicle (such as on a ship or satellite), or a defined point of an image.</skos:definition>
    <rdfs:isDefinedBy>http://standards.iso.org/iso/19111/ed-3/en/</rdfs:isDefinedBy>
    <rdfs:subClassOf rdf:resource="&iso19111;Datum"/>
  </owl:Class>

  <!--++++++++++++++++++++++-->
  <!-- Class: TemporalDatum -->
  <!--++++++++++++++++++++++-->
  <owl:Class rdf:about="&iso19111;TemporalDatum">
    <rdfs:label>TemporalDatum</rdfs:label>
    <skos:definition>definition of the relationship of a temporal coordinate system to an objectNote: The object is normally time on the Earth.</skos:definition>
    <rdfs:isDefinedBy>http://standards.iso.org/iso/19111/ed-3/en/</rdfs:isDefinedBy>
    <rdfs:subClassOf rdf:resource="&iso19111_4044;CD_Datum"/>
    <rdfs:subClassOf rdf:resource="&iso19111;Datum"/>
    <rdfs:subClassOf>
      <owl:Restriction>
        <owl:onProperty rdf:resource="&iso19111;TemporalDatum.origin"/>
        <owl:cardinality rdf:datatype="&xsd;nonNegativeInteger">1</owl:cardinality>
      </owl:Restriction>
    </rdfs:subClassOf>
    <rdfs:subClassOf>
      <owl:Restriction>
        <owl:onProperty rdf:resource="&iso19111;TemporalDatum.origin"/>
        <owl:allValuesFrom rdf:resource="&xsd;dateTime"/>
      </owl:Restriction>
    </rdfs:subClassOf>
    <rdfs:subClassOf>
      <owl:Restriction>
        <owl:onProperty rdf:resource="&iso19111;TemporalDatum.calendar"/>
        <owl:cardinality rdf:datatype="&xsd;nonNegativeInteger">1</owl:cardinality>
      </owl:Restriction>
    </rdfs:subClassOf>
    <rdfs:subClassOf>
      <owl:Restriction>
        <owl:onProperty rdf:resource="&iso19111;TemporalDatum.calendar"/>
        <owl:allValuesFrom rdf:resource="&iso19111;Calendar"/>
      </owl:Restriction>
    </rdfs:subClassOf>
  </owl:Class>

  <!--++++++++++++++++++++++-->
  <!-- Class: DatumEnsemble -->
  <!--++++++++++++++++++++++-->
  <owl:Class rdf:about="&iso19111;DatumEnsemble">
    <rdfs:label>DatumEnsemble</rdfs:label>
    <skos:definition>A collection of two or more datums (or if geodetic or vertical, a collection of two or more reference frames) that are realizations of one Conventional Reference System and which for all but the highest accuracy requirements may be considered to be insignificantly different from each other.Note: Within the datum ensemble every frame or datum is constrained to be a realization of the same reference system.</skos:definition>
    <rdfs:isDefinedBy>http://standards.iso.org/iso/19111/ed-3/en/</rdfs:isDefinedBy>
    <iso19150-2:constraint>datum -.gt.forAll(p1, p2 | p1.conventionalRS.eq.p2.conventionalRS)</iso19150-2:constraint>
    <rdfs:subClassOf rdf:resource="&iso19111_7020;ObjectUsage"/>
    <rdfs:subClassOf>
      <owl:Restriction>
        <owl:onProperty rdf:resource="&iso19111;DatumEnsemble.ensembleAccuracy"/>
        <owl:cardinality rdf:datatype="&xsd;nonNegativeInteger">1</owl:cardinality>
      </owl:Restriction>
    </rdfs:subClassOf>
    <rdfs:subClassOf>
      <owl:Restriction>
        <owl:onProperty rdf:resource="&iso19111;DatumEnsemble.ensembleAccuracy"/>
        <owl:allValuesFrom rdf:resource="&iso19157_4482;DQ_PositionalAccuracy"/>
      </owl:Restriction>
    </rdfs:subClassOf>
    <rdfs:subClassOf>
      <owl:Restriction>
        <owl:onProperty rdf:resource="&iso19111;DatumEnsemble.datum"/>
        <owl:minCardinality rdf:datatype="&xsd;nonNegativeInteger">2</owl:minCardinality>
      </owl:Restriction>
    </rdfs:subClassOf>
    <rdfs:subClassOf>
      <owl:Restriction>
        <owl:onProperty rdf:resource="&iso19111;DatumEnsemble.datum"/>
        <owl:allValuesFrom rdf:resource="&iso19111;Datum"/>
      </owl:Restriction>
    </rdfs:subClassOf>
  </owl:Class>

  <!--++++++++++++++++++++++++++++++++++++++++++-->
  <!-- DatatypeProperty: Datum.anchorDefinition -->
  <!--++++++++++++++++++++++++++++++++++++++++++-->
  <owl:DatatypeProperty rdf:about="&iso19111;Datum.anchorDefinition">
    <rdfs:label>anchorDefinition</rdfs:label>
    <skos:definition>description, possibly including coordinates of an identified point or points, of the relationship used to anchor a coordinate system to the Earth or alternate object Note: For modern geodetic reference frames the anchor may be a set of station coordinates; if the reference frame is dynamic it will also include coordinate velocities. For a traditional geodetic datum, the anchor may be a point known as the fundamental point, which is traditionally the point where the relationship between geoid and ellipsoid is defined, together with a direction from that point.- For a vertical reference frame the anchor may be the zero level at one or more defined locations or a conventionally defined surface. - For an engineering datum, the anchor may be an identified physical point with the orientation defined relative to the object.</skos:definition>
    <rdfs:isDefinedBy>http://standards.iso.org/iso/19111/ed-3/en/</rdfs:isDefinedBy>
    <rdfs:domain rdf:resource="&iso19111;Datum"/>
    <rdfs:range rdf:resource="&xsd;string"/>
  </owl:DatatypeProperty>

  <!--+++++++++++++++++++++++++++++++++++++++++-->
  <!-- DatatypeProperty: Datum.publicationDate -->
  <!--+++++++++++++++++++++++++++++++++++++++++-->
  <owl:DatatypeProperty rdf:about="&iso19111;Datum.publicationDate">
    <rdfs:label>publicationDate</rdfs:label>
    <skos:definition>date on which the datum definition was published</skos:definition>
    <rdfs:isDefinedBy>http://standards.iso.org/iso/19111/ed-3/en/</rdfs:isDefinedBy>
    <rdfs:domain rdf:resource="&iso19111;Datum"/>
    <rdfs:range rdf:resource="&rdf;XMLLiteral"/>
  </owl:DatatypeProperty>

  <!--++++++++++++++++++++++++++++++++++++++-->
  <!-- ObjectProperty: Datum.conventionalRS -->
  <!--++++++++++++++++++++++++++++++++++++++-->
  <owl:ObjectProperty rdf:about="&iso19111;Datum.conventionalRS">
    <rdfs:label>conventionalRS</rdfs:label>
    <skos:definition>name, identifier, alias and remarks for the terrestrial reference system or vertical reference system realized by this reference frameExamples: .gu.ITRS.gu. for ITRF88 through ITRF2008 and ITRF2014, or .gu.EVRS.gu. for EVRF2000 and EVRF2007.</skos:definition>
    <rdfs:isDefinedBy>http://standards.iso.org/iso/19111/ed-3/en/</rdfs:isDefinedBy>
    <rdfs:domain rdf:resource="&iso19111;Datum"/>
    <rdfs:range rdf:resource="&iso19111_7020;IdentifiedObject"/>
  </owl:ObjectProperty>

  <!--+++++++++++++++++++++++++++++++++++++++++++++++++++++++++++++++++++-->
  <!-- ObjectProperty: DynamicGeodeticReferenceFrame.frameReferenceEpoch -->
  <!--+++++++++++++++++++++++++++++++++++++++++++++++++++++++++++++++++++-->
  <owl:ObjectProperty rdf:about="&iso19111;DynamicGeodeticReferenceFrame.frameReferenceEpoch">
    <rdfs:label>frameReferenceEpoch</rdfs:label>
    <skos:definition>epoch to which the coordinates of stations defining the dynamic geodetic reference frame are referenced, expressed as a decimal year in the Gregorian calendarExample: 2016,47.</skos:definition>
    <rdfs:isDefinedBy>http://standards.iso.org/iso/19111/ed-3/en/</rdfs:isDefinedBy>
    <rdfs:domain rdf:resource="&iso19111;DynamicGeodeticReferenceFrame"/>
    <rdfs:range rdf:resource="&iso19103_5905;Measure"/>
  </owl:ObjectProperty>

  <!--++++++++++++++++++++++++++++++++++++++++++++++++++-->
  <!-- ObjectProperty: PrimeMeridian.greenwichLongitude -->
  <!--++++++++++++++++++++++++++++++++++++++++++++++++++-->
  <owl:ObjectProperty rdf:about="&iso19111;PrimeMeridian.greenwichLongitude">
    <rdfs:label>greenwichLongitude</rdfs:label>
    <skos:definition>longitude of the prime meridian measured from the internationally-recognised reference meridian ('Greenwich meridian'), positive eastwardNote 1: Default value: 0 degrees. Note 2: If the value of the prime meridian name is “Greenwich” then the value of greenwichLongitude is required to be 0 degrees.</skos:definition>
    <rdfs:isDefinedBy>http://standards.iso.org/iso/19111/ed-3/en/</rdfs:isDefinedBy>
    <rdfs:domain rdf:resource="&iso19111;PrimeMeridian"/>
    <rdfs:range rdf:resource="&iso19103_5905;Angle"/>
  </owl:ObjectProperty>

  <!--+++++++++++++++++++++++++++++++++++++++++-->
  <!-- ObjectProperty: Ellipsoid.semiMajorAxis -->
  <!--+++++++++++++++++++++++++++++++++++++++++-->
  <owl:ObjectProperty rdf:about="&iso19111;Ellipsoid.semiMajorAxis">
    <rdfs:label>semiMajorAxis</rdfs:label>
    <skos:definition>length of the semi-major axis of the ellipsoid</skos:definition>
    <rdfs:isDefinedBy>http://standards.iso.org/iso/19111/ed-3/en/</rdfs:isDefinedBy>
    <rdfs:domain rdf:resource="&iso19111;Ellipsoid"/>
    <rdfs:range rdf:resource="&iso19103_5905;Length"/>
  </owl:ObjectProperty>

  <!--+++++++++++++++++++++++++++++++++++++++++++++++++++-->
  <!-- ObjectProperty: Ellipsoid.secondDefiningParameter -->
  <!--+++++++++++++++++++++++++++++++++++++++++++++++++++-->
  <owl:ObjectProperty rdf:about="&iso19111;Ellipsoid.secondDefiningParameter">
    <rdfs:label>secondDefiningParameter</rdfs:label>
    <skos:definition>definition of the second parameter that describes the shape of this ellipsoid</skos:definition>
    <rdfs:isDefinedBy>http://standards.iso.org/iso/19111/ed-3/en/</rdfs:isDefinedBy>
    <rdfs:domain rdf:resource="&iso19111;Ellipsoid"/>
    <rdfs:range rdf:resource="&iso19111;SecondDefiningParameter"/>
  </owl:ObjectProperty>

  <!--++++++++++++++++++++++++++++++++++++++++++-->
  <!-- ObjectProperty: Ellipsoid.semiMedianAxis -->
  <!--++++++++++++++++++++++++++++++++++++++++++-->
  <owl:ObjectProperty rdf:about="&iso19111;Ellipsoid.semiMedianAxis">
    <rdfs:label>semiMedianAxis</rdfs:label>
    <skos:definition>length of the semi-median axis of a triaxial ellipsoidNote: This parameter is not required for a biaxial ellipsoid.</skos:definition>
    <rdfs:isDefinedBy>http://standards.iso.org/iso/19111/ed-3/en/</rdfs:isDefinedBy>
    <rdfs:domain rdf:resource="&iso19111;Ellipsoid"/>
    <rdfs:range rdf:resource="&iso19103_5905;Length"/>
  </owl:ObjectProperty>

  <!--+++++++++++++++++++++++++++++++++++-->
  <!-- ObjectProperty: inverseFlattening -->
  <!--+++++++++++++++++++++++++++++++++++-->
  <owl:ObjectProperty rdf:about="&iso19111;uInverseFlattening.inverseFlattening">
    <skos:prefLabel>inverseFlattening</skos:prefLabel>
    <rdfs:isDefinedBy>http://standards.iso.org/iso/19111/ed-3/en/</rdfs:isDefinedBy>
    <rdfs:domain rdf:resource="&iso19111;uInverseFlattening"/>
    <rdfs:range rdf:resource="&iso19103_5905;Scale"/>
  </owl:ObjectProperty>

  <!--+++++++++++++++++++++++++++++++-->
  <!-- ObjectProperty: semiMinorAxis -->
  <!--+++++++++++++++++++++++++++++++-->
  <owl:ObjectProperty rdf:about="&iso19111;uSemiMinorAxis.semiMinorAxis">
    <skos:prefLabel>semiMinorAxis</skos:prefLabel>
    <rdfs:isDefinedBy>http://standards.iso.org/iso/19111/ed-3/en/</rdfs:isDefinedBy>
    <rdfs:domain rdf:resource="&iso19111;uSemiMinorAxis"/>
    <rdfs:range rdf:resource="&iso19103_5905;Length"/>
  </owl:ObjectProperty>

  <!--++++++++++++++++++++++++++++-->
  <!-- DatatypeProperty: isSphere -->
  <!--++++++++++++++++++++++++++++-->
  <owl:DatatypeProperty rdf:about="&iso19111;uIsSphere.isSphere">
    <rdfs:label>isSphere</rdfs:label>
    <rdfs:isDefinedBy>http://standards.iso.org/iso/19111/ed-3/en/</rdfs:isDefinedBy>
    <rdfs:domain rdf:resource="&iso19111;uIsSphere"/>
    <rdfs:range rdf:resource="&xsd;boolean"/>
  </owl:DatatypeProperty>

  <!--++++++++++++++++++++++++++++++++++++++++++++++++++++++++++-->
  <!-- ObjectProperty: VerticalReferenceFrame.realizationMethod -->
  <!--++++++++++++++++++++++++++++++++++++++++++++++++++++++++++-->
  <owl:ObjectProperty rdf:about="&iso19111;VerticalReferenceFrame.realizationMethod">
    <rdfs:label>realizationMethod</rdfs:label>
    <skos:definition>method through which this vertical reference frame is realized</skos:definition>
    <rdfs:isDefinedBy>http://standards.iso.org/iso/19111/ed-3/en/</rdfs:isDefinedBy>
    <rdfs:domain rdf:resource="&iso19111;VerticalReferenceFrame"/>
    <rdfs:range rdf:resource="&iso19111;RealizationMethod"/>
  </owl:ObjectProperty>

  <!--+++++++++++++++++++++++++++++++++++++++++++++++++++++++++++++++++++-->
  <!-- ObjectProperty: DynamicVerticalReferenceFrame.frameReferenceEpoch -->
  <!--+++++++++++++++++++++++++++++++++++++++++++++++++++++++++++++++++++-->
  <owl:ObjectProperty rdf:about="&iso19111;DynamicVerticalReferenceFrame.frameReferenceEpoch">
    <rdfs:label>frameReferenceEpoch</rdfs:label>
    <skos:definition>epoch to which the coordinates of stations defining the dynamic vertical reference frame are referenced, expressed as a decimal year in the Gregorian calendarExample: 2016,47.</skos:definition>
    <rdfs:isDefinedBy>http://standards.iso.org/iso/19111/ed-3/en/</rdfs:isDefinedBy>
    <rdfs:domain rdf:resource="&iso19111;DynamicVerticalReferenceFrame"/>
    <rdfs:range rdf:resource="&iso19103_5905;Measure"/>
  </owl:ObjectProperty>

  <!--++++++++++++++++++++++++++++++++++++++++++++++++++++++++-->
  <!-- ObjectProperty: ParametricDatum.datumDefiningParameter -->
  <!--++++++++++++++++++++++++++++++++++++++++++++++++++++++++-->
  <owl:ObjectProperty rdf:about="&iso19111;ParametricDatum.datumDefiningParameter">
    <rdfs:label>datumDefiningParameter</rdfs:label>
    <skos:definition>parameter used to define the parametric datum</skos:definition>
    <rdfs:isDefinedBy>http://standards.iso.org/iso/19111/ed-3/en/</rdfs:isDefinedBy>
    <rdfs:domain rdf:resource="&iso19111;ParametricDatum"/>
    <rdfs:range rdf:resource="&iso19111;DefiningParameter"/>
  </owl:ObjectProperty>

  <!--++++++++++++++++++++++++++++++++++++++++++++++++++-->
  <!-- ObjectProperty: DefiningParameter.parameterValue -->
  <!--++++++++++++++++++++++++++++++++++++++++++++++++++-->
  <owl:ObjectProperty rdf:about="&iso19111;DefiningParameter.parameterValue">
    <rdfs:label>parameterValue</rdfs:label>
    <skos:definition>value of the datum-defining parameter</skos:definition>
    <rdfs:isDefinedBy>http://standards.iso.org/iso/19111/ed-3/en/</rdfs:isDefinedBy>
    <rdfs:domain rdf:resource="&iso19111;DefiningParameter"/>
    <rdfs:range rdf:resource="&iso19111_7025;ParameterValue"/>
  </owl:ObjectProperty>

  <!--++++++++++++++++++++++++++++++++++++++++-->
  <!-- DatatypeProperty: TemporalDatum.origin -->
  <!--++++++++++++++++++++++++++++++++++++++++-->
  <owl:DatatypeProperty rdf:about="&iso19111;TemporalDatum.origin">
    <rdfs:label>origin</rdfs:label>
    <skos:definition>date and time to which temporal coordinates are referenced, expressed in conformance with ISO 8601</skos:definition>
    <rdfs:isDefinedBy>http://standards.iso.org/iso/19111/ed-3/en/</rdfs:isDefinedBy>
    <rdfs:domain rdf:resource="&iso19111;TemporalDatum"/>
    <rdfs:range rdf:resource="&xsd;dateTime"/>
  </owl:DatatypeProperty>

  <!--++++++++++++++++++++++++++++++++++++++++-->
  <!-- ObjectProperty: TemporalDatum.calendar -->
  <!--++++++++++++++++++++++++++++++++++++++++-->
  <owl:ObjectProperty rdf:about="&iso19111;TemporalDatum.calendar">
    <rdfs:label>calendar</rdfs:label>
    <skos:definition>calendar to which the temporal origin is referencedNote: Default value is prolepticGregorian</skos:definition>
    <rdfs:isDefinedBy>http://standards.iso.org/iso/19111/ed-3/en/</rdfs:isDefinedBy>
    <rdfs:domain rdf:resource="&iso19111;TemporalDatum"/>
    <rdfs:range rdf:resource="&iso19111;Calendar"/>
  </owl:ObjectProperty>

  <!--++++++++++++++++++++++++++++++++++++++++++++++++-->
  <!-- ObjectProperty: DatumEnsemble.ensembleAccuracy -->
  <!--++++++++++++++++++++++++++++++++++++++++++++++++-->
  <owl:ObjectProperty rdf:about="&iso19111;DatumEnsemble.ensembleAccuracy">
    <rdfs:label>ensembleAccuracy</rdfs:label>
    <skos:definition>inaccuracy introduced through use of this collection of reference frames or datumsNote: It is an indication of the differences in coordinate values at all points between the various realizations that have been grouped into this datum ensemble.</skos:definition>
    <rdfs:isDefinedBy>http://standards.iso.org/iso/19111/ed-3/en/</rdfs:isDefinedBy>
    <rdfs:domain rdf:resource="&iso19111;DatumEnsemble"/>
    <rdfs:range rdf:resource="&iso19157_4482;DQ_PositionalAccuracy"/>
  </owl:ObjectProperty>

  <!--++++++++++++++++++++++++++++++++++++++++++++++++++-->
  <!-- ObjectProperty: GeodeticReferenceFrame.ellipsoid -->
  <!--++++++++++++++++++++++++++++++++++++++++++++++++++-->
  <owl:ObjectProperty rdf:about="&iso19111;GeodeticReferenceFrame.ellipsoid">
    <rdfs:label>ellipsoid</rdfs:label>
    <rdfs:isDefinedBy>http://standards.iso.org/iso/19111/ed-3/en/</rdfs:isDefinedBy>
    <iso19150-2:aggregationType>partOfSharedAggregation</iso19150-2:aggregationType>
    <rdfs:domain rdf:resource="&iso19111;GeodeticReferenceFrame"/>
    <rdfs:range rdf:resource="&iso19111;Ellipsoid"/>
  </owl:ObjectProperty>

  <!--++++++++++++++++++++++++++++++++++++++++++++++++++++++-->
  <!-- ObjectProperty: GeodeticReferenceFrame.primeMeridian -->
  <!--++++++++++++++++++++++++++++++++++++++++++++++++++++++-->
  <owl:ObjectProperty rdf:about="&iso19111;GeodeticReferenceFrame.primeMeridian">
    <rdfs:label>primeMeridian</rdfs:label>
    <rdfs:isDefinedBy>http://standards.iso.org/iso/19111/ed-3/en/</rdfs:isDefinedBy>
    <iso19150-2:aggregationType>partOfSharedAggregation</iso19150-2:aggregationType>
    <rdfs:domain rdf:resource="&iso19111;GeodeticReferenceFrame"/>
    <rdfs:range rdf:resource="&iso19111;PrimeMeridian"/>
  </owl:ObjectProperty>

  <!--+++++++++++++++++++++++++++++++++++++-->
  <!-- ObjectProperty: DatumEnsemble.datum -->
  <!--+++++++++++++++++++++++++++++++++++++-->
  <owl:ObjectProperty rdf:about="&iso19111;DatumEnsemble.datum">
    <rdfs:label>datum</rdfs:label>
    <rdfs:isDefinedBy>http://standards.iso.org/iso/19111/ed-3/en/</rdfs:isDefinedBy>
    <rdfs:domain rdf:resource="&iso19111;DatumEnsemble"/>
    <rdfs:range rdf:resource="&iso19111;Datum"/>
  </owl:ObjectProperty>

  <!--++++++++++++++++++++++++++++++++-->
  <!-- Class: SecondDefiningParameter -->
  <!--++++++++++++++++++++++++++++++++-->
  <owl:Class rdf:about="&iso19111;SecondDefiningParameter">
    <rdfs:label>SecondDefiningParameter</rdfs:label>
    <skos:definition>definition of the second parameter that defines the shape of a biaxial ellipsoid, or the third parameter that defines a triaxial ellipsoidNote: A biaxial ellipsoid requires two defining parameters: a semi-major axis and inverse flattening or a semi-major axis and a semi-minor axis. When the reference body is a sphere rather than an ellipsoid, only a single defining parameter is required, namely the radius of the sphere; in that case, the semi-major axis “degenerates” into the radius of the sphere.</skos:definition>
    <rdfs:isDefinedBy>http://standards.iso.org/iso/19111/ed-3/en/</rdfs:isDefinedBy>
    <owl:equivalentClass>
      <owl:Class>
        <owl:unionOf rdf:parseType="Collection">
          <owl:Class rdf:about="&iso19111;uInverseFlattening"/>
          <owl:Class rdf:about="&iso19111;uSemiMinorAxis"/>
          <owl:Class rdf:about="&iso19111;uIsSphere"/>
        </owl:unionOf>
      </owl:Class>
    </owl:equivalentClass>
  </owl:Class>

  <!--+++++++++++++++++++++++++++++-->
  <!-- Codelist: RealizationMethod -->
  <!--+++++++++++++++++++++++++++++-->
  <owl:Class rdf:about="&iso19111;RealizationMethod">
    <rdfs:label>RealizationMethod</rdfs:label>
    <rdfs:isDefinedBy>http://standards.iso.org/iso/19111/ed-3/en/</rdfs:isDefinedBy>
    <rdfs:subClassOf rdf:resource="&skos;Concept"/>
  </owl:Class>
  <skos:ConceptScheme rdf:about="&iso19111Code;RealizationMethod">
    <skos:prefLabel>RealizationMethod - ConceptScheme</skos:prefLabel>
    <rdfs:isDefinedBy>http://standards.iso.org/iso/19111/ed-3/en/</rdfs:isDefinedBy>
    <dct:isFormatOf rdf:resource="&iso19111;RealizationMethod"/>
  </skos:ConceptScheme>
  <iso19111:RealizationMethod rdf:about="&iso19111Code;RealizationMethod/levelling">
    <rdf:type rdf:resource="&skos;Concept"/>
    <skos:prefLabel>levelling</skos:prefLabel>
    <skos:inScheme rdf:resource="&iso19111Code;RealizationMethod"/>
    <rdfs:isDefinedBy>http://standards.iso.org/iso/19111/ed-3/en/</rdfs:isDefinedBy>
    <skos:definition>realization is by adjustment of a levelling network fixed to one or more tide gauges</skos:definition>
  </iso19111:RealizationMethod>
  <iso19111:RealizationMethod rdf:about="&iso19111Code;RealizationMethod/geoid">
    <rdf:type rdf:resource="&skos;Concept"/>
    <skos:prefLabel>geoid</skos:prefLabel>
    <skos:inScheme rdf:resource="&iso19111Code;RealizationMethod"/>
    <rdfs:isDefinedBy>http://standards.iso.org/iso/19111/ed-3/en/</rdfs:isDefinedBy>
    <skos:definition>realization is through a geoid height model or a height correction modelNote: This is applied to a specified geodetic CRS. </skos:definition>
  </iso19111:RealizationMethod>
  <iso19111:RealizationMethod rdf:about="&iso19111Code;RealizationMethod/tidal">
    <rdf:type rdf:resource="&skos;Concept"/>
    <skos:prefLabel>tidal</skos:prefLabel>
    <skos:inScheme rdf:resource="&iso19111Code;RealizationMethod"/>
    <rdfs:isDefinedBy>http://standards.iso.org/iso/19111/ed-3/en/</rdfs:isDefinedBy>
    <skos:definition>realization is through a tidal model or by tidal predictions</skos:definition>
  </iso19111:RealizationMethod>
  <skos:Collection rdf:about="&iso19111Code;RealizationMethodCollection">
    <skos:prefLabel>RealizationMethod - Collection</skos:prefLabel>
    <skos:member rdf:resource="&iso19111Code;RealizationMethod/levelling"/>
    <skos:member rdf:resource="&iso19111Code;RealizationMethod/geoid"/>
    <skos:member rdf:resource="&iso19111Code;RealizationMethod/tidal"/>
  </skos:Collection>

  <!--++++++++++++++++++++-->
  <!-- Codelist: Calendar -->
  <!--++++++++++++++++++++-->
  <owl:Class rdf:about="&iso19111;Calendar">
    <rdfs:label>Calendar</rdfs:label>
    <rdfs:isDefinedBy>http://standards.iso.org/iso/19111/ed-3/en/</rdfs:isDefinedBy>
    <rdfs:subClassOf rdf:resource="&skos;Concept"/>
  </owl:Class>
  <skos:ConceptScheme rdf:about="&iso19111Code;Calendar">
    <skos:prefLabel>Calendar - ConceptScheme</skos:prefLabel>
    <rdfs:isDefinedBy>http://standards.iso.org/iso/19111/ed-3/en/</rdfs:isDefinedBy>
    <dct:isFormatOf rdf:resource="&iso19111;Calendar"/>
  </skos:ConceptScheme>
  <iso19111:Calendar rdf:about="&iso19111Code;Calendar/prolepticGregorian">
    <rdf:type rdf:resource="&skos;Concept"/>
    <skos:prefLabel>prolepticGregorian</skos:prefLabel>
    <skos:inScheme rdf:resource="&iso19111Code;Calendar"/>
    <rdfs:isDefinedBy>http://standards.iso.org/iso/19111/ed-3/en/</rdfs:isDefinedBy>
    <skos:definition>proleptic Gregorian calendar as defined in ISO 8601Note: This is the default value.</skos:definition>
  </iso19111:Calendar>
  <skos:Collection rdf:about="&iso19111Code;CalendarCollection">
    <skos:prefLabel>Calendar - Collection</skos:prefLabel>
    <skos:member rdf:resource="&iso19111Code;Calendar/prolepticGregorian"/>
  </skos:Collection>

</rdf:RDF>

