PREFIX : <http://def.isotc211.org/iso19157/-1/20yy/DataQualityEvaluation/code/EvaluationMethodTypeCode/>
PREFIX cs: <http://def.isotc211.org/iso19157/-1/20yy/DataQualityEvaluation/code/EvaluationMethodTypeCode>
PREFIX schema: <https://schema.org/>
PREFIX prov: <http://www.w3.org/ns/prov#>
PREFIX rdfs: <http://www.w3.org/2000/01/rdf-schema#>
PREFIX reg: <http://purl.org/linked-data/registry#>
PREFIX skos: <http://www.w3.org/2004/02/skos/core#>
PREFIX status: <http://def.isotc211.org/iso19135/-1/2015/CoreModel/code/RE_ItemStatus/>
PREFIX xsd: <http://www.w3.org/2001/XMLSchema#>

:directExternal
    a skos:Concept ;
    schema:identifier "directExternal"^^xsd:token ;
    schema:provenance "Presented in the original standard's codelist"@en ;
    reg:status status:original ;
    rdfs:isDefinedBy cs: ;
    skos:definition "method of evaluating the quality of a dataset based on inspection of items within the dataset, where reference data external to the dataset being evaluated is required"@en ;
    skos:inScheme cs: ;
    skos:prefLabel "direct external"@en ;
    skos:topConceptOf cs: ;
.

:directInternal
    a skos:Concept ;
    schema:identifier "directInternal"^^xsd:token ;
    schema:provenance "Presented in the original standard's codelist"@en ;
    reg:status status:original ;
    rdfs:isDefinedBy cs: ;
    skos:definition "method of evaluating the quality of a dataset based on inspection of items within the dataset, where all data required is internal to the dataset being evaluated"@en ;
    skos:inScheme cs: ;
    skos:prefLabel "direct internal"@en ;
    skos:topConceptOf cs: ;
.

:indirect
    a skos:Concept ;
    schema:identifier "indirect"^^xsd:token ;
    schema:provenance "Presented in the original standard's codelist"@en ;
    reg:status status:original ;
    rdfs:isDefinedBy cs: ;
    skos:definition "method of evaluating the quality of a dataset based on external knowledge"@en ;
    skos:inScheme cs: ;
    skos:prefLabel "indirect"@en ;
    skos:topConceptOf cs: ;
.

cs:
    a skos:ConceptScheme ;
    schema:dateCreated "2000-01-01"^^xsd:date ;
    schema:creator <https://committee.iso.org/home/tc211> ;
    schema:identifier "EvaluationMethodTypeCode"^^xsd:token ;
    schema:isFormatOf <http://def.isotc211.org/iso19115/-1/2018/CitationAndResponsiblePartyInformation#CI_DateTypeCode> ;
    schema:issued "2000-01-01"^^xsd:date ;
    schema:dateModified "2000-01-01"^^xsd:date ;
    schema:provenance "Derived from TC211-produced RDF versions of the standard's UML"@en ;
    schema:publisher <https://committee.iso.org/home/tc211> ;
    schema:citation "http://standards.iso.org/iso/19157/-1/ed-1/en/"^^xsd:anyURI ;
    reg:status status:valid ;
    skos:definition "Methods of evaluating the quality of a dataset"@en ;
    skos:hasTopConcept
        :directExternal ,
        :directInternal ,
        :indirect ;
    skos:prefLabel "Evaluation Method Type Code"@en ;
    prov:qualifiedDerivation [
            prov:entity <http://example.com/none> ;
            prov:hadRole <https://linked.data.gov.au/def/vocab-derivation-modes/none>
        ] ;
.

