<?xml version="1.0"?>

<!DOCTYPE rdf:RDF [
  <!ENTITY owl "http://www.w3.org/2002/07/owl#" >
  <!ENTITY xsd "http://www.w3.org/2001/XMLSchema#" >
  <!ENTITY rdfs "http://www.w3.org/2000/01/rdf-schema#" >
  <!ENTITY rdf "http://www.w3.org/1999/02/22-rdf-syntax-ns#" >
  <!ENTITY dc "http://purl.org/dc/elements/1.1/" >
  <!ENTITY dct "http://purl.org/dc/terms/" >
  <!ENTITY skos "http://www.w3.org/2004/02/skos/core#" >
  <!ENTITY iso19150-2 "http://def.isotc211.org/iso19150/-2/2012/base#" >
  <!ENTITY iso19103_340 "http://def.isotc211.org/iso19103/2005/Enumerations#" >
  <!ENTITY iso19103_335 "http://def.isotc211.org/iso19103/2005/Collections#" >
  <!ENTITY iso19133 "http://def.isotc211.org/iso19133/2005/NewBasicTypes#" >

]>

  <!--++++++++++++++++++++++++++++++++++++++++++++++-->
  <!-- File name:         iso19133NewBasicTypes.rdf -->
  <!-- Generator:         GOM_Technologies::UML2OWL -->
  <!-- Generator version: 2.5                       -->
  <!-- File date:         14-11-2016                -->
  <!--++++++++++++++++++++++++++++++++++++++++++++++-->

<rdf:RDF xmlns="http://def.isotc211.org/iso19133/2005/NewBasicTypes#"
  xml:base="http://def.isotc211.org/iso19133/2005/NewBasicTypes"
  xmlns:owl="http://www.w3.org/2002/07/owl#"
  xmlns:xsd="http://www.w3.org/2001/XMLSchema#"
  xmlns:rdfs="http://www.w3.org/2000/01/rdf-schema#"
  xmlns:rdf="http://www.w3.org/1999/02/22-rdf-syntax-ns#"
  xmlns:dc="http://purl.org/dc/elements/1.1/"
  xmlns:dct="http://purl.org/dc/terms/"
  xmlns:skos="http://www.w3.org/2004/02/skos/core#"
  xmlns:iso19150-2="http://def.isotc211.org/iso19150/-2/2012/base#"
  xmlns:iso19103_340="http://def.isotc211.org/iso19103/2005/Enumerations#"
  xmlns:iso19103_335="http://def.isotc211.org/iso19103/2005/Collections#"
  xmlns:iso19133="http://def.isotc211.org/iso19133/2005/NewBasicTypes#">

  <!--++++++++++++++++++++++++++++++++++++++++++-->
  <!-- Ontology: ISO 19133:2005 New Basic Types -->
  <!--++++++++++++++++++++++++++++++++++++++++++-->
  <owl:Ontology rdf:about="http://def.isotc211.org/iso19133/2005/NewBasicTypes">
    <rdfs:label>ISO 19133:2005 New Basic Types</rdfs:label>
    <dct:source>http://standards.iso.org/iso/19133/ed-1/en/</dct:source>
    <owl:versionInfo>2005-10-15</owl:versionInfo>
    <!--owl:imports rdf:resource="http://def.isotc211.org/iso19103/2005/Enumerations"/-->
    <!--owl:imports rdf:resource="http://def.isotc211.org/iso19103/2005/Collections"/-->
    <owl:imports rdf:resource="http://def.isotc211.org/iso19150/-2/2012/base"/>
  </owl:Ontology>

  <!--+++++++++++++++++++-->
  <!-- Class: BinaryData -->
  <!--+++++++++++++++++++-->
  <owl:Class rdf:about="&iso19133;BinaryData">
    <rdfs:label>BinaryData</rdfs:label>
    <rdfs:isDefinedBy>http://standards.iso.org/iso/19133/ed-1/en/</rdfs:isDefinedBy>
    <rdfs:subClassOf rdf:resource="&iso19133;Sequence.lt.Bit.gt."/>
  </owl:Class>

  <!--++++++++++++++-->
  <!-- Class: Image -->
  <!--++++++++++++++-->
  <owl:Class rdf:about="&iso19133;Image">
    <rdfs:label>Image</rdfs:label>
    <skos:definition>.lt.UsedBy.gt..lt.NameSpace.gt.ISO 19133 Tracking and Navigation.lt..sl.NameSpace.gt..lt.Class.gt.NS_Instruction.lt..sl.Class.gt..lt.Operation.gt.renderAsGoundLevelView.lt..sl.Operation.gt..lt.Parameter.gt.Return.lt..sl.Parameter.gt..lt.Type.gt.Image.lt..sl.Type.gt..lt.UsedBy.gt.</skos:definition>
    <rdfs:isDefinedBy>http://standards.iso.org/iso/19133/ed-1/en/</rdfs:isDefinedBy>
    <rdfs:subClassOf rdf:resource="&iso19133;BinaryData"/>
  </owl:Class>

  <!--++++++++++++-->
  <!-- Class: Map -->
  <!--++++++++++++-->
  <owl:Class rdf:about="&iso19133;Map">
    <rdfs:label>Map</rdfs:label>
    <skos:definition>.lt.UsedBy.gt..lt.NameSpace.gt.ISO 19133 Tracking and Navigation.lt..sl.NameSpace.gt..lt.Class.gt.NS_Instruction.lt..sl.Class.gt..lt.Operation.gt.renderAsMap.lt..sl.Operation.gt..lt.Parameter.gt.Return.lt..sl.Parameter.gt..lt.Type.gt.Map.lt..sl.Type.gt..lt.UsedBy.gt.</skos:definition>
    <rdfs:isDefinedBy>http://standards.iso.org/iso/19133/ed-1/en/</rdfs:isDefinedBy>
    <rdfs:subClassOf rdf:resource="&iso19133;BinaryData"/>
  </owl:Class>

  <!--++++++++++++++++++++++++++++-->
  <!-- Class: Sequence.lt.Bit.gt. -->
  <!--++++++++++++++++++++++++++++-->
  <owl:Class rdf:about="&iso19133;Sequence.lt.Bit.gt.">
    <rdfs:label>Sequence.lt.Bit.gt.</rdfs:label>
    <rdfs:isDefinedBy>http://standards.iso.org/iso/19133/ed-1/en/</rdfs:isDefinedBy>
    <rdfs:subClassOf rdf:resource="&iso19103_335;Sequence"/>
    <rdfs:subClassOf>
      <owl:Restriction>
        <owl:onProperty rdf:resource="&iso19133;Sequence.lt.Bit.gt..bit"/>
        <owl:minCardinality rdf:datatype="&xsd;nonNegativeInteger">1</owl:minCardinality>
      </owl:Restriction>
    </rdfs:subClassOf>
    <rdfs:subClassOf>
      <owl:Restriction>
        <owl:onProperty rdf:resource="&iso19133;Sequence.lt.Bit.gt..bit"/>
        <owl:allValuesFrom rdf:resource="&iso19103_340;Bit"/>
      </owl:Restriction>
    </rdfs:subClassOf>
  </owl:Class>

  <!--++++++++++++++++++++-->
  <!-- Class: VoiceStream -->
  <!--++++++++++++++++++++-->
  <owl:Class rdf:about="&iso19133;VoiceStream">
    <rdfs:label>VoiceStream</rdfs:label>
    <skos:definition>.lt.UsedBy.gt..lt.NameSpace.gt.ISO 19133 Tracking and Navigation.lt..sl.NameSpace.gt..lt.Class.gt.NS_Instruction.lt..sl.Class.gt..lt.Operation.gt.renderAsVoice.lt..sl.Operation.gt..lt.Parameter.gt.Return.lt..sl.Parameter.gt..lt.Type.gt.VoiceStream.lt..sl.Type.gt..lt.UsedBy.gt.</skos:definition>
    <rdfs:isDefinedBy>http://standards.iso.org/iso/19133/ed-1/en/</rdfs:isDefinedBy>
    <rdfs:subClassOf rdf:resource="&iso19133;BinaryData"/>
  </owl:Class>

  <!--++++++++++++++++++++++++++++++++++++++++-->
  <!-- ObjectProperty: Sequence.lt.Bit.gt..bit -->
  <!--++++++++++++++++++++++++++++++++++++++++-->
  <owl:ObjectProperty rdf:about="&iso19133;Sequence.lt.Bit.gt..bit">
    <rdfs:label>Sequence.lt.Bit.gt..bit</rdfs:label>
    <rdfs:isDefinedBy>http://standards.iso.org/iso/19133/ed-1/en/</rdfs:isDefinedBy>
    <rdfs:domain rdf:resource="&iso19133;Sequence.lt.Bit.gt."/>
    <rdfs:range rdf:resource="&iso19103_340;Bit"/>
  </owl:ObjectProperty>

</rdf:RDF>

