<?xml version="1.0"?>

<!DOCTYPE rdf:RDF [
  <!ENTITY owl "http://www.w3.org/2002/07/owl#" >
  <!ENTITY xsd "http://www.w3.org/2001/XMLSchema#" >
  <!ENTITY rdfs "http://www.w3.org/2000/01/rdf-schema#" >
  <!ENTITY rdf "http://www.w3.org/1999/02/22-rdf-syntax-ns#" >
  <!ENTITY dc "http://purl.org/dc/elements/1.1/" >
  <!ENTITY dct "http://purl.org/dc/terms/" >
  <!ENTITY skos "http://www.w3.org/2004/02/skos/core#" >
  <!ENTITY iso19150-2 "http://def.isotc211.org/iso19150/-2/2012/base#" >
  <!ENTITY iso19115-1_1505 "http://def.isotc211.org/iso19115/-1/2014/CitationAndResponsiblePartyInformation#" >
  <!ENTITY iso19135-1_1058 "http://def.isotc211.org/iso19135/-1/2015/ExtendedModel#" >
  <!ENTITY iso19135-1_1057 "http://def.isotc211.org/iso19135/-1/2015/CoreModel#" >
  <!ENTITY iso19104 "http://def.isotc211.org/iso19104/2015/TermRegister#" >

]>

  <!--++++++++++++++++++++++++++++++++++++++++++++++-->
  <!-- File name:         iso19104TermRegister.rdf  -->
  <!-- Generator:         GOM_Technologies::UML2OWL -->
  <!-- Generator version: 2.5                       -->
  <!-- File date:         19-10-2016                -->
  <!--++++++++++++++++++++++++++++++++++++++++++++++-->

<rdf:RDF xmlns="http://def.isotc211.org/iso19104/2015/TermRegister#"
  xml:base="http://def.isotc211.org/iso19104/2015/TermRegister"
  xmlns:owl="http://www.w3.org/2002/07/owl#"
  xmlns:xsd="http://www.w3.org/2001/XMLSchema#"
  xmlns:rdfs="http://www.w3.org/2000/01/rdf-schema#"
  xmlns:rdf="http://www.w3.org/1999/02/22-rdf-syntax-ns#"
  xmlns:dc="http://purl.org/dc/elements/1.1/"
  xmlns:dct="http://purl.org/dc/terms/"
  xmlns:skos="http://www.w3.org/2004/02/skos/core#"
  xmlns:iso19150-2="http://def.isotc211.org/iso19150/-2/2012/base#"
  xmlns:iso19115-1_1505="http://def.isotc211.org/iso19115/-1/2014/CitationAndResponsiblePartyInformation#"
  xmlns:iso19135-1_1058="http://def.isotc211.org/iso19135/-1/2015/ExtendedModel#"
  xmlns:iso19135-1_1057="http://def.isotc211.org/iso19135/-1/2015/CoreModel#"
  xmlns:iso19104="http://def.isotc211.org/iso19104/2015/TermRegister#">

  <!--+++++++++++++++++++++++++++++++++++++++-->
  <!-- Ontology: ISO 19104:2015 TermRegister -->
  <!--+++++++++++++++++++++++++++++++++++++++-->
  <owl:Ontology rdf:about="http://def.isotc211.org/iso19104/2015/TermRegister">
    <rdfs:label>ISO 19104:2015 TermRegister</rdfs:label>
    <dct:source>http://standards.iso.org/iso/19104/ed-1/en/</dct:source>
    <owl:versionInfo>2016-10-01</owl:versionInfo>
    <!--owl:imports rdf:resource="http://def.isotc211.org/iso19115/-1/2014/CitationAndResponsiblePartyInformation"/>
    <owl:imports rdf:resource="http://def.isotc211.org/iso19135/-1/2015/ExtendedModel"/>
    <owl:imports rdf:resource="http://def.isotc211.org/iso19135/-1/2015/CoreModel"/-->
    <owl:imports rdf:resource="http://def.isotc211.org/iso19150/-2/2012/base"/>
  </owl:Ontology>

  <!--++++++++++++++++-->
  <!-- Class: Example -->
  <!--++++++++++++++++-->
  <owl:Class rdf:about="&iso19104;Example">
    <rdfs:label>Example</rdfs:label>
    <skos:definition>Model element for recording instances of the data category .gu.example.gu..</skos:definition>
    <rdfs:isDefinedBy>http://standards.iso.org/iso/19104/ed-1/en/</rdfs:isDefinedBy>
    <rdfs:subClassOf>
      <owl:Restriction>
        <owl:onProperty rdf:resource="&iso19104;Example.example"/>
        <owl:cardinality rdf:datatype="&xsd;nonNegativeInteger">1</owl:cardinality>
      </owl:Restriction>
    </rdfs:subClassOf>
    <rdfs:subClassOf>
      <owl:Restriction>
        <owl:onProperty rdf:resource="&iso19104;Example.example"/>
        <owl:allValuesFrom rdf:resource="&xsd;string"/>
      </owl:Restriction>
    </rdfs:subClassOf>
    <rdfs:subClassOf>
      <owl:Restriction>
        <owl:onProperty rdf:resource="&iso19104;Example.termEntry"/>
        <owl:minCardinality rdf:datatype="&xsd;nonNegativeInteger">1</owl:minCardinality>
      </owl:Restriction>
    </rdfs:subClassOf>
    <rdfs:subClassOf>
      <owl:Restriction>
        <owl:onProperty rdf:resource="&iso19104;Example.termEntry"/>
        <owl:allValuesFrom rdf:resource="&iso19104;TermRegisterEntry"/>
      </owl:Restriction>
    </rdfs:subClassOf>
  </owl:Class>

  <!--++++++++++++++++++++-->
  <!-- Class: NoteToEntry -->
  <!--++++++++++++++++++++-->
  <owl:Class rdf:about="&iso19104;NoteToEntry">
    <rdfs:label>NoteToEntry</rdfs:label>
    <skos:definition>Model element for recording instances of the data category .gu.note to entry.gu..</skos:definition>
    <rdfs:isDefinedBy>http://standards.iso.org/iso/19104/ed-1/en/</rdfs:isDefinedBy>
    <rdfs:subClassOf>
      <owl:Restriction>
        <owl:onProperty rdf:resource="&iso19104;NoteToEntry.noteToEntry"/>
        <owl:cardinality rdf:datatype="&xsd;nonNegativeInteger">1</owl:cardinality>
      </owl:Restriction>
    </rdfs:subClassOf>
    <rdfs:subClassOf>
      <owl:Restriction>
        <owl:onProperty rdf:resource="&iso19104;NoteToEntry.noteToEntry"/>
        <owl:allValuesFrom rdf:resource="&xsd;string"/>
      </owl:Restriction>
    </rdfs:subClassOf>
    <rdfs:subClassOf>
      <owl:Restriction>
        <owl:onProperty rdf:resource="&iso19104;NoteToEntry.termEntry"/>
        <owl:minCardinality rdf:datatype="&xsd;nonNegativeInteger">1</owl:minCardinality>
      </owl:Restriction>
    </rdfs:subClassOf>
    <rdfs:subClassOf>
      <owl:Restriction>
        <owl:onProperty rdf:resource="&iso19104;NoteToEntry.termEntry"/>
        <owl:allValuesFrom rdf:resource="&iso19104;TermRegisterEntry"/>
      </owl:Restriction>
    </rdfs:subClassOf>
  </owl:Class>

  <!--+++++++++++++++++++++-->
  <!-- Class: TermAddition -->
  <!--+++++++++++++++++++++-->
  <owl:Class rdf:about="&iso19104;TermAddition">
    <rdfs:label>TermAddition</rdfs:label>
    <skos:definition>The class TermAddition is a subclass of RE_AdditionInformation (ISO 19135-1:2015, B.2.7.2). It specifies elements of management information to be recorded for each proposal to add a register item.</skos:definition>
    <rdfs:isDefinedBy>http://standards.iso.org/iso/19104/ed-1/en/</rdfs:isDefinedBy>
    <rdfs:subClassOf rdf:resource="&iso19135-1_1058;RE_AdditionInformation"/>
  </owl:Class>

  <!--++++++++++++++++++++++-->
  <!-- Class: TermAmendment -->
  <!--++++++++++++++++++++++-->
  <owl:Class rdf:about="&iso19104;TermAmendment">
    <rdfs:label>TermAmendment</rdfs:label>
    <skos:definition>The class TermAmendment is a subclass of RE_AmendmentInformation (ISO 19135:2015, B.2.7.3). It specifies elements of management information to be recorded for each proposal to amend a register item.</skos:definition>
    <rdfs:isDefinedBy>http://standards.iso.org/iso/19104/ed-1/en/</rdfs:isDefinedBy>
    <rdfs:subClassOf rdf:resource="&iso19135-1_1058;RE_AmendmentInformation"/>
  </owl:Class>

  <!--++++++++++++++++++++++++++-->
  <!-- Class: TermClarification -->
  <!--++++++++++++++++++++++++++-->
  <owl:Class rdf:about="&iso19104;TermClarification">
    <rdfs:label>TermClarification</rdfs:label>
    <skos:definition>The class TermClarification is a subclass of RE_ClarificationInformation (ISO 19135-1:2015, B.2.7.4). It specifies elements of management information to be recorded for each proposal to clarify a register item.</skos:definition>
    <rdfs:isDefinedBy>http://standards.iso.org/iso/19104/ed-1/en/</rdfs:isDefinedBy>
    <rdfs:subClassOf rdf:resource="&iso19135-1_1058;RE_ClarificationInformation"/>
  </owl:Class>

  <!--+++++++++++++++++++++-->
  <!-- Class: TermRegister -->
  <!--+++++++++++++++++++++-->
  <owl:Class rdf:about="&iso19104;TermRegister">
    <rdfs:label>TermRegister</rdfs:label>
    <skos:definition>The class TermRegister is a subclass of RE_Register specified in ISO 19135-1:2015, B.2.2.2. It specifies information items for describing a terminology register or subregister.</skos:definition>
    <rdfs:isDefinedBy>http://standards.iso.org/iso/19104/ed-1/en/</rdfs:isDefinedBy>
    <rdfs:subClassOf rdf:resource="&iso19135-1_1058;RE_Register"/>
  </owl:Class>

  <!--++++++++++++++++++++++++++-->
  <!-- Class: TermRegisterEntry -->
  <!--++++++++++++++++++++++++++-->
  <owl:Class rdf:about="&iso19104;TermRegisterEntry">
    <rdfs:label>TermRegisterEntry</rdfs:label>
    <skos:definition>The class TermRegisterEntry is a subclass of RE_RegisterItem (ISO 19135-1:2015, B.2.3.2). It specifies elements of information to be recorded for each terminological entry in a simple register, reference language subregister or submitted language subregister. TermRegisterEntry is not used to record entries in a principal register. Entries in a principal register are recorded using instances of TermSubregisterDescription as described in ISO 19104:2016, 10.5.14.</skos:definition>
    <rdfs:isDefinedBy>http://standards.iso.org/iso/19104/ed-1/en/</rdfs:isDefinedBy>
    <rdfs:subClassOf rdf:resource="&iso19135-1_1058;RE_RegisterItem"/>
    <rdfs:subClassOf>
      <owl:Restriction>
        <owl:onProperty rdf:resource="&iso19104;TermRegisterEntry.termClassification"/>
        <owl:cardinality rdf:datatype="&xsd;nonNegativeInteger">1</owl:cardinality>
      </owl:Restriction>
    </rdfs:subClassOf>
    <rdfs:subClassOf>
      <owl:Restriction>
        <owl:onProperty rdf:resource="&iso19104;TermRegisterEntry.termClassification"/>
        <owl:allValuesFrom rdf:resource="&iso19104;TermClassification"/>
      </owl:Restriction>
    </rdfs:subClassOf>
    <rdfs:subClassOf>
      <owl:Restriction>
        <owl:onProperty rdf:resource="&iso19104;TermRegisterEntry.termAbbreviation"/>
        <owl:maxCardinality rdf:datatype="&xsd;nonNegativeInteger">1</owl:maxCardinality>
      </owl:Restriction>
    </rdfs:subClassOf>
    <rdfs:subClassOf>
      <owl:Restriction>
        <owl:onProperty rdf:resource="&iso19104;TermRegisterEntry.termAbbreviation"/>
        <owl:allValuesFrom rdf:resource="&xsd;string"/>
      </owl:Restriction>
    </rdfs:subClassOf>
    <rdfs:subClassOf>
      <owl:Restriction>
        <owl:onProperty rdf:resource="&iso19104;TermRegisterEntry.symbol"/>
        <owl:allValuesFrom rdf:resource="&iso19115-1_1505;CI_Citation"/>
      </owl:Restriction>
    </rdfs:subClassOf>
    <rdfs:subClassOf>
      <owl:Restriction>
        <owl:onProperty rdf:resource="&iso19104;TermRegisterEntry.nonVerbalRep"/>
        <owl:allValuesFrom rdf:resource="&iso19115-1_1505;CI_Citation"/>
      </owl:Restriction>
    </rdfs:subClassOf>
    <rdfs:subClassOf>
      <owl:Restriction>
        <owl:onProperty rdf:resource="&iso19104;TermRegisterEntry.correspondence"/>
        <owl:maxCardinality rdf:datatype="&xsd;nonNegativeInteger">1</owl:maxCardinality>
      </owl:Restriction>
    </rdfs:subClassOf>
    <rdfs:subClassOf>
      <owl:Restriction>
        <owl:onProperty rdf:resource="&iso19104;TermRegisterEntry.correspondence"/>
        <owl:allValuesFrom rdf:resource="&iso19104;Correspondence"/>
      </owl:Restriction>
    </rdfs:subClassOf>
    <rdfs:subClassOf>
      <owl:Restriction>
        <owl:onProperty rdf:resource="&iso19104;TermRegisterEntry.deprecatedEntry"/>
        <owl:allValuesFrom rdf:resource="&iso19104;TermRegisterEntry"/>
      </owl:Restriction>
    </rdfs:subClassOf>
    <rdfs:subClassOf>
      <owl:Restriction>
        <owl:onProperty rdf:resource="&iso19104;TermRegisterEntry.currentEntry"/>
        <owl:minCardinality rdf:datatype="&xsd;nonNegativeInteger">1</owl:minCardinality>
      </owl:Restriction>
    </rdfs:subClassOf>
    <rdfs:subClassOf>
      <owl:Restriction>
        <owl:onProperty rdf:resource="&iso19104;TermRegisterEntry.currentEntry"/>
        <owl:allValuesFrom rdf:resource="&iso19104;TermRegisterEntry"/>
      </owl:Restriction>
    </rdfs:subClassOf>
    <rdfs:subClassOf>
      <owl:Restriction>
        <owl:onProperty rdf:resource="&iso19104;TermRegisterEntry.admittedEntry"/>
        <owl:allValuesFrom rdf:resource="&iso19104;TermRegisterEntry"/>
      </owl:Restriction>
    </rdfs:subClassOf>
    <rdfs:subClassOf>
      <owl:Restriction>
        <owl:onProperty rdf:resource="&iso19104;TermRegisterEntry.preferredEntry"/>
        <owl:cardinality rdf:datatype="&xsd;nonNegativeInteger">1</owl:cardinality>
      </owl:Restriction>
    </rdfs:subClassOf>
    <rdfs:subClassOf>
      <owl:Restriction>
        <owl:onProperty rdf:resource="&iso19104;TermRegisterEntry.preferredEntry"/>
        <owl:allValuesFrom rdf:resource="&iso19104;TermRegisterEntry"/>
      </owl:Restriction>
    </rdfs:subClassOf>
    <rdfs:subClassOf>
      <owl:Restriction>
        <owl:onProperty rdf:resource="&iso19104;TermRegisterEntry.example"/>
        <owl:allValuesFrom rdf:resource="&iso19104;Example"/>
      </owl:Restriction>
    </rdfs:subClassOf>
    <rdfs:subClassOf>
      <owl:Restriction>
        <owl:onProperty rdf:resource="&iso19104;TermRegisterEntry.note"/>
        <owl:allValuesFrom rdf:resource="&iso19104;NoteToEntry"/>
      </owl:Restriction>
    </rdfs:subClassOf>
  </owl:Class>

  <!--++++++++++++++++++++++++-->
  <!-- Class: TermStakeholder -->
  <!--++++++++++++++++++++++++-->
  <owl:Class rdf:about="&iso19104;TermStakeholder">
    <rdfs:label>TermStakeholder</rdfs:label>
    <skos:definition>The class TermStakeholder is a subclass of RegisterStakeholder, specified in ISO 19135-1:2015, 7.3.2. It specifies information items for identifying the owner and manager of a terminology register or subregister. It also specifies information items for identifying each party that submits entries to that register or subregister.</skos:definition>
    <rdfs:isDefinedBy>http://standards.iso.org/iso/19104/ed-1/en/</rdfs:isDefinedBy>
    <rdfs:subClassOf rdf:resource="&iso19135-1_1057;RegisterStakeholder"/>
  </owl:Class>

  <!--+++++++++++++++++++++++++++++++++++-->
  <!-- Class: TermSubregisterDescription -->
  <!--+++++++++++++++++++++++++++++++++++-->
  <owl:Class rdf:about="&iso19104;TermSubregisterDescription">
    <rdfs:label>TermSubregisterDescription</rdfs:label>
    <skos:definition>The class TermSubregisterDescription is a subclass of RE_SubregisterDescription [ISO 19135-1:2015, B.2.8.2]. It is used in a principal register to describe affiliated subregisters.</skos:definition>
    <rdfs:isDefinedBy>http://standards.iso.org/iso/19104/ed-1/en/</rdfs:isDefinedBy>
    <rdfs:subClassOf rdf:resource="&iso19135-1_1058;RE_SubregisterDescription"/>
    <rdfs:subClassOf>
      <owl:Restriction>
        <owl:onProperty rdf:resource="&iso19104;TermSubregisterDescription.contentSummary"/>
        <owl:cardinality rdf:datatype="&xsd;nonNegativeInteger">1</owl:cardinality>
      </owl:Restriction>
    </rdfs:subClassOf>
    <rdfs:subClassOf>
      <owl:Restriction>
        <owl:onProperty rdf:resource="&iso19104;TermSubregisterDescription.contentSummary"/>
        <owl:allValuesFrom rdf:resource="&xsd;string"/>
      </owl:Restriction>
    </rdfs:subClassOf>
    <rdfs:subClassOf>
      <owl:Restriction>
        <owl:onProperty rdf:resource="&iso19104;TermSubregisterDescription.reference"/>
        <owl:cardinality rdf:datatype="&xsd;nonNegativeInteger">1</owl:cardinality>
      </owl:Restriction>
    </rdfs:subClassOf>
    <rdfs:subClassOf>
      <owl:Restriction>
        <owl:onProperty rdf:resource="&iso19104;TermSubregisterDescription.reference"/>
        <owl:allValuesFrom rdf:resource="&xsd;boolean"/>
      </owl:Restriction>
    </rdfs:subClassOf>
    <rdfs:subClassOf>
      <owl:Restriction>
        <owl:onProperty rdf:resource="&iso19104;TermSubregisterDescription.alternativeLanguages"/>
        <owl:cardinality rdf:datatype="&xsd;nonNegativeInteger">1</owl:cardinality>
      </owl:Restriction>
    </rdfs:subClassOf>
    <rdfs:subClassOf>
      <owl:Restriction>
        <owl:onProperty rdf:resource="&iso19104;TermSubregisterDescription.alternativeLanguages"/>
        <owl:allValuesFrom rdf:resource="&iso19135-1_1058;RE_Locale"/>
      </owl:Restriction>
    </rdfs:subClassOf>
  </owl:Class>

  <!--+++++++++++++++++++++++++++++++++++-->
  <!-- DatatypeProperty: Example.example -->
  <!--+++++++++++++++++++++++++++++++++++-->
  <owl:DatatypeProperty rdf:about="&iso19104;Example.example">
    <rdfs:label>example</rdfs:label>
    <skos:definition>Description that illustrates the application of a concept.</skos:definition>
    <rdfs:isDefinedBy>http://standards.iso.org/iso/19104/ed-1/en/</rdfs:isDefinedBy>
    <rdfs:domain rdf:resource="&iso19104;Example"/>
    <rdfs:range rdf:resource="&xsd;string"/>
  </owl:DatatypeProperty>

  <!--+++++++++++++++++++++++++++++++++++++++++++-->
  <!-- DatatypeProperty: NoteToEntry.noteToEntry -->
  <!--+++++++++++++++++++++++++++++++++++++++++++-->
  <owl:DatatypeProperty rdf:about="&iso19104;NoteToEntry.noteToEntry">
    <rdfs:label>noteToEntry</rdfs:label>
    <skos:definition>Description that elaborates the context, characteristics or application of a concept.</skos:definition>
    <rdfs:isDefinedBy>http://standards.iso.org/iso/19104/ed-1/en/</rdfs:isDefinedBy>
    <rdfs:domain rdf:resource="&iso19104;NoteToEntry"/>
    <rdfs:range rdf:resource="&xsd;string"/>
  </owl:DatatypeProperty>

  <!--++++++++++++++++++++++++++++++++++++++++++++++++++++++-->
  <!-- ObjectProperty: TermRegisterEntry.termClassification -->
  <!--++++++++++++++++++++++++++++++++++++++++++++++++++++++-->
  <owl:ObjectProperty rdf:about="&iso19104;TermRegisterEntry.termClassification">
    <rdfs:label>termClassification</rdfs:label>
    <skos:definition>Classification of the term, represented as an instance of the enumeration TermClassification.</skos:definition>
    <rdfs:isDefinedBy>http://standards.iso.org/iso/19104/ed-1/en/</rdfs:isDefinedBy>
    <rdfs:domain rdf:resource="&iso19104;TermRegisterEntry"/>
    <rdfs:range rdf:resource="&iso19104;TermClassification"/>
  </owl:ObjectProperty>

  <!--++++++++++++++++++++++++++++++++++++++++++++++++++++++-->
  <!-- DatatypeProperty: TermRegisterEntry.termAbbreviation -->
  <!--++++++++++++++++++++++++++++++++++++++++++++++++++++++-->
  <owl:DatatypeProperty rdf:about="&iso19104;TermRegisterEntry.termAbbreviation">
    <rdfs:label>termAbbreviation</rdfs:label>
    <skos:definition>.lt.i.gt.designation.lt..sl.i.gt. formed by omitting words or letters from a longer form.</skos:definition>
    <rdfs:isDefinedBy>http://standards.iso.org/iso/19104/ed-1/en/</rdfs:isDefinedBy>
    <rdfs:domain rdf:resource="&iso19104;TermRegisterEntry"/>
    <rdfs:range rdf:resource="&xsd;string"/>
  </owl:DatatypeProperty>

  <!--++++++++++++++++++++++++++++++++++++++++++-->
  <!-- ObjectProperty: TermRegisterEntry.symbol -->
  <!--++++++++++++++++++++++++++++++++++++++++++-->
  <owl:ObjectProperty rdf:about="&iso19104;TermRegisterEntry.symbol">
    <rdfs:label>symbol</rdfs:label>
    <skos:definition>Reference to a resource containing a representation of the symbol.</skos:definition>
    <rdfs:isDefinedBy>http://standards.iso.org/iso/19104/ed-1/en/</rdfs:isDefinedBy>
    <rdfs:domain rdf:resource="&iso19104;TermRegisterEntry"/>
    <rdfs:range rdf:resource="&iso19115-1_1505;CI_Citation"/>
  </owl:ObjectProperty>

  <!--++++++++++++++++++++++++++++++++++++++++++++++++-->
  <!-- ObjectProperty: TermRegisterEntry.nonVerbalRep -->
  <!--++++++++++++++++++++++++++++++++++++++++++++++++-->
  <owl:ObjectProperty rdf:about="&iso19104;TermRegisterEntry.nonVerbalRep">
    <rdfs:label>nonVerbalRep</rdfs:label>
    <skos:definition>Reference to a resource containing the non-verbal representation, presented as an instance of CI_Citation (ISO 19115-1:2014, B.16).</skos:definition>
    <rdfs:isDefinedBy>http://standards.iso.org/iso/19104/ed-1/en/</rdfs:isDefinedBy>
    <rdfs:domain rdf:resource="&iso19104;TermRegisterEntry"/>
    <rdfs:range rdf:resource="&iso19115-1_1505;CI_Citation"/>
  </owl:ObjectProperty>

  <!--++++++++++++++++++++++++++++++++++++++++++++++++++-->
  <!-- ObjectProperty: TermRegisterEntry.correspondence -->
  <!--++++++++++++++++++++++++++++++++++++++++++++++++++-->
  <owl:ObjectProperty rdf:about="&iso19104;TermRegisterEntry.correspondence">
    <rdfs:label>correspondence</rdfs:label>
    <skos:definition>Degree to which the technical content of a culturally and.sl.or linguistically adapted terminological entry corresponds to that of the entry in the reference language, represented as an instance of the enumeration Correspondence.Note to entry:	This attribute shall only be included if the terminological entry forms part of a submitted language subregister.</skos:definition>
    <rdfs:isDefinedBy>http://standards.iso.org/iso/19104/ed-1/en/</rdfs:isDefinedBy>
    <rdfs:domain rdf:resource="&iso19104;TermRegisterEntry"/>
    <rdfs:range rdf:resource="&iso19104;Correspondence"/>
  </owl:ObjectProperty>

  <!--+++++++++++++++++++++++++++++++++++++++++++++++++++++++++++++-->
  <!-- DatatypeProperty: TermSubregisterDescription.contentSummary -->
  <!--+++++++++++++++++++++++++++++++++++++++++++++++++++++++++++++-->
  <owl:DatatypeProperty rdf:about="&iso19104;TermSubregisterDescription.contentSummary">
    <rdfs:label>contentSummary</rdfs:label>
    <skos:definition>General statement of the purpose for which items in the subregister are made available to potential usersEXAMPLE	.gu.A compilation of terminological entries published in ISO.sl.TC 211-sponsored International Standards and Technical Specifications, presented in English for use by the geospatial community..gu.</skos:definition>
    <rdfs:isDefinedBy>http://standards.iso.org/iso/19104/ed-1/en/</rdfs:isDefinedBy>
    <rdfs:domain rdf:resource="&iso19104;TermSubregisterDescription"/>
    <rdfs:range rdf:resource="&xsd;string"/>
  </owl:DatatypeProperty>

  <!--++++++++++++++++++++++++++++++++++++++++++++++++++++++++-->
  <!-- DatatypeProperty: TermSubregisterDescription.reference -->
  <!--++++++++++++++++++++++++++++++++++++++++++++++++++++++++-->
  <owl:DatatypeProperty rdf:about="&iso19104;TermSubregisterDescription.reference">
    <rdfs:label>reference</rdfs:label>
    <skos:definition>Specifies whether the subregister is the reference language subregister</skos:definition>
    <rdfs:isDefinedBy>http://standards.iso.org/iso/19104/ed-1/en/</rdfs:isDefinedBy>
    <rdfs:domain rdf:resource="&iso19104;TermSubregisterDescription"/>
    <rdfs:range rdf:resource="&xsd;boolean"/>
  </owl:DatatypeProperty>

  <!--+++++++++++++++++++++++++++++++++++++++++++++++++++++++++++++++++-->
  <!-- ObjectProperty: TermSubregisterDescription.alternativeLanguages -->
  <!--+++++++++++++++++++++++++++++++++++++++++++++++++++++++++++++++++-->
  <owl:ObjectProperty rdf:about="&iso19104;TermSubregisterDescription.alternativeLanguages">
    <rdfs:label>alternativeLanguages</rdfs:label>
    <skos:definition>Summary of alternative locales used by items in a subregister, represented as instances of the class RE_Locale (ISO 19135-1:2015, B.2.2.3)</skos:definition>
    <rdfs:isDefinedBy>http://standards.iso.org/iso/19104/ed-1/en/</rdfs:isDefinedBy>
    <rdfs:domain rdf:resource="&iso19104;TermSubregisterDescription"/>
    <rdfs:range rdf:resource="&iso19135-1_1058;RE_Locale"/>
  </owl:ObjectProperty>

  <!--+++++++++++++++++++++++++++++++++++++++++++-->
  <!-- ObjectProperty: TermRegisterEntry.example -->
  <!--+++++++++++++++++++++++++++++++++++++++++++-->
  <owl:ObjectProperty rdf:about="&iso19104;TermRegisterEntry.example">
    <rdfs:label>example</rdfs:label>
    <rdfs:isDefinedBy>http://standards.iso.org/iso/19104/ed-1/en/</rdfs:isDefinedBy>
    <iso19150-2:associationName>HasExample</iso19150-2:associationName>
    <rdfs:domain rdf:resource="&iso19104;TermRegisterEntry"/>
    <rdfs:range rdf:resource="&iso19104;Example"/>
  </owl:ObjectProperty>

  <!--+++++++++++++++++++++++++++++++++++-->
  <!-- ObjectProperty: Example.termEntry -->
  <!--+++++++++++++++++++++++++++++++++++-->
  <owl:ObjectProperty rdf:about="&iso19104;Example.termEntry">
    <rdfs:label>termEntry</rdfs:label>
    <rdfs:isDefinedBy>http://standards.iso.org/iso/19104/ed-1/en/</rdfs:isDefinedBy>
    <iso19150-2:associationName>HasExample</iso19150-2:associationName>
    <rdfs:domain rdf:resource="&iso19104;Example"/>
    <rdfs:range rdf:resource="&iso19104;TermRegisterEntry"/>
    <owl:inverseOf rdf:resource="&iso19104;TermRegisterEntry.example"/>
  </owl:ObjectProperty>

  <!--++++++++++++++++++++++++++++++++++++++++-->
  <!-- ObjectProperty: TermRegisterEntry.note -->
  <!--++++++++++++++++++++++++++++++++++++++++-->
  <owl:ObjectProperty rdf:about="&iso19104;TermRegisterEntry.note">
    <rdfs:label>note</rdfs:label>
    <rdfs:isDefinedBy>http://standards.iso.org/iso/19104/ed-1/en/</rdfs:isDefinedBy>
    <iso19150-2:associationName>HasNote</iso19150-2:associationName>
    <rdfs:domain rdf:resource="&iso19104;TermRegisterEntry"/>
    <rdfs:range rdf:resource="&iso19104;NoteToEntry"/>
  </owl:ObjectProperty>

  <!--+++++++++++++++++++++++++++++++++++++++-->
  <!-- ObjectProperty: NoteToEntry.termEntry -->
  <!--+++++++++++++++++++++++++++++++++++++++-->
  <owl:ObjectProperty rdf:about="&iso19104;NoteToEntry.termEntry">
    <rdfs:label>termEntry</rdfs:label>
    <rdfs:isDefinedBy>http://standards.iso.org/iso/19104/ed-1/en/</rdfs:isDefinedBy>
    <iso19150-2:associationName>HasNote</iso19150-2:associationName>
    <rdfs:domain rdf:resource="&iso19104;NoteToEntry"/>
    <rdfs:range rdf:resource="&iso19104;TermRegisterEntry"/>
    <owl:inverseOf rdf:resource="&iso19104;TermRegisterEntry.note"/>
  </owl:ObjectProperty>

  <!--+++++++++++++++++++++++++++++++++++++++++++++++++++-->
  <!-- ObjectProperty: TermRegisterEntry.deprecatedEntry -->
  <!--+++++++++++++++++++++++++++++++++++++++++++++++++++-->
  <owl:ObjectProperty rdf:about="&iso19104;TermRegisterEntry.deprecatedEntry">
    <rdfs:label>deprecatedEntry</rdfs:label>
    <rdfs:isDefinedBy>http://standards.iso.org/iso/19104/ed-1/en/</rdfs:isDefinedBy>
    <iso19150-2:associationName>Deprecated</iso19150-2:associationName>
    <rdfs:domain rdf:resource="&iso19104;TermRegisterEntry"/>
    <rdfs:range rdf:resource="&iso19104;TermRegisterEntry"/>
  </owl:ObjectProperty>

  <!--++++++++++++++++++++++++++++++++++++++++++++++++-->
  <!-- ObjectProperty: TermRegisterEntry.currentEntry -->
  <!--++++++++++++++++++++++++++++++++++++++++++++++++-->
  <owl:ObjectProperty rdf:about="&iso19104;TermRegisterEntry.currentEntry">
    <rdfs:label>currentEntry</rdfs:label>
    <rdfs:isDefinedBy>http://standards.iso.org/iso/19104/ed-1/en/</rdfs:isDefinedBy>
    <iso19150-2:associationName>Deprecated</iso19150-2:associationName>
    <rdfs:domain rdf:resource="&iso19104;TermRegisterEntry"/>
    <rdfs:range rdf:resource="&iso19104;TermRegisterEntry"/>
    <owl:inverseOf rdf:resource="&iso19104;TermRegisterEntry.deprecatedEntry"/>
  </owl:ObjectProperty>

  <!--+++++++++++++++++++++++++++++++++++++++++++++++++-->
  <!-- ObjectProperty: TermRegisterEntry.admittedEntry -->
  <!--+++++++++++++++++++++++++++++++++++++++++++++++++-->
  <owl:ObjectProperty rdf:about="&iso19104;TermRegisterEntry.admittedEntry">
    <rdfs:label>admittedEntry</rdfs:label>
    <rdfs:isDefinedBy>http://standards.iso.org/iso/19104/ed-1/en/</rdfs:isDefinedBy>
    <iso19150-2:associationName>Admitted</iso19150-2:associationName>
    <rdfs:domain rdf:resource="&iso19104;TermRegisterEntry"/>
    <rdfs:range rdf:resource="&iso19104;TermRegisterEntry"/>
  </owl:ObjectProperty>

  <!--++++++++++++++++++++++++++++++++++++++++++++++++++-->
  <!-- ObjectProperty: TermRegisterEntry.preferredEntry -->
  <!--++++++++++++++++++++++++++++++++++++++++++++++++++-->
  <owl:ObjectProperty rdf:about="&iso19104;TermRegisterEntry.preferredEntry">
    <rdfs:label>preferredEntry</rdfs:label>
    <rdfs:isDefinedBy>http://standards.iso.org/iso/19104/ed-1/en/</rdfs:isDefinedBy>
    <iso19150-2:associationName>Admitted</iso19150-2:associationName>
    <rdfs:domain rdf:resource="&iso19104;TermRegisterEntry"/>
    <rdfs:range rdf:resource="&iso19104;TermRegisterEntry"/>
    <owl:inverseOf rdf:resource="&iso19104;TermRegisterEntry.admittedEntry"/>
  </owl:ObjectProperty>

  <!--+++++++++++++++++++++++++++++-->
  <!-- Enumeration: Correspondence -->
  <!--+++++++++++++++++++++++++++++-->
  <rdfs:Datatype rdf:about="&iso19104;Correspondence">
    <rdfs:label>Correspondence</rdfs:label>
    <rdfs:isDefinedBy>http://standards.iso.org/iso/19104/ed-1/en/</rdfs:isDefinedBy>
    <owl:equivalentClass>
      <rdfs:Datatype>
        <owl:oneOf>
          <rdf:List>
            <rdf:first rdf:datatype="&xsd;string">identical</rdf:first>
            <rdf:rest>
              <rdf:List>
                <rdf:first rdf:datatype="&xsd;string">modified</rdf:first>
                <rdf:rest>
                  <rdf:List>
                    <rdf:first rdf:datatype="&xsd;string">notEquivalent</rdf:first>
                    <rdf:rest rdf:resource="&rdf;nil"/>
                  </rdf:List>
                </rdf:rest>
              </rdf:List>
            </rdf:rest>
          </rdf:List>
        </owl:oneOf>
      </rdfs:Datatype>
    </owl:equivalentClass>
  </rdfs:Datatype>

  <!--+++++++++++++++++++++++++++++++++-->
  <!-- Enumeration: TermClassification -->
  <!--+++++++++++++++++++++++++++++++++-->
  <rdfs:Datatype rdf:about="&iso19104;TermClassification">
    <rdfs:label>TermClassification</rdfs:label>
    <rdfs:isDefinedBy>http://standards.iso.org/iso/19104/ed-1/en/</rdfs:isDefinedBy>
    <owl:equivalentClass>
      <rdfs:Datatype>
        <owl:oneOf>
          <rdf:List>
            <rdf:first rdf:datatype="&xsd;string">preferred</rdf:first>
            <rdf:rest>
              <rdf:List>
                <rdf:first rdf:datatype="&xsd;string">admitted</rdf:first>
                <rdf:rest>
                  <rdf:List>
                    <rdf:first rdf:datatype="&xsd;string">deprecated</rdf:first>
                    <rdf:rest>
                      <rdf:List>
                        <rdf:first rdf:datatype="&xsd;string">equivalent</rdf:first>
                        <rdf:rest rdf:resource="&rdf;nil"/>
                      </rdf:List>
                    </rdf:rest>
                  </rdf:List>
                </rdf:rest>
              </rdf:List>
            </rdf:rest>
          </rdf:List>
        </owl:oneOf>
      </rdfs:Datatype>
    </owl:equivalentClass>
  </rdfs:Datatype>

</rdf:RDF>

