<?xml version="1.0"?>

<!DOCTYPE rdf:RDF [
  <!ENTITY owl "http://www.w3.org/2002/07/owl#" >
  <!ENTITY xsd "http://www.w3.org/2001/XMLSchema#" >
  <!ENTITY rdfs "http://www.w3.org/2000/01/rdf-schema#" >
  <!ENTITY rdf "http://www.w3.org/1999/02/22-rdf-syntax-ns#" >
  <!ENTITY dc "http://purl.org/dc/elements/1.1/" >
  <!ENTITY dct "http://purl.org/dc/terms/" >
  <!ENTITY skos "http://www.w3.org/2004/02/skos/core#" >
  <!ENTITY iso19150-2 "http://def.isotc211.org/iso19150/-2/2012/base#" >
  <!ENTITY iso19107_401 "http://def.isotc211.org/iso19107/2003/GeometryRoot#" >
  <!ENTITY iso19115_515 "http://def.isotc211.org/iso19115/2006/ExtentInformation#" >
  <!ENTITY iso19108_407 "http://def.isotc211.org/iso19108/2006/TemporalObjects#" >
  <!ENTITY iso19115_516 "http://def.isotc211.org/iso19115/2006/CitationAndResponsiblePartyInformation#" >
  <!ENTITY iso19103_336 "http://def.isotc211.org/iso19103/2005/Names#" >
  <!ENTITY iso19103_333 "http://def.isotc211.org/iso19103/2005/UnitsOfMeasure#" >
  <!ENTITY iso19156_1677 "http://def.isotc211.org/iso19156/2011/SamplingFeature#" >
  <!ENTITY iso19156 "http://def.isotc211.org/iso19156/2011/Specimen#" >

]>

  <!--++++++++++++++++++++++++++++++++++++++++++++++-->
  <!-- File name:         iso19156Specimen.rdf      -->
  <!-- Generator:         GOM_Technologies::UML2OWL -->
  <!-- Generator version: 2.5                       -->
  <!-- File date:         26-10-2016                -->
  <!--++++++++++++++++++++++++++++++++++++++++++++++-->

<rdf:RDF xmlns="http://def.isotc211.org/iso19156/2011/Specimen#"
  xml:base="http://def.isotc211.org/iso19156/2011/Specimen"
  xmlns:owl="http://www.w3.org/2002/07/owl#"
  xmlns:xsd="http://www.w3.org/2001/XMLSchema#"
  xmlns:rdfs="http://www.w3.org/2000/01/rdf-schema#"
  xmlns:rdf="http://www.w3.org/1999/02/22-rdf-syntax-ns#"
  xmlns:dc="http://purl.org/dc/elements/1.1/"
  xmlns:dct="http://purl.org/dc/terms/"
  xmlns:skos="http://www.w3.org/2004/02/skos/core#"
  xmlns:iso19150-2="http://def.isotc211.org/iso19150/-2/2012/base#"
  xmlns:iso19107_401="http://def.isotc211.org/iso19107/2003/GeometryRoot#"
  xmlns:iso19115_515="http://def.isotc211.org/iso19115/2006/ExtentInformation#"
  xmlns:iso19108_407="http://def.isotc211.org/iso19108/2006/TemporalObjects#"
  xmlns:iso19115_516="http://def.isotc211.org/iso19115/2006/CitationAndResponsiblePartyInformation#"
  xmlns:iso19103_336="http://def.isotc211.org/iso19103/2005/Names#"
  xmlns:iso19103_333="http://def.isotc211.org/iso19103/2005/UnitsOfMeasure#"
  xmlns:iso19156_1677="http://def.isotc211.org/iso19156/2011/SamplingFeature#"
  xmlns:iso19156="http://def.isotc211.org/iso19156/2011/Specimen#">

  <!--+++++++++++++++++++++++++++++++++++-->
  <!-- Ontology: ISO 19156:2011 specimen -->
  <!--+++++++++++++++++++++++++++++++++++-->
  <owl:Ontology rdf:about="http://def.isotc211.org/iso19156/2011/Specimen">
    <rdfs:label>ISO 19156:2011 specimen</rdfs:label>
    <dct:source>http://standards.iso.org/iso/19156/ed-1/en/</dct:source>
    <owl:versionInfo>2011-12-15</owl:versionInfo>
    <!--owl:imports rdf:resource="http://def.isotc211.org/iso19107/2003/GeometryRoot"/>
    <owl:imports rdf:resource="http://def.isotc211.org/iso19115/2006/ExtentInformation"/>
    <owl:imports rdf:resource="http://def.isotc211.org/iso19108/2006/TemporalObjects"/>
    <owl:imports rdf:resource="http://def.isotc211.org/iso19115/2006/CitationAndResponsiblePartyInformation"/>
    <owl:imports rdf:resource="http://def.isotc211.org/iso19103/2005/Names"/>
    <owl:imports rdf:resource="http://def.isotc211.org/iso19103/2005/UnitsOfMeasure"/-->
    <owl:imports rdf:resource="http://def.isotc211.org/iso19156/2011/SamplingFeature"/>
    <owl:imports rdf:resource="http://def.isotc211.org/iso19150/-2/2012/base"/>
  </owl:Ontology>

  <!--+++++++++++++++++++++++++-->
  <!-- Class: GeometryLocation -->
  <!--+++++++++++++++++++++++++-->
  <owl:Class rdf:about="&iso19156;uGeometryLocation">
    <rdfs:label>GeometryLocation</rdfs:label>
    <skos:definition>The attribute .lt.i.gt.geometryLocation:GM_Object .lt..sl.i.gt.shall select a geometric representation of the location. </skos:definition>
    <rdfs:isDefinedBy>http://standards.iso.org/iso/19156/ed-1/en/</rdfs:isDefinedBy>
    <rdfs:subClassOf>
      <owl:Restriction>
        <owl:onProperty rdf:resource="&iso19156;uGeometryLocation.geometryLocation"/>
        <owl:cardinality rdf:datatype="&xsd;nonNegativeInteger">1</owl:cardinality>
      </owl:Restriction>
    </rdfs:subClassOf>
    <rdfs:subClassOf>
      <owl:Restriction>
        <owl:onProperty rdf:resource="&iso19156;uGeometryLocation.geometryLocation"/>
        <owl:allValuesFrom rdf:resource="&iso19107_401;GM_Object"/>
      </owl:Restriction>
    </rdfs:subClassOf>
  </owl:Class>

  <!--+++++++++++++++++++++-->
  <!-- Class: NameLocation -->
  <!--+++++++++++++++++++++-->
  <owl:Class rdf:about="&iso19156;uNameLocation">
    <rdfs:label>NameLocation</rdfs:label>
    <skos:definition>The attribute .lt.i.gt.nameLocation:EX_GeographicDescription .lt..sl.i.gt.shall select a description of the location using text or an identifier. </skos:definition>
    <rdfs:isDefinedBy>http://standards.iso.org/iso/19156/ed-1/en/</rdfs:isDefinedBy>
    <rdfs:subClassOf>
      <owl:Restriction>
        <owl:onProperty rdf:resource="&iso19156;uNameLocation.nameLocation"/>
        <owl:cardinality rdf:datatype="&xsd;nonNegativeInteger">1</owl:cardinality>
      </owl:Restriction>
    </rdfs:subClassOf>
    <rdfs:subClassOf>
      <owl:Restriction>
        <owl:onProperty rdf:resource="&iso19156;uNameLocation.nameLocation"/>
        <owl:allValuesFrom rdf:resource="&iso19115_515;EX_GeographicDescription"/>
      </owl:Restriction>
    </rdfs:subClassOf>
  </owl:Class>

  <!--++++++++++++++++++++++++-->
  <!-- Class: PreparationStep -->
  <!--++++++++++++++++++++++++-->
  <owl:Class rdf:about="&iso19156;PreparationStep">
    <rdfs:label>PreparationStep</rdfs:label>
    <skos:definition>In many applications specimen preparation procedures are applied to the material prior to its use in an observation. The class .lt.i.gt.PreparationStep.lt..sl.i.gt. (Figure 13) shall link a SF_Specimen to a OM_Process that describes a phase of the specimen preparation.  It shall support one attribute. </skos:definition>
    <rdfs:isDefinedBy>http://standards.iso.org/iso/19156/ed-1/en/</rdfs:isDefinedBy>
    <rdfs:subClassOf>
      <owl:Restriction>
        <owl:onProperty rdf:resource="&iso19156;PreparationStep.time"/>
        <owl:cardinality rdf:datatype="&xsd;nonNegativeInteger">1</owl:cardinality>
      </owl:Restriction>
    </rdfs:subClassOf>
    <rdfs:subClassOf>
      <owl:Restriction>
        <owl:onProperty rdf:resource="&iso19156;PreparationStep.time"/>
        <owl:allValuesFrom rdf:resource="&iso19108_407;TM_Object"/>
      </owl:Restriction>
    </rdfs:subClassOf>
    <rdfs:subClassOf>
      <owl:Restriction>
        <owl:onProperty rdf:resource="&iso19156;PreparationStep.processOperator"/>
        <owl:maxCardinality rdf:datatype="&xsd;nonNegativeInteger">1</owl:maxCardinality>
      </owl:Restriction>
    </rdfs:subClassOf>
    <rdfs:subClassOf>
      <owl:Restriction>
        <owl:onProperty rdf:resource="&iso19156;PreparationStep.processOperator"/>
        <owl:allValuesFrom rdf:resource="&iso19115_516;CI_ResponsibleParty"/>
      </owl:Restriction>
    </rdfs:subClassOf>
    <rdfs:subClassOf>
      <owl:Restriction>
        <owl:onProperty rdf:resource="&iso19156;PreparationStep.processingDetails"/>
        <owl:cardinality rdf:datatype="&xsd;nonNegativeInteger">1</owl:cardinality>
      </owl:Restriction>
    </rdfs:subClassOf>
    <rdfs:subClassOf>
      <owl:Restriction>
        <owl:onProperty rdf:resource="&iso19156;PreparationStep.processingDetails"/>
        <owl:allValuesFrom rdf:resource="&iso19156;PreparationStep"/>
      </owl:Restriction>
    </rdfs:subClassOf>
  </owl:Class>

  <!--+++++++++++++++++++-->
  <!-- Class: SF_Process -->
  <!--+++++++++++++++++++-->
  <owl:Class rdf:about="&iso19156;SF_Process">
    <rdfs:label>SF_Process</rdfs:label>
    <skos:definition>The class SF_Process (Figure 13) is an instance of the .og.metaclass.cg. GF_FeatureType (ISO 19109:2005), which therefore represents a feature type. SF_Process is abstract, and has no attributes, operations or associations. It serves as the base class for processes associated with the design and preparation of sampling features. The purpose of a sampling process is to generate or transform a sampling feature.  </skos:definition>
    <rdfs:isDefinedBy>http://standards.iso.org/iso/19156/ed-1/en/</rdfs:isDefinedBy>
    <iso19150-2:isAbstract rdf:datatype="&xsd;boolean">true</iso19150-2:isAbstract>
  </owl:Class>

  <!--++++++++++++++++++++-->
  <!-- Class: SF_Specimen -->
  <!--++++++++++++++++++++-->
  <owl:Class rdf:about="&iso19156;SF_Specimen">
    <rdfs:label>SF_Specimen</rdfs:label>
    <skos:definition>A Specimen is a physical sample, obtained for observation(s) carried out .lt.i.gt.ex situ, .lt..sl.i.gt.sometimes in a laboratory. </skos:definition>
    <rdfs:isDefinedBy>http://standards.iso.org/iso/19156/ed-1/en/</rdfs:isDefinedBy>
    <rdfs:subClassOf rdf:resource="&iso19156_1677;SF_SamplingFeature"/>
    <rdfs:subClassOf>
      <owl:Restriction>
        <owl:onProperty rdf:resource="&iso19156;SF_Specimen.materialClass"/>
        <owl:cardinality rdf:datatype="&xsd;nonNegativeInteger">1</owl:cardinality>
      </owl:Restriction>
    </rdfs:subClassOf>
    <rdfs:subClassOf>
      <owl:Restriction>
        <owl:onProperty rdf:resource="&iso19156;SF_Specimen.materialClass"/>
        <owl:allValuesFrom rdf:resource="&iso19103_336;GenericName"/>
      </owl:Restriction>
    </rdfs:subClassOf>
    <rdfs:subClassOf>
      <owl:Restriction>
        <owl:onProperty rdf:resource="&iso19156;SF_Specimen.samplingTime"/>
        <owl:cardinality rdf:datatype="&xsd;nonNegativeInteger">1</owl:cardinality>
      </owl:Restriction>
    </rdfs:subClassOf>
    <rdfs:subClassOf>
      <owl:Restriction>
        <owl:onProperty rdf:resource="&iso19156;SF_Specimen.samplingTime"/>
        <owl:allValuesFrom rdf:resource="&iso19108_407;TM_Object"/>
      </owl:Restriction>
    </rdfs:subClassOf>
    <rdfs:subClassOf>
      <owl:Restriction>
        <owl:onProperty rdf:resource="&iso19156;SF_Specimen.samplingLocation"/>
        <owl:maxCardinality rdf:datatype="&xsd;nonNegativeInteger">1</owl:maxCardinality>
      </owl:Restriction>
    </rdfs:subClassOf>
    <rdfs:subClassOf>
      <owl:Restriction>
        <owl:onProperty rdf:resource="&iso19156;SF_Specimen.samplingLocation"/>
        <owl:allValuesFrom rdf:resource="&iso19107_401;GM_Object"/>
      </owl:Restriction>
    </rdfs:subClassOf>
    <rdfs:subClassOf>
      <owl:Restriction>
        <owl:onProperty rdf:resource="&iso19156;SF_Specimen.samplingMethod"/>
        <owl:maxCardinality rdf:datatype="&xsd;nonNegativeInteger">1</owl:maxCardinality>
      </owl:Restriction>
    </rdfs:subClassOf>
    <rdfs:subClassOf>
      <owl:Restriction>
        <owl:onProperty rdf:resource="&iso19156;SF_Specimen.samplingMethod"/>
        <owl:allValuesFrom rdf:resource="&iso19156;SF_Process"/>
      </owl:Restriction>
    </rdfs:subClassOf>
    <rdfs:subClassOf>
      <owl:Restriction>
        <owl:onProperty rdf:resource="&iso19156;SF_Specimen.currentLocation"/>
        <owl:maxCardinality rdf:datatype="&xsd;nonNegativeInteger">1</owl:maxCardinality>
      </owl:Restriction>
    </rdfs:subClassOf>
    <rdfs:subClassOf>
      <owl:Restriction>
        <owl:onProperty rdf:resource="&iso19156;SF_Specimen.currentLocation"/>
        <owl:allValuesFrom rdf:resource="&iso19156;Location"/>
      </owl:Restriction>
    </rdfs:subClassOf>
    <rdfs:subClassOf>
      <owl:Restriction>
        <owl:onProperty rdf:resource="&iso19156;SF_Specimen.specimenType"/>
        <owl:maxCardinality rdf:datatype="&xsd;nonNegativeInteger">1</owl:maxCardinality>
      </owl:Restriction>
    </rdfs:subClassOf>
    <rdfs:subClassOf>
      <owl:Restriction>
        <owl:onProperty rdf:resource="&iso19156;SF_Specimen.specimenType"/>
        <owl:allValuesFrom rdf:resource="&iso19103_336;GenericName"/>
      </owl:Restriction>
    </rdfs:subClassOf>
    <rdfs:subClassOf>
      <owl:Restriction>
        <owl:onProperty rdf:resource="&iso19156;SF_Specimen.size"/>
        <owl:maxCardinality rdf:datatype="&xsd;nonNegativeInteger">1</owl:maxCardinality>
      </owl:Restriction>
    </rdfs:subClassOf>
    <rdfs:subClassOf>
      <owl:Restriction>
        <owl:onProperty rdf:resource="&iso19156;SF_Specimen.size"/>
        <owl:allValuesFrom rdf:resource="&iso19103_333;Measure"/>
      </owl:Restriction>
    </rdfs:subClassOf>
    <rdfs:subClassOf>
      <owl:Restriction>
        <owl:onProperty rdf:resource="&iso19156;SF_Specimen.thePreparationStep"/>
        <owl:allValuesFrom rdf:resource="&iso19156;PreparationStep"/>
      </owl:Restriction>
    </rdfs:subClassOf>
  </owl:Class>

  <!--++++++++++++++++++++++++++++++++++-->
  <!-- ObjectProperty: geometryLocation -->
  <!--++++++++++++++++++++++++++++++++++-->
  <owl:ObjectProperty rdf:about="&iso19156;uGeometryLocation.geometryLocation">
    <skos:prefLabel>geometryLocation</skos:prefLabel>
    <rdfs:isDefinedBy>http://standards.iso.org/iso/19156/ed-1/en/</rdfs:isDefinedBy>
    <rdfs:domain rdf:resource="&iso19156;uGeometryLocation"/>
    <rdfs:range rdf:resource="&iso19107_401;GM_Object"/>
  </owl:ObjectProperty>

  <!--++++++++++++++++++++++++++++++-->
  <!-- ObjectProperty: nameLocation -->
  <!--++++++++++++++++++++++++++++++-->
  <owl:ObjectProperty rdf:about="&iso19156;uNameLocation.nameLocation">
    <skos:prefLabel>nameLocation</skos:prefLabel>
    <rdfs:isDefinedBy>http://standards.iso.org/iso/19156/ed-1/en/</rdfs:isDefinedBy>
    <rdfs:domain rdf:resource="&iso19156;uNameLocation"/>
    <rdfs:range rdf:resource="&iso19115_515;EX_GeographicDescription"/>
  </owl:ObjectProperty>

  <!--++++++++++++++++++++++++++++++++++++++-->
  <!-- ObjectProperty: PreparationStep.time -->
  <!--++++++++++++++++++++++++++++++++++++++-->
  <owl:ObjectProperty rdf:about="&iso19156;PreparationStep.time">
    <rdfs:label>time</rdfs:label>
    <skos:definition>The attribute .lt.i.gt.time:TM_Object .lt..sl.i.gt.shall describe the time that the OM_Process was applied to the SP_Specimen. It supports ordering of preparation steps.</skos:definition>
    <rdfs:isDefinedBy>http://standards.iso.org/iso/19156/ed-1/en/</rdfs:isDefinedBy>
    <rdfs:domain rdf:resource="&iso19156;PreparationStep"/>
    <rdfs:range rdf:resource="&iso19108_407;TM_Object"/>
  </owl:ObjectProperty>

  <!--+++++++++++++++++++++++++++++++++++++++++++++++++-->
  <!-- ObjectProperty: PreparationStep.processOperator -->
  <!--+++++++++++++++++++++++++++++++++++++++++++++++++-->
  <owl:ObjectProperty rdf:about="&iso19156;PreparationStep.processOperator">
    <rdfs:label>processOperator</rdfs:label>
    <skos:definition>If present, the attribute .lt.i.gt.processOperator:CI_ResponsibleParty .lt..sl.i.gt.shall describe the operator of the process involved in the preparation step. </skos:definition>
    <rdfs:isDefinedBy>http://standards.iso.org/iso/19156/ed-1/en/</rdfs:isDefinedBy>
    <rdfs:domain rdf:resource="&iso19156;PreparationStep"/>
    <rdfs:range rdf:resource="&iso19115_516;CI_ResponsibleParty"/>
  </owl:ObjectProperty>

  <!--+++++++++++++++++++++++++++++++++++++++++++-->
  <!-- ObjectProperty: SF_Specimen.materialClass -->
  <!--+++++++++++++++++++++++++++++++++++++++++++-->
  <owl:ObjectProperty rdf:about="&iso19156;SF_Specimen.materialClass">
    <rdfs:label>materialClass</rdfs:label>
    <skos:definition>The attribute .lt.i.gt.materialClass:GenericName .lt..sl.i.gt.shall provide a basic classification of the material type of the specimen. EXAMPLE	soil, water, rock, aqueous, liquid, tissue, vegetation, food. </skos:definition>
    <rdfs:isDefinedBy>http://standards.iso.org/iso/19156/ed-1/en/</rdfs:isDefinedBy>
    <rdfs:domain rdf:resource="&iso19156;SF_Specimen"/>
    <rdfs:range rdf:resource="&iso19103_336;GenericName"/>
  </owl:ObjectProperty>

  <!--++++++++++++++++++++++++++++++++++++++++++-->
  <!-- ObjectProperty: SF_Specimen.samplingTime -->
  <!--++++++++++++++++++++++++++++++++++++++++++-->
  <owl:ObjectProperty rdf:about="&iso19156;SF_Specimen.samplingTime">
    <rdfs:label>samplingTime</rdfs:label>
    <skos:definition>The attribute .lt.i.gt.samplingTime:TM_Object .lt..sl.i.gt.shall record when the specimen was retrieved from the sampled feature.</skos:definition>
    <rdfs:isDefinedBy>http://standards.iso.org/iso/19156/ed-1/en/</rdfs:isDefinedBy>
    <rdfs:domain rdf:resource="&iso19156;SF_Specimen"/>
    <rdfs:range rdf:resource="&iso19108_407;TM_Object"/>
  </owl:ObjectProperty>

  <!--++++++++++++++++++++++++++++++++++++++++++++++-->
  <!-- ObjectProperty: SF_Specimen.samplingLocation -->
  <!--++++++++++++++++++++++++++++++++++++++++++++++-->
  <owl:ObjectProperty rdf:about="&iso19156;SF_Specimen.samplingLocation">
    <rdfs:label>samplingLocation</rdfs:label>
    <skos:definition>If present, the attribute .lt.i.gt.samplingLocation:GM_Object .lt..sl.i.gt.shall describe the location from where the specimen was obtained. NOTE	Where a specimen has a relatedSamplingFeature whose location provides an unambiguous location then this attribute is not required. However, if the specific sampling location within the sampledFeature is important, then this attribute supports its description. </skos:definition>
    <rdfs:isDefinedBy>http://standards.iso.org/iso/19156/ed-1/en/</rdfs:isDefinedBy>
    <rdfs:domain rdf:resource="&iso19156;SF_Specimen"/>
    <rdfs:range rdf:resource="&iso19107_401;GM_Object"/>
  </owl:ObjectProperty>

  <!--++++++++++++++++++++++++++++++++++++++++++++-->
  <!-- ObjectProperty: SF_Specimen.samplingMethod -->
  <!--++++++++++++++++++++++++++++++++++++++++++++-->
  <owl:ObjectProperty rdf:about="&iso19156;SF_Specimen.samplingMethod">
    <rdfs:label>samplingMethod</rdfs:label>
    <skos:definition>If present, the attribute .lt.i.gt.samplingMethod:SF_Process .lt..sl.i.gt.shall describe the method used to obtain the specimen from its sampledFeature. </skos:definition>
    <rdfs:isDefinedBy>http://standards.iso.org/iso/19156/ed-1/en/</rdfs:isDefinedBy>
    <rdfs:domain rdf:resource="&iso19156;SF_Specimen"/>
    <rdfs:range rdf:resource="&iso19156;SF_Process"/>
  </owl:ObjectProperty>

  <!--+++++++++++++++++++++++++++++++++++++++++++++-->
  <!-- ObjectProperty: SF_Specimen.currentLocation -->
  <!--+++++++++++++++++++++++++++++++++++++++++++++-->
  <owl:ObjectProperty rdf:about="&iso19156;SF_Specimen.currentLocation">
    <rdfs:label>currentLocation</rdfs:label>
    <skos:definition>If present, the attribute .lt.i.gt.currentLocation:Location .lt..sl.i.gt.shall describe the location of a physical specimen. This may be a storage location, such as a shelf in a warehouse or a drawer in a museum. NOTE	If a specimen no longer exists, for example it was destroyed in connection with an observation act, then the currentLocation should be omitted or carry a suitable null indicator. </skos:definition>
    <rdfs:isDefinedBy>http://standards.iso.org/iso/19156/ed-1/en/</rdfs:isDefinedBy>
    <rdfs:domain rdf:resource="&iso19156;SF_Specimen"/>
    <rdfs:range rdf:resource="&iso19156;Location"/>
  </owl:ObjectProperty>

  <!--++++++++++++++++++++++++++++++++++++++++++-->
  <!-- ObjectProperty: SF_Specimen.specimenType -->
  <!--++++++++++++++++++++++++++++++++++++++++++-->
  <owl:ObjectProperty rdf:about="&iso19156;SF_Specimen.specimenType">
    <rdfs:label>specimenType</rdfs:label>
    <skos:definition>If present, the attribute .lt.i.gt.specimenType:GenericName .lt..sl.i.gt.shall describe the basic form of the specimen. EXAMPLE	polished section; core; pulp; solution. </skos:definition>
    <rdfs:isDefinedBy>http://standards.iso.org/iso/19156/ed-1/en/</rdfs:isDefinedBy>
    <rdfs:domain rdf:resource="&iso19156;SF_Specimen"/>
    <rdfs:range rdf:resource="&iso19103_336;GenericName"/>
  </owl:ObjectProperty>

  <!--++++++++++++++++++++++++++++++++++-->
  <!-- ObjectProperty: SF_Specimen.size -->
  <!--++++++++++++++++++++++++++++++++++-->
  <owl:ObjectProperty rdf:about="&iso19156;SF_Specimen.size">
    <rdfs:label>size</rdfs:label>
    <skos:definition>If present, the attribute .lt.i.gt.size:Measure .lt..sl.i.gt.shall describe a physical extent of the specimen. This may be length, mass, volume, etc as appropriate for the specimen instance and its material class. </skos:definition>
    <rdfs:isDefinedBy>http://standards.iso.org/iso/19156/ed-1/en/</rdfs:isDefinedBy>
    <rdfs:domain rdf:resource="&iso19156;SF_Specimen"/>
    <rdfs:range rdf:resource="&iso19103_333;Measure"/>
  </owl:ObjectProperty>

  <!--+++++++++++++++++++++++++++++++++++++++++++++++-->
  <!-- ObjectProperty: PreparationStep.processingDetails -->
  <!--+++++++++++++++++++++++++++++++++++++++++++++++-->
  <owl:ObjectProperty rdf:about="&iso19156;PreparationStep.processingDetails">
    <rdfs:label>thePreparationStep</rdfs:label>
    <rdfs:isDefinedBy>http://standards.iso.org/iso/19156/ed-1/en/</rdfs:isDefinedBy>
    <rdfs:domain rdf:resource="&iso19156;PreparationStep"/>
    <rdfs:range rdf:resource="&iso19156;SF_Process"/>
  </owl:ObjectProperty>

  <!--+++++++++++++++++-->
  <!-- Class: Location -->
  <!--+++++++++++++++++-->
  <owl:Class rdf:about="&iso19156;Location">
    <rdfs:label>Location</rdfs:label>
    <skos:definition>Location (Figure 13) is a union class (choice) that shall support two attributes. </skos:definition>
    <rdfs:isDefinedBy>http://standards.iso.org/iso/19156/ed-1/en/</rdfs:isDefinedBy>
    <owl:equivalentClass>
      <owl:Class>
        <owl:unionOf rdf:parseType="Collection">
          <owl:Class rdf:about="&iso19156;uGeometryLocation"/>
          <owl:Class rdf:about="&iso19156;uNameLocation"/>
        </owl:unionOf>
      </owl:Class>
    </owl:equivalentClass>
  </owl:Class>

</rdf:RDF>

