<?xml version="1.0"?>

<!DOCTYPE rdf:RDF [
  <!ENTITY owl "http://www.w3.org/2002/07/owl#" >
  <!ENTITY xsd "http://www.w3.org/2001/XMLSchema#" >
  <!ENTITY rdfs "http://www.w3.org/2000/01/rdf-schema#" >
  <!ENTITY rdf "http://www.w3.org/1999/02/22-rdf-syntax-ns#" >
  <!ENTITY dc "http://purl.org/dc/elements/1.1/" >
  <!ENTITY dct "http://purl.org/dc/terms/" >
  <!ENTITY skos "http://www.w3.org/2004/02/skos/core#" >
  <!ENTITY iso19150-2 "http://def.isotc211.org/iso19150/-2/2012/base#" >
  <!ENTITY iso19108_407 "http://def.isotc211.org/iso19108/2006/TemporalObjects#" >
  <!ENTITY iso19123_1041 "http://def.isotc211.org/iso19123/2005/DiscreteCoverages#" >
  <!ENTITY iso19123_1040 "http://def.isotc211.org/iso19123/2005/CoverageCore#" >
  <!ENTITY iso19156 "http://def.isotc211.org/iso19156/2011/TemporalCoverage#" >

]>

  <!--+++++++++++++++++++++++++++++++++++++++++++++++++-->
  <!-- File name:         iso19156TemporalCoverage.rdf -->
  <!-- Generator:         GOM_Technologies::UML2OWL    -->
  <!-- Generator version: 2.5                          -->
  <!-- File date:         26-10-2016                   -->
  <!--+++++++++++++++++++++++++++++++++++++++++++++++++-->

<rdf:RDF xmlns="http://def.isotc211.org/iso19156/2011/TemporalCoverage#"
  xml:base="http://def.isotc211.org/iso19156/2011/TemporalCoverage"
  xmlns:owl="http://www.w3.org/2002/07/owl#"
  xmlns:xsd="http://www.w3.org/2001/XMLSchema#"
  xmlns:rdfs="http://www.w3.org/2000/01/rdf-schema#"
  xmlns:rdf="http://www.w3.org/1999/02/22-rdf-syntax-ns#"
  xmlns:dc="http://purl.org/dc/elements/1.1/"
  xmlns:dct="http://purl.org/dc/terms/"
  xmlns:skos="http://www.w3.org/2004/02/skos/core#"
  xmlns:iso19150-2="http://def.isotc211.org/iso19150/-2/2012/base#"
  xmlns:iso19108_407="http://def.isotc211.org/iso19108/2006/TemporalObjects#"
  xmlns:iso19123_1041="http://def.isotc211.org/iso19123/2005/DiscreteCoverages#"
  xmlns:iso19123_1040="http://def.isotc211.org/iso19123/2005/CoverageCore#"
  xmlns:iso19156="http://def.isotc211.org/iso19156/2011/TemporalCoverage#">

  <!--++++++++++++++++++++++++++++++++++++++++++++-->
  <!-- Ontology: ISO 19156:2011 Temporal Coverage -->
  <!--++++++++++++++++++++++++++++++++++++++++++++-->
  <owl:Ontology rdf:about="http://def.isotc211.org/iso19156/2011/TemporalCoverage">
    <rdfs:label>ISO 19156:2011 Temporal Coverage</rdfs:label>
    <dct:source>http://standards.iso.org/iso/19156/ed-1/en/</dct:source>
    <owl:versionInfo>2011-12-15</owl:versionInfo>
    <!--owl:imports rdf:resource="http://def.isotc211.org/iso19108/2006/TemporalObjects"/>
    <owl:imports rdf:resource="http://def.isotc211.org/iso19123/2005/DiscreteCoverages"/>
    <owl:imports rdf:resource="http://def.isotc211.org/iso19123/2005/CoverageCore"/-->
    <owl:imports rdf:resource="http://def.isotc211.org/iso19150/-2/2012/base"/>
  </owl:Ontology>

  <!--++++++++++++++++++++++++++++++++++++++++-->
  <!-- Class: CVT_DiscreteTimeInstantCoverage -->
  <!--++++++++++++++++++++++++++++++++++++++++-->
  <owl:Class rdf:about="&iso19156;CVT_DiscreteTimeInstantCoverage">
    <rdfs:label>CVT_DiscreteTimeInstantCoverage</rdfs:label>
    <skos:definition>The class .lt.i.gt.CT_DiscreteTimeInstantCoverage.lt..sl.i.gt. (Figure 5) is a specialization of CV_DiscreteCoverage (ISO 19123). CT_DiscreteTimeInstantCoverage shall support one association.  </skos:definition>
    <rdfs:isDefinedBy>http://standards.iso.org/iso/19156/ed-1/en/</rdfs:isDefinedBy>
    <rdfs:subClassOf rdf:resource="&iso19123_1041;CV_DiscreteCoverage"/>
    <rdfs:subClassOf>
      <owl:Restriction>
        <owl:onProperty rdf:resource="&iso19156;CVT_DiscreteTimeInstantCoverage.element"/>
        <owl:allValuesFrom rdf:resource="&iso19156;CVT_TimeInstantValuePair"/>
      </owl:Restriction>
    </rdfs:subClassOf>
  </owl:Class>

  <!--+++++++++++++++++++++++++++++++++-->
  <!-- Class: CVT_TimeInstantValuePair -->
  <!--+++++++++++++++++++++++++++++++++-->
  <owl:Class rdf:about="&iso19156;CVT_TimeInstantValuePair">
    <rdfs:label>CVT_TimeInstantValuePair</rdfs:label>
    <skos:definition>The class .lt.i.gt.CVT_TimeInstantValuePair.lt..sl.i.gt. (Figure 12) is a specialization of CV_GeometryValuePair (ISO 19123). CVT_TimeInstantValuePair shall redefine one attribute inherited from CV_GeometryValuePair.   </skos:definition>
    <rdfs:isDefinedBy>http://standards.iso.org/iso/19156/ed-1/en/</rdfs:isDefinedBy>
    <rdfs:subClassOf rdf:resource="&iso19123_1040;CV_GeometryValuePair"/>
    <rdfs:subClassOf>
      <owl:Restriction>
        <owl:onProperty rdf:resource="&iso19156;CVT_TimeInstantValuePair.geometry"/>
        <owl:cardinality rdf:datatype="&xsd;nonNegativeInteger">1</owl:cardinality>
      </owl:Restriction>
    </rdfs:subClassOf>
    <rdfs:subClassOf>
      <owl:Restriction>
        <owl:onProperty rdf:resource="&iso19156;CVT_TimeInstantValuePair.geometry"/>
        <owl:allValuesFrom rdf:resource="&iso19108_407;TM_Instant"/>
      </owl:Restriction>
    </rdfs:subClassOf>
  </owl:Class>

  <!--+++++++++++++++++++++++++++++++++++++++++++++++++++-->
  <!-- ObjectProperty: CVT_TimeInstantValuePair.geometry -->
  <!--+++++++++++++++++++++++++++++++++++++++++++++++++++-->
  <owl:ObjectProperty rdf:about="&iso19156;CVT_TimeInstantValuePair.geometry">
    <rdfs:label>geometry</rdfs:label>
    <skos:definition>The attribute geometry:TM_Instant shall redefine the type of the geometry attribute inheritted from CV_GeometryValuePair. </skos:definition>
    <rdfs:isDefinedBy>http://standards.iso.org/iso/19156/ed-1/en/</rdfs:isDefinedBy>
    <rdfs:domain rdf:resource="&iso19156;CVT_TimeInstantValuePair"/>
    <rdfs:range rdf:resource="&iso19108_407;TM_Instant"/>
  </owl:ObjectProperty>

  <!--+++++++++++++++++++++++++++++++++++++++++++++++++++++++++-->
  <!-- ObjectProperty: CVT_DiscreteTimeInstantCoverage.element -->
  <!--+++++++++++++++++++++++++++++++++++++++++++++++++++++++++-->
  <owl:ObjectProperty rdf:about="&iso19156;CVT_DiscreteTimeInstantCoverage.element">
    <rdfs:label>element</rdfs:label>
    <rdfs:isDefinedBy>http://standards.iso.org/iso/19156/ed-1/en/</rdfs:isDefinedBy>
    <iso19150-2:aggregationType>partOfSharedAggregation</iso19150-2:aggregationType>
    <iso19150-2:associationName>CoverageFunction</iso19150-2:associationName>
    <rdfs:domain rdf:resource="&iso19156;CVT_DiscreteTimeInstantCoverage"/>
    <rdfs:range rdf:resource="&iso19156;CVT_TimeInstantValuePair"/>
  </owl:ObjectProperty>

</rdf:RDF>

