<?xml version="1.0"?>

<!DOCTYPE rdf:RDF [
  <!ENTITY owl "http://www.w3.org/2002/07/owl#" >
  <!ENTITY xsd "http://www.w3.org/2001/XMLSchema#" >
  <!ENTITY rdfs "http://www.w3.org/2000/01/rdf-schema#" >
  <!ENTITY rdf "http://www.w3.org/1999/02/22-rdf-syntax-ns#" >
  <!ENTITY dc "http://purl.org/dc/elements/1.1/" >
  <!ENTITY dct "http://purl.org/dc/terms/" >
  <!ENTITY skos "http://www.w3.org/2004/02/skos/core#" >
  <!ENTITY iso19150-2 "http://def.isotc211.org/iso19150/-2/2012/base#" >
  <!ENTITY iso19103_336 "http://def.isotc211.org/iso19103/2005/Names#" >
  <!ENTITY iso19103_337 "http://def.isotc211.org/iso19103/2005/RecordsAndClassMetadata#" >
  <!ENTITY iso19108_407 "http://def.isotc211.org/iso19108/2006/TemporalObjects#" >
  <!ENTITY iso19115_506 "http://def.isotc211.org/iso19115/2006/DataQualityInformation#" >
  <!ENTITY iso19115_503 "http://def.isotc211.org/iso19115/2006/MetadataEntitySetInformation#" >
  <!ENTITY iso19109_449 "http://def.isotc211.org/iso19109/2005/GeneralFeatureModel#" >
  <!ENTITY iso19156_1687 "http://def.isotc211.org/iso19156/2011/GeneralFeatureInstance#" >
  <!ENTITY iso19156 "http://def.isotc211.org/iso19156/2011/Observation#" >

]>

  <!--++++++++++++++++++++++++++++++++++++++++++++++-->
  <!-- File name:         iso19156Observation.rdf   -->
  <!-- Generator:         GOM_Technologies::UML2OWL -->
  <!-- Generator version: 2.5                       -->
  <!-- File date:         26-10-2016                -->
  <!--++++++++++++++++++++++++++++++++++++++++++++++-->

<rdf:RDF xmlns="http://def.isotc211.org/iso19156/2011/Observation#"
  xml:base="http://def.isotc211.org/iso19156/2011/Observation"
  xmlns:owl="http://www.w3.org/2002/07/owl#"
  xmlns:xsd="http://www.w3.org/2001/XMLSchema#"
  xmlns:rdfs="http://www.w3.org/2000/01/rdf-schema#"
  xmlns:rdf="http://www.w3.org/1999/02/22-rdf-syntax-ns#"
  xmlns:dc="http://purl.org/dc/elements/1.1/"
  xmlns:dct="http://purl.org/dc/terms/"
  xmlns:skos="http://www.w3.org/2004/02/skos/core#"
  xmlns:iso19150-2="http://def.isotc211.org/iso19150/-2/2012/base#"
  xmlns:iso19103_336="http://def.isotc211.org/iso19103/2005/Names#"
  xmlns:iso19103_337="http://def.isotc211.org/iso19103/2005/RecordsAndClassMetadata#"
  xmlns:iso19108_407="http://def.isotc211.org/iso19108/2006/TemporalObjects#"
  xmlns:iso19115_506="http://def.isotc211.org/iso19115/2006/DataQualityInformation#"
  xmlns:iso19115_503="http://def.isotc211.org/iso19115/2006/MetadataEntitySetInformation#"
  xmlns:iso19109_449="http://def.isotc211.org/iso19109/2005/GeneralFeatureModel#"
  xmlns:iso19156_1687="http://def.isotc211.org/iso19156/2011/GeneralFeatureInstance#"
  xmlns:iso19156="http://def.isotc211.org/iso19156/2011/Observation#">

  <!--++++++++++++++++++++++++++++++++++++++-->
  <!-- Ontology: ISO 19156:2011 observation -->
  <!--++++++++++++++++++++++++++++++++++++++-->
  <owl:Ontology rdf:about="http://def.isotc211.org/iso19156/2011/Observation">
    <rdfs:label>ISO 19156:2011 observation</rdfs:label>
    <dct:source>http://standards.iso.org/iso/19156/ed-1/en/</dct:source>
    <owl:versionInfo>2011-12-15</owl:versionInfo>
    <!--owl:imports rdf:resource="http://def.isotc211.org/iso19103/2005/Names"/>
    <owl:imports rdf:resource="http://def.isotc211.org/iso19103/2005/RecordsAndClassMetadata"/>
    <owl:imports rdf:resource="http://def.isotc211.org/iso19108/2006/TemporalObjects"/>
    <owl:imports rdf:resource="http://def.isotc211.org/iso19115/2006/DataQualityInformation"/>
    <owl:imports rdf:resource="http://def.isotc211.org/iso19115/2006/MetadataEntitySetInformation"/>
    <owl:imports rdf:resource="http://def.isotc211.org/iso19109/2005/GeneralFeatureModel"/>
    <owl:imports rdf:resource="http://def.isotc211.org/iso19156/2011/GeneralFeatureInstance"/-->
    <owl:imports rdf:resource="http://def.isotc211.org/iso19150/-2/2012/base"/>
  </owl:Ontology>

  <!--+++++++++++++++++++-->
  <!-- Class: NamedValue -->
  <!--+++++++++++++++++++-->
  <owl:Class rdf:about="&iso19156;NamedValue">
    <rdfs:label>NamedValue</rdfs:label>
    <skos:definition>The class .lt.i.gt.NamedValue.lt..sl.i.gt. provides for a generic soft-typed parameter value. NamedValue shall support two attributes. </skos:definition>
    <rdfs:isDefinedBy>http://standards.iso.org/iso/19156/ed-1/en/</rdfs:isDefinedBy>
    <rdfs:subClassOf>
      <owl:Restriction>
        <owl:onProperty rdf:resource="&iso19156;NamedValue.name"/>
        <owl:cardinality rdf:datatype="&xsd;nonNegativeInteger">1</owl:cardinality>
      </owl:Restriction>
    </rdfs:subClassOf>
    <rdfs:subClassOf>
      <owl:Restriction>
        <owl:onProperty rdf:resource="&iso19156;NamedValue.name"/>
        <owl:allValuesFrom rdf:resource="&iso19103_336;GenericName"/>
      </owl:Restriction>
    </rdfs:subClassOf>
    <rdfs:subClassOf>
      <owl:Restriction>
        <owl:onProperty rdf:resource="&iso19156;NamedValue.value"/>
        <owl:cardinality rdf:datatype="&xsd;nonNegativeInteger">1</owl:cardinality>
      </owl:Restriction>
    </rdfs:subClassOf>
    <rdfs:subClassOf>
      <owl:Restriction>
        <owl:onProperty rdf:resource="&iso19156;NamedValue.value"/>
        <owl:allValuesFrom rdf:resource="&iso19103_337;Any"/>
      </owl:Restriction>
    </rdfs:subClassOf>
  </owl:Class>

  <!--+++++++++++++++++++++++++++-->
  <!-- Class: ObservationContext -->
  <!--+++++++++++++++++++++++++++-->
  <owl:Class rdf:about="&iso19156;ObservationContext">
    <rdfs:label>ObservationContext</rdfs:label>
    <skos:definition>Some observations depend on other observations to provide context which is important, sometimes essential, in understanding the result. These dependencies are stronger than mere spatio-temporal coincidences, requiring explicit representation. If present, the association class class .lt.i.gt.ObservationContext.lt..sl.i.gt. (Figure 2) shall link a OM_Observation to another OM_Observation, with the role name relatedObservation for the target. It shall support one attribute.EXAMPLES	Some examples include the conditions associated with experimental replicates (e.g., experimental plots and treatments used), biotic factors (e.g., ecological community), interactions among features (e.g., predator-prey), or other temporary relationships occurring at the time of observation that are are not inherent to the observed features themselves (i.e., they change over time), or the related observation may provide input to a process that generates a new result.This association complements the Intention association which describes relationships between a sampling feature and domain features.   </skos:definition>
    <rdfs:isDefinedBy>http://standards.iso.org/iso/19156/ed-1/en/</rdfs:isDefinedBy>
    <rdfs:subClassOf>
      <owl:Restriction>
        <owl:onProperty rdf:resource="&iso19156;ObservationContext.role"/>
        <owl:cardinality rdf:datatype="&xsd;nonNegativeInteger">1</owl:cardinality>
      </owl:Restriction>
    </rdfs:subClassOf>
    <rdfs:subClassOf>
      <owl:Restriction>
        <owl:onProperty rdf:resource="&iso19156;ObservationContext.role"/>
        <owl:allValuesFrom rdf:resource="&iso19103_336;GenericName"/>
      </owl:Restriction>
    </rdfs:subClassOf>
    <rdfs:subClassOf>
      <owl:Restriction>
        <owl:onProperty rdf:resource="&iso19156;ObservationContext.relatedObservation"/>
        <owl:cardinality rdf:datatype="&xsd;nonNegativeInteger">1</owl:cardinality>
      </owl:Restriction>
    </rdfs:subClassOf>
    <rdfs:subClassOf>
      <owl:Restriction>
        <owl:onProperty rdf:resource="&iso19156;ObservationContext.relatedObservation"/>
        <owl:allValuesFrom rdf:resource="&iso19156;OM_Observation"/>
      </owl:Restriction>
    </rdfs:subClassOf>
  </owl:Class>

  <!--+++++++++++++++++++++++-->
  <!-- Class: OM_Observation -->
  <!--+++++++++++++++++++++++-->
  <owl:Class rdf:about="&iso19156;OM_Observation">
    <rdfs:label>OM_Observation</rdfs:label>
    <skos:definition>An observation is an act that results in the estimation of the value of a feature property, and involves application of a specified procedure, such as a sensor, instrument, algorithm or process chain. The procedure may be applied in-situ, remotely, or ex-situ with respect to the sampling location. Use of a common model allows observation data using different procedures to be combined unambiguously. Observation details are also important for data discovery and for data quality estimation. Observation feature types are defined by the properties that support these applications. An observation is an act associated with a discrete time instant or period through which a number, term or other symbol is assigned to a phenomenon [2]. The result of an observation is an estimate of the value of a property of some feature, so the details of the observation are metadata concerning the value of the feature property. The observation itself is also a feature, since it has properties and identity. </skos:definition>
    <rdfs:isDefinedBy>http://standards.iso.org/iso/19156/ed-1/en/</rdfs:isDefinedBy>
    <iso19150-2:constraint>result type shall be suitable for observedProperty</iso19150-2:constraint>
    <iso19150-2:constraint>result type shall be suitable for observedProperty</iso19150-2:constraint>
    <iso19150-2:constraint>result type shall be suitable for observedProperty</iso19150-2:constraint>
    <iso19150-2:constraint>result type shall be suitable for observedProperty</iso19150-2:constraint>
    <rdfs:subClassOf>
      <owl:Restriction>
        <owl:onProperty rdf:resource="&iso19156;OM_Observation.phenomenonTime"/>
        <owl:cardinality rdf:datatype="&xsd;nonNegativeInteger">1</owl:cardinality>
      </owl:Restriction>
    </rdfs:subClassOf>
    <rdfs:subClassOf>
      <owl:Restriction>
        <owl:onProperty rdf:resource="&iso19156;OM_Observation.phenomenonTime"/>
        <owl:allValuesFrom rdf:resource="&iso19108_407;TM_Object"/>
      </owl:Restriction>
    </rdfs:subClassOf>
    <rdfs:subClassOf>
      <owl:Restriction>
        <owl:onProperty rdf:resource="&iso19156;OM_Observation.resultTime"/>
        <owl:cardinality rdf:datatype="&xsd;nonNegativeInteger">1</owl:cardinality>
      </owl:Restriction>
    </rdfs:subClassOf>
    <rdfs:subClassOf>
      <owl:Restriction>
        <owl:onProperty rdf:resource="&iso19156;OM_Observation.resultTime"/>
        <owl:allValuesFrom rdf:resource="&iso19108_407;TM_Instant"/>
      </owl:Restriction>
    </rdfs:subClassOf>
    <rdfs:subClassOf>
      <owl:Restriction>
        <owl:onProperty rdf:resource="&iso19156;OM_Observation.validTime"/>
        <owl:maxCardinality rdf:datatype="&xsd;nonNegativeInteger">1</owl:maxCardinality>
      </owl:Restriction>
    </rdfs:subClassOf>
    <rdfs:subClassOf>
      <owl:Restriction>
        <owl:onProperty rdf:resource="&iso19156;OM_Observation.validTime"/>
        <owl:allValuesFrom rdf:resource="&iso19108_407;TM_Period"/>
      </owl:Restriction>
    </rdfs:subClassOf>
    <rdfs:subClassOf>
      <owl:Restriction>
        <owl:onProperty rdf:resource="&iso19156;OM_Observation.resultQuality"/>
        <owl:allValuesFrom rdf:resource="&iso19115_506;DQ_Element"/>
      </owl:Restriction>
    </rdfs:subClassOf>
    <rdfs:subClassOf>
      <owl:Restriction>
        <owl:onProperty rdf:resource="&iso19156;OM_Observation.parameter"/>
        <owl:allValuesFrom rdf:resource="&iso19156;NamedValue"/>
      </owl:Restriction>
    </rdfs:subClassOf>
    <rdfs:subClassOf>
      <owl:Restriction>
        <owl:onProperty rdf:resource="&iso19156;OM_Observation.metadata"/>
        <owl:maxCardinality rdf:datatype="&xsd;nonNegativeInteger">1</owl:maxCardinality>
      </owl:Restriction>
    </rdfs:subClassOf>
    <rdfs:subClassOf>
      <owl:Restriction>
        <owl:onProperty rdf:resource="&iso19156;OM_Observation.metadata"/>
        <owl:allValuesFrom rdf:resource="&iso19115_503;MD_Metadata"/>
      </owl:Restriction>
    </rdfs:subClassOf>
    <rdfs:subClassOf>
      <owl:Restriction>
        <owl:onProperty rdf:resource="&iso19156;OM_Observation.result"/>
        <owl:cardinality rdf:datatype="&xsd;nonNegativeInteger">1</owl:cardinality>
      </owl:Restriction>
    </rdfs:subClassOf>
    <rdfs:subClassOf>
      <owl:Restriction>
        <owl:onProperty rdf:resource="&iso19156;OM_Observation.result"/>
        <owl:allValuesFrom rdf:resource="&iso19103_337;Any"/>
      </owl:Restriction>
    </rdfs:subClassOf>
    <rdfs:subClassOf>
      <owl:Restriction>
        <owl:onProperty rdf:resource="&iso19156;OM_Observation.observedProperty"/>
        <owl:cardinality rdf:datatype="&xsd;nonNegativeInteger">1</owl:cardinality>
      </owl:Restriction>
    </rdfs:subClassOf>
    <rdfs:subClassOf>
      <owl:Restriction>
        <owl:onProperty rdf:resource="&iso19156;OM_Observation.observedProperty"/>
        <owl:allValuesFrom rdf:resource="&iso19109_449;GF_PropertyType"/>
      </owl:Restriction>
    </rdfs:subClassOf>
    <rdfs:subClassOf>
      <owl:Restriction>
        <owl:onProperty rdf:resource="&iso19156;OM_Observation.procedure"/>
        <owl:cardinality rdf:datatype="&xsd;nonNegativeInteger">1</owl:cardinality>
      </owl:Restriction>
    </rdfs:subClassOf>
    <rdfs:subClassOf>
      <owl:Restriction>
        <owl:onProperty rdf:resource="&iso19156;OM_Observation.procedure"/>
        <owl:allValuesFrom rdf:resource="&iso19156;OM_Process"/>
      </owl:Restriction>
    </rdfs:subClassOf>
    <rdfs:subClassOf>
      <owl:Restriction>
        <owl:onProperty rdf:resource="&iso19156;OM_Observation.featureOfInterest"/>
        <owl:cardinality rdf:datatype="&xsd;nonNegativeInteger">1</owl:cardinality>
      </owl:Restriction>
    </rdfs:subClassOf>
    <rdfs:subClassOf>
      <owl:Restriction>
        <owl:onProperty rdf:resource="&iso19156;OM_Observation.featureOfInterest"/>
        <owl:allValuesFrom rdf:resource="&iso19156_1687;GFI_Feature"/>
      </owl:Restriction>
    </rdfs:subClassOf>
    <rdfs:subClassOf>
      <owl:Restriction>
        <owl:onProperty rdf:resource="&iso19156;OM_Observation.theObservationContext"/>
        <owl:allValuesFrom rdf:resource="&iso19156;ObservationContext"/>
      </owl:Restriction>
    </rdfs:subClassOf>
  </owl:Class>

  <!--+++++++++++++++++++-->
  <!-- Class: OM_Process -->
  <!--+++++++++++++++++++-->
  <owl:Class rdf:about="&iso19156;OM_Process">
    <rdfs:label>OM_Process</rdfs:label>
    <skos:definition>The class OM_Process (Figure 2) is an instance of the .og.metaclass.cg. GF_FeatureType (ISO 19109:2005), which therefore represents a feature type. OM_Process is abstract, and has no attributes, operations or associations. It serves as the base class for observation processes. The purpose of an observation process is to generate an observation result. An instance of OM_Process is often an instrument or sensor, but may be a human observer, a simulator, or a process or algorithm applied to more primitive results used as inputs. NOTE	ISO 19115-2:2008 provides MI_Instrument, LE_Processing and LE_Algorithm, which could all be modelled as specializations of OM_Process. OGC SensorML [10] provides a model which is suitable for many observation procedures. </skos:definition>
    <rdfs:isDefinedBy>http://standards.iso.org/iso/19156/ed-1/en/</rdfs:isDefinedBy>
    <iso19150-2:isAbstract rdf:datatype="&xsd;boolean">true</iso19150-2:isAbstract>
  </owl:Class>

  <!--+++++++++++++++++++++++++++++++++-->
  <!-- ObjectProperty: NamedValue.name -->
  <!--+++++++++++++++++++++++++++++++++-->
  <owl:ObjectProperty rdf:about="&iso19156;NamedValue.name">
    <rdfs:label>name</rdfs:label>
    <skos:definition>The attribute name:GenericName shall indicate the meaning of the named value. Its value should be taken from a well-governed source if possible. EXAMPLES	When used as the value of an Observation:;parameter, the name might take values like .lq.procedureOperator.rq., .lq.detectionLimit.rq., .lq.amplifierGain.rq., .lq.samplingDepth.rq.. </skos:definition>
    <rdfs:isDefinedBy>http://standards.iso.org/iso/19156/ed-1/en/</rdfs:isDefinedBy>
    <rdfs:domain rdf:resource="&iso19156;NamedValue"/>
    <rdfs:range rdf:resource="&iso19103_336;GenericName"/>
  </owl:ObjectProperty>

  <!--++++++++++++++++++++++++++++++++++-->
  <!-- ObjectProperty: NamedValue.value -->
  <!--++++++++++++++++++++++++++++++++++-->
  <owl:ObjectProperty rdf:about="&iso19156;NamedValue.value">
    <rdfs:label>value</rdfs:label>
    <skos:definition>The attribute value:Any shall provide the value. The type Any should be substituted by a suitable concrete type, such as CI_ResponsibleParty or Measure. </skos:definition>
    <rdfs:isDefinedBy>http://standards.iso.org/iso/19156/ed-1/en/</rdfs:isDefinedBy>
    <rdfs:domain rdf:resource="&iso19156;NamedValue"/>
    <rdfs:range rdf:resource="&iso19103_337;Any"/>
  </owl:ObjectProperty>

  <!--+++++++++++++++++++++++++++++++++++++++++-->
  <!-- ObjectProperty: ObservationContext.role -->
  <!--+++++++++++++++++++++++++++++++++++++++++-->
  <owl:ObjectProperty rdf:about="&iso19156;ObservationContext.role">
    <rdfs:label>role</rdfs:label>
    <skos:definition>The attribute .lt.i.gt.role:GenericName .lt..sl.i.gt.shall describe the relationship of the target OM_Observation to the source OM_Observation. </skos:definition>
    <rdfs:isDefinedBy>http://standards.iso.org/iso/19156/ed-1/en/</rdfs:isDefinedBy>
    <rdfs:domain rdf:resource="&iso19156;ObservationContext"/>
    <rdfs:range rdf:resource="&iso19103_336;GenericName"/>
  </owl:ObjectProperty>

  <!--+++++++++++++++++++++++++++++++++++++++++++++++-->
  <!-- ObjectProperty: OM_Observation.phenomenonTime -->
  <!--+++++++++++++++++++++++++++++++++++++++++++++++-->
  <owl:ObjectProperty rdf:about="&iso19156;OM_Observation.phenomenonTime">
    <rdfs:label>phenomenonTime</rdfs:label>
    <skos:definition>The attribute .lt.i.gt.phenomenonTime:TM_Object.lt..sl.i.gt. shall describe the time that the result (6.2.2.9) applies to the property of the feature-of-interest (6.2.2.7). This is often the time of interaction by a sampling procedure (8.2) or observation procedure (6.2.2.10) with a real-world feature. NOTE 1	The phenomenon time is the temporal parameter normally used in geospatial analysis of the result. NOTE 2	If the observedProperty of an observation is .lq.occurrence time.rq. then the result should be the same as the phenomenonTime</skos:definition>
    <rdfs:isDefinedBy>http://standards.iso.org/iso/19156/ed-1/en/</rdfs:isDefinedBy>
    <rdfs:domain rdf:resource="&iso19156;OM_Observation"/>
    <rdfs:range rdf:resource="&iso19108_407;TM_Object"/>
  </owl:ObjectProperty>

  <!--+++++++++++++++++++++++++++++++++++++++++++-->
  <!-- ObjectProperty: OM_Observation.resultTime -->
  <!--+++++++++++++++++++++++++++++++++++++++++++-->
  <owl:ObjectProperty rdf:about="&iso19156;OM_Observation.resultTime">
    <rdfs:label>resultTime</rdfs:label>
    <skos:definition>The attribute .lt.i.gt.resultTime:TM_Instant.lt..sl.i.gt. shall describe the time when the result became available, typically when the procedure (6.2.2.10) associated with the observation was completed For some observations this is identical to the phenomenonTime. However, there are important cases where they differ. EXAMPLE 1	Where a measurement is made on a specimen in a laboratory, the phenomenonTime is the time the specimen was retrieved from its host, while the resultTime is the time the laboratory procedure was applied. EXAMPLE 2	The resultTime also supports disambiguation of repeat measurements made of the same property of a feature using the same procedure. EXAMPLE 3	Where sensor observation results are post-processed, the resultTime is the post-processing time, while the phenomenonTime is the time of initial interaction with the world. EXAMPLE 4	Simulations may be used to estimate the values for phenomena in the future or past. The phenomenonTime is the time that the result applies to, while the resultTime is the time that the simulation was executed. </skos:definition>
    <rdfs:isDefinedBy>http://standards.iso.org/iso/19156/ed-1/en/</rdfs:isDefinedBy>
    <rdfs:domain rdf:resource="&iso19156;OM_Observation"/>
    <rdfs:range rdf:resource="&iso19108_407;TM_Instant"/>
  </owl:ObjectProperty>

  <!--++++++++++++++++++++++++++++++++++++++++++-->
  <!-- ObjectProperty: OM_Observation.validTime -->
  <!--++++++++++++++++++++++++++++++++++++++++++-->
  <owl:ObjectProperty rdf:about="&iso19156;OM_Observation.validTime">
    <rdfs:label>validTime</rdfs:label>
    <skos:definition>If present, the attribute .lt.i.gt.validTime:TM_Period.lt..sl.i.gt. shall describe the time period during which the result is intended to be used. NOTE	This attribute is commonly required in forecasting applications. </skos:definition>
    <rdfs:isDefinedBy>http://standards.iso.org/iso/19156/ed-1/en/</rdfs:isDefinedBy>
    <rdfs:domain rdf:resource="&iso19156;OM_Observation"/>
    <rdfs:range rdf:resource="&iso19108_407;TM_Period"/>
  </owl:ObjectProperty>

  <!--++++++++++++++++++++++++++++++++++++++++++++++-->
  <!-- ObjectProperty: OM_Observation.resultQuality -->
  <!--++++++++++++++++++++++++++++++++++++++++++++++-->
  <owl:ObjectProperty rdf:about="&iso19156;OM_Observation.resultQuality">
    <rdfs:label>resultQuality</rdfs:label>
    <skos:definition>If present, the attributes .lt.i.gt.resultQuality:DQ_Element.lt..sl.i.gt. shall describe the quality of the result (6.2.2.9). This instance-specific description complements the description of the observation procedure (6.2.2.10), which provides information concerning the quality of all observations using this procedure. Quality of a result may be assessed following the procedures in ISO 19114:2003.Multiple measures may be provided (ISO.sl.TS 19138:2006). </skos:definition>
    <rdfs:isDefinedBy>http://standards.iso.org/iso/19156/ed-1/en/</rdfs:isDefinedBy>
    <rdfs:domain rdf:resource="&iso19156;OM_Observation"/>
    <rdfs:range rdf:resource="&iso19115_506;DQ_Element"/>
  </owl:ObjectProperty>

  <!--++++++++++++++++++++++++++++++++++++++++++-->
  <!-- ObjectProperty: OM_Observation.parameter -->
  <!--++++++++++++++++++++++++++++++++++++++++++-->
  <owl:ObjectProperty rdf:about="&iso19156;OM_Observation.parameter">
    <rdfs:label>parameter</rdfs:label>
    <skos:definition>If present, the attributes .lt.i.gt.parameter:NamedValue.lt..sl.i.gt. shall describe an arbitrary event-specific parameter. This might be an environmental parameter, an instrument setting or input, or an event-specific sampling parameter that is not tightly bound to either the feature-of-interest (6.2.2.7) or to the observation procedure (6.2.2.10). To avoid ambiguity, there shall be no more than one parameter with the same name. NOTE	Parameters that are tightly bound to the procedure may be recorded as part of the procedure description. In some contexts the .lt.i.gt.Observation::procedure.lt..sl.i.gt. (6.2.2.10) is a generic or standard procedure, rather than an event-specific process. In this context, parameters bound to the observation act, such as instrument settings, calibrations or inputs, local position, detection limits, asset identifer, operator, may augment the description of a standard procedure. EXAMPLE	A time sequence of observations of water quality in a well may be made at variable depths within the well. While these may be associated with specimens taken from the well at this depth as the features-of-interest, a more common approach is to identify the well itself as the feature-of-interest, and add a .ldq.samplingDepth.rdq. parameter to the observation (Figure 3). The sampling depth is of secondary interest compared to the temporal variation of water quality at the site. </skos:definition>
    <rdfs:isDefinedBy>http://standards.iso.org/iso/19156/ed-1/en/</rdfs:isDefinedBy>
    <rdfs:domain rdf:resource="&iso19156;OM_Observation"/>
    <rdfs:range rdf:resource="&iso19156;NamedValue"/>
  </owl:ObjectProperty>

  <!--+++++++++++++++++++++++++++++++++++++++++-->
  <!-- ObjectProperty: OM_Observation.metadata -->
  <!--+++++++++++++++++++++++++++++++++++++++++-->
  <owl:ObjectProperty rdf:about="&iso19156;OM_Observation.metadata">
    <rdfs:label>metadata</rdfs:label>
    <rdfs:isDefinedBy>http://standards.iso.org/iso/19156/ed-1/en/</rdfs:isDefinedBy>
    <iso19150-2:associationName>Metadata</iso19150-2:associationName>
    <rdfs:domain rdf:resource="&iso19156;OM_Observation"/>
    <rdfs:range rdf:resource="&iso19115_503;MD_Metadata"/>
  </owl:ObjectProperty>

  <!--+++++++++++++++++++++++++++++++++++++++-->
  <!-- ObjectProperty: OM_Observation.result -->
  <!--+++++++++++++++++++++++++++++++++++++++-->
  <owl:ObjectProperty rdf:about="&iso19156;OM_Observation.result">
    <rdfs:label>result</rdfs:label>
    <rdfs:isDefinedBy>http://standards.iso.org/iso/19156/ed-1/en/</rdfs:isDefinedBy>
    <iso19150-2:aggregationType>partOfCompositeAggregation</iso19150-2:aggregationType>
    <iso19150-2:associationName>Range</iso19150-2:associationName>
    <rdfs:domain rdf:resource="&iso19156;OM_Observation"/>
    <rdfs:range rdf:resource="&iso19103_337;Any"/>
  </owl:ObjectProperty>

  <!--+++++++++++++++++++++++++++++++++++++++++++++++++-->
  <!-- ObjectProperty: OM_Observation.observedProperty -->
  <!--+++++++++++++++++++++++++++++++++++++++++++++++++-->
  <owl:ObjectProperty rdf:about="&iso19156;OM_Observation.observedProperty">
    <rdfs:label>observedProperty</rdfs:label>
    <rdfs:isDefinedBy>http://standards.iso.org/iso/19156/ed-1/en/</rdfs:isDefinedBy>
    <iso19150-2:associationName>Phenomenon</iso19150-2:associationName>
    <rdfs:domain rdf:resource="&iso19156;OM_Observation"/>
    <rdfs:range rdf:resource="&iso19109_449;GF_PropertyType"/>
  </owl:ObjectProperty>

  <!--++++++++++++++++++++++++++++++++++++++++++-->
  <!-- ObjectProperty: OM_Observation.procedure -->
  <!--++++++++++++++++++++++++++++++++++++++++++-->
  <owl:ObjectProperty rdf:about="&iso19156;OM_Observation.procedure">
    <rdfs:label>procedure</rdfs:label>
    <rdfs:isDefinedBy>http://standards.iso.org/iso/19156/ed-1/en/</rdfs:isDefinedBy>
    <iso19150-2:associationName>ProcessUsed</iso19150-2:associationName>
    <rdfs:domain rdf:resource="&iso19156;OM_Observation"/>
    <rdfs:range rdf:resource="&iso19156;OM_Process"/>
  </owl:ObjectProperty>

  <!--++++++++++++++++++++++++++++++++++++++++++++++++++-->
  <!-- ObjectProperty: OM_Observation.featureOfInterest -->
  <!--++++++++++++++++++++++++++++++++++++++++++++++++++-->
  <owl:ObjectProperty rdf:about="&iso19156;OM_Observation.featureOfInterest">
    <rdfs:label>featureOfInterest</rdfs:label>
    <rdfs:isDefinedBy>http://standards.iso.org/iso/19156/ed-1/en/</rdfs:isDefinedBy>
    <iso19150-2:associationName>Domain</iso19150-2:associationName>
    <rdfs:domain rdf:resource="&iso19156;OM_Observation"/>
    <rdfs:range rdf:resource="&iso19156_1687;GFI_Feature"/>
  </owl:ObjectProperty>

  <!--++++++++++++++++++++++++++++++++++++++++++++++++++++++-->
  <!-- ObjectProperty: OM_Observation.theObservationContext -->
  <!--++++++++++++++++++++++++++++++++++++++++++++++++++++++-->
  <owl:ObjectProperty rdf:about="&iso19156;OM_Observation.theObservationContext">
    <rdfs:label>theObservationContext</rdfs:label>
    <rdfs:isDefinedBy>http://standards.iso.org/iso/19156/ed-1/en/</rdfs:isDefinedBy>
    <rdfs:domain rdf:resource="&iso19156;OM_Observation"/>
    <rdfs:range rdf:resource="&iso19156;ObservationContext"/>
  </owl:ObjectProperty>

  <!--+++++++++++++++++++++++++++++++++++++++++++++++++++++++-->
  <!-- ObjectProperty: ObservationContext.relatedObservation -->
  <!--+++++++++++++++++++++++++++++++++++++++++++++++++++++++-->
  <owl:ObjectProperty rdf:about="&iso19156;ObservationContext.relatedObservation">
    <rdfs:label>relatedObservation</rdfs:label>
    <rdfs:isDefinedBy>http://standards.iso.org/iso/19156/ed-1/en/</rdfs:isDefinedBy>
    <rdfs:domain rdf:resource="&iso19156;ObservationContext"/>
    <rdfs:range rdf:resource="&iso19156;OM_Observation"/>
  </owl:ObjectProperty>

</rdf:RDF>

